<?xml version="1.0" encoding="UTF-8"?>
<rdf:RDF
    xmlns:gr="http://purl.org/goodrelations/v1#"
    xmlns:rdf="http://www.w3.org/1999/02/22-rdf-syntax-ns#"
    xmlns:xsd="http://www.w3.org/2001/XMLSchema#"
    xmlns:rdfs="http://www.w3.org/2000/01/rdf-schema#"
    xmlns:owl="http://www.w3.org/2002/07/owl#"
    xmlns:dc="http://purl.org/dc/elements/1.1/"
    xmlns="http://www.ebusiness-unibw.org/ontologies/consumerelectronics/v1#"
  xml:base="http://www.ebusiness-unibw.org/ontologies/consumerelectronics/v1">
  <owl:Ontology rdf:about="">
    <rdfs:label xml:lang="en">CEO: Consumer Electronics Ontology - An Ontology for Consumer Electronics Products and Services</rdfs:label>
    <rdfs:comment xml:lang="en">The CEO: Consumer Electronics Ontology is a vocabulary for describing typical consumer electronics products and services and their features, e.g. digital cameras, camcorders, etc.
It can be used in combination with GoodRelations, http://purl.org/goodrelations/ for making your e-commerce offerings available in the new Web of Data.

Several descriptions of conceptual elements in this ontology are partly based on or reuse content from respective Wikipedia articles in the English Wikipedia http://en.wikipedia.org/wiki/. Thus, this ontology is also licensed under the GNU Free Documentation License, http://www.gnu.org/copyleft/fdl.html.</rdfs:comment>
    <dc:creator xml:lang="en">Xaver Brandl, Christian Deckert, Felix Frommer, Daniel Karl, Daniel Koslowski, Daniel Schley, David Sonntag, Andreas Wechselberger, and Martin Hepp</dc:creator>
    <dc:title xml:lang="en">CEO: Consumer Electronics Ontology - An Ontology for Consumer Electronics Products and Services</dc:title>
    <dc:rights xml:lang="en">http://creativecommons.org/licenses/by/3.0/</dc:rights>
    <owl:imports rdf:resource="http://purl.org/goodrelations/v1"/>
    <rdfs:seeAlso rdf:resource="http://www.rdf4ecommerce.org/"/>
    <dc:subject xml:lang="en">E-Commerce, E-Business, GoodRelations, Ontology, MP3 player, TV, Printer, DigitalCamera, Camcorder</dc:subject>
  </owl:Ontology>
  <owl:Class rdf:ID="DataFormatVideo">
    <rdfs:label xml:lang="de">Video Datenformat</rdfs:label>
    <rdfs:label xml:lang="en">Data Format Video</rdfs:label>
    <rdfs:subClassOf rdf:resource="#DataFormat"/>
    <rdfs:isDefinedBy rdf:resource="http://www.ebusiness-unibw.org/ontologies/consumerelectronics/v1"/>
    <belongsToModule xml:lang="en">MP3Player, DigitalCamera, Camcorder</belongsToModule>
    <rdfs:comment xml:lang="en">A data format is a particular way to encode information for storage in a computer file (refers to video data).

(This description is partly based on or reuses content from the Wikipedia article "File Format" (http://en.wikipedia.org/wiki/File_format) and is licensed under the GNU Free Documentation License (http://www.gnu.org/copyleft/fdl.html).)</rdfs:comment>
  </owl:Class>
  <owl:Class rdf:ID="SensorType">
    <rdfs:isDefinedBy rdf:resource="http://www.ebusiness-unibw.org/ontologies/consumerelectronics/v1"/>
    <rdfs:comment xml:lang="en">Type of device that measures a physical quantity and converts it into a signal which can be read by an observer or by an instrument.

(This description is partly based on or reuses content from the Wikipedia article "Sensor" (http://en.wikipedia.org/wiki/Sensor) and is licensed under the GNU Free Documentation License (http://www.gnu.org/copyleft/fdl.html).)</rdfs:comment>
    <rdfs:label xml:lang="en">Sensor type</rdfs:label>
    <rdfs:label xml:lang="de">Sensorart</rdfs:label>
    <belongsToModule xml:lang="en">Camcorder</belongsToModule>
    <rdfs:subClassOf rdf:resource="http://purl.org/goodrelations/v1#QualitativeValue"/>
  </owl:Class>
  <owl:Class rdf:ID="DataInterfaceType">
    <rdfs:isDefinedBy rdf:resource="http://www.ebusiness-unibw.org/ontologies/consumerelectronics/v1"/>
    <rdfs:comment xml:lang="en">Interface generally refers to an abstraction that an entity provides of itself to the outside.

(This description is partly based on or reuses content from the Wikipedia article "Interface (computer science)" (http://en.wikipedia.org/wiki/Interface_(computer_science)) and is licensed under the GNU Free Documentation License (http://www.gnu.org/copyleft/fdl.html).)</rdfs:comment>
    <rdfs:label xml:lang="en">Data Interface Type</rdfs:label>
    <rdfs:label xml:lang="de">Datenschnittstellentyp</rdfs:label>
    <belongsToModule xml:lang="en">MP3Player, Printer, DigitalCamera, Camcorder</belongsToModule>
    <rdfs:subClassOf rdf:resource="http://purl.org/goodrelations/v1#QualitativeValue"/>
  </owl:Class>
  <owl:Class rdf:ID="USB">
    <rdfs:isDefinedBy rdf:resource="http://www.ebusiness-unibw.org/ontologies/consumerelectronics/v1"/>
    <rdfs:label xml:lang="en">USB</rdfs:label>
    <rdfs:label xml:lang="de">USB</rdfs:label>
    <belongsToModule xml:lang="en">MP3Player, Printer, DigitalCamera, Camcorder</belongsToModule>
    <rdfs:subClassOf rdf:resource="#EnergySource"/>
    <rdfs:comment xml:lang="en">Universal Serial Bus (USB) is a serial bus standard to connect devices to a host computer.

(This description is partly based on or reuses content from the Wikipedia article "Universal Serial Bus" (http://en.wikipedia.org/wiki/Universal_Serial_Bus) and is licensed under the GNU Free Documentation License (http://www.gnu.org/copyleft/fdl.html).)</rdfs:comment>
  </owl:Class>
  <owl:Class rdf:ID="Accessory">
    <rdfs:subClassOf rdf:resource="http://purl.org/goodrelations/v1#QualitativeValue"/>
    <rdfs:isDefinedBy rdf:resource="http://www.ebusiness-unibw.org/ontologies/consumerelectronics/v1"/>
    <rdfs:label xml:lang="en">Accessory</rdfs:label>
    <rdfs:label xml:lang="de">Zubehör</rdfs:label>
    <belongsToModule xml:lang="en">Camcorder</belongsToModule>
    <rdfs:comment xml:lang="en">A subordinate or supplementary item; an adjunct.</rdfs:comment>
  </owl:Class>
  <owl:Class rdf:ID="LensSystem">
    <rdfs:comment xml:lang="en">A lens is an optical device with perfect or approximate axial symmetry which transmits and refracts light, converging or diverging the beam.

(This description is partly based on or reuses content from the Wikipedia article "Lens (optics)" (http://en.wikipedia.org/wiki/Lens_(optics)) and is licensed under the GNU Free Documentation License (http://www.gnu.org/copyleft/fdl.html).)</rdfs:comment>
    <belongsToModule xml:lang="en">Camcorder</belongsToModule>
    <rdfs:isDefinedBy rdf:resource="http://www.ebusiness-unibw.org/ontologies/consumerelectronics/v1"/>
    <rdfs:label xml:lang="en">Lens system</rdfs:label>
    <rdfs:label xml:lang="de">Objektivsystem</rdfs:label>
    <rdfs:subClassOf rdf:resource="http://purl.org/goodrelations/v1#QualitativeValue"/>
  </owl:Class>
  <owl:Class rdf:ID="EnergySource">
    <rdfs:isDefinedBy rdf:resource="http://www.ebusiness-unibw.org/ontologies/consumerelectronics/v1"/>
    <belongsToModule xml:lang="en">MP3Player, Printer, DigitalCamera, Camcorder</belongsToModule>
    <rdfs:label xml:lang="en">Energy Source</rdfs:label>
    <rdfs:label xml:lang="de">Energiequelle</rdfs:label>
    <rdfs:subClassOf rdf:resource="http://purl.org/goodrelations/v1#QualitativeValue"/>
    <rdfs:comment xml:lang="en">Methods of energy storage have been developed, which transform electrical energy into forms of potential energy.

(This description is partly based on or reuses content from the Wikipedia article "Energy development" (http://en.wikipedia.org/wiki/Energy_development) and is licensed under the GNU Free Documentation License (http://www.gnu.org/copyleft/fdl.html).)</rdfs:comment>
  </owl:Class>
  <owl:Class rdf:ID="Camcorder">
    <rdfs:isDefinedBy rdf:resource="http://www.ebusiness-unibw.org/ontologies/consumerelectronics/v1"/>
    <rdfs:comment xml:lang="en">A camcorder is a portable consumer electronics device for recording video and audio using a built-in recorder unit.</rdfs:comment>
    <belongsToModule xml:lang="en">Camcorder</belongsToModule>
    <rdfs:subClassOf rdf:resource="http://purl.org/goodrelations/v1#ProductOrService"/>
    <rdfs:label xml:lang="en">Camcorder</rdfs:label>
    <rdfs:label xml:lang="de">Camcorder</rdfs:label>
  </owl:Class>
  <owl:Class rdf:ID="TVDisplayResolution">
    <rdfs:isDefinedBy rdf:resource="http://www.ebusiness-unibw.org/ontologies/consumerelectronics/v1"/>
    <belongsToModule xml:lang="en">TV</belongsToModule>
    <rdfs:label xml:lang="de">Fernsehbildschirmauflösung</rdfs:label>
    <rdfs:label xml:lang="en">TV display resolution</rdfs:label>
    <rdfs:comment rdf:datatype="http://www.w3.org/2001/XMLSchema#string"
    >The display resolution of a digital television or display typically refers to the number of distinct pixels in each dimension that can be displayed.

(This description is partly based on or reuses content from the Wikipedia article "Display resolution" (http://en.wikipedia.org/wiki/Display_resolution) and is licensed under the GNU Free Documentation License (http://www.gnu.org/copyleft/fdl.html).)</rdfs:comment>
    <rdfs:subClassOf rdf:resource="#SupportedResolution"/>
  </owl:Class>
  <owl:Class rdf:ID="SignalFormat">
    <belongsToModule xml:lang="en">TV</belongsToModule>
    <rdfs:subClassOf rdf:resource="#TVTuner"/>
    <rdfs:isDefinedBy rdf:resource="http://www.ebusiness-unibw.org/ontologies/consumerelectronics/v1"/>
    <rdfs:label xml:lang="en">Signal format</rdfs:label>
    <rdfs:label xml:lang="de">Signalformat</rdfs:label>
    <rdfs:comment xml:lang="en">Type of the transmitted video format signal that is displayed by a monitor or TV panel.</rdfs:comment>
  </owl:Class>
  <owl:Class rdf:ID="DataFormat">
    <rdfs:subClassOf rdf:resource="http://purl.org/goodrelations/v1#QualitativeValue"/>
    <rdfs:label xml:lang="de">Datenformat</rdfs:label>
    <rdfs:label xml:lang="en">Data Format</rdfs:label>
    <belongsToModule xml:lang="en">MP3Player, DigitalCamera, Camcorder</belongsToModule>
    <rdfs:isDefinedBy rdf:resource="http://www.ebusiness-unibw.org/ontologies/consumerelectronics/v1"/>
    <rdfs:comment xml:lang="en">A data format is a particular way to encode information for storage in a computer file.

(This description is partly based on or reuses content from the Wikipedia article "File Format" (http://en.wikipedia.org/wiki/File_format) and is licensed under the GNU Free Documentation License (http://www.gnu.org/copyleft/fdl.html).)</rdfs:comment>
  </owl:Class>
  <owl:Class rdf:ID="LaserPrinter">
    <rdfs:isDefinedBy rdf:resource="http://www.ebusiness-unibw.org/ontologies/consumerelectronics/v1"/>
    <belongsToModule xml:lang="en">Printer</belongsToModule>
    <rdfs:label xml:lang="en">Laser printer</rdfs:label>
    <rdfs:label xml:lang="de">Laserdrucker</rdfs:label>
    <rdfs:comment xml:lang="en">A laser printer is a common type of computer printer that rapidly produces high quality text and graphics on plain paper.

(This description is partly based on or reuses content from the Wikipedia article "Laser printer" (http://en.wikipedia.org/wiki/Laser_printer) and is licensed under the GNU Free Documentation License (http://www.gnu.org/copyleft/fdl.html).)</rdfs:comment>
    <rdfs:subClassOf rdf:resource="#Printer"/>
  </owl:Class>
  <owl:Class rdf:ID="WhiteBalance">
    <rdfs:subClassOf rdf:resource="http://purl.org/goodrelations/v1#QualitativeValue"/>
    <rdfs:isDefinedBy rdf:resource="http://www.ebusiness-unibw.org/ontologies/consumerelectronics/v1"/>
    <rdfs:label xml:lang="en">White balance</rdfs:label>
    <rdfs:label xml:lang="de">Weißabgleich</rdfs:label>
    <rdfs:comment xml:lang="en">Is the global adjustment of the intensities of the colors (typically red, green, and blue primary colors). An important goal of this adjustment is to render specific colors - particularly neutral colors - correctly; hence, the general method is sometimes called gray balance, neutral balance, or white balance.

(This description is partly based on or reuses content from the Wikipedia article "White Balance" (http://en.wikipedia.org/wiki/White_Balance) and is licensed under the GNU Free Documentation License (http://www.gnu.org/copyleft/fdl.html).)</rdfs:comment>
    <belongsToModule xml:lang="en">Camcorder</belongsToModule>
  </owl:Class>
  <owl:Class rdf:ID="DataFormatOffice">
    <rdfs:comment xml:lang="en">A data format is a particular way to encode information for storage in a computer file (refers to office data).

(This description is partly based on or reuses content from the Wikipedia article "File Format" (http://en.wikipedia.org/wiki/File_format) and is licensed under the GNU Free Documentation License (http://www.gnu.org/copyleft/fdl.html).)</rdfs:comment>
    <rdfs:isDefinedBy rdf:resource="http://www.ebusiness-unibw.org/ontologies/consumerelectronics/v1"/>
    <belongsToModule xml:lang="en">MP3Player, DigitalCamera</belongsToModule>
    <rdfs:label xml:lang="de">Büro Datenformat</rdfs:label>
    <rdfs:label xml:lang="en">Data Format Office</rdfs:label>
    <rdfs:subClassOf rdf:resource="#DataFormat"/>
  </owl:Class>
  <owl:Class rdf:ID="Connectivity">
    <belongsToModule xml:lang="en">TV</belongsToModule>
    <rdfs:subClassOf rdf:resource="http://purl.org/goodrelations/v1#QualitativeValue"/>
    <rdfs:comment xml:lang="en">A generic term for linking devices to each other and allow sending data in one or both directions.</rdfs:comment>
    <rdfs:isDefinedBy rdf:resource="http://www.ebusiness-unibw.org/ontologies/consumerelectronics/v1"/>
    <rdfs:label xml:lang="en">Connectivity</rdfs:label>
    <rdfs:label xml:lang="de">Verbindungsmöglichkeit</rdfs:label>
  </owl:Class>
  <owl:Class rdf:ID="AudioFeatures">
    <rdfs:isDefinedBy rdf:resource="http://www.ebusiness-unibw.org/ontologies/consumerelectronics/v1"/>
    <rdfs:comment xml:lang="en">Additional audio equipment and abilities.</rdfs:comment>
    <belongsToModule xml:lang="en">TV</belongsToModule>
    <rdfs:label xml:lang="de">Audio Eigenschaften</rdfs:label>
    <rdfs:label xml:lang="en">Audio Features</rdfs:label>
    <rdfs:subClassOf rdf:resource="#Features"/>
  </owl:Class>
  <owl:Class rdf:ID="PowerSupplyUnit">
    <belongsToModule xml:lang="en">MP3Player, Printer, DigitalCamera, Camcorder</belongsToModule>
    <rdfs:comment xml:lang="en">A Power Supply Adapter is used to convert 120 or 240 volt AC supplied by a utility company to a well-regulated lower voltage DC for electronic devices.

(This description is partly based on or reuses content from the Wikipedia article "Power supply" (http://en.wikipedia.org/wiki/Power_supply) and is licensed under the GNU Free Documentation License (http://www.gnu.org/copyleft/fdl.html).)</rdfs:comment>
    <rdfs:label xml:lang="en">Power Supply Unit</rdfs:label>
    <rdfs:label xml:lang="de">Netzgerät</rdfs:label>
    <rdfs:isDefinedBy rdf:resource="http://www.ebusiness-unibw.org/ontologies/consumerelectronics/v1"/>
    <rdfs:subClassOf rdf:resource="#EnergySource"/>
  </owl:Class>
  <owl:Class rdf:ID="CompatibleOperatingSystems">
    <rdfs:comment xml:lang="en">Ability to communicate with different kinds of operating systems.</rdfs:comment>
    <rdfs:isDefinedBy rdf:resource="http://www.ebusiness-unibw.org/ontologies/consumerelectronics/v1"/>
    <rdfs:subClassOf rdf:resource="http://purl.org/goodrelations/v1#QualitativeValue"/>
    <belongsToModule xml:lang="en">MP3Player, Printer, DigitalCamera, Camcorder</belongsToModule>
    <rdfs:label xml:lang="de">Kompatible Betriebssyteme</rdfs:label>
    <rdfs:label xml:lang="en">Compatible Operating Systems</rdfs:label>
  </owl:Class>
  <owl:Class rdf:ID="SupportedResolution">
    <rdfs:isDefinedBy rdf:resource="http://www.ebusiness-unibw.org/ontologies/consumerelectronics/v1"/>
    <rdfs:subClassOf rdf:resource="http://purl.org/goodrelations/v1#QualitativeValue"/>
    <rdfs:label xml:lang="en">Supported resolution</rdfs:label>
    <rdfs:label xml:lang="en">Unterstützte Auflösung</rdfs:label>
    <belongsToModule xml:lang="en">TV</belongsToModule>
    <rdfs:comment xml:lang="en">Resolution supported by an electronical device.</rdfs:comment>
  </owl:Class>
  <owl:Class rdf:ID="VideoFeatures">
    <rdfs:label xml:lang="de">Video Eigenschaften</rdfs:label>
    <rdfs:label xml:lang="en">Video Features</rdfs:label>
    <belongsToModule xml:lang="en">TV</belongsToModule>
    <rdfs:comment xml:lang="en">Additional video equipment and abilities.</rdfs:comment>
    <rdfs:subClassOf rdf:resource="#Features"/>
    <rdfs:isDefinedBy rdf:resource="http://www.ebusiness-unibw.org/ontologies/consumerelectronics/v1"/>
  </owl:Class>
  <owl:Class rdf:ID="StorageMedia">
    <belongsToModule xml:lang="en">MP3Player, DigitalCamera, Camcorder</belongsToModule>
    <rdfs:subClassOf rdf:resource="http://purl.org/goodrelations/v1#QualitativeValue"/>
    <rdfs:label xml:lang="en">Storage Media</rdfs:label>
    <rdfs:label xml:lang="de">Speichermedium</rdfs:label>
    <rdfs:isDefinedBy rdf:resource="http://www.ebusiness-unibw.org/ontologies/consumerelectronics/v1"/>
    <rdfs:comment xml:lang="en">A data storage device is a device for recording (storing) information (data).
 
(This description is partly based on or reuses content from the Wikipedia article "Data Storage Device" (http://en.wikipedia.org/wiki/Data_storage_device) and is licensed under the GNU Free Documentation License (http://www.gnu.org/copyleft/fdl.html).)</rdfs:comment>
  </owl:Class>
  <owl:Class rdf:ID="Color">
    <rdfs:label xml:lang="de">Farbe</rdfs:label>
    <rdfs:label xml:lang="en">Color</rdfs:label>
    <rdfs:comment xml:lang="en">Color derives from the spectrum of light interacting in the eye with the spectral sensitivities of the light receptors.

(This description is partly based on or reuses content from the Wikipedia article "Color" (http://en.wikipedia.org/wiki/Color) and is licensed under the GNU Free Documentation License (http://www.gnu.org/copyleft/fdl.html).)</rdfs:comment>
    <rdfs:subClassOf rdf:resource="http://purl.org/goodrelations/v1#QualitativeValue"/>
    <rdfs:isDefinedBy rdf:resource="http://www.ebusiness-unibw.org/ontologies/consumerelectronics/v1"/>
    <belongsToModule xml:lang="en">MP3Player, TV, Printer, DigitalCamera, Camcorder</belongsToModule>
  </owl:Class>
  <owl:Class rdf:ID="ViewFinder">
    <rdfs:label xml:lang="de">Bildsucher</rdfs:label>
    <rdfs:label xml:lang="en">Viewfinder</rdfs:label>
    <rdfs:isDefinedBy rdf:resource="http://www.ebusiness-unibw.org/ontologies/consumerelectronics/v1"/>
    <belongsToModule xml:lang="en">DigitalCamera, Camcorder</belongsToModule>
    <rdfs:subClassOf rdf:resource="http://purl.org/goodrelations/v1#QualitativeValue"/>
    <rdfs:comment xml:lang="en">A viewfinder is what the photographer looks through to compose, and in many cases to focus, the picture.

(This description is partly based on or reuses content from the Wikipedia article "Viewfinder" (http://en.wikipedia.org/wiki/Viewfinder) and is licensed under the GNU Free Documentation License (http://www.gnu.org/copyleft/fdl.html).)</rdfs:comment>
  </owl:Class>
  <owl:Class rdf:ID="InkjetPrinter">
    <rdfs:label xml:lang="de">Tintenstrahldrucker</rdfs:label>
    <rdfs:label xml:lang="en">Inkjet printer</rdfs:label>
    <rdfs:subClassOf rdf:resource="#Printer"/>
    <rdfs:comment xml:lang="en">Inkjet printers operate by propelling variably-sized droplets of liquid or molten material (ink) onto almost any sized page.

(This description is partly based on or reuses content from the Wikipedia article "Inkjet printer" (http://en.wikipedia.org/wiki/Inkjet_printer) and is licensed under the GNU Free Documentation License (http://www.gnu.org/copyleft/fdl.html).)</rdfs:comment>
    <belongsToModule xml:lang="en">Printer</belongsToModule>
    <rdfs:isDefinedBy rdf:resource="http://www.ebusiness-unibw.org/ontologies/consumerelectronics/v1"/>
  </owl:Class>
  <owl:Class rdf:ID="DataFormatImage">
    <belongsToModule xml:lang="en">MP3Player, DigitalCamera, Camcorder</belongsToModule>
    <rdfs:isDefinedBy rdf:resource="http://www.ebusiness-unibw.org/ontologies/consumerelectronics/v1"/>
    <rdfs:comment xml:lang="en">A data format is a particular way to encode information for storage in a computer file (refers to image data).

(This description is partly based on or reuses content from the Wikipedia article "File Format" (http://en.wikipedia.org/wiki/File_format) and is licensed under the GNU Free Documentation License (http://www.gnu.org/copyleft/fdl.html).)</rdfs:comment>
    <rdfs:subClassOf rdf:resource="#DataFormat"/>
    <rdfs:label xml:lang="en">Data Format Image</rdfs:label>
    <rdfs:label xml:lang="de">Graphik Datenformat</rdfs:label>
  </owl:Class>
  <owl:Class rdf:ID="DataFormatAudio">
    <rdfs:isDefinedBy rdf:resource="http://www.ebusiness-unibw.org/ontologies/consumerelectronics/v1"/>
    <rdfs:label xml:lang="de">Audio Datenformat</rdfs:label>
    <rdfs:label xml:lang="en">Data Format Audio</rdfs:label>
    <belongsToModule xml:lang="en">MP3Player, DigitalCamera, Camcorder</belongsToModule>
    <rdfs:subClassOf rdf:resource="#DataFormat"/>
    <rdfs:comment xml:lang="en">A data format is a particular way to encode information for storage in a computer file (refers to audiodata).

(This description is partly based on or reuses content from the Wikipedia article "File Format" (http://en.wikipedia.org/wiki/File_format) and is licensed under the GNU Free Documentation License (http://www.gnu.org/copyleft/fdl.html).)</rdfs:comment>
  </owl:Class>
  <owl:Class rdf:ID="DisplayType">
    <belongsToModule xml:lang="en">MP3Player, TV, Printer, Camcorder</belongsToModule>
    <rdfs:isDefinedBy rdf:resource="http://www.ebusiness-unibw.org/ontologies/consumerelectronics/v1"/>
    <rdfs:subClassOf rdf:resource="http://purl.org/goodrelations/v1#QualitativeValue"/>
    <rdfs:comment xml:lang="en">A display device is an output device for presentation of information for visual, tactile or auditive reception, acquired, stored, or transmitted in various forms.

(This description is partly based on or reuses content from the Wikipedia article "Display device" (http://en.wikipedia.org/wiki/Display_device) and is licensed under the GNU Free Documentation License (http://www.gnu.org/copyleft/fdl.html).)</rdfs:comment>
    <rdfs:label xml:lang="en">Display Type</rdfs:label>
    <rdfs:label xml:lang="de">Bildschirmtyp</rdfs:label>
  </owl:Class>
  <owl:Class rdf:ID="DigitalCamera">
    <rdfs:isDefinedBy rdf:resource="http://www.ebusiness-unibw.org/ontologies/consumerelectronics/v1"/>
    <belongsToModule rdf:datatype="http://www.w3.org/2001/XMLSchema#string"
    >DigitalCamera</belongsToModule>
    <rdfs:comment xml:lang="en">A digital camera (or digicam for short) is a camera that takes video or still photographs, or both, digitally by recording images via an electronic image sensor.

(This description is partly based on or reuses content from the Wikipedia article "Digital camera" (http://en.wikipedia.org/wiki/Digital_camera) and is licensed under the GNU Free Documentation License (http://www.gnu.org/copyleft/fdl.html).)</rdfs:comment>
    <rdfs:subClassOf rdf:resource="http://purl.org/goodrelations/v1#ProductOrService"/>
    <rdfs:label xml:lang="de">Digitalkamera</rdfs:label>
    <rdfs:label xml:lang="en">Digital camera</rdfs:label>
  </owl:Class>
  <owl:Class rdf:ID="Zoom">
    <rdfs:subClassOf rdf:resource="http://purl.org/goodrelations/v1#QualitativeValue"/>
    <belongsToModule xml:lang="en">DigitalCamera, Camcorder</belongsToModule>
    <rdfs:isDefinedBy rdf:resource="http://www.ebusiness-unibw.org/ontologies/consumerelectronics/v1"/>
    <rdfs:comment xml:lang="en">Zoom is a method of decreasing (narrowing) the apparent angle of view of a photographic or video image.

(This description is partly based on or reuses content from the Wikipedia article "Digital zoom" (http://en.wikipedia.org/wiki/Digital_zoom) and is licensed under the GNU Free Documentation License (http://www.gnu.org/copyleft/fdl.html).)</rdfs:comment>
    <rdfs:label xml:lang="de">Zoom</rdfs:label>
    <rdfs:label xml:lang="en">Zoom</rdfs:label>
  </owl:Class>
  <owl:Class rdf:ID="TVTuner">
    <rdfs:label xml:lang="en">TV Tuner</rdfs:label>
    <rdfs:label xml:lang="de">TV Tuner</rdfs:label>
    <belongsToModule xml:lang="en">TV</belongsToModule>
    <rdfs:comment rdf:datatype="http://www.w3.org/2001/XMLSchema#string"
    >A television tuner converts an RF television transmission into audio and video signals which can be further processed to produce sound and a picture.

(This description is partly based on or reuses content from the Wikipedia article "Tuner (electronics)" (http://en.wikipedia.org/wiki/Tuner_(electronics)) and is licensed under the GNU Free Documentation License (http://www.gnu.org/copyleft/fdl.html).)</rdfs:comment>
    <rdfs:subClassOf rdf:resource="http://purl.org/goodrelations/v1#QualitativeValue"/>
    <rdfs:isDefinedBy rdf:resource="http://www.ebusiness-unibw.org/ontologies/consumerelectronics/v1"/>
  </owl:Class>
  <owl:Class rdf:ID="DisposableEnergySource">
    <rdfs:subClassOf rdf:resource="#EnergySource"/>
    <belongsToModule xml:lang="en">MP3Player, DigitalCamera, Camcorder</belongsToModule>
    <rdfs:isDefinedBy rdf:resource="http://www.ebusiness-unibw.org/ontologies/consumerelectronics/v1"/>
    <rdfs:comment xml:lang="en">Disposable batteries are non-rechargeable batteries. When they are out of power you have to dispose them.</rdfs:comment>
    <rdfs:label xml:lang="en">Disposable Energy Source</rdfs:label>
    <rdfs:label xml:lang="de">Einweg-Energiequelle</rdfs:label>
  </owl:Class>
  <owl:Class rdf:ID="MP3Player">
    <rdfs:isDefinedBy rdf:resource="http://www.ebusiness-unibw.org/ontologies/consumerelectronics/v1"/>
    <rdfs:subClassOf rdf:resource="http://purl.org/goodrelations/v1#ProductOrService"/>
    <rdfs:comment xml:lang="en">Playback equipment for certain data formats, especially audio data. Product is often equipped with some scope of delivery. Especially earphones, booklet, sotwareCD, charger and datacable.</rdfs:comment>
    <belongsToModule xml:lang="en">MP3Player</belongsToModule>
    <rdfs:label xml:lang="en">MP3-Player</rdfs:label>
    <rdfs:label xml:lang="de">MP3-Player</rdfs:label>
  </owl:Class>
  <owl:Class rdf:ID="MediaType">
    <rdfs:subClassOf rdf:resource="http://purl.org/goodrelations/v1#QualitativeValue"/>
    <rdfs:label rdf:datatype="http://www.w3.org/2001/XMLSchema#string"
    >Media type</rdfs:label>
    <rdfs:label xml:lang="en">Mediumart</rdfs:label>
    <rdfs:comment xml:lang="en">The type of paper a device is able to handle.</rdfs:comment>
    <belongsToModule xml:lang="en">Printer</belongsToModule>
    <rdfs:isDefinedBy rdf:resource="http://www.ebusiness-unibw.org/ontologies/consumerelectronics/v1"/>
  </owl:Class>
  <owl:Class rdf:ID="RechargeableEnergySource">
    <rdfs:subClassOf rdf:resource="#EnergySource"/>
    <rdfs:isDefinedBy rdf:resource="http://www.ebusiness-unibw.org/ontologies/consumerelectronics/v1"/>
    <belongsToModule xml:lang="en">MP3Player, DigitalCamera, Camcorder</belongsToModule>
    <rdfs:label xml:lang="de">Wiederaufladbare Energiequelle</rdfs:label>
    <rdfs:label xml:lang="en">Rechargeable Energy Source</rdfs:label>
    <rdfs:comment xml:lang="en">A rechargeable battery is a kind of energy source that is able to be reused by refilling it with a charger.</rdfs:comment>
  </owl:Class>
  <owl:Class rdf:ID="PrintResolution">
    <rdfs:label xml:lang="de">Druckauflösung</rdfs:label>
    <rdfs:label xml:lang="en">Print resolution</rdfs:label>
    <belongsToModule xml:lang="en">Printer</belongsToModule>
    <rdfs:isDefinedBy rdf:resource="http://www.ebusiness-unibw.org/ontologies/consumerelectronics/v1"/>
    <rdfs:comment xml:lang="en">Defines the maximum digital resolution the device is able to print.</rdfs:comment>
    <rdfs:subClassOf rdf:resource="#SupportedResolution"/>
  </owl:Class>
  <owl:Class rdf:ID="PhotoPrinter">
    <rdfs:subClassOf rdf:resource="#Printer"/>
    <rdfs:comment xml:lang="en">A photo printer is a printer that is specifically designed to print high quality digital photos on photo paper.

(This description is partly based on or reuses content from the Wikipedia article "Photo printer" (http://en.wikipedia.org/wiki/Photo_printer) and is licensed under the GNU Free Documentation License (http://www.gnu.org/copyleft/fdl.html).)</rdfs:comment>
    <rdfs:isDefinedBy rdf:resource="http://www.ebusiness-unibw.org/ontologies/consumerelectronics/v1"/>
    <rdfs:label xml:lang="en">Photo printer</rdfs:label>
    <rdfs:label xml:lang="de">Fotodrucker</rdfs:label>
    <belongsToModule xml:lang="en">Printer</belongsToModule>
  </owl:Class>
  <owl:Class rdf:ID="ProcessorType">
    <rdfs:label xml:lang="en">Processor type</rdfs:label>
    <rdfs:label xml:lang="de">Prozessorart</rdfs:label>
    <rdfs:subClassOf rdf:resource="http://purl.org/goodrelations/v1#QualitativeValue"/>
    <rdfs:comment xml:lang="en">The type of central processing unit (CPU) as an electronic circuit that can execute printing tasks or programs.</rdfs:comment>
    <rdfs:isDefinedBy rdf:resource="http://www.ebusiness-unibw.org/ontologies/consumerelectronics/v1"/>
    <belongsToModule xml:lang="en">Printer</belongsToModule>
  </owl:Class>
  <owl:Class rdf:ID="Focus">
    <rdfs:isDefinedBy rdf:resource="http://www.ebusiness-unibw.org/ontologies/consumerelectronics/v1"/>
    <rdfs:subClassOf rdf:resource="http://purl.org/goodrelations/v1#QualitativeValue"/>
    <rdfs:comment xml:lang="en">A focus, also called an image point, is the point where light rays originating from a point on the object converge.

(This description is partly based on or reuses content from the Wikipedia article "Focus (optics)" (http://en.wikipedia.org/wiki/Focus_(optics)) and is licensed under the GNU Free Documentation License (http://www.gnu.org/copyleft/fdl.html).)</rdfs:comment>
    <rdfs:label xml:lang="de">Fokus</rdfs:label>
    <rdfs:label xml:lang="en">Focus</rdfs:label>
    <belongsToModule xml:lang="en">DigitalCamera, Camcorder</belongsToModule>
  </owl:Class>
  <owl:Class rdf:ID="LabelPrinter">
    <belongsToModule xml:lang="en">Printer</belongsToModule>
    <rdfs:comment xml:lang="en">A label printer is a computer peripheral that prints on self-adhesive label material and sometimes card-stock (also called tags).</rdfs:comment>
    <rdfs:label xml:lang="de">Etikettendrucker</rdfs:label>
    <rdfs:label xml:lang="en">Label printer</rdfs:label>
    <rdfs:subClassOf rdf:resource="#Printer"/>
    <rdfs:isDefinedBy rdf:resource="http://www.ebusiness-unibw.org/ontologies/consumerelectronics/v1"/>
  </owl:Class>
  <owl:Class rdf:ID="SceneMode">
    <rdfs:subClassOf rdf:resource="http://purl.org/goodrelations/v1#QualitativeValue"/>
    <belongsToModule xml:lang="en">Camcorder</belongsToModule>
    <rdfs:isDefinedBy rdf:resource="http://www.ebusiness-unibw.org/ontologies/consumerelectronics/v1"/>
    <rdfs:label xml:lang="de">Szenenmodus</rdfs:label>
    <rdfs:label xml:lang="en">Scene mode</rdfs:label>
    <rdfs:comment xml:lang="en">A projection of information from any physical environment into any sensory system.</rdfs:comment>
  </owl:Class>
  <owl:Class rdf:ID="MediaFormat">
    <rdfs:label xml:lang="en">Media format</rdfs:label>
    <rdfs:label xml:lang="de">Medienformat</rdfs:label>
    <belongsToModule xml:lang="en">Printer</belongsToModule>
    <rdfs:comment xml:lang="en">Sizes and shapes of the paper.</rdfs:comment>
    <rdfs:isDefinedBy rdf:resource="http://www.ebusiness-unibw.org/ontologies/consumerelectronics/v1"/>
    <rdfs:subClassOf rdf:resource="http://purl.org/goodrelations/v1#QualitativeValue"/>
  </owl:Class>
  <owl:Class rdf:ID="TunerType">
    <belongsToModule xml:lang="en">TV</belongsToModule>
    <rdfs:isDefinedBy rdf:resource="http://www.ebusiness-unibw.org/ontologies/consumerelectronics/v1"/>
    <rdfs:label xml:lang="en">Tuner type</rdfs:label>
    <rdfs:label xml:lang="de">Tuner Typ</rdfs:label>
    <rdfs:subClassOf rdf:resource="#TVTuner"/>
    <rdfs:comment xml:lang="en">Type of TV tuner that is used to convert RF television transmissions into audio and video signals.

(This description is partly based on or reuses content from the Wikipedia article "Tuner (electronics)" (http://en.wikipedia.org/wiki/Tuner_(electronics)) and is licensed under the GNU Free Documentation License (http://www.gnu.org/copyleft/fdl.html).)</rdfs:comment>
  </owl:Class>
  <owl:Class rdf:ID="TV">
    <belongsToModule xml:lang="en">Printer</belongsToModule>
    <rdfs:comment xml:lang="en">Television (TV) is a widely used telecommunication medium for transmitting and receiving moving images, either monochromatic ("black and white") or color, usually accompanied by sound. Is often deliverd with a remote control and a manual.

(This description is partly based on or reuses content from the Wikipedia article "TV" (http://en.wikipedia.org/wiki/Tv) and is licensed under the GNU Free Documentation License (http://www.gnu.org/copyleft/fdl.html).)</rdfs:comment>
    <rdfs:isDefinedBy rdf:resource="http://www.ebusiness-unibw.org/ontologies/consumerelectronics/v1"/>
    <rdfs:subClassOf rdf:resource="http://purl.org/goodrelations/v1#ProductOrService"/>
    <rdfs:label xml:lang="en">TV</rdfs:label>
    <rdfs:label xml:lang="de">TV</rdfs:label>
  </owl:Class>
  <owl:Class rdf:ID="Features">
    <rdfs:comment xml:lang="en">Additional equipment and abilities.</rdfs:comment>
    <rdfs:isDefinedBy rdf:resource="http://www.ebusiness-unibw.org/ontologies/consumerelectronics/v1"/>
    <rdfs:subClassOf rdf:resource="http://purl.org/goodrelations/v1#QualitativeValue"/>
    <belongsToModule xml:lang="en">MP3Player, TV, DigitalCamera, Camcorder</belongsToModule>
    <rdfs:label xml:lang="en">Features</rdfs:label>
    <rdfs:label xml:lang="de">Eigenschaften</rdfs:label>
  </owl:Class>
  <owl:Class rdf:ID="Printer">
    <rdfs:isDefinedBy rdf:resource="http://www.ebusiness-unibw.org/ontologies/consumerelectronics/v1"/>
    <belongsToModule xml:lang="en">Printer</belongsToModule>
    <rdfs:subClassOf rdf:resource="http://purl.org/goodrelations/v1#ProductOrService"/>
    <rdfs:label xml:lang="en">Printer</rdfs:label>
    <rdfs:label xml:lang="de">Drucker</rdfs:label>
    <rdfs:comment xml:lang="en">A peripheral which produces a hard copy (permanent human-readable text and/or graphics) of documents stored in electronic form, usually on physical print media such as paper or transparencies.

(This description is partly based on or reuses content from the Wikipedia article "Printer" (http://en.wikipedia.org/wiki/Computer_printer) and is licensed under the GNU Free Documentation License (http://www.gnu.org/copyleft/fdl.html).)</rdfs:comment>
  </owl:Class>
  <owl:Class rdf:ID="Certificate">
    <rdfs:comment xml:lang="en">A certificate is an official document affirming some fact like quality standards.

(This description is partly based on or reuses content from the Wikipedia article "Certificate" (http://en.wikipedia.org/wiki/Certificate) and is licensed under the GNU Free Documentation License (http://www.gnu.org/copyleft/fdl.html).)</rdfs:comment>
    <rdfs:label xml:lang="en">Certificate</rdfs:label>
    <rdfs:label xml:lang="de">Zertifikat</rdfs:label>
    <belongsToModule xml:lang="en">TV</belongsToModule>
    <rdfs:isDefinedBy rdf:resource="http://www.ebusiness-unibw.org/ontologies/consumerelectronics/v1"/>
    <rdfs:subClassOf rdf:resource="http://purl.org/goodrelations/v1#QualitativeValue"/>
  </owl:Class>
  <owl:Class rdf:ID="GeneralFeatures">
    <rdfs:comment xml:lang="en">Additional general equipment and abilities.</rdfs:comment>
    <rdfs:subClassOf rdf:resource="#Features"/>
    <rdfs:label xml:lang="de">Allgemeine Eigenschaften</rdfs:label>
    <rdfs:label xml:lang="en">General Features</rdfs:label>
    <rdfs:isDefinedBy rdf:resource="http://www.ebusiness-unibw.org/ontologies/consumerelectronics/v1"/>
    <belongsToModule xml:lang="en">TV</belongsToModule>
  </owl:Class>
  <owl:Class rdf:ID="ComputerDisplayResolution">
    <rdfs:subClassOf rdf:resource="#SupportedResolution"/>
    <belongsToModule xml:lang="en">TV</belongsToModule>
    <rdfs:label xml:lang="de">Computerbildschirmauflösung</rdfs:label>
    <rdfs:label xml:lang="en">Computer display resolution</rdfs:label>
    <rdfs:comment xml:lang="en">The display resolution of a computer display typically refers to the number of distinct pixels in each dimension that can be displayed.

(This description is partly based on or reuses content from the Wikipedia article "Display resolution" (http://en.wikipedia.org/wiki/Display_resolution) and is licensed under the GNU Free Documentation License (http://www.gnu.org/copyleft/fdl.html).)</rdfs:comment>
    <rdfs:isDefinedBy rdf:resource="http://www.ebusiness-unibw.org/ontologies/consumerelectronics/v1"/>
  </owl:Class>
  <owl:Class rdf:ID="AudioInterfaceType">
    <rdfs:label xml:lang="en">Audio Interface Type</rdfs:label>
    <rdfs:label xml:lang="de">Audioschnittstellentyp</rdfs:label>
    <rdfs:comment xml:lang="en">Interface generally refers to an abstraction that an entity provides of itself to the outside (refers to audio output).

(This description is partly based on or reuses content from the Wikipedia article "Interface (computer science)" (http://en.wikipedia.org/wiki/Interface_(computer_science)) and is licensed under the GNU Free Documentation License (http://www.gnu.org/copyleft/fdl.html).)</rdfs:comment>
    <belongsToModule xml:lang="en">MP3Player</belongsToModule>
    <rdfs:subClassOf rdf:resource="http://purl.org/goodrelations/v1#QualitativeValue"/>
    <rdfs:isDefinedBy rdf:resource="http://www.ebusiness-unibw.org/ontologies/consumerelectronics/v1"/>
  </owl:Class>
  <owl:ObjectProperty rdf:ID="hasFocalLength">
    <rdfs:comment xml:lang="en">Defines a measure of how strongly it converges (focuses) or diverges (diffuses) light.

(This description is partly based on or reuses content from the Wikipedia article "Focal length" (http://en.wikipedia.org/wiki/Focal_length) and is licensed under the GNU Free Documentation License (http://www.gnu.org/copyleft/fdl.html).)</rdfs:comment>
    <rdfs:range rdf:resource="http://purl.org/goodrelations/v1#QuantitativeValueFloat"/>
    <rdfs:label xml:lang="de">Brennweite</rdfs:label>
    <rdfs:label xml:lang="en">focal length</rdfs:label>
    <rdfs:isDefinedBy rdf:resource="http://www.ebusiness-unibw.org/ontologies/consumerelectronics/v1"/>
    <belongsToModule xml:lang="en">Camcorder</belongsToModule>
    <rdfs:subPropertyOf rdf:resource="http://purl.org/goodrelations/v1#quantitativeProductOrServiceProperty"/>
  </owl:ObjectProperty>
  <owl:ObjectProperty rdf:ID="hasCompatibleOperatingSystem">
    <rdfs:isDefinedBy rdf:resource="http://www.ebusiness-unibw.org/ontologies/consumerelectronics/v1"/>
    <rdfs:comment xml:lang="en">Defines the possible external operating systems to communicate with.</rdfs:comment>
    <belongsToModule xml:lang="en">MP3Player, Printer, DigitalCamera, Camcorder</belongsToModule>
    <rdfs:label xml:lang="de">kompatibles Betriebssystem</rdfs:label>
    <rdfs:label xml:lang="en">compatible operating system</rdfs:label>
    <rdfs:range rdf:resource="#CompatibleOperatingSystems"/>
    <rdfs:subPropertyOf rdf:resource="http://purl.org/goodrelations/v1#qualitativeProductOrServiceProperty"/>
  </owl:ObjectProperty>
  <owl:ObjectProperty rdf:ID="hasPackageWeight">
    <rdfs:comment xml:lang="en">Defines the measurement of the gravitational force acting on an object with its package (Common unit of measurement gramm, GRM).</rdfs:comment>
    <belongsToModule xml:lang="en">TV</belongsToModule>
    <rdfs:label xml:lang="de">Verpackungsgewicht</rdfs:label>
    <rdfs:label xml:lang="en">package weight</rdfs:label>
    <rdfs:subPropertyOf rdf:resource="http://purl.org/goodrelations/v1#quantitativeProductOrServiceProperty"/>
    <rdfs:isDefinedBy rdf:resource="http://www.ebusiness-unibw.org/ontologies/consumerelectronics/v1"/>
    <rdfs:range rdf:resource="http://purl.org/goodrelations/v1#QuantitativeValueFloat"/>
  </owl:ObjectProperty>
  <owl:ObjectProperty rdf:ID="hasViewFinder">
    <rdfs:comment xml:lang="en">A viewfinder is what the photographer looks through to compose, and in many cases to focus, the picture.

(This description is partly based on or reuses content from the Wikipedia article "Viewfinder" (http://en.wikipedia.org/wiki/Viewfinder) and is licensed under the GNU Free Documentation License (http://www.gnu.org/copyleft/fdl.html).)</rdfs:comment>
    <rdfs:isDefinedBy rdf:resource="http://www.ebusiness-unibw.org/ontologies/consumerelectronics/v1"/>
    <rdfs:range rdf:resource="#ViewFinder"/>
    <rdfs:subPropertyOf rdf:resource="http://purl.org/goodrelations/v1#qualitativeProductOrServiceProperty"/>
    <belongsToModule xml:lang="en">DigitalCamera, Camcorder</belongsToModule>
    <rdfs:label xml:lang="de">Bildsucher</rdfs:label>
    <rdfs:label xml:lang="en">viewfinder</rdfs:label>
  </owl:ObjectProperty>
  <owl:ObjectProperty rdf:ID="hasMaxRelativeHumidity">
    <rdfs:subPropertyOf rdf:resource="http://purl.org/goodrelations/v1#quantitativeProductOrServiceProperty"/>
    <rdfs:range rdf:resource="http://purl.org/goodrelations/v1#QuantitativeValueFloat"/>
    <belongsToModule xml:lang="en">TV, Printer</belongsToModule>
    <rdfs:isDefinedBy rdf:resource="http://www.ebusiness-unibw.org/ontologies/consumerelectronics/v1"/>
    <rdfs:comment xml:lang="en">Defines the maximum level of relative humidity, non-condensing, within which the product can operate.</rdfs:comment>
    <rdfs:label xml:lang="de">maximale Luftfeuchtigkeit</rdfs:label>
    <rdfs:label xml:lang="en">max relative humidity</rdfs:label>
  </owl:ObjectProperty>
  <owl:ObjectProperty rdf:ID="hasWhiteBalance">
    <rdfs:isDefinedBy rdf:resource="http://www.ebusiness-unibw.org/ontologies/consumerelectronics/v1"/>
    <rdfs:label xml:lang="de">Weißabgleich</rdfs:label>
    <rdfs:label xml:lang="en">white balance</rdfs:label>
    <belongsToModule xml:lang="en">Camcorder</belongsToModule>
    <rdfs:range rdf:resource="#WhiteBalance"/>
    <rdfs:comment xml:lang="en">Defines the global adjustment of the intensities of the colors.</rdfs:comment>
    <rdfs:subPropertyOf rdf:resource="http://purl.org/goodrelations/v1#qualitativeProductOrServiceProperty"/>
  </owl:ObjectProperty>
  <owl:ObjectProperty rdf:ID="hasResolution">
    <rdfs:isDefinedBy rdf:resource="http://www.ebusiness-unibw.org/ontologies/consumerelectronics/v1"/>
    <rdfs:subPropertyOf rdf:resource="http://purl.org/goodrelations/v1#qualitativeProductOrServiceProperty"/>
    <belongsToModule rdf:datatype="http://www.w3.org/2001/XMLSchema#string"
    >TV</belongsToModule>
    <rdfs:comment xml:lang="en">Defines the type of resolution a screen is able to display.</rdfs:comment>
    <rdfs:label xml:lang="de">Auflösung</rdfs:label>
    <rdfs:label xml:lang="en">resolution</rdfs:label>
    <rdfs:range rdf:resource="#SupportedResolution"/>
  </owl:ObjectProperty>
  <owl:ObjectProperty rdf:ID="hasNumberOfHDMIPorts">
    <belongsToModule xml:lang="en">Camcorder</belongsToModule>
    <rdfs:range rdf:resource="http://purl.org/goodrelations/v1#QuantitativeValueInteger"/>
    <rdfs:label xml:lang="de">Anzahl HDMI Anschlussmöglichkeiten</rdfs:label>
    <rdfs:label xml:lang="en">number of HDMI ports</rdfs:label>
    <rdfs:isDefinedBy rdf:resource="http://www.ebusiness-unibw.org/ontologies/consumerelectronics/v1"/>
    <rdfs:subPropertyOf rdf:resource="http://purl.org/goodrelations/v1#quantitativeProductOrServiceProperty"/>
    <rdfs:comment xml:lang="en">Number of compact audio/video interface ports for transmitting uncompressed digital data.</rdfs:comment>
  </owl:ObjectProperty>
  <owl:ObjectProperty rdf:ID="hasUSBPortsQuantity">
    <belongsToModule xml:lang="en">Camcorder</belongsToModule>
    <rdfs:range rdf:resource="http://purl.org/goodrelations/v1#QuantitativeValueInteger"/>
    <rdfs:label xml:lang="de">Anzahl USB Anschlussmöglichkeiten</rdfs:label>
    <rdfs:label xml:lang="en">number of USB ports</rdfs:label>
    <rdfs:isDefinedBy rdf:resource="http://www.ebusiness-unibw.org/ontologies/consumerelectronics/v1"/>
    <rdfs:subPropertyOf rdf:resource="http://purl.org/goodrelations/v1#quantitativeProductOrServiceProperty"/>
    <rdfs:comment xml:lang="en">Number of serial bus standard ports to connect devices to a host computer.</rdfs:comment>
  </owl:ObjectProperty>
  <owl:ObjectProperty rdf:ID="hasSpeakerQuantity">
    <belongsToModule xml:lang="en">TV</belongsToModule>
    <rdfs:range rdf:resource="http://purl.org/goodrelations/v1#QuantitativeValueInteger"/>
    <rdfs:label xml:lang="de">Anzahl an Lautsprecher</rdfs:label>
    <rdfs:label xml:lang="en">speaker quantity</rdfs:label>
    <rdfs:isDefinedBy rdf:resource="http://www.ebusiness-unibw.org/ontologies/consumerelectronics/v1"/>
    <rdfs:subPropertyOf rdf:resource="http://purl.org/goodrelations/v1#quantitativeProductOrServiceProperty"/>
    <rdfs:comment xml:lang="en">Defines the number of integrated speakers an object includes.</rdfs:comment>
  </owl:ObjectProperty>
  <owl:ObjectProperty rdf:ID="hasMinRelativeHumidity">
    <rdfs:isDefinedBy rdf:resource="http://www.ebusiness-unibw.org/ontologies/consumerelectronics/v1"/>
    <rdfs:range rdf:resource="http://purl.org/goodrelations/v1#QuantitativeValueFloat"/>
    <belongsToModule xml:lang="en">TV, Printer</belongsToModule>
    <rdfs:label xml:lang="de">minimale Luftfeuchtigkeit</rdfs:label>
    <rdfs:label xml:lang="en">min relative humidity</rdfs:label>
    <rdfs:subPropertyOf rdf:resource="http://purl.org/goodrelations/v1#quantitativeProductOrServiceProperty"/>
    <rdfs:comment xml:lang="en">Defines the minimum level of relative humidity, non-condensing, within which the product can operate.</rdfs:comment>
  </owl:ObjectProperty>
  <owl:ObjectProperty rdf:ID="hasMaxBlackWhitePrintSpeedBestQuality">
    <rdfs:comment xml:lang="en">Amount of pages per minute the product is able to print in the mode of black-printig best quality.</rdfs:comment>
    <rdfs:subPropertyOf rdf:resource="http://purl.org/goodrelations/v1#quantitativeProductOrServiceProperty"/>
    <rdfs:label xml:lang="de">maximale Druckgeschwindigkeit Schwarz/Weiß beste Qualität</rdfs:label>
    <rdfs:label xml:lang="en">max black white print speed best quality</rdfs:label>
    <rdfs:isDefinedBy rdf:resource="http://www.ebusiness-unibw.org/ontologies/consumerelectronics/v1"/>
    <rdfs:range rdf:resource="http://purl.org/goodrelations/v1#QuantitativeValueFloat"/>
    <belongsToModule xml:lang="en">Printer</belongsToModule>
  </owl:ObjectProperty>
  <owl:ObjectProperty rdf:ID="hasChannelQuantity">
    <rdfs:subPropertyOf rdf:resource="http://purl.org/goodrelations/v1#quantitativeProductOrServiceProperty"/>
    <rdfs:range rdf:resource="http://purl.org/goodrelations/v1#QuantitativeValueInteger"/>
    <rdfs:comment xml:lang="en">Defines the number of channels of a television that can be used to save specific transmitted signals.</rdfs:comment>
    <rdfs:label xml:lang="de">Anzahl von Kanäle</rdfs:label>
    <rdfs:label xml:lang="en">channel quantity</rdfs:label>
    <belongsToModule xml:lang="en">TV</belongsToModule>
    <rdfs:isDefinedBy rdf:resource="http://www.ebusiness-unibw.org/ontologies/consumerelectronics/v1"/>
  </owl:ObjectProperty>
  <owl:ObjectProperty rdf:ID="hasMaxPrintCapacity">
    <rdfs:range rdf:resource="http://purl.org/goodrelations/v1#QuantitativeValueInteger"/>
    <rdfs:isDefinedBy rdf:resource="http://www.ebusiness-unibw.org/ontologies/consumerelectronics/v1"/>
    <rdfs:subPropertyOf rdf:resource="http://purl.org/goodrelations/v1#quantitativeProductOrServiceProperty"/>
    <rdfs:label xml:lang="de">maximale Druckkapazität</rdfs:label>
    <rdfs:label xml:lang="en">max print capacity</rdfs:label>
    <belongsToModule xml:lang="en">Printer</belongsToModule>
    <rdfs:comment xml:lang="en">Describes the maximum printed sites per month.</rdfs:comment>
  </owl:ObjectProperty>
  <owl:ObjectProperty rdf:ID="hasSwivel">
    <rdfs:isDefinedBy rdf:resource="http://www.ebusiness-unibw.org/ontologies/consumerelectronics/v1"/>
    <rdfs:range rdf:resource="http://purl.org/goodrelations/v1#QuantitativeValueFloat"/>
    <rdfs:subPropertyOf rdf:resource="http://purl.org/goodrelations/v1#quantitativeProductOrServiceProperty"/>
    <rdfs:label xml:lang="de">Schwenkarm</rdfs:label>
    <rdfs:label xml:lang="en">swivel</rdfs:label>
    <rdfs:comment xml:lang="en">Defines the possibilty to rotate or turn an object into different directions (Common unit of measurement degree, DD).</rdfs:comment>
    <belongsToModule xml:lang="en">TV</belongsToModule>
  </owl:ObjectProperty>
  <owl:ObjectProperty rdf:ID="hasMaxPrintableResolutionBlackWhiteVertical">
    <rdfs:label xml:lang="en">max printable resolution black white vertical</rdfs:label>
    <rdfs:label xml:lang="de">maximale vertikale druckbare Auflösung Schwarz/Weiß</rdfs:label>
    <rdfs:comment xml:lang="en">Defines the maximum digital resolution of the vertical axe (Common unit of measurement pixel, E37) for black/white prints.</rdfs:comment>
    <rdfs:subPropertyOf rdf:resource="http://purl.org/goodrelations/v1#quantitativeProductOrServiceProperty"/>
    <belongsToModule xml:lang="en">Printer</belongsToModule>
    <rdfs:range rdf:resource="http://purl.org/goodrelations/v1#QuantitativeValueInteger"/>
    <rdfs:isDefinedBy rdf:resource="http://www.ebusiness-unibw.org/ontologies/consumerelectronics/v1"/>
  </owl:ObjectProperty>
  <owl:ObjectProperty rdf:ID="hasWarmupTime">
    <belongsToModule xml:lang="en">Printer</belongsToModule>
    <rdfs:isDefinedBy rdf:resource="http://www.ebusiness-unibw.org/ontologies/consumerelectronics/v1"/>
    <rdfs:range rdf:resource="http://purl.org/goodrelations/v1#QuantitativeValueFloat"/>
    <rdfs:comment xml:lang="en">Defines the amount of time the device needs to be ready.</rdfs:comment>
    <rdfs:label xml:lang="de">Warmlaufzeit</rdfs:label>
    <rdfs:label xml:lang="en">warmup time</rdfs:label>
    <rdfs:subPropertyOf rdf:resource="http://purl.org/goodrelations/v1#quantitativeProductOrServiceProperty"/>
  </owl:ObjectProperty>
  <owl:ObjectProperty rdf:ID="hasApertureRange">
    <rdfs:comment xml:lang="en">Defines the hole or an opening through which light is admitted.</rdfs:comment>
    <rdfs:range rdf:resource="http://purl.org/goodrelations/v1#QuantitativeValueFloat"/>
    <rdfs:isDefinedBy rdf:resource="http://www.ebusiness-unibw.org/ontologies/consumerelectronics/v1"/>
    <belongsToModule xml:lang="en">Camcorder</belongsToModule>
    <rdfs:subPropertyOf rdf:resource="http://purl.org/goodrelations/v1#quantitativeProductOrServiceProperty"/>
    <rdfs:label xml:lang="de">Blendenbereich</rdfs:label>
    <rdfs:label xml:lang="en">aperture range</rdfs:label>
  </owl:ObjectProperty>
  <owl:ObjectProperty rdf:ID="hasWeight">
    <rdfs:range rdf:resource="http://purl.org/goodrelations/v1#QuantitativeValueFloat"/>
    <rdfs:label xml:lang="de">Gewicht</rdfs:label>
    <rdfs:label xml:lang="en">weight</rdfs:label>
    <rdfs:comment xml:lang="en">Defines the measurement of the gravitational force acting on an object (Common unit of measurement gramm, GRM).</rdfs:comment>
    <belongsToModule xml:lang="en">MP3Player, TV, Printer, DigitalCamera, Camcorder</belongsToModule>
    <rdfs:subPropertyOf rdf:resource="http://purl.org/goodrelations/v1#quantitativeProductOrServiceProperty"/>
    <rdfs:isDefinedBy rdf:resource="http://www.ebusiness-unibw.org/ontologies/consumerelectronics/v1"/>
  </owl:ObjectProperty>
  <owl:ObjectProperty rdf:ID="hasPhotographicFilterSize">
    <belongsToModule xml:lang="en">Camcorder</belongsToModule>
    <rdfs:comment xml:lang="en">Size of a camera accessory consisting of an optical filter that can be inserted in the optical path.

(This description is partly based on or reuses content from the Wikipedia article "Photographic filter" (http://en.wikipedia.org/wiki/Photographic_filter) and is licensed under the GNU Free Documentation License (http://www.gnu.org/copyleft/fdl.html).)</rdfs:comment>
    <rdfs:range rdf:resource="http://purl.org/goodrelations/v1#QuantitativeValueFloat"/>
    <rdfs:isDefinedBy rdf:resource="http://www.ebusiness-unibw.org/ontologies/consumerelectronics/v1"/>
    <rdfs:label xml:lang="de">Filtergröße</rdfs:label>
    <rdfs:label xml:lang="en">filter size</rdfs:label>
    <rdfs:subPropertyOf rdf:resource="http://purl.org/goodrelations/v1#quantitativeProductOrServiceProperty"/>
  </owl:ObjectProperty>
  <owl:ObjectProperty rdf:ID="hasMaxBlackWhitePrintSpeedNormal">
    <belongsToModule xml:lang="en">Printer</belongsToModule>
    <rdfs:range rdf:resource="http://purl.org/goodrelations/v1#QuantitativeValueFloat"/>
    <rdfs:subPropertyOf rdf:resource="http://purl.org/goodrelations/v1#quantitativeProductOrServiceProperty"/>
    <rdfs:comment xml:lang="en">Amount of pages per minute the product is able to print in the mode of black-printig normal quality.</rdfs:comment>
    <rdfs:isDefinedBy rdf:resource="http://www.ebusiness-unibw.org/ontologies/consumerelectronics/v1"/>
    <rdfs:label xml:lang="de">maximale Druckgeschwindigkeit Schwarz/Weiß normal</rdfs:label>
    <rdfs:label xml:lang="en">max black white print speed draft</rdfs:label>
  </owl:ObjectProperty>
  <owl:ObjectProperty rdf:ID="hasMinIllumination">
    <rdfs:comment xml:lang="en">Minimum deliberate application of light to achieve some aesthetic or practical effect (common unit of measurement: Lux; LUX).</rdfs:comment>
    <rdfs:label xml:lang="de">minimale Belichtung</rdfs:label>
    <rdfs:label xml:lang="en">min illumination</rdfs:label>
    <belongsToModule xml:lang="en">Camcorder</belongsToModule>
    <rdfs:subPropertyOf rdf:resource="http://purl.org/goodrelations/v1#quantitativeProductOrServiceProperty"/>
    <rdfs:isDefinedBy rdf:resource="http://www.ebusiness-unibw.org/ontologies/consumerelectronics/v1"/>
    <rdfs:range rdf:resource="http://purl.org/goodrelations/v1#QuantitativeValueFloat"/>
  </owl:ObjectProperty>
  <owl:ObjectProperty rdf:ID="hasProcessorClockSpeed">
    <rdfs:comment xml:lang="en">Defines the frequency of the clock in any synchronous circuit (common unit of measurement: hertz, HTZ).</rdfs:comment>
    <rdfs:subPropertyOf rdf:resource="http://purl.org/goodrelations/v1#quantitativeProductOrServiceProperty"/>
    <rdfs:isDefinedBy rdf:resource="http://www.ebusiness-unibw.org/ontologies/consumerelectronics/v1"/>
    <belongsToModule xml:lang="en">Printer</belongsToModule>
    <rdfs:label xml:lang="de">Prozessortaktrate</rdfs:label>
    <rdfs:label xml:lang="en">processor clock speed</rdfs:label>
    <rdfs:range rdf:resource="http://purl.org/goodrelations/v1#QuantitativeValueFloat"/>
  </owl:ObjectProperty>
  <owl:ObjectProperty rdf:ID="hasMaxMediaWeight">
    <rdfs:label xml:lang="de">maximales Mediengewicht</rdfs:label>
    <rdfs:label xml:lang="en">max media weight</rdfs:label>
    <rdfs:subPropertyOf rdf:resource="http://purl.org/goodrelations/v1#quantitativeProductOrServiceProperty"/>
    <rdfs:comment xml:lang="en">Describes the maximum weight of the media format (Common unit of measurement gram per square metre, GM).</rdfs:comment>
    <rdfs:isDefinedBy rdf:resource="http://www.ebusiness-unibw.org/ontologies/consumerelectronics/v1"/>
    <belongsToModule xml:lang="en">Printer</belongsToModule>
    <rdfs:range rdf:resource="http://purl.org/goodrelations/v1#QuantitativeValueFloat"/>
  </owl:ObjectProperty>
  <owl:ObjectProperty rdf:ID="hasMinMediaWeight">
    <rdfs:comment xml:lang="en">Describes the minimum weight of the media format (Common unit of measurement gram per square metre, GM).</rdfs:comment>
    <rdfs:isDefinedBy rdf:resource="http://www.ebusiness-unibw.org/ontologies/consumerelectronics/v1"/>
    <rdfs:range rdf:resource="http://purl.org/goodrelations/v1#QuantitativeValueFloat"/>
    <rdfs:subPropertyOf rdf:resource="http://purl.org/goodrelations/v1#quantitativeProductOrServiceProperty"/>
    <belongsToModule xml:lang="en">Printer</belongsToModule>
    <rdfs:label xml:lang="de">minimales Mediengewicht</rdfs:label>
    <rdfs:label xml:lang="en">min media weight</rdfs:label>
  </owl:ObjectProperty>
  <owl:ObjectProperty rdf:ID="hasConnectivity">
    <belongsToModule xml:lang="en">TV</belongsToModule>
    <rdfs:subPropertyOf rdf:resource="http://purl.org/goodrelations/v1#qualitativeProductOrServiceProperty"/>
    <rdfs:isDefinedBy rdf:resource="http://www.ebusiness-unibw.org/ontologies/consumerelectronics/v1"/>
    <rdfs:range rdf:resource="#Connectivity"/>
    <rdfs:comment xml:lang="en">Defines the possibilities to connect different kinds of electronical devices.</rdfs:comment>
    <rdfs:label xml:lang="de">Verbindungsmöglichkeit</rdfs:label>
    <rdfs:label xml:lang="en">connectivity</rdfs:label>
  </owl:ObjectProperty>
  <owl:ObjectProperty rdf:ID="hasViewingAngleVertical">
    <rdfs:comment xml:lang="en">Defines the angle in a vertical axe where a viewer is still able to see the picture on a screen (Common unit of measurement degree, DD).</rdfs:comment>
    <belongsToModule xml:lang="en">TV</belongsToModule>
    <rdfs:isDefinedBy rdf:resource="http://www.ebusiness-unibw.org/ontologies/consumerelectronics/v1"/>
    <rdfs:subPropertyOf rdf:resource="http://purl.org/goodrelations/v1#quantitativeProductOrServiceProperty"/>
    <rdfs:range rdf:resource="http://purl.org/goodrelations/v1#QuantitativeValueFloat"/>
    <rdfs:label xml:lang="de">vertikaler Betrachtungswinkel</rdfs:label>
    <rdfs:label xml:lang="en">viewing angle vertical</rdfs:label>
  </owl:ObjectProperty>
  <owl:ObjectProperty rdf:ID="hasDataFormat">
    <rdfs:label xml:lang="de">Datenformat</rdfs:label>
    <rdfs:label xml:lang="en">data format</rdfs:label>
    <rdfs:isDefinedBy rdf:resource="http://www.ebusiness-unibw.org/ontologies/consumerelectronics/v1"/>
    <rdfs:range rdf:resource="#DataFormat"/>
    <rdfs:comment xml:lang="en">Defines the supported data formats.</rdfs:comment>
    <rdfs:subPropertyOf rdf:resource="http://purl.org/goodrelations/v1#qualitativeProductOrServiceProperty"/>
    <belongsToModule xml:lang="en">MP3Player, DigitalCamera, Camcorder</belongsToModule>
  </owl:ObjectProperty>
  <owl:ObjectProperty rdf:ID="hasMaxColorPrintSpeedDraft">
    <rdfs:subPropertyOf rdf:resource="http://purl.org/goodrelations/v1#quantitativeProductOrServiceProperty"/>
    <rdfs:range rdf:resource="http://purl.org/goodrelations/v1#QuantitativeValueFloat"/>
    <rdfs:comment xml:lang="en">Amount of pages per minute the product is able to print in the mode of color-printig of drafts.</rdfs:comment>
    <rdfs:isDefinedBy rdf:resource="http://www.ebusiness-unibw.org/ontologies/consumerelectronics/v1"/>
    <belongsToModule xml:lang="en">Printer</belongsToModule>
    <rdfs:label xml:lang="de">maximale Druckgeschwindigkeit Farbe Entwurf</rdfs:label>
    <rdfs:label xml:lang="en">max color print speed draft</rdfs:label>
  </owl:ObjectProperty>
  <owl:ObjectProperty rdf:ID="hasMediaWeightTray2">
    <rdfs:comment xml:lang="en">Describes the weight of the media format (Common unit of measurement gram per square metre, GM) hold in tray 2.</rdfs:comment>
    <rdfs:subPropertyOf rdf:resource="http://purl.org/goodrelations/v1#quantitativeProductOrServiceProperty"/>
    <rdfs:label xml:lang="de">Mediengewicht Kassette 1</rdfs:label>
    <rdfs:label xml:lang="en">media weight tray 2</rdfs:label>
    <rdfs:isDefinedBy rdf:resource="http://www.ebusiness-unibw.org/ontologies/consumerelectronics/v1"/>
    <rdfs:range rdf:resource="http://purl.org/goodrelations/v1#QuantitativeValueFloat"/>
    <belongsToModule xml:lang="en">Printer</belongsToModule>
  </owl:ObjectProperty>
  <owl:ObjectProperty rdf:ID="hasStandardOutputCapacity">
    <rdfs:isDefinedBy rdf:resource="http://www.ebusiness-unibw.org/ontologies/consumerelectronics/v1"/>
    <rdfs:subPropertyOf rdf:resource="http://purl.org/goodrelations/v1#quantitativeProductOrServiceProperty"/>
    <rdfs:label xml:lang="de">Standard Ausgabkapazität</rdfs:label>
    <rdfs:label xml:lang="en">standard output capacity</rdfs:label>
    <rdfs:comment xml:lang="en">Number of sheets the product can hold in all available output trays as a standard.</rdfs:comment>
    <rdfs:range rdf:resource="http://purl.org/goodrelations/v1#QuantitativeValueInteger"/>
  </owl:ObjectProperty>
  <owl:ObjectProperty rdf:ID="hasOutputPower">
    <rdfs:comment xml:lang="en">Defines the rate of energy conversion (Common unit of Measurement milliwatt, C31).</rdfs:comment>
    <belongsToModule xml:lang="en">MP3Player, Printer</belongsToModule>
    <rdfs:subPropertyOf rdf:resource="http://purl.org/goodrelations/v1#quantitativeProductOrServiceProperty"/>
    <rdfs:isDefinedBy rdf:resource="http://www.ebusiness-unibw.org/ontologies/consumerelectronics/v1"/>
    <rdfs:label xml:lang="de">Ausgangsleistung</rdfs:label>
    <rdfs:label xml:lang="en">output power</rdfs:label>
    <rdfs:range rdf:resource="http://purl.org/goodrelations/v1#QuantitativeValueFloat"/>
  </owl:ObjectProperty>
  <owl:ObjectProperty rdf:ID="hasSoundEmission">
    <rdfs:isDefinedBy rdf:resource="http://www.ebusiness-unibw.org/ontologies/consumerelectronics/v1"/>
    <rdfs:subPropertyOf rdf:resource="http://purl.org/goodrelations/v1#quantitativeProductOrServiceProperty"/>
    <rdfs:range rdf:resource="http://purl.org/goodrelations/v1#QuantitativeValueFloat"/>
    <belongsToModule xml:lang="en">Printer</belongsToModule>
    <rdfs:comment xml:lang="en">Level of sound power during the printing (Common unit of measurement decibel, 2N).</rdfs:comment>
    <rdfs:label xml:lang="de">Geräuschentwicklung</rdfs:label>
    <rdfs:label xml:lang="en">sound emission</rdfs:label>
  </owl:ObjectProperty>
  <owl:ObjectProperty rdf:ID="hasPowerRequirementsAC">
    <rdfs:isDefinedBy rdf:resource="http://www.ebusiness-unibw.org/ontologies/consumerelectronics/v1"/>
    <rdfs:label xml:lang="de">Strombedarf AC</rdfs:label>
    <rdfs:label xml:lang="en">power requirements AC</rdfs:label>
    <rdfs:range rdf:resource="http://purl.org/goodrelations/v1#QuantitativeValueFloat"/>
    <rdfs:comment xml:lang="en">Defines the requirements of power an electronical device needs to operate (Common unit of measurement Ampere, AMP).</rdfs:comment>
    <belongsToModule xml:lang="en">TV</belongsToModule>
    <rdfs:subPropertyOf rdf:resource="http://purl.org/goodrelations/v1#quantitativeProductOrServiceProperty"/>
  </owl:ObjectProperty>
  <owl:ObjectProperty rdf:ID="hasDataInterfaceType">
    <rdfs:isDefinedBy rdf:resource="http://www.ebusiness-unibw.org/ontologies/consumerelectronics/v1"/>
    <rdfs:comment xml:lang="en">Defines the type of interfaces used to exchange data.</rdfs:comment>
    <rdfs:subPropertyOf rdf:resource="http://purl.org/goodrelations/v1#qualitativeProductOrServiceProperty"/>
    <rdfs:label xml:lang="de">Datenschnittstellentyp</rdfs:label>
    <rdfs:label xml:lang="en">data interface type</rdfs:label>
    <belongsToModule xml:lang="en">MP3Player, DigitalCamera, Camcorder</belongsToModule>
    <rdfs:range rdf:resource="#DataInterfaceType"/>
  </owl:ObjectProperty>
  <owl:ObjectProperty rdf:ID="hasNumberOfPrintCartridges">
    <rdfs:label xml:lang="de">Anzahl von Druckerkassetten</rdfs:label>
    <rdfs:label xml:lang="en">number of print cartridges</rdfs:label>
    <rdfs:comment xml:lang="en">Number of replaceable components of a printer that contains the ink that is spread on paper during printing.</rdfs:comment>
    <rdfs:range rdf:resource="http://purl.org/goodrelations/v1#QuantitativeValueInteger"/>
    <rdfs:isDefinedBy rdf:resource="http://www.ebusiness-unibw.org/ontologies/consumerelectronics/v1"/>
    <rdfs:subPropertyOf rdf:resource="http://purl.org/goodrelations/v1#quantitativeProductOrServiceProperty"/>
    <belongsToModule xml:lang="en">Printer</belongsToModule>
  </owl:ObjectProperty>
  <owl:ObjectProperty rdf:ID="hasPrintBorderTop">
    <rdfs:label xml:lang="de">Druckgrenze oben</rdfs:label>
    <rdfs:label xml:lang="en">print border top</rdfs:label>
    <rdfs:range rdf:resource="http://purl.org/goodrelations/v1#QuantitativeValueFloat"/>
    <rdfs:subPropertyOf rdf:resource="http://purl.org/goodrelations/v1#quantitativeProductOrServiceProperty"/>
    <belongsToModule xml:lang="en">Printer</belongsToModule>
    <rdfs:comment xml:lang="en">Defines the area which can not be printed on the top side of a paper (A4) (Common unit of measurement millimetre, MMT).</rdfs:comment>
    <rdfs:isDefinedBy rdf:resource="http://www.ebusiness-unibw.org/ontologies/consumerelectronics/v1"/>
  </owl:ObjectProperty>
  <owl:ObjectProperty rdf:ID="hasDurationToPrintFirstPage">
    <belongsToModule xml:lang="en">Printer</belongsToModule>
    <rdfs:isDefinedBy rdf:resource="http://www.ebusiness-unibw.org/ontologies/consumerelectronics/v1"/>
    <rdfs:label xml:lang="de">Zeitspanne bis Druck erster Seite</rdfs:label>
    <rdfs:label xml:lang="en">duration to print first page</rdfs:label>
    <rdfs:comment xml:lang="en">Amount of time the printer needs to start printing the first page.</rdfs:comment>
    <rdfs:subPropertyOf rdf:resource="http://purl.org/goodrelations/v1#quantitativeProductOrServiceProperty"/>
    <rdfs:range rdf:resource="http://purl.org/goodrelations/v1#QuantitativeValueFloat"/>
  </owl:ObjectProperty>
  <owl:ObjectProperty rdf:ID="hasMaxPrintableResolutionColorVertical">
    <rdfs:comment xml:lang="en">Defines the maximum digital resolution of the vertical axe (Common unit of measurement pixel, E37)  for color prints.</rdfs:comment>
    <rdfs:range rdf:resource="http://purl.org/goodrelations/v1#QuantitativeValueInteger"/>
    <rdfs:isDefinedBy rdf:resource="http://www.ebusiness-unibw.org/ontologies/consumerelectronics/v1"/>
    <belongsToModule xml:lang="en">Printer</belongsToModule>
    <rdfs:label xml:lang="de">maximale vertikale druckbare Auflösung Farbe</rdfs:label>
    <rdfs:label xml:lang="en">max printable resolution color vertical</rdfs:label>
    <rdfs:subPropertyOf rdf:resource="http://purl.org/goodrelations/v1#quantitativeProductOrServiceProperty"/>
  </owl:ObjectProperty>
  <owl:ObjectProperty rdf:ID="hasMaxOutputCapacity">
    <rdfs:range rdf:resource="http://purl.org/goodrelations/v1#QuantitativeValueInteger"/>
    <belongsToModule xml:lang="en">Printer</belongsToModule>
    <rdfs:comment xml:lang="en">Maximum number of sheets the product can hold in all available standard and optional output trays.</rdfs:comment>
    <rdfs:isDefinedBy rdf:resource="http://www.ebusiness-unibw.org/ontologies/consumerelectronics/v1"/>
    <rdfs:subPropertyOf rdf:resource="http://purl.org/goodrelations/v1#quantitativeProductOrServiceProperty"/>
    <rdfs:label xml:lang="de">maximale Größe Ausgabefach</rdfs:label>
    <rdfs:label xml:lang="en">max output capacity</rdfs:label>
  </owl:ObjectProperty>
  <owl:ObjectProperty rdf:ID="hasNormalPrintableResolutionColorHorizontal">
    <rdfs:subPropertyOf rdf:resource="http://purl.org/goodrelations/v1#quantitativeProductOrServiceProperty"/>
    <belongsToModule xml:lang="en">Printer</belongsToModule>
    <rdfs:comment xml:lang="en">Defines the digital resolution of the horizontal axe (Common unit of measurement pixel, E37) for color prints for normal prints.</rdfs:comment>
    <rdfs:label xml:lang="de">horizontale druckbare Auflösung Farbe normal</rdfs:label>
    <rdfs:label xml:lang="en">normal printable resolution color horizontal</rdfs:label>
    <rdfs:isDefinedBy rdf:resource="http://www.ebusiness-unibw.org/ontologies/consumerelectronics/v1"/>
    <rdfs:range rdf:resource="http://purl.org/goodrelations/v1#QuantitativeValueInteger"/>
  </owl:ObjectProperty>
  <owl:ObjectProperty rdf:ID="hasStorageMedia">
    <rdfs:comment xml:lang="en">Defines the type of storage media the object uses to store data.</rdfs:comment>
    <rdfs:range rdf:resource="#StorageMedia"/>
    <rdfs:subPropertyOf rdf:resource="http://purl.org/goodrelations/v1#qualitativeProductOrServiceProperty"/>
    <rdfs:isDefinedBy rdf:resource="http://www.ebusiness-unibw.org/ontologies/consumerelectronics/v1"/>
    <rdfs:label xml:lang="de">Speichermedium</rdfs:label>
    <rdfs:label xml:lang="en">storage media</rdfs:label>
    <belongsToModule xml:lang="en">MP3Player, DigitalCamera, Camcorder</belongsToModule>
  </owl:ObjectProperty>
  <owl:ObjectProperty rdf:ID="hasHeightWithStand">
    <belongsToModule xml:lang="en">TV</belongsToModule>
    <rdfs:isDefinedBy rdf:resource="http://www.ebusiness-unibw.org/ontologies/consumerelectronics/v1"/>
    <rdfs:range rdf:resource="http://purl.org/goodrelations/v1#QuantitativeValueFloat"/>
    <rdfs:comment xml:lang="en">Defines the measurement of vertical distance of an object with its stand (Common unit of measurement centimetre, CMT).</rdfs:comment>
    <rdfs:subPropertyOf rdf:resource="http://purl.org/goodrelations/v1#quantitativeProductOrServiceProperty"/>
    <rdfs:label xml:lang="de">Höhe mit Standfuß</rdfs:label>
    <rdfs:label xml:lang="en">height with stand</rdfs:label>
  </owl:ObjectProperty>
  <owl:ObjectProperty rdf:ID="hasDepth">
    <belongsToModule xml:lang="en">MP3Player, TV, Printer, DigitalCamera, Camcorder</belongsToModule>
    <rdfs:comment xml:lang="en">Defines the distance from side to side, measuring across the object at right angles to the width (Common unit of measurement centimetre, CMT).

(This description is partly based on or reuses content from the Wikipedia article "Length" (http://en.wikipedia.org/wiki/Length) and is licensed under the GNU Free Documentation License (http://www.gnu.org/copyleft/fdl.html).)</rdfs:comment>
    <rdfs:subPropertyOf rdf:resource="http://purl.org/goodrelations/v1#quantitativeProductOrServiceProperty"/>
    <rdfs:range rdf:resource="http://purl.org/goodrelations/v1#QuantitativeValueFloat"/>
    <rdfs:isDefinedBy rdf:resource="http://www.ebusiness-unibw.org/ontologies/consumerelectronics/v1"/>
    <rdfs:label xml:lang="de">Tiefe</rdfs:label>
    <rdfs:label xml:lang="en">depth</rdfs:label>
  </owl:ObjectProperty>
  <owl:ObjectProperty rdf:ID="hasPictureResolution">
    <rdfs:isDefinedBy rdf:resource="http://www.ebusiness-unibw.org/ontologies/consumerelectronics/v1"/>
    <rdfs:subPropertyOf rdf:resource="http://purl.org/goodrelations/v1#quantitativeProductOrServiceProperty"/>
    <belongsToModule xml:lang="en">DigitalCamera, Camcorder</belongsToModule>
    <rdfs:comment xml:lang="en">Defines the digital resolution of the pictures (Common unit of measurement pixel, E37).</rdfs:comment>
    <rdfs:label xml:lang="de">Fotoauflösung</rdfs:label>
    <rdfs:label xml:lang="en">picture resolution</rdfs:label>
    <rdfs:range rdf:resource="http://purl.org/goodrelations/v1#QuantitativeValueFloat"/>
  </owl:ObjectProperty>
  <owl:ObjectProperty rdf:ID="hasMediaWeightTray1">
    <rdfs:comment xml:lang="en">Describes the weight of the media format (Common unit of measurement gram per square metre, GM) hold in tray 1.</rdfs:comment>
    <rdfs:range rdf:resource="http://purl.org/goodrelations/v1#QuantitativeValueFloat"/>
    <rdfs:label xml:lang="de">Mediengewicht Kassette 1</rdfs:label>
    <rdfs:label xml:lang="en">media weight tray 1</rdfs:label>
    <rdfs:subPropertyOf rdf:resource="http://purl.org/goodrelations/v1#quantitativeProductOrServiceProperty"/>
    <belongsToModule xml:lang="en">Printer</belongsToModule>
    <rdfs:isDefinedBy rdf:resource="http://www.ebusiness-unibw.org/ontologies/consumerelectronics/v1"/>
  </owl:ObjectProperty>
  <owl:ObjectProperty rdf:ID="hasOperatingTime">
    <rdfs:comment xml:lang="en">Average time the object operates (Common unit of measurement hour, HUR).</rdfs:comment>
    <rdfs:label xml:lang="de">Betriebsdauer</rdfs:label>
    <rdfs:label xml:lang="en">operating time</rdfs:label>
    <belongsToModule xml:lang="en">MP3Player, DigitalCamera, Camcorder</belongsToModule>
    <rdfs:isDefinedBy rdf:resource="http://www.ebusiness-unibw.org/ontologies/consumerelectronics/v1"/>
    <rdfs:range rdf:resource="http://purl.org/goodrelations/v1#QuantitativeValueFloat"/>
    <rdfs:subPropertyOf rdf:resource="http://purl.org/goodrelations/v1#quantitativeProductOrServiceProperty"/>
  </owl:ObjectProperty>
  <owl:ObjectProperty rdf:ID="hasMinOperatingTemperature">
    <rdfs:range rdf:resource="http://purl.org/goodrelations/v1#QuantitativeValueFloat"/>
    <rdfs:label xml:lang="de">minimale Betriebstemperatur</rdfs:label>
    <rdfs:label xml:lang="en">min operating temperature</rdfs:label>
    <rdfs:comment xml:lang="en">Defines the minimum temperature the product is able to operate (Common unit of measurement grad celsius, CEL).</rdfs:comment>
    <belongsToModule xml:lang="en">TV, Printer</belongsToModule>
    <rdfs:subPropertyOf rdf:resource="http://purl.org/goodrelations/v1#quantitativeProductOrServiceProperty"/>
    <rdfs:isDefinedBy rdf:resource="http://www.ebusiness-unibw.org/ontologies/consumerelectronics/v1"/>
  </owl:ObjectProperty>
  <owl:ObjectProperty rdf:ID="hasSensorType">
    <rdfs:comment xml:lang="en">Defines type of device that measures a physical quantity and converts it into a signal which can be read by an observer or by an instrument.</rdfs:comment>
    <rdfs:subPropertyOf rdf:resource="http://purl.org/goodrelations/v1#qualitativeProductOrServiceProperty"/>
    <rdfs:range rdf:resource="#SensorType"/>
    <belongsToModule xml:lang="en">Camcorder</belongsToModule>
    <rdfs:label xml:lang="de">Sensorart</rdfs:label>
    <rdfs:label xml:lang="en">sensor type</rdfs:label>
    <rdfs:isDefinedBy rdf:resource="http://www.ebusiness-unibw.org/ontologies/consumerelectronics/v1"/>
  </owl:ObjectProperty>
  <owl:ObjectProperty rdf:ID="hasEqualizerBandsQuantity">
    <rdfs:comment xml:lang="en">Defines the number of supported equalizers.</rdfs:comment>
    <rdfs:label xml:lang="de">Anzahl von Equalizer</rdfs:label>
    <rdfs:label xml:lang="en">equalizer bands qunatity</rdfs:label>
    <rdfs:isDefinedBy rdf:resource="http://www.ebusiness-unibw.org/ontologies/consumerelectronics/v1"/>
    <rdfs:range rdf:resource="http://purl.org/goodrelations/v1#QuantitativeValueInteger"/>
    <belongsToModule xml:lang="en">MP3Player, TV</belongsToModule>
    <rdfs:subPropertyOf rdf:resource="http://purl.org/goodrelations/v1#quantitativeProductOrServiceProperty"/>
  </owl:ObjectProperty>
  <owl:ObjectProperty rdf:ID="hasNumberOfInputPaperTrays">
    <rdfs:isDefinedBy rdf:resource="http://www.ebusiness-unibw.org/ontologies/consumerelectronics/v1"/>
    <rdfs:subPropertyOf rdf:resource="http://purl.org/goodrelations/v1#quantitativeProductOrServiceProperty"/>
    <rdfs:comment xml:lang="en">Counts the trays which feed the printer with paper.</rdfs:comment>
    <rdfs:label xml:lang="de">Anzahl an Papierkassetten Zuführung</rdfs:label>
    <rdfs:label xml:lang="en">number of input paper trays</rdfs:label>
    <rdfs:range rdf:resource="http://purl.org/goodrelations/v1#QuantitativeValueInteger"/>
    <belongsToModule xml:lang="en">Printer</belongsToModule>
  </owl:ObjectProperty>
  <owl:ObjectProperty rdf:ID="hasPackageHeight">
    <rdfs:isDefinedBy rdf:resource="http://www.ebusiness-unibw.org/ontologies/consumerelectronics/v1"/>
    <rdfs:label xml:lang="de">Verpackungshöhe</rdfs:label>
    <rdfs:label xml:lang="en">package height</rdfs:label>
    <rdfs:comment xml:lang="en">Defines the measurement of vertical distance of an object with its package (Common unit of measurement centimetre, CMT).</rdfs:comment>
    <belongsToModule xml:lang="en">TV</belongsToModule>
    <rdfs:subPropertyOf rdf:resource="http://purl.org/goodrelations/v1#quantitativeProductOrServiceProperty"/>
    <rdfs:range rdf:resource="http://purl.org/goodrelations/v1#QuantitativeValueFloat"/>
  </owl:ObjectProperty>
  <owl:ObjectProperty rdf:ID="hasFeature">
    <rdfs:label xml:lang="de">Eigenschaft</rdfs:label>
    <rdfs:label xml:lang="en">feature</rdfs:label>
    <rdfs:range rdf:resource="#Features"/>
    <rdfs:isDefinedBy rdf:resource="http://www.ebusiness-unibw.org/ontologies/consumerelectronics/v1"/>
    <rdfs:comment xml:lang="en">Defines the type of special functions the object is capable of.</rdfs:comment>
    <rdfs:subPropertyOf rdf:resource="http://purl.org/goodrelations/v1#qualitativeProductOrServiceProperty"/>
    <belongsToModule xml:lang="en">MP3Player, TV, DigitalCamera, Camcorder</belongsToModule>
  </owl:ObjectProperty>
  <owl:ObjectProperty rdf:ID="hasProcessorType">
    <rdfs:isDefinedBy rdf:resource="http://www.ebusiness-unibw.org/ontologies/consumerelectronics/v1"/>
    <rdfs:subPropertyOf rdf:resource="http://purl.org/goodrelations/v1#qualitativeProductOrServiceProperty"/>
    <rdfs:range rdf:resource="#ProcessorType"/>
    <rdfs:label xml:lang="de">Prozessorart</rdfs:label>
    <rdfs:label xml:lang="en">processor type</rdfs:label>
    <rdfs:comment xml:lang="en">The type of central processing unit (CPU) as an electronic circuit that can execute printing tasks or programs.</rdfs:comment>
    <belongsToModule xml:lang="en">Printer</belongsToModule>
  </owl:ObjectProperty>
  <owl:ObjectProperty rdf:ID="hasPrintBorderLeft">
    <rdfs:range rdf:resource="http://purl.org/goodrelations/v1#QuantitativeValueFloat"/>
    <rdfs:comment xml:lang="en">Defines the area which can not be printed on the left side of a paper (DIN A4) (Common unit of measurement millimetre, MMT).</rdfs:comment>
    <rdfs:label xml:lang="de">Druckgrenze links</rdfs:label>
    <rdfs:label xml:lang="en">print border left</rdfs:label>
    <rdfs:subPropertyOf rdf:resource="http://purl.org/goodrelations/v1#quantitativeProductOrServiceProperty"/>
    <rdfs:isDefinedBy rdf:resource="http://www.ebusiness-unibw.org/ontologies/consumerelectronics/v1"/>
  </owl:ObjectProperty>
  <owl:ObjectProperty rdf:ID="hasDigitalZoomFactor">
    <rdfs:comment xml:lang="en">Defines the stages an object can be zoomed digitally.</rdfs:comment>
    <rdfs:range rdf:resource="http://purl.org/goodrelations/v1#QuantitativeValueFloat"/>
    <rdfs:label xml:lang="de">digitaler Zoomfaktor</rdfs:label>
    <rdfs:label xml:lang="en">digital zoom factor</rdfs:label>
    <belongsToModule xml:lang="en">DigitalCamera, Camcorder</belongsToModule>
    <rdfs:isDefinedBy rdf:resource="http://www.ebusiness-unibw.org/ontologies/consumerelectronics/v1"/>
    <rdfs:subPropertyOf rdf:resource="http://purl.org/goodrelations/v1#quantitativeProductOrServiceProperty"/>
  </owl:ObjectProperty>
  <owl:ObjectProperty rdf:ID="hasDigitalVideoCaptureSpeed">
    <rdfs:comment xml:lang="en">Speed of the process of converting an analog video signal—such as that produced by a video camera or DVD player—to digital form.</rdfs:comment>
    <rdfs:range rdf:resource="http://purl.org/goodrelations/v1#QuantitativeValueFloat"/>
    <rdfs:isDefinedBy rdf:resource="http://www.ebusiness-unibw.org/ontologies/consumerelectronics/v1"/>
    <rdfs:label xml:lang="de">digitale Videoaufnahmgeschwindigkeit</rdfs:label>
    <rdfs:label xml:lang="en">digital video capture speed</rdfs:label>
    <belongsToModule xml:lang="en">Camcorder</belongsToModule>
    <rdfs:subPropertyOf rdf:resource="http://purl.org/goodrelations/v1#quantitativeProductOrServiceProperty"/>
  </owl:ObjectProperty>
  <owl:ObjectProperty rdf:ID="hasMaxColorPrintSpeedBestQuality">
    <rdfs:subPropertyOf rdf:resource="http://purl.org/goodrelations/v1#quantitativeProductOrServiceProperty"/>
    <rdfs:range rdf:resource="http://purl.org/goodrelations/v1#QuantitativeValueFloat"/>
    <belongsToModule xml:lang="en">Printer</belongsToModule>
    <rdfs:label xml:lang="de">maximale Druckgeschwindigkeit Farbe beste Qualität</rdfs:label>
    <rdfs:label xml:lang="en">max color print speed best quality</rdfs:label>
    <rdfs:comment xml:lang="en">Amount of pages per minute the product is able to print in the mode of color-printig best quality.</rdfs:comment>
    <rdfs:isDefinedBy rdf:resource="http://www.ebusiness-unibw.org/ontologies/consumerelectronics/v1"/>
  </owl:ObjectProperty>
  <owl:ObjectProperty rdf:ID="hasMaxInputCapacityForEnvelopes">
    <belongsToModule xml:lang="en">Printer</belongsToModule>
    <rdfs:comment xml:lang="en">Defines the maximum ability to hold for envelopes.</rdfs:comment>
    <rdfs:range rdf:resource="http://purl.org/goodrelations/v1#QuantitativeValueInteger"/>
    <rdfs:label xml:lang="de">maximale Menge an Briefkuvert</rdfs:label>
    <rdfs:label xml:lang="en">max input capacity for envelopes</rdfs:label>
    <rdfs:isDefinedBy rdf:resource="http://www.ebusiness-unibw.org/ontologies/consumerelectronics/v1"/>
    <rdfs:subPropertyOf rdf:resource="http://purl.org/goodrelations/v1#quantitativeProductOrServiceProperty"/>
  </owl:ObjectProperty>
  <owl:ObjectProperty rdf:ID="hasNormalPrintableResolutionColorVertical">
    <rdfs:isDefinedBy rdf:resource="http://www.ebusiness-unibw.org/ontologies/consumerelectronics/v1"/>
    <rdfs:range rdf:resource="http://purl.org/goodrelations/v1#QuantitativeValueInteger"/>
    <rdfs:subPropertyOf rdf:resource="http://purl.org/goodrelations/v1#quantitativeProductOrServiceProperty"/>
    <belongsToModule xml:lang="en">Printer</belongsToModule>
    <rdfs:label xml:lang="de">vertikale durckbare Aufslösung Farbe normal</rdfs:label>
    <rdfs:label xml:lang="en">normal printable resolution color vertical</rdfs:label>
    <rdfs:comment xml:lang="en">Defines the digital resolution of the vertical axe (Common unit of measurement pixel, E37)  for color prints for normal prints.</rdfs:comment>
  </owl:ObjectProperty>
  <owl:ObjectProperty rdf:ID="hasNumberOfStandardInputTrays">
    <rdfs:subPropertyOf rdf:resource="http://purl.org/goodrelations/v1#quantitativeProductOrServiceProperty"/>
    <rdfs:label xml:lang="de">Anzahl an Standard Papierkassetten</rdfs:label>
    <rdfs:label xml:lang="en">number of standard input trays</rdfs:label>
    <rdfs:comment xml:lang="en">Defines the number of trays able to hold sheets of paper to be printed.</rdfs:comment>
    <rdfs:isDefinedBy rdf:resource="http://www.ebusiness-unibw.org/ontologies/consumerelectronics/v1"/>
    <rdfs:range rdf:resource="http://purl.org/goodrelations/v1#QuantitativeValueInteger"/>
    <belongsToModule xml:lang="en">Printer</belongsToModule>
  </owl:ObjectProperty>
  <owl:ObjectProperty rdf:ID="hasOpticalSensorSize">
    <rdfs:subPropertyOf rdf:resource="http://purl.org/goodrelations/v1#quantitativeProductOrServiceProperty"/>
    <rdfs:comment xml:lang="en">Size of the device that measures a physical quantity and converts it into a signal which can be read by an observer or by an instrument (common unit of measurement: inch; INH).</rdfs:comment>
    <rdfs:label xml:lang="de">optischer Sensorgröße</rdfs:label>
    <rdfs:label xml:lang="en">optical sensor size</rdfs:label>
    <rdfs:range rdf:resource="http://purl.org/goodrelations/v1#QuantitativeValueFloat"/>
    <belongsToModule xml:lang="en">Camcorder</belongsToModule>
    <rdfs:seeAlso rdf:resource="http://www.ebusiness-unibw.org/ontologies/consumerelectronics/v1"/>
  </owl:ObjectProperty>
  <owl:ObjectProperty rdf:ID="hasStandardInputCapacity">
    <rdfs:comment xml:lang="en">Amount of sheets the product can hold as standard.</rdfs:comment>
    <rdfs:isDefinedBy rdf:resource="http://www.ebusiness-unibw.org/ontologies/consumerelectronics/v1"/>
    <belongsToModule xml:lang="en">Printer</belongsToModule>
    <rdfs:subPropertyOf rdf:resource="http://purl.org/goodrelations/v1#quantitativeProductOrServiceProperty"/>
    <rdfs:label xml:lang="de">Standard Eingabekapazität</rdfs:label>
    <rdfs:label xml:lang="en">standard input capacity</rdfs:label>
    <rdfs:range rdf:resource="http://purl.org/goodrelations/v1#QuantitativeValueInteger"/>
  </owl:ObjectProperty>
  <owl:ObjectProperty rdf:ID="hasFocus">
    <rdfs:isDefinedBy rdf:resource="http://www.ebusiness-unibw.org/ontologies/consumerelectronics/v1"/>
    <rdfs:label xml:lang="de">Fokus</rdfs:label>
    <rdfs:label xml:lang="en">focus</rdfs:label>
    <rdfs:comment xml:lang="en">A focus, also called an image point, is the point where light rays originating from a point on the object converge.

(This description is partly based on or reuses content from the Wikipedia article "Focus (optics)" (http://en.wikipedia.org/wiki/Focus_(optics)) and is licensed under the GNU Free Documentation License (http://www.gnu.org/copyleft/fdl.html).)</rdfs:comment>
    <belongsToModule xml:lang="en">DigitalCamera, Camcorder</belongsToModule>
    <rdfs:range rdf:resource="#Focus"/>
    <rdfs:subPropertyOf rdf:resource="http://purl.org/goodrelations/v1#qualitativeProductOrServiceProperty"/>
  </owl:ObjectProperty>
  <owl:ObjectProperty rdf:ID="hasNumberOfHyptertextPages">
    <belongsToModule xml:lang="en">TV</belongsToModule>
    <rdfs:label xml:lang="de">Anzahl von Teletextseiten</rdfs:label>
    <rdfs:label xml:lang="en">number of hypertext pages</rdfs:label>
    <rdfs:subPropertyOf rdf:resource="http://purl.org/goodrelations/v1#quantitativeProductOrServiceProperty"/>
    <rdfs:comment xml:lang="en">Defines the number of hypertext pages that can be displayed on the main screen of a device.</rdfs:comment>
    <rdfs:range rdf:resource="http://purl.org/goodrelations/v1#QuantitativeValueInteger"/>
    <rdfs:isDefinedBy rdf:resource="http://www.ebusiness-unibw.org/ontologies/consumerelectronics/v1"/>
  </owl:ObjectProperty>
  <owl:ObjectProperty rdf:ID="hasViewingAngleHorizontal">
    <rdfs:comment xml:lang="en">Defines the angle in a horizontal axe where a viewer is still able to see the picture on a screen (Common unit of measurement degree, DD).</rdfs:comment>
    <rdfs:label xml:lang="de">horizontaler Betrachtungswinkel</rdfs:label>
    <rdfs:label xml:lang="en">viewing angle horizontal</rdfs:label>
    <belongsToModule xml:lang="en">TV</belongsToModule>
    <rdfs:range rdf:resource="http://purl.org/goodrelations/v1#QuantitativeValueFloat"/>
    <rdfs:subPropertyOf rdf:resource="http://purl.org/goodrelations/v1#quantitativeProductOrServiceProperty"/>
    <rdfs:isDefinedBy rdf:resource="http://www.ebusiness-unibw.org/ontologies/consumerelectronics/v1"/>
  </owl:ObjectProperty>
  <owl:ObjectProperty rdf:ID="hasFrequencyRange">
    <rdfs:label xml:lang="de">Frequenzberich</rdfs:label>
    <rdfs:label xml:lang="en">frequency range</rdfs:label>
    <belongsToModule xml:lang="en">MP3Player</belongsToModule>
    <rdfs:range rdf:resource="http://purl.org/goodrelations/v1#QuantitativeValueFloat"/>
    <rdfs:subPropertyOf rdf:resource="http://purl.org/goodrelations/v1#quantitativeProductOrServiceProperty"/>
    <rdfs:isDefinedBy rdf:resource="http://www.ebusiness-unibw.org/ontologies/consumerelectronics/v1"/>
    <rdfs:comment xml:lang="en">Defines the range of supported frequency signals (Common unit of measurement megahertz, MHZ).</rdfs:comment>
  </owl:ObjectProperty>
  <owl:ObjectProperty rdf:ID="hasMaxInputCapacity">
    <rdfs:isDefinedBy rdf:resource="http://www.ebusiness-unibw.org/ontologies/consumerelectronics/v1"/>
    <rdfs:comment xml:lang="en">Maximum number of sheets the device can hold in all available standard and optional output trays.</rdfs:comment>
    <rdfs:label xml:lang="de">maximale Medienkapazität</rdfs:label>
    <rdfs:label xml:lang="en">max input capacity</rdfs:label>
    <rdfs:range rdf:resource="http://purl.org/goodrelations/v1#QuantitativeValueInteger"/>
    <belongsToModule xml:lang="en">Printer</belongsToModule>
    <rdfs:subPropertyOf rdf:resource="http://purl.org/goodrelations/v1#quantitativeProductOrServiceProperty"/>
  </owl:ObjectProperty>
  <owl:ObjectProperty rdf:ID="hasDisplayResolutionVertical">
    <rdfs:isDefinedBy rdf:resource="http://www.ebusiness-unibw.org/ontologies/consumerelectronics/v1"/>
    <rdfs:subPropertyOf rdf:resource="http://purl.org/goodrelations/v1#quantitativeProductOrServiceProperty"/>
    <rdfs:label xml:lang="de">vertikale Bildschirmauflösung</rdfs:label>
    <rdfs:label xml:lang="en">display resolution vertical</rdfs:label>
    <belongsToModule xml:lang="en">MP3Player, TV, DigitalCamera, Camcorder</belongsToModule>
    <rdfs:comment xml:lang="en">Defines the digital resolution of the vertical axe (Common unit of measurement pixel, E37).</rdfs:comment>
    <rdfs:range rdf:resource="http://purl.org/goodrelations/v1#QuantitativeValueInteger"/>
  </owl:ObjectProperty>
  <owl:ObjectProperty rdf:ID="hasWidth">
    <rdfs:range rdf:resource="http://purl.org/goodrelations/v1#QuantitativeValueFloat"/>
    <belongsToModule xml:lang="en">MP3Player, TV, Printer, DigitalCamera, Camcorder</belongsToModule>
    <rdfs:subPropertyOf rdf:resource="http://purl.org/goodrelations/v1#quantitativeProductOrServiceProperty"/>
    <rdfs:label xml:lang="de">Breite</rdfs:label>
    <rdfs:label xml:lang="en">width</rdfs:label>
    <rdfs:isDefinedBy rdf:resource="http://www.ebusiness-unibw.org/ontologies/consumerelectronics/v1"/>
    <rdfs:comment xml:lang="en">Defines the distance between the ends of an object, its linear extent as measured from end to end (Common unit of measurement centimetre, CMT).</rdfs:comment>
  </owl:ObjectProperty>
  <owl:ObjectProperty rdf:ID="hasNumberOfOnScreenLanguages">
    <rdfs:label xml:lang="de">Anzahl von verfügbaren Sprachen</rdfs:label>
    <rdfs:label xml:lang="en">number of on screen languages</rdfs:label>
    <rdfs:range rdf:resource="http://purl.org/goodrelations/v1#QuantitativeValueInteger"/>
    <rdfs:subPropertyOf rdf:resource="http://purl.org/goodrelations/v1#quantitativeProductOrServiceProperty"/>
    <rdfs:isDefinedBy rdf:resource="http://www.ebusiness-unibw.org/ontologies/consumerelectronics/v1"/>
    <belongsToModule xml:lang="en">TV</belongsToModule>
    <rdfs:comment xml:lang="en">Defines the available languages that can be chosen to be displayed on the main screen of a device.</rdfs:comment>
  </owl:ObjectProperty>
  <owl:ObjectProperty rdf:ID="hasAudioInterfaceType">
    <rdfs:subPropertyOf rdf:resource="http://purl.org/goodrelations/v1#qualitativeProductOrServiceProperty"/>
    <rdfs:range rdf:resource="#AudioInterfaceType"/>
    <rdfs:isDefinedBy rdf:resource="http://www.ebusiness-unibw.org/ontologies/consumerelectronics/v1"/>
    <rdfs:comment xml:lang="en">Defines the type of interfaces used to transfer audio signals.</rdfs:comment>
    <rdfs:label xml:lang="de">Audioschnittstellentyp</rdfs:label>
    <rdfs:label xml:lang="en">audio interface type</rdfs:label>
    <belongsToModule xml:lang="en">MP3Player</belongsToModule>
  </owl:ObjectProperty>
  <owl:ObjectProperty rdf:ID="hasSleepModePowerConsumption">
    <rdfs:subPropertyOf rdf:resource="http://purl.org/goodrelations/v1#quantitativeProductOrServiceProperty"/>
    <rdfs:comment xml:lang="en">Defines the ability to use a mode that saves significant electrical consumption compared to leaving a device fully on and idle but allows the user to avoid having to reset programming codes (Common unit of measurement Watt, WTT).

(This description is partly based on or reuses content from the Wikipedia article "Sleep mode" (http://en.wikipedia.org/wiki/Sleep_mode) and is licensed under the GNU Free Documentation License (http://www.gnu.org/copyleft/fdl.html).)</rdfs:comment>
    <belongsToModule xml:lang="en">TV</belongsToModule>
    <rdfs:label xml:lang="de">Stromverbrauch im Ruhezustand</rdfs:label>
    <rdfs:label xml:lang="en">sleep mode power consumption</rdfs:label>
    <rdfs:range rdf:resource="http://purl.org/goodrelations/v1#QuantitativeValueFloat"/>
    <rdfs:isDefinedBy rdf:resource="http://www.ebusiness-unibw.org/ontologies/consumerelectronics/v1"/>
  </owl:ObjectProperty>
  <owl:ObjectProperty rdf:ID="hasPowerRequirementsHTZ">
    <rdfs:label xml:lang="de">Strombedarf HTZ</rdfs:label>
    <rdfs:label xml:lang="en">power requirements HTZ</rdfs:label>
    <rdfs:comment xml:lang="en">Defines the power requirements of an electronical device (Common unit of measurement hertz, HTZ).</rdfs:comment>
    <rdfs:isDefinedBy rdf:resource="http://www.ebusiness-unibw.org/ontologies/consumerelectronics/v1"/>
    <rdfs:range rdf:resource="http://purl.org/goodrelations/v1#QuantitativeValueFloat"/>
    <rdfs:subPropertyOf rdf:resource="http://purl.org/goodrelations/v1#quantitativeProductOrServiceProperty"/>
  </owl:ObjectProperty>
  <owl:ObjectProperty rdf:ID="hasMaxPrintableResolutionBlackWhiteHorizontal">
    <rdfs:isDefinedBy rdf:resource="http://www.ebusiness-unibw.org/ontologies/consumerelectronics/v1"/>
    <rdfs:comment xml:lang="en">Defines the maximum digital resolution of the horizontal axe (Common unit of measurement pixel, E37) for black/white prints.</rdfs:comment>
    <belongsToModule xml:lang="en">Printer</belongsToModule>
    <rdfs:label xml:lang="de">maximale horizontale druckbare Auflösung Schwarz/Weiß</rdfs:label>
    <rdfs:label xml:lang="en">max printable resolution black white horizontal</rdfs:label>
    <rdfs:range rdf:resource="http://purl.org/goodrelations/v1#QuantitativeValueInteger"/>
    <rdfs:subPropertyOf rdf:resource="http://purl.org/goodrelations/v1#quantitativeProductOrServiceProperty"/>
  </owl:ObjectProperty>
  <owl:ObjectProperty rdf:ID="hasInternalMemoryCapacity">
    <rdfs:label xml:lang="de">interner Speicherplatz</rdfs:label>
    <rdfs:label xml:lang="en">internal memory capacity</rdfs:label>
    <rdfs:isDefinedBy rdf:resource="http://www.ebusiness-unibw.org/ontologies/consumerelectronics/v1"/>
    <belongsToModule xml:lang="en">MP3Player, Printer, DigitalCamera, Camcorder</belongsToModule>
    <rdfs:range rdf:resource="http://purl.org/goodrelations/v1#QuantitativeValueFloat"/>
    <rdfs:subPropertyOf rdf:resource="http://purl.org/goodrelations/v1#quantitativeProductOrServiceProperty"/>
    <rdfs:comment xml:lang="en">Defines the capacity to store data on internal memory (Common unit of measurement Megabyte, 4L).</rdfs:comment>
  </owl:ObjectProperty>
  <owl:ObjectProperty rdf:ID="hasOpticalSensorResolution">
    <rdfs:isDefinedBy rdf:resource="http://www.ebusiness-unibw.org/ontologies/consumerelectronics/v1"/>
    <rdfs:subPropertyOf rdf:resource="http://purl.org/goodrelations/v1#quantitativeProductOrServiceProperty"/>
    <rdfs:range rdf:resource="http://purl.org/goodrelations/v1#QuantitativeValueFloat"/>
    <belongsToModule xml:lang="en">Camcorder</belongsToModule>
    <rdfs:comment xml:lang="en">Describes the ability of an imaging system to resolve detail in the object that is being imaged.</rdfs:comment>
    <rdfs:label xml:lang="de">Auflösung optischer Sensor</rdfs:label>
    <rdfs:label xml:lang="en">optical sensor resolution</rdfs:label>
  </owl:ObjectProperty>
  <owl:ObjectProperty rdf:ID="hasSceneMode">
    <rdfs:label xml:lang="de">Szenenmodus</rdfs:label>
    <rdfs:label xml:lang="en">scene mode</rdfs:label>
    <rdfs:comment xml:lang="en">Defines a projection of information from any physical environment into any sensory system.</rdfs:comment>
    <rdfs:subPropertyOf rdf:resource="http://purl.org/goodrelations/v1#qualitativeProductOrServiceProperty"/>
    <belongsToModule xml:lang="en">Camcorder</belongsToModule>
    <rdfs:range rdf:resource="#SceneMode"/>
    <rdfs:isDefinedBy rdf:resource="http://www.ebusiness-unibw.org/ontologies/consumerelectronics/v1"/>
  </owl:ObjectProperty>
  <owl:ObjectProperty rdf:ID="hasDisplaySize">
    <belongsToModule xml:lang="en">MP3Player, TV, Printer, DigitalCamera, Camcorder</belongsToModule>
    <rdfs:isDefinedBy rdf:resource="http://www.ebusiness-unibw.org/ontologies/consumerelectronics/v1"/>
    <rdfs:comment xml:lang="en">Defines the diagonal length from the upper left to the lower right angle (Common unit of measurement centimetre, CMT; or inch, INH).</rdfs:comment>
    <rdfs:subPropertyOf rdf:resource="http://purl.org/goodrelations/v1#quantitativeProductOrServiceProperty"/>
    <rdfs:range rdf:resource="http://purl.org/goodrelations/v1#QuantitativeValueFloat"/>
    <rdfs:label xml:lang="de">Bildschirmgröße</rdfs:label>
    <rdfs:label xml:lang="en">display size</rdfs:label>
  </owl:ObjectProperty>
  <owl:ObjectProperty rdf:ID="hasPrintBorderBottom">
    <rdfs:label xml:lang="de">Druckgrenze unten</rdfs:label>
    <rdfs:label xml:lang="en">print border bottom</rdfs:label>
    <rdfs:comment xml:lang="en">Defines the area which can not be printed on the bottom side of a paper (A4) (Common unit of measurement millimetre, MMT).</rdfs:comment>
    <belongsToModule xml:lang="en">Printer</belongsToModule>
    <rdfs:range rdf:resource="http://purl.org/goodrelations/v1#QuantitativeValueFloat"/>
    <rdfs:isDefinedBy rdf:resource="http://www.ebusiness-unibw.org/ontologies/consumerelectronics/v1"/>
    <rdfs:subPropertyOf rdf:resource="http://purl.org/goodrelations/v1#quantitativeProductOrServiceProperty"/>
  </owl:ObjectProperty>
  <owl:ObjectProperty rdf:ID="hasWeightWithStand">
    <belongsToModule xml:lang="en">TV</belongsToModule>
    <rdfs:subPropertyOf rdf:resource="http://purl.org/goodrelations/v1#quantitativeProductOrServiceProperty"/>
    <rdfs:comment xml:lang="en">Defines the measurement of the gravitational force acting on an object with its stand (Common unit of measurement gramm, GRM).</rdfs:comment>
    <rdfs:label xml:lang="de">Gewicht mit Standfuß</rdfs:label>
    <rdfs:label xml:lang="en">weight with stand</rdfs:label>
    <rdfs:range rdf:resource="http://purl.org/goodrelations/v1#QuantitativeValueFloat"/>
    <rdfs:isDefinedBy rdf:resource="http://www.ebusiness-unibw.org/ontologies/consumerelectronics/v1"/>
  </owl:ObjectProperty>
  <owl:ObjectProperty rdf:ID="hasEnergySource">
    <rdfs:comment xml:lang="en">Defines the used energy source.</rdfs:comment>
    <rdfs:label xml:lang="de">Energiequelle</rdfs:label>
    <rdfs:label xml:lang="en">energy source</rdfs:label>
    <rdfs:range rdf:resource="#EnergySource"/>
    <rdfs:isDefinedBy rdf:resource="http://www.ebusiness-unibw.org/ontologies/consumerelectronics/v1"/>
    <belongsToModule xml:lang="en">MP3Player, Printer, DigitalCamera, Camcorder</belongsToModule>
    <rdfs:subPropertyOf rdf:resource="http://purl.org/goodrelations/v1#qualitativeProductOrServiceProperty"/>
  </owl:ObjectProperty>
  <owl:ObjectProperty rdf:ID="hasOpticalZoomFactor">
    <belongsToModule xml:lang="en">DigitalCamera, Camcorder</belongsToModule>
    <rdfs:label xml:lang="de">optischer Zoomfaktor</rdfs:label>
    <rdfs:label xml:lang="en">optical zoom factor</rdfs:label>
    <rdfs:range rdf:resource="http://purl.org/goodrelations/v1#QuantitativeValueFloat"/>
    <rdfs:comment xml:lang="en">Defines the stages an object can be zoomed optically.</rdfs:comment>
    <rdfs:isDefinedBy rdf:resource="http://www.ebusiness-unibw.org/ontologies/consumerelectronics/v1"/>
    <rdfs:subPropertyOf rdf:resource="http://purl.org/goodrelations/v1#quantitativeProductOrServiceProperty"/>
  </owl:ObjectProperty>
  <owl:ObjectProperty rdf:ID="hasZoom">
    <rdfs:label xml:lang="de">Zoom</rdfs:label>
    <rdfs:label xml:lang="en">zoom</rdfs:label>
    <rdfs:isDefinedBy rdf:resource="http://www.ebusiness-unibw.org/ontologies/consumerelectronics/v1"/>
    <rdfs:comment xml:lang="en">Zoom is a method of decreasing (narrowing) the apparent angle of view of a photographic or video image.

(This description is partly based on or reuses content from the Wikipedia article "Digital zoom" (http://en.wikipedia.org/wiki/Digital_zoom) and is licensed under the GNU Free Documentation License (http://www.gnu.org/copyleft/fdl.html).)</rdfs:comment>
    <belongsToModule xml:lang="en">DigitalCamera, Camcorder</belongsToModule>
    <rdfs:subPropertyOf rdf:resource="http://purl.org/goodrelations/v1#qualitativeProductOrServiceProperty"/>
    <rdfs:range rdf:resource="#Zoom"/>
  </owl:ObjectProperty>
  <owl:ObjectProperty rdf:ID="hasPackageDepth">
    <rdfs:subPropertyOf rdf:resource="http://purl.org/goodrelations/v1#quantitativeProductOrServiceProperty"/>
    <rdfs:isDefinedBy rdf:resource="http://www.ebusiness-unibw.org/ontologies/consumerelectronics/v1"/>
    <belongsToModule xml:lang="en">TV</belongsToModule>
    <rdfs:comment xml:lang="en">Defines the distance from side to side, measuring across the object with its package at right angles to the width (Common unit of measurement centimetre, CMT).

(This description is partly based on or reuses content from the Wikipedia article "Length" (http://en.wikipedia.org/wiki/Length) and is licensed under the GNU Free Documentation License (http://www.gnu.org/copyleft/fdl.html).)</rdfs:comment>
    <rdfs:range rdf:resource="http://purl.org/goodrelations/v1#QuantitativeValueFloat"/>
    <rdfs:label xml:lang="de">Verpackungstiefe</rdfs:label>
    <rdfs:label xml:lang="en">package depth</rdfs:label>
  </owl:ObjectProperty>
  <owl:ObjectProperty rdf:ID="hasMaxOperatingTemperature">
    <rdfs:subPropertyOf rdf:resource="http://purl.org/goodrelations/v1#quantitativeProductOrServiceProperty"/>
    <rdfs:comment xml:lang="en">Defines the maximum temperature the product is able to operate (Common unit of measurement grad celsius, CEL).</rdfs:comment>
    <belongsToModule xml:lang="en">TV, Printer</belongsToModule>
    <rdfs:label xml:lang="de">maximale Betriebstemperatur</rdfs:label>
    <rdfs:label xml:lang="en">max operating temperatur</rdfs:label>
    <rdfs:isDefinedBy rdf:resource="http://www.ebusiness-unibw.org/ontologies/consumerelectronics/v1"/>
    <rdfs:range rdf:resource="http://purl.org/goodrelations/v1#QuantitativeValueFloat"/>
  </owl:ObjectProperty>
  <owl:ObjectProperty rdf:ID="hasAccessory">
    <rdfs:label xml:lang="de">Zubehör</rdfs:label>
    <rdfs:label xml:lang="en">accessory</rdfs:label>
    <rdfs:range rdf:resource="#Accessory"/>
    <rdfs:isDefinedBy rdf:resource="http://www.ebusiness-unibw.org/ontologies/consumerelectronics/v1"/>
    <rdfs:subPropertyOf rdf:resource="http://purl.org/goodrelations/v1#qualitativeProductOrServiceProperty"/>
    <rdfs:comment xml:lang="en">Defines subordinate or supplementary items.</rdfs:comment>
    <belongsToModule xml:lang="en">Camcorder</belongsToModule>
  </owl:ObjectProperty>
  <owl:ObjectProperty rdf:ID="hasAudioOutputPower">
    <belongsToModule rdf:datatype="http://www.w3.org/2001/XMLSchema#string"
    >TV</belongsToModule>
    <rdfs:comment xml:lang="en">Defines the rate of energy conversion (Common unit of Measurement milliwatt, C31).</rdfs:comment>
    <rdfs:label xml:lang="de">Audioausgangsleistung</rdfs:label>
    <rdfs:label xml:lang="en">audio output power</rdfs:label>
    <rdfs:isDefinedBy rdf:resource="http://www.ebusiness-unibw.org/ontologies/consumerelectronics/v1"/>
    <rdfs:subPropertyOf rdf:resource="#hasOutputPower"/>
  </owl:ObjectProperty>
  <owl:ObjectProperty rdf:ID="hasBodyColor">
    <rdfs:subPropertyOf rdf:resource="http://purl.org/goodrelations/v1#qualitativeProductOrServiceProperty"/>
    <rdfs:comment xml:lang="en">Defines the major color of an objects body.</rdfs:comment>
    <rdfs:range rdf:resource="#Color"/>
    <rdfs:isDefinedBy rdf:resource="http://www.ebusiness-unibw.org/ontologies/consumerelectronics/v1"/>
    <rdfs:label xml:lang="de">Farbe</rdfs:label>
    <rdfs:label xml:lang="en">body color</rdfs:label>
    <belongsToModule xml:lang="en">MP3Player, TV, Printer, DigitalCamera, Camcorder</belongsToModule>
  </owl:ObjectProperty>
  <owl:ObjectProperty rdf:ID="hasTVTuner">
    <rdfs:label xml:lang="de">TV Tuner</rdfs:label>
    <rdfs:label rdf:datatype="http://www.w3.org/2001/XMLSchema#string"
    >TV Tuner</rdfs:label>
    <rdfs:domain rdf:resource="#TV"/>
    <rdfs:comment xml:lang="en">Defines the type of included TV tuner.</rdfs:comment>
    <rdfs:subPropertyOf rdf:resource="http://purl.org/goodrelations/v1#qualitativeProductOrServiceProperty"/>
    <belongsToModule xml:lang="en">TV</belongsToModule>
    <rdfs:range rdf:resource="#TVTuner"/>
    <rdfs:isDefinedBy rdf:resource="http://www.ebusiness-unibw.org/ontologies/consumerelectronics/v1"/>
  </owl:ObjectProperty>
  <owl:ObjectProperty rdf:ID="hasNormalPrintableResolutionBlackWhiteHorizontal">
    <rdfs:subPropertyOf rdf:resource="http://purl.org/goodrelations/v1#quantitativeProductOrServiceProperty"/>
    <rdfs:comment xml:lang="en">Defines the digital resolution of the horizontal axe (Common unit of measurement pixel, E37) for black/white prints for normal prints.</rdfs:comment>
    <rdfs:range rdf:resource="http://purl.org/goodrelations/v1#QuantitativeValueInteger"/>
    <rdfs:isDefinedBy rdf:resource="http://www.ebusiness-unibw.org/ontologies/consumerelectronics/v1"/>
    <rdfs:label xml:lang="de">horizontale druckbare Auflösung Schwarz/Weiß normal</rdfs:label>
    <rdfs:label xml:lang="en">normal printable resolution black white horizontal</rdfs:label>
    <belongsToModule xml:lang="en">Printer</belongsToModule>
  </owl:ObjectProperty>
  <owl:ObjectProperty rdf:ID="hasDraftPrintableResolutionColorVertical">
    <rdfs:label xml:lang="de">vertikale druckbare Auflösung Farbe Entwurf</rdfs:label>
    <rdfs:label xml:lang="en">draft printable resolution color vertical</rdfs:label>
    <rdfs:isDefinedBy rdf:resource="http://www.ebusiness-unibw.org/ontologies/consumerelectronics/v1"/>
    <rdfs:comment xml:lang="en">Defines the digital resolution of the vertical axe (Common unit of measurement pixel, E37) for black/white prints for draft prints.</rdfs:comment>
    <belongsToModule xml:lang="en">Printer</belongsToModule>
    <rdfs:range rdf:resource="http://purl.org/goodrelations/v1#QuantitativeValueInteger"/>
    <rdfs:subPropertyOf rdf:resource="http://purl.org/goodrelations/v1#quantitativeProductOrServiceProperty"/>
  </owl:ObjectProperty>
  <owl:ObjectProperty rdf:ID="hasMaxPrintableResolutionColorHorizontal">
    <rdfs:label xml:lang="de">maximale horizontale druckbare Auflösung Farbe</rdfs:label>
    <rdfs:label xml:lang="en">max printable resolution color horizontal</rdfs:label>
    <rdfs:range rdf:resource="http://purl.org/goodrelations/v1#QuantitativeValueInteger"/>
    <rdfs:subPropertyOf rdf:resource="http://purl.org/goodrelations/v1#quantitativeProductOrServiceProperty"/>
    <belongsToModule xml:lang="en">Printer</belongsToModule>
    <rdfs:comment xml:lang="en">Defines the maximum digital resolution of the horizontal axe (Common unit of measurement pixel, E37) for color prints.</rdfs:comment>
    <rdfs:isDefinedBy rdf:resource="http://www.ebusiness-unibw.org/ontologies/consumerelectronics/v1"/>
  </owl:ObjectProperty>
  <owl:ObjectProperty rdf:ID="hasDraftPrintableResolutionBlackWhiteVertical">
    <rdfs:comment xml:lang="en">Defines the digital resolution of the vertical axe (Common unit of measurement pixel, E37) for black/white prints for draft prints.</rdfs:comment>
    <rdfs:range rdf:resource="http://purl.org/goodrelations/v1#QuantitativeValueInteger"/>
    <belongsToModule xml:lang="en">Printer</belongsToModule>
    <rdfs:subPropertyOf rdf:resource="http://purl.org/goodrelations/v1#quantitativeProductOrServiceProperty"/>
    <rdfs:isDefinedBy rdf:resource="http://www.ebusiness-unibw.org/ontologies/consumerelectronics/v1"/>
    <rdfs:label xml:lang="de">vertikale druckbare Auflösung Schwarz/Weiß Entwurf</rdfs:label>
    <rdfs:label xml:lang="en">draft printable resolution black white vertical</rdfs:label>
  </owl:ObjectProperty>
  <owl:ObjectProperty rdf:ID="hasFocusSize">
    <rdfs:comment xml:lang="en">Focus, also called an image point, is the point where light rays originating from a point on the object converge.

(This description is partly based on or reuses content from the Wikipedia article "Focus (optics)" (http://en.wikipedia.org/wiki/Focus_(optics)) and is licensed under the GNU Free Documentation License (http://www.gnu.org/copyleft/fdl.html).)</rdfs:comment>
    <belongsToModule xml:lang="en">Camcorder</belongsToModule>
    <rdfs:label xml:lang="de">Fokusgröße</rdfs:label>
    <rdfs:label xml:lang="en">focus size</rdfs:label>
    <rdfs:isDefinedBy rdf:resource="http://www.ebusiness-unibw.org/ontologies/consumerelectronics/v1"/>
    <rdfs:range rdf:resource="http://purl.org/goodrelations/v1#QuantitativeValueFloat"/>
    <rdfs:subPropertyOf rdf:resource="http://purl.org/goodrelations/v1#quantitativeProductOrServiceProperty"/>
  </owl:ObjectProperty>
  <owl:ObjectProperty rdf:ID="hasStandardOutputCapacityForTransperancies">
    <rdfs:comment xml:lang="en">Defines the maximum amount of transparancies the product is able to print.</rdfs:comment>
    <rdfs:subPropertyOf rdf:resource="http://purl.org/goodrelations/v1#quantitativeProductOrServiceProperty"/>
    <rdfs:range rdf:resource="http://purl.org/goodrelations/v1#QuantitativeValueInteger"/>
    <belongsToModule xml:lang="en">Printer</belongsToModule>
    <rdfs:isDefinedBy rdf:resource="http://www.ebusiness-unibw.org/ontologies/consumerelectronics/v1"/>
    <rdfs:label xml:lang="de">Standard Ausgabekapazität für Folien</rdfs:label>
    <rdfs:label xml:lang="en">standard output capacity for transperancies</rdfs:label>
  </owl:ObjectProperty>
  <owl:ObjectProperty rdf:ID="hasDraftPrintableResolutionColorHorizontal">
    <rdfs:comment xml:lang="en">Defines the digital resolution of the horizontal axe (Common unit of measurement pixel, E37) for black/white prints for draft prints.</rdfs:comment>
    <belongsToModule xml:lang="en">Printer</belongsToModule>
    <rdfs:range rdf:resource="http://purl.org/goodrelations/v1#QuantitativeValueInteger"/>
    <rdfs:isDefinedBy rdf:resource="http://www.ebusiness-unibw.org/ontologies/consumerelectronics/v1"/>
    <rdfs:subPropertyOf rdf:resource="http://purl.org/goodrelations/v1#quantitativeProductOrServiceProperty"/>
    <rdfs:label xml:lang="de">horizontale druckbare Auflösung Farbe Entwurf</rdfs:label>
    <rdfs:label xml:lang="en">draft printable resolution color horizontal</rdfs:label>
  </owl:ObjectProperty>
  <owl:ObjectProperty rdf:ID="hasShutterLag">
    <rdfs:range rdf:resource="http://purl.org/goodrelations/v1#QuantitativeValueFloat"/>
    <rdfs:label xml:lang="de">Auslöseverzögerung</rdfs:label>
    <rdfs:label xml:lang="en">shutter lag</rdfs:label>
    <rdfs:subPropertyOf rdf:resource="http://purl.org/goodrelations/v1#quantitativeProductOrServiceProperty"/>
    <rdfs:comment xml:lang="en">Defines the delay between triggering the shutter and when the photograph is actually recorded (Common unit of measurement seconds, SEC).</rdfs:comment>
    <rdfs:isDefinedBy rdf:resource="http://www.ebusiness-unibw.org/ontologies/consumerelectronics/v1"/>
    <belongsToModule xml:lang="en">DigitalCamera, Camcorder</belongsToModule>
  </owl:ObjectProperty>
  <owl:ObjectProperty rdf:ID="hasStandbyPowerConsumption">
    <belongsToModule xml:lang="en">TV, Printer</belongsToModule>
    <rdfs:subPropertyOf rdf:resource="http://purl.org/goodrelations/v1#quantitativeProductOrServiceProperty"/>
    <rdfs:range rdf:resource="http://purl.org/goodrelations/v1#QuantitativeValueFloat"/>
    <rdfs:comment xml:lang="en">Defines the amount of consumed energy while the device is in the standby mode (Common unit of measurement Watt, WTT).</rdfs:comment>
    <rdfs:isDefinedBy rdf:resource="http://www.ebusiness-unibw.org/ontologies/consumerelectronics/v1"/>
    <rdfs:label xml:lang="de">Standby Stromverbrauch</rdfs:label>
    <rdfs:label xml:lang="en">standby power consumption</rdfs:label>
  </owl:ObjectProperty>
  <owl:ObjectProperty rdf:ID="hasPaperFormat">
    <rdfs:range rdf:resource="#MediaFormat"/>
    <rdfs:label xml:lang="de">Papierformat</rdfs:label>
    <rdfs:label xml:lang="en">paper format</rdfs:label>
    <rdfs:comment xml:lang="en">Defines the supported paper formats.</rdfs:comment>
    <belongsToModule xml:lang="en">Printer</belongsToModule>
    <rdfs:isDefinedBy rdf:resource="http://www.ebusiness-unibw.org/ontologies/consumerelectronics/v1"/>
    <rdfs:subPropertyOf rdf:resource="http://purl.org/goodrelations/v1#qualitativeProductOrServiceProperty"/>
  </owl:ObjectProperty>
  <owl:ObjectProperty rdf:ID="hasDepthWithStand">
    <belongsToModule xml:lang="en">TV</belongsToModule>
    <rdfs:label xml:lang="de">Tiefe mit Standfuß</rdfs:label>
    <rdfs:label xml:lang="en">depth with stand</rdfs:label>
    <rdfs:subPropertyOf rdf:resource="http://purl.org/goodrelations/v1#quantitativeProductOrServiceProperty"/>
    <rdfs:isDefinedBy rdf:resource="http://www.ebusiness-unibw.org/ontologies/consumerelectronics/v1"/>
    <rdfs:comment xml:lang="en">Defines the distance from side to side, measuring across the object with its stand at right angles to the width (Common unit of measurement centimetre, CMT).

(This description is partly based on or reuses content from the Wikipedia article "Length" (http://en.wikipedia.org/wiki/Length) and is licensed under the GNU Free Documentation License (http://www.gnu.org/copyleft/fdl.html).)</rdfs:comment>
    <rdfs:range rdf:resource="http://purl.org/goodrelations/v1#QuantitativeValueFloat"/>
  </owl:ObjectProperty>
  <owl:ObjectProperty rdf:ID="hasPrintBorderRight">
    <rdfs:isDefinedBy rdf:resource="http://www.ebusiness-unibw.org/ontologies/consumerelectronics/v1"/>
    <rdfs:subPropertyOf rdf:resource="http://purl.org/goodrelations/v1#quantitativeProductOrServiceProperty"/>
    <rdfs:comment xml:lang="en">Defines the area which can not be printed on the right side of a paper (A4) (Common unit of measurement millimetre, MMT).</rdfs:comment>
    <rdfs:range rdf:resource="http://purl.org/goodrelations/v1#QuantitativeValueFloat"/>
    <rdfs:label xml:lang="de">Druckgrenze rechts</rdfs:label>
    <rdfs:label xml:lang="en">print border right</rdfs:label>
    <belongsToModule xml:lang="en">Printer</belongsToModule>
  </owl:ObjectProperty>
  <owl:ObjectProperty rdf:ID="hasNumberOfDisplayColors">
    <rdfs:isDefinedBy rdf:resource="http://www.ebusiness-unibw.org/ontologies/consumerelectronics/v1"/>
    <rdfs:range rdf:resource="http://purl.org/goodrelations/v1#QuantitativeValueInteger"/>
    <rdfs:label xml:lang="de">Anzahl von Bildschirmfarben</rdfs:label>
    <rdfs:label xml:lang="en">number of display colors</rdfs:label>
    <rdfs:subPropertyOf rdf:resource="http://purl.org/goodrelations/v1#quantitativeProductOrServiceProperty"/>
    <rdfs:comment xml:lang="en">Defines the number of colors an electronical device is able to display on a screen.</rdfs:comment>
    <belongsToModule xml:lang="en">MP3Player, TV, Printer, DigitalCamera, Camcorder</belongsToModule>
  </owl:ObjectProperty>
  <owl:ObjectProperty rdf:ID="hasPackageWidth">
    <rdfs:subPropertyOf rdf:resource="http://purl.org/goodrelations/v1#quantitativeProductOrServiceProperty"/>
    <rdfs:comment xml:lang="en">Defines the distance between the ends of an object, its linear extent as measured from end to end with its package (Common unit of measurement centimetre, CMT).</rdfs:comment>
    <rdfs:range rdf:resource="http://purl.org/goodrelations/v1#QuantitativeValueFloat"/>
    <rdfs:label xml:lang="de">Verpackungsbreite</rdfs:label>
    <rdfs:label xml:lang="en">package width</rdfs:label>
    <rdfs:isDefinedBy rdf:resource="http://www.ebusiness-unibw.org/ontologies/consumerelectronics/v1"/>
    <belongsToModule xml:lang="en">TV</belongsToModule>
  </owl:ObjectProperty>
  <owl:ObjectProperty rdf:ID="hasStandardOutputCapacityForEnvelopes">
    <rdfs:isDefinedBy rdf:resource="http://www.ebusiness-unibw.org/ontologies/consumerelectronics/v1"/>
    <rdfs:comment xml:lang="en">Defines the maximum amount of envelopes the product is able to print.</rdfs:comment>
    <belongsToModule xml:lang="en">Printer</belongsToModule>
    <rdfs:label xml:lang="de">Standard Ausgabekapazität für Briefkuvert</rdfs:label>
    <rdfs:label xml:lang="en">standard output capacity for envelopes</rdfs:label>
    <rdfs:range rdf:resource="http://purl.org/goodrelations/v1#QuantitativeValueInteger"/>
    <rdfs:subPropertyOf rdf:resource="http://purl.org/goodrelations/v1#quantitativeProductOrServiceProperty"/>
  </owl:ObjectProperty>
  <owl:ObjectProperty rdf:ID="hasLensSystem">
    <rdfs:label xml:lang="de">Objektivsystem</rdfs:label>
    <rdfs:label xml:lang="en">lens system</rdfs:label>
    <rdfs:range rdf:resource="#LensSystem"/>
    <belongsToModule xml:lang="en">Camcorder</belongsToModule>
    <rdfs:subPropertyOf rdf:resource="http://purl.org/goodrelations/v1#qualitativeProductOrServiceProperty"/>
    <rdfs:comment xml:lang="en">Defines the perfect or approximate axial symmetry which transmits and refracts light.</rdfs:comment>
    <rdfs:isDefinedBy rdf:resource="http://www.ebusiness-unibw.org/ontologies/consumerelectronics/v1"/>
  </owl:ObjectProperty>
  <owl:ObjectProperty rdf:ID="hasMaxColorPrintSpeedNormal">
    <rdfs:subPropertyOf rdf:resource="http://purl.org/goodrelations/v1#quantitativeProductOrServiceProperty"/>
    <rdfs:label xml:lang="de">maximale Druckgeschwindigkeit Farbe normal</rdfs:label>
    <rdfs:label xml:lang="en">max color print speed normal</rdfs:label>
    <rdfs:range rdf:resource="http://purl.org/goodrelations/v1#QuantitativeValueFloat"/>
    <rdfs:isDefinedBy rdf:resource="http://www.ebusiness-unibw.org/ontologies/consumerelectronics/v1"/>
    <belongsToModule xml:lang="en">Printer</belongsToModule>
    <rdfs:comment xml:lang="en">Amount of pages per minute the product is able to print in the mode of color-printig normal quality.</rdfs:comment>
  </owl:ObjectProperty>
  <owl:ObjectProperty rdf:ID="hasCertificate">
    <rdfs:comment xml:lang="en">Defines the type of certificate of a product used to attest quality standards.</rdfs:comment>
    <rdfs:label xml:lang="de">Zertifikat</rdfs:label>
    <rdfs:label xml:lang="en">certificate</rdfs:label>
    <rdfs:isDefinedBy rdf:resource="http://www.ebusiness-unibw.org/ontologies/consumerelectronics/v1"/>
    <rdfs:range rdf:resource="#Certificate"/>
    <rdfs:subPropertyOf rdf:resource="http://purl.org/goodrelations/v1#qualitativeProductOrServiceProperty"/>
    <belongsToModule xml:lang="en">TV</belongsToModule>
  </owl:ObjectProperty>
  <owl:ObjectProperty rdf:ID="hasDraftPrintableResolutionBlackWhiteHorizontal">
    <rdfs:label xml:lang="de">horizontale druckbare Auflösung Schwarz/Weiß Entwurf</rdfs:label>
    <rdfs:label xml:lang="en">draft printable resolution black white horizontal</rdfs:label>
    <belongsToModule xml:lang="en">Printer</belongsToModule>
    <rdfs:subPropertyOf rdf:resource="http://purl.org/goodrelations/v1#quantitativeProductOrServiceProperty"/>
    <rdfs:comment xml:lang="en">Defines the digital resolution of the horizontal axe (Common unit of measurement pixel, E37) for black/white prints for draft prints.</rdfs:comment>
    <rdfs:isDefinedBy rdf:resource="http://www.ebusiness-unibw.org/ontologies/consumerelectronics/v1"/>
    <rdfs:range rdf:resource="http://purl.org/goodrelations/v1#QuantitativeValueInteger"/>
  </owl:ObjectProperty>
  <owl:ObjectProperty rdf:ID="hasMaxMediaFormat">
    <rdfs:isDefinedBy rdf:resource="http://www.ebusiness-unibw.org/ontologies/consumerelectronics/v1"/>
    <rdfs:label xml:lang="de">maximale Mediengröße</rdfs:label>
    <rdfs:label xml:lang="en">max media format</rdfs:label>
    <belongsToModule xml:lang="en">Printer</belongsToModule>
    <rdfs:comment xml:lang="en">Defines the maximum size of the printed media format.</rdfs:comment>
    <rdfs:range rdf:resource="#MediaFormat"/>
    <rdfs:subPropertyOf rdf:resource="http://purl.org/goodrelations/v1#qualitativeProductOrServiceProperty"/>
  </owl:ObjectProperty>
  <owl:ObjectProperty rdf:ID="hasMaxInternalMemoryCapacity">
    <rdfs:comment xml:lang="en">Defines the maximum amount of memory that can be installed in the systems hardware (common unit of measurement: megabyte(MB): 4L).</rdfs:comment>
    <rdfs:label xml:lang="de">maximaler interner Speicherplatz</rdfs:label>
    <rdfs:label xml:lang="en">max internal memory capacity</rdfs:label>
    <rdfs:subPropertyOf rdf:resource="http://purl.org/goodrelations/v1#quantitativeProductOrServiceProperty"/>
    <rdfs:isDefinedBy rdf:resource="http://www.ebusiness-unibw.org/ontologies/consumerelectronics/v1"/>
    <rdfs:range rdf:resource="http://purl.org/goodrelations/v1#QuantitativeValueFloat"/>
    <belongsToModule xml:lang="en">Printer</belongsToModule>
  </owl:ObjectProperty>
  <owl:ObjectProperty rdf:ID="hasWidthWithStand">
    <rdfs:label xml:lang="de">Breite mit Standfuß</rdfs:label>
    <rdfs:label xml:lang="en">width with stand</rdfs:label>
    <rdfs:isDefinedBy rdf:resource="http://www.ebusiness-unibw.org/ontologies/consumerelectronics/v1"/>
    <rdfs:range rdf:resource="http://purl.org/goodrelations/v1#QuantitativeValueFloat"/>
    <belongsToModule xml:lang="en">TV</belongsToModule>
    <rdfs:comment xml:lang="en">Defines the distance between the ends of an object, its linear extent as measured from end to end with its stand (Common unit of measurement centimetre, CMT).</rdfs:comment>
    <rdfs:subPropertyOf rdf:resource="http://purl.org/goodrelations/v1#quantitativeProductOrServiceProperty"/>
  </owl:ObjectProperty>
  <owl:ObjectProperty rdf:ID="hasUsagePowerConsumption">
    <rdfs:comment xml:lang="en">Defines the necessary power for an electronical object while the device is used (Common unit of measurement Watt, WTT).</rdfs:comment>
    <rdfs:subPropertyOf rdf:resource="http://purl.org/goodrelations/v1#quantitativeProductOrServiceProperty"/>
    <rdfs:isDefinedBy rdf:resource="http://www.ebusiness-unibw.org/ontologies/consumerelectronics/v1"/>
    <belongsToModule xml:lang="en">TV, Printer</belongsToModule>
    <rdfs:range rdf:resource="http://purl.org/goodrelations/v1#QuantitativeValueFloat"/>
    <rdfs:label xml:lang="de">Stromverbrauch in Betrieb</rdfs:label>
    <rdfs:label xml:lang="en">usage power consumption</rdfs:label>
  </owl:ObjectProperty>
  <owl:ObjectProperty rdf:ID="hasMaxMemoryCapacity">
    <rdfs:subPropertyOf rdf:resource="http://purl.org/goodrelations/v1#quantitativeProductOrServiceProperty"/>
    <rdfs:isDefinedBy rdf:resource="http://www.ebusiness-unibw.org/ontologies/consumerelectronics/v1"/>
    <rdfs:label xml:lang="de">maximale Speicherkapazität</rdfs:label>
    <rdfs:label xml:lang="en">maximale memory capacity</rdfs:label>
    <rdfs:comment xml:lang="en">Defines the maxium capacity that can be provided by using external memory (Common unit of measurement megabyte, 4L).</rdfs:comment>
    <rdfs:range rdf:resource="http://purl.org/goodrelations/v1#QuantitativeValueFloat"/>
    <belongsToModule xml:lang="en">MP3Player, DigitalCamera, Camcorder</belongsToModule>
  </owl:ObjectProperty>
  <owl:ObjectProperty rdf:ID="hasHeight">
    <belongsToModule xml:lang="en">MP3Player, TV, Printer, DigitalCamera, Camcorder</belongsToModule>
    <rdfs:subPropertyOf rdf:resource="http://purl.org/goodrelations/v1#quantitativeProductOrServiceProperty"/>
    <rdfs:range rdf:resource="http://purl.org/goodrelations/v1#QuantitativeValueFloat"/>
    <rdfs:isDefinedBy rdf:resource="http://www.ebusiness-unibw.org/ontologies/consumerelectronics/v1"/>
    <rdfs:label xml:lang="de">Höhe</rdfs:label>
    <rdfs:label xml:lang="en">height</rdfs:label>
    <rdfs:comment xml:lang="en">Defines the measurement of vertical distance (Common unit of measurement centimetre, CMT).</rdfs:comment>
  </owl:ObjectProperty>
  <owl:ObjectProperty rdf:ID="hasDigitalFrequency">
    <rdfs:label xml:lang="de">Digitale Frequenz</rdfs:label>
    <rdfs:label xml:lang="en">digital frequency</rdfs:label>
    <rdfs:range rdf:resource="http://purl.org/goodrelations/v1#QuantitativeValueFloat"/>
    <rdfs:comment xml:lang="en">Digital frequency is the analogue for discrete signals as frequency is to continuous signals (Common unit of measurement hertz, HTZ).

(This description is partly based on or reuses content from the Wikipedia article "Digital frequency" (http://en.wikipedia.org/wiki/Digital_frequency) and is licensed under the GNU Free Documentation License (http://www.gnu.org/copyleft/fdl.html).)</rdfs:comment>
    <rdfs:isDefinedBy rdf:resource="http://www.ebusiness-unibw.org/ontologies/consumerelectronics/v1"/>
    <belongsToModule xml:lang="en">TV</belongsToModule>
    <rdfs:subPropertyOf rdf:resource="http://purl.org/goodrelations/v1#quantitativeProductOrServiceProperty"/>
  </owl:ObjectProperty>
  <owl:ObjectProperty rdf:ID="hasDisplayType">
    <rdfs:comment xml:lang="en">Defines the type of the display like LCD or Plasma.</rdfs:comment>
    <rdfs:range rdf:resource="#DisplayType"/>
    <rdfs:subPropertyOf rdf:resource="http://purl.org/goodrelations/v1#qualitativeProductOrServiceProperty"/>
    <rdfs:label xml:lang="de">Bildschirmtyp</rdfs:label>
    <rdfs:label xml:lang="en">display type</rdfs:label>
    <belongsToModule xml:lang="en">MP3Player, TV, Printer, Camcorder</belongsToModule>
    <rdfs:isDefinedBy rdf:resource="http://www.ebusiness-unibw.org/ontologies/consumerelectronics/v1"/>
  </owl:ObjectProperty>
  <owl:ObjectProperty rdf:ID="hasMaxBlackWhitePrintSpeedDraft">
    <rdfs:isDefinedBy rdf:resource="http://www.ebusiness-unibw.org/ontologies/consumerelectronics/v1"/>
    <rdfs:comment xml:lang="en">Amount of pages per minute the product is able to print in the mode of black-printig of drafts.</rdfs:comment>
    <belongsToModule xml:lang="en">Printer</belongsToModule>
    <rdfs:subPropertyOf rdf:resource="http://purl.org/goodrelations/v1#quantitativeProductOrServiceProperty"/>
    <rdfs:label xml:lang="de">maximale Druckgeschwindigkeit schwarz/weiß Entwurf</rdfs:label>
    <rdfs:label xml:lang="en">max black white print speed draft</rdfs:label>
    <rdfs:range rdf:resource="http://purl.org/goodrelations/v1#QuantitativeValueFloat"/>
  </owl:ObjectProperty>
  <owl:ObjectProperty rdf:ID="hasNormalPrintableResolutionBlackWhiteVertical">
    <rdfs:isDefinedBy rdf:resource="http://www.ebusiness-unibw.org/ontologies/consumerelectronics/v1"/>
    <rdfs:range rdf:resource="http://purl.org/goodrelations/v1#QuantitativeValueInteger"/>
    <rdfs:subPropertyOf rdf:resource="http://purl.org/goodrelations/v1#quantitativeProductOrServiceProperty"/>
    <rdfs:label xml:lang="de">vertikale druckbare Auflösung Schwarz/Weiß normal</rdfs:label>
    <rdfs:label xml:lang="en">normal printable resolution black white vertical</rdfs:label>
    <rdfs:comment xml:lang="en">Defines the  digital resolution of the vertical axe (Common unit of measurement pixel, E37) for black/white prints for normal prints.</rdfs:comment>
    <belongsToModule xml:lang="en">Printer</belongsToModule>
  </owl:ObjectProperty>
  <owl:ObjectProperty rdf:ID="hasDisplayResolutionHorizontal">
    <rdfs:comment xml:lang="en">Defines the digital resolution of the horizontal axe (Common unit of measurement pixel, E37).</rdfs:comment>
    <rdfs:range rdf:resource="http://purl.org/goodrelations/v1#QuantitativeValueInteger"/>
    <rdfs:isDefinedBy rdf:resource="http://www.ebusiness-unibw.org/ontologies/consumerelectronics/v1"/>
    <rdfs:label xml:lang="de">horizontale Bildschirmauflösung</rdfs:label>
    <rdfs:label xml:lang="en">display resolution horizontal</rdfs:label>
    <belongsToModule xml:lang="en">MP3Player, TV, DigitalCamera, Camcorder</belongsToModule>
    <rdfs:subPropertyOf rdf:resource="http://purl.org/goodrelations/v1#quantitativeProductOrServiceProperty"/>
  </owl:ObjectProperty>
  <owl:ObjectProperty rdf:ID="hasBatteryRechargeTime">
    <rdfs:label xml:lang="de">Akkuladezeit</rdfs:label>
    <rdfs:label xml:lang="en">battery recharge time</rdfs:label>
    <belongsToModule xml:lang="en">MP3Player, DigitalCamera, Camcorder</belongsToModule>
    <rdfs:isDefinedBy rdf:resource="http://www.ebusiness-unibw.org/ontologies/consumerelectronics/v1"/>
    <rdfs:comment xml:lang="en">Total time needed to fully recharge a completely discharged rechargeable energy source for this mp3 player (Common unit of measurement hour, HUR).</rdfs:comment>
    <rdfs:range rdf:resource="http://purl.org/goodrelations/v1#QuantitativeValueFloat"/>
    <rdfs:subPropertyOf rdf:resource="http://purl.org/goodrelations/v1#quantitativeProductOrServiceProperty"/>
  </owl:ObjectProperty>  
  <owl:ObjectProperty rdf:ID="hasResponseTime">
    <rdfs:label xml:lang="de">Reaktionszeit</rdfs:label>
    <rdfs:label xml:lang="en">response time</rdfs:label>
    <rdfs:comment xml:lang="en">Defines the time an electronical device needs to react on a signal (Common unit of measurement millisecond, C26).</rdfs:comment>
    <belongsToModule xml:lang="en">TV</belongsToModule>
    <rdfs:range rdf:resource="http://purl.org/goodrelations/v1#QuantitativeValueFloat"/>
    <rdfs:subPropertyOf rdf:resource="http://purl.org/goodrelations/v1#quantitativeProductOrServiceProperty"/>
    <rdfs:isDefinedBy rdf:resource="http://www.ebusiness-unibw.org/ontologies/consumerelectronics/v1"/>
  </owl:ObjectProperty>  
  <owl:DatatypeProperty rdf:ID="hasID3Support">
    <rdfs:subPropertyOf rdf:resource="http://purl.org/goodrelations/v1#datatypeProductOrServiceProperty"/>
    <rdfs:range rdf:resource="http://www.w3.org/2001/XMLSchema#boolean"/>
    <rdfs:isDefinedBy rdf:resource="http://www.ebusiness-unibw.org/ontologies/consumerelectronics/v1"/>
    <rdfs:comment xml:lang="en">Defines the support of information such as the title, artist, album, track number, or other information about the file to be stored in the file itself.</rdfs:comment>
    <rdfs:label xml:lang="de">ID3 Unterstützung</rdfs:label>
    <rdfs:label xml:lang="en">ID3 support</rdfs:label>
    <belongsToModule xml:lang="de">MP3Player</belongsToModule>
  </owl:DatatypeProperty>
  <owl:DatatypeProperty rdf:ID="hasColorBalance">
    <rdfs:isDefinedBy rdf:resource="http://creativecommons.org/licenses/by/3.0/"/>
    <rdfs:range rdf:resource="http://www.w3.org/2001/XMLSchema#boolean"/>
    <belongsToModule xml:lang="en">DigitalCamera</belongsToModule>
    <rdfs:comment xml:lang="en">In photography and image processing, color balance is the global adjustment of the intensities of the colors (typically red, green, and blue primary colors).

(This description is partly based on or reuses content from the Wikipedia article "White balance" (http://en.wikipedia.org/wiki/White_balance) and is licensed under the GNU Free Documentation License (http://www.gnu.org/copyleft/fdl.html).)</rdfs:comment>
    <rdfs:label xml:lang="de">Farbabgleich</rdfs:label>
    <rdfs:label xml:lang="en">color balance</rdfs:label>
    <rdfs:subPropertyOf rdf:resource="http://purl.org/goodrelations/v1#datatypeProductOrServiceProperty"/>
  </owl:DatatypeProperty>
  <owl:DatatypeProperty rdf:ID="hasDigitalZoom">
    <belongsToModule xml:lang="en">DigitalCamera, Camcorder</belongsToModule>
    <rdfs:isDefinedBy rdf:resource="http://www.ebusiness-unibw.org/ontologies/consumerelectronics/v1"/>
    <rdfs:comment xml:lang="en">Zoom is a method of decreasing (narrowing) the apparent angle of view of a photographic or video image.

(This description is partly based on or reuses content from the Wikipedia article "Digital zoom" (http://en.wikipedia.org/wiki/Digital_zoom) and is licensed under the GNU Free Documentation License (http://www.gnu.org/copyleft/fdl.html).)</rdfs:comment>
    <rdfs:label xml:lang="de">digitaler Zoom</rdfs:label>
    <rdfs:label xml:lang="en">digital zoom</rdfs:label>
    <rdfs:subPropertyOf rdf:resource="http://purl.org/goodrelations/v1#datatypeProductOrServiceProperty"/>
    <rdfs:range rdf:resource="http://www.w3.org/2001/XMLSchema#boolean"/>
  </owl:DatatypeProperty>
  <owl:DatatypeProperty rdf:ID="hasExpansionSlot">
    <rdfs:comment xml:lang="en">Defines the ability to add devices (e.g. cards) to maximize the storage capacity.</rdfs:comment>
    <rdfs:isDefinedBy rdf:resource="http://www.ebusiness-unibw.org/ontologies/consumerelectronics/v1"/>
    <belongsToModule xml:lang="en">Camcorder</belongsToModule>
    <rdfs:subPropertyOf rdf:resource="http://purl.org/goodrelations/v1#datatypeProductOrServiceProperty"/>
    <rdfs:label xml:lang="de">Erweiterungsplätze</rdfs:label>
    <rdfs:label xml:lang="en">expansion slot</rdfs:label>
    <rdfs:range rdf:resource="http://www.w3.org/2001/XMLSchema#boolean"/>
  </owl:DatatypeProperty>
  <owl:DatatypeProperty rdf:ID="hasFlash">
    <rdfs:comment xml:lang="en">Device for instantaneous illumination for picture taking.</rdfs:comment>
    <rdfs:subPropertyOf rdf:resource="http://purl.org/goodrelations/v1#datatypeProductOrServiceProperty"/>
    <rdfs:label xml:lang="de">Blitz</rdfs:label>
    <rdfs:label xml:lang="en">flash</rdfs:label>
    <rdfs:isDefinedBy rdf:resource="http://www.ebusiness-unibw.org/ontologies/consumerelectronics/v1"/>
    <belongsToModule xml:lang="en">DigitalCamera</belongsToModule>
    <rdfs:range rdf:resource="http://www.w3.org/2001/XMLSchema#boolean"/>
  </owl:DatatypeProperty>
  <owl:DatatypeProperty rdf:ID="hasOpticalZoom">
    <rdfs:label xml:lang="de">optischer Zoom</rdfs:label>
    <rdfs:label xml:lang="en">optical zoom</rdfs:label>
    <rdfs:range rdf:resource="http://www.w3.org/2001/XMLSchema#boolean"/>
    <belongsToModule xml:lang="en">DigitalCamera</belongsToModule>
    <rdfs:isDefinedBy rdf:resource="http://www.ebusiness-unibw.org/ontologies/consumerelectronics/v1"/>
    <rdfs:comment xml:lang="en">Defines a method of decreasing (narrowing) the apparent angle of view of a digital photographic or video image with a higher optical resolution than the digital zoom.</rdfs:comment>
    <rdfs:subPropertyOf rdf:resource="http://purl.org/goodrelations/v1#datatypeProductOrServiceProperty"/>
  </owl:DatatypeProperty>
  <owl:DatatypeProperty rdf:ID="hasNumberOfComponentVideoPorts">
    <rdfs:isDefinedBy rdf:resource="http://www.ebusiness-unibw.org/ontologies/consumerelectronics/v1"/>
    <rdfs:label xml:lang="de">Anzahl an Component Vido Ports</rdfs:label>
    <rdfs:label xml:lang="en">number of component video ports</rdfs:label>
    <rdfs:subPropertyOf rdf:resource="http://purl.org/goodrelations/v1#datatypeProductOrServiceProperty"/>
    <rdfs:range rdf:resource="http://www.w3.org/2001/XMLSchema#int"/>
    <rdfs:comment xml:lang="en">Defines the number of component video ports a device offers.</rdfs:comment>
    <belongsToModule xml:lang="en">Camcorder</belongsToModule>
  </owl:DatatypeProperty>
  <owl:DatatypeProperty rdf:ID="hasSelfTimer">
    <rdfs:comment xml:lang="en">Defines whether the product is able  to give a delay between the pressing of the shutter release and the shutter firing.</rdfs:comment>
    <rdfs:subPropertyOf rdf:resource="http://purl.org/goodrelations/v1#datatypeProductOrServiceProperty"/>
    <belongsToModule xml:lang="en">DigitalCamera</belongsToModule>
    <rdfs:range rdf:resource="http://www.w3.org/2001/XMLSchema#boolean"/>
    <rdfs:label xml:lang="de">Selbstauslöser</rdfs:label>
    <rdfs:label xml:lang="en">self-timer</rdfs:label>
    <rdfs:isDefinedBy rdf:resource="http://www.ebusiness-unibw.org/ontologies/consumerelectronics/v1"/>
  </owl:DatatypeProperty>
  <owl:DatatypeProperty rdf:ID="hasAspectRatioVertical">
    <rdfs:subPropertyOf rdf:resource="http://purl.org/goodrelations/v1#datatypeProductOrServiceProperty"/>
    <rdfs:range rdf:resource="http://www.w3.org/2001/XMLSchema#float"/>
    <rdfs:isDefinedBy rdf:resource="http://www.ebusiness-unibw.org/ontologies/consumerelectronics/v1"/>
    <rdfs:comment xml:lang="en">The aspect ratio of a shape is the ratio of its longer dimension to its shorter dimension. The vertical dimension is the shorter one.

(This description is partly based on or reuses content from the Wikipedia article "Aspect ratio" (http://en.wikipedia.org/wiki/Aspect_ratio) and is licensed under the GNU Free Documentation License (http://www.gnu.org/copyleft/fdl.html).)</rdfs:comment>
    <belongsToModule xml:lang="en">TV</belongsToModule>
    <rdfs:label xml:lang="de">vertikales Bildseitenverhältnis</rdfs:label>
    <rdfs:label rdf:datatype="http://www.w3.org/2001/XMLSchema#string"
    >aspect ratio vertical</rdfs:label>
  </owl:DatatypeProperty>
  <owl:DatatypeProperty rdf:ID="hasLightExposureControl">
    <rdfs:subPropertyOf rdf:resource="http://purl.org/goodrelations/v1#datatypeProductOrServiceProperty"/>
    <rdfs:label xml:lang="de">Belichtungsregelung</rdfs:label>
    <rdfs:label xml:lang="en">light exposure control</rdfs:label>
    <rdfs:range rdf:resource="http://www.w3.org/2001/XMLSchema#boolean"/>
    <belongsToModule xml:lang="en">Camcorder</belongsToModule>
    <rdfs:isDefinedBy rdf:resource="http://www.ebusiness-unibw.org/ontologies/consumerelectronics/v1"/>
    <rdfs:comment xml:lang="en">Defines the total amount of light allowed to fall on the photographic medium (photographic film or image sensor) during the process of taking a photograph.</rdfs:comment>
  </owl:DatatypeProperty>
  <owl:DatatypeProperty rdf:ID="hasDisplayBrightness">
    <belongsToModule xml:lang="en">TV</belongsToModule>
    <rdfs:subPropertyOf rdf:resource="http://purl.org/goodrelations/v1#datatypeProductOrServiceProperty"/>
    <rdfs:isDefinedBy rdf:resource="http://www.ebusiness-unibw.org/ontologies/consumerelectronics/v1"/>
    <rdfs:label xml:lang="de">Bildhelligkeit</rdfs:label>
    <rdfs:label xml:lang="en">display brightness</rdfs:label>
    <rdfs:range rdf:resource="http://www.w3.org/2001/XMLSchema#float"/>
    <rdfs:comment xml:lang="en">Defines the brightness of a display or screen. Brightness is an attribute of visual perception in which a source appears to be radiating or reflecting light.

(This description is partly based on or reuses content from the Wikipedia article "Brightness" (http://en.wikipedia.org/wiki/Brightness) and is licensed under the GNU Free Documentation License (http://www.gnu.org/copyleft/fdl.html).)</rdfs:comment>
  </owl:DatatypeProperty>
  <owl:DatatypeProperty rdf:ID="has35mmCameraLensEquivalentRange">
    <rdfs:label xml:lang="de">35mm Kameraobjektiv</rdfs:label>
    <rdfs:label xml:lang="en">35mm camera lens equivalent range</rdfs:label>
    <rdfs:isDefinedBy rdf:resource="http://www.ebusiness-unibw.org/ontologies/consumerelectronics/v1"/>
    <belongsToModule xml:lang="en">Camcorder</belongsToModule>
    <rdfs:subPropertyOf rdf:resource="http://purl.org/goodrelations/v1#datatypeProductOrServiceProperty"/>
    <rdfs:range rdf:resource="http://www.w3.org/2001/XMLSchema#boolean"/>
    <rdfs:comment xml:lang="en">Defines an optical lens or assembly of lenses used in conjunction with a camera body and mechanism to make images of objects either on photographic film or on other media capable of storing an image chemically or electronically.</rdfs:comment>
  </owl:DatatypeProperty>
  <owl:DatatypeProperty rdf:ID="hasBatterySize">
    <rdfs:comment xml:lang="en">Defines the size of used energy source. (Use ASIN code here. For more information we refer to http://en.wikipedia.org/wiki/List_of_battery_sizes)</rdfs:comment>
    <rdfs:range rdf:resource="http://www.w3.org/2001/XMLSchema#string"/>
    <rdfs:subPropertyOf rdf:resource="http://purl.org/goodrelations/v1#datatypeProductOrServiceProperty"/>
    <rdfs:isDefinedBy rdf:resource="http://www.ebusiness-unibw.org/ontologies/consumerelectronics/v1"/>
    <belongsToModule xml:lang="en">MP3Player, DigitalCamera, Camcorder</belongsToModule>
    <rdfs:label xml:lang="de">Batteriegröße</rdfs:label>
    <rdfs:label xml:lang="en">battery size</rdfs:label>
  </owl:DatatypeProperty>
  <owl:DatatypeProperty rdf:ID="hasEconomicPrintMode">
    <rdfs:isDefinedBy rdf:resource="http://www.ebusiness-unibw.org/ontologies/consumerelectronics/v1"/>
    <rdfs:label xml:lang="de">Energiespardruckmodus</rdfs:label>
    <rdfs:label xml:lang="en">economic print mode</rdfs:label>
    <rdfs:comment xml:lang="en">Describes whether or not the product is equipped with features that allow economical printing.</rdfs:comment>
    <rdfs:range rdf:resource="http://www.w3.org/2001/XMLSchema#boolean"/>
    <rdfs:subPropertyOf rdf:resource="http://purl.org/goodrelations/v1#datatypeProductOrServiceProperty"/>
    <belongsToModule xml:lang="en">Printer</belongsToModule>
  </owl:DatatypeProperty>
  <owl:DatatypeProperty rdf:ID="hasWallMountability">
    <belongsToModule xml:lang="en">TV</belongsToModule>
    <rdfs:label xml:lang="de">Wandmontagemöglichkeit</rdfs:label>
    <rdfs:label xml:lang="en">wall mountability</rdfs:label>
    <rdfs:comment xml:lang="en">Defines if an object can be installed at a wall.</rdfs:comment>
    <rdfs:range rdf:resource="http://www.w3.org/2001/XMLSchema#boolean"/>
    <rdfs:subPropertyOf rdf:resource="http://purl.org/goodrelations/v1#datatypeProductOrServiceProperty"/>
    <rdfs:isDefinedBy rdf:resource="http://www.ebusiness-unibw.org/ontologies/consumerelectronics/v1"/>
  </owl:DatatypeProperty>
  <owl:DatatypeProperty rdf:ID="hasPictureInPicture">
    <rdfs:isDefinedBy rdf:resource="http://www.ebusiness-unibw.org/ontologies/consumerelectronics/v1"/>
    <rdfs:comment xml:lang="en">Defines that an electronical screen can display minimum two pictures on one screen.</rdfs:comment>
    <belongsToModule xml:lang="en">TV</belongsToModule>
    <rdfs:label xml:lang="de">Bild-in-Bild Funktion</rdfs:label>
    <rdfs:label xml:lang="en">picture in picture</rdfs:label>
    <rdfs:range rdf:resource="http://www.w3.org/2001/XMLSchema#boolean"/>
    <rdfs:subPropertyOf rdf:resource="http://purl.org/goodrelations/v1#datatypeProductOrServiceProperty"/>
  </owl:DatatypeProperty>
  <owl:DatatypeProperty rdf:ID="hasContrastRatio">
    <rdfs:isDefinedBy rdf:resource="http://www.ebusiness-unibw.org/ontologies/consumerelectronics/v1"/>
    <belongsToModule xml:lang="en">TV</belongsToModule>
    <rdfs:subPropertyOf rdf:resource="http://purl.org/goodrelations/v1#datatypeProductOrServiceProperty"/>
    <rdfs:range rdf:resource="http://www.w3.org/2001/XMLSchema#string"/>
    <rdfs:comment xml:lang="en">The contrast ratio is a measure of a display system, defined as the ratio of the luminance of the brightest color (white) to that of the darkest color (black) that the system is capable of producing.

(This description is partly based on or reuses content from the Wikipedia article "Contrast ratio" (http://en.wikipedia.org/wiki/Contrast_ratio) and is licensed under the GNU Free Documentation License (http://www.gnu.org/copyleft/fdl.html).)</rdfs:comment>
    <rdfs:label xml:lang="de">Kontrastverhältnis</rdfs:label>
    <rdfs:label xml:lang="en">contrast ratio</rdfs:label>
  </owl:DatatypeProperty>
  <owl:DatatypeProperty rdf:ID="hasEnvelopeFeeder">
    <rdfs:comment xml:lang="en">Indicates wheter this feature is available on this product.</rdfs:comment>
    <belongsToModule xml:lang="en">Printer</belongsToModule>
    <rdfs:isDefinedBy rdf:resource="http://www.ebusiness-unibw.org/ontologies/consumerelectronics/v1"/>
    <rdfs:subPropertyOf rdf:resource="http://purl.org/goodrelations/v1#datatypeProductOrServiceProperty"/>
    <rdfs:range rdf:resource="http://www.w3.org/2001/XMLSchema#boolean"/>
    <rdfs:label xml:lang="de">Kuvertzuführeinrichtung</rdfs:label>
    <rdfs:label xml:lang="en">envelope feeder</rdfs:label>
  </owl:DatatypeProperty>
  <owl:DatatypeProperty rdf:ID="hasEqualizer">
    <rdfs:label xml:lang="de">Equalizer</rdfs:label>
    <rdfs:label xml:lang="en">Equalizer</rdfs:label>
    <rdfs:comment xml:lang="en">Defines the possibility to vary the audio presentation of sound.</rdfs:comment>
    <belongsToModule xml:lang="en">MP3Player</belongsToModule>
    <rdfs:subPropertyOf rdf:resource="http://purl.org/goodrelations/v1#datatypeProductOrServiceProperty"/>
    <rdfs:range rdf:resource="http://www.w3.org/2001/XMLSchema#boolean"/>
    <rdfs:isDefinedBy rdf:resource="http://www.ebusiness-unibw.org/ontologies/consumerelectronics/v1"/>
  </owl:DatatypeProperty>
  <owl:DatatypeProperty rdf:ID="hasAspectRatioHorizontal">
    <rdfs:isDefinedBy rdf:resource="http://www.ebusiness-unibw.org/ontologies/consumerelectronics/v1"/>
    <rdfs:subPropertyOf rdf:resource="http://purl.org/goodrelations/v1#datatypeProductOrServiceProperty"/>
    <belongsToModule xml:lang="en">TV</belongsToModule>
    <rdfs:comment xml:lang="en">The aspect ratio of a shape is the ratio of its longer dimension to its shorter dimension. The vertical dimension is the longer one.

(This description is partly based on or reuses content from the Wikipedia article "Aspect ratio" (http://en.wikipedia.org/wiki/Aspect_ratio) and is licensed under the GNU Free Documentation License (http://www.gnu.org/copyleft/fdl.html).)</rdfs:comment>
    <rdfs:range rdf:resource="http://www.w3.org/2001/XMLSchema#float"/>
    <rdfs:label xml:lang="de">horizontales Bildseitenverhältnis</rdfs:label>
    <rdfs:label xml:lang="en">aspect ratio horizontal</rdfs:label>
  </owl:DatatypeProperty>
  <owl:DatatypeProperty rdf:ID="hasAnalogVideoSignal">
    <rdfs:comment xml:lang="en">Defines whether an analog video signal is supported.</rdfs:comment>
    <rdfs:isDefinedBy rdf:resource="http://www.ebusiness-unibw.org/ontologies/consumerelectronics/v1"/>
    <rdfs:label xml:lang="de">analoges Videosignal</rdfs:label>
    <rdfs:label xml:lang="en">analog video signal</rdfs:label>
    <belongsToModule xml:lang="en">DigitalCamera</belongsToModule>
    <rdfs:range rdf:resource="http://www.w3.org/2001/XMLSchema#boolean"/>
    <rdfs:subPropertyOf rdf:resource="http://purl.org/goodrelations/v1#datatypeProductOrServiceProperty"/>
  </owl:DatatypeProperty>
  <owl:DatatypeProperty rdf:ID="hasDisplay">
    <belongsToModule xml:lang="en">MP3Player, Printer, DigitalCamera, Camcorder</belongsToModule>
    <rdfs:label xml:lang="de">Bildschirm</rdfs:label>
    <rdfs:label xml:lang="en">display</rdfs:label>
    <rdfs:range rdf:resource="http://www.w3.org/2001/XMLSchema#boolean"/>
    <rdfs:isDefinedBy rdf:resource="http://www.ebusiness-unibw.org/ontologies/consumerelectronics/v1"/>
    <rdfs:comment xml:lang="en">Defines if object includes a screen.</rdfs:comment>
    <rdfs:subPropertyOf rdf:resource="http://purl.org/goodrelations/v1#datatypeProductOrServiceProperty"/>
  </owl:DatatypeProperty>
  <owl:DatatypeProperty rdf:ID="hasRedEyeReduction">
    <rdfs:subPropertyOf rdf:resource="http://purl.org/goodrelations/v1#datatypeProductOrServiceProperty"/>
    <rdfs:range rdf:resource="http://www.w3.org/2001/XMLSchema#boolean"/>
    <rdfs:isDefinedBy rdf:resource="http://www.ebusiness-unibw.org/ontologies/consumerelectronics/v1"/>
    <rdfs:comment xml:lang="en">The red-eye effect in photography is the common appearance of red pupils in color photographs of eyes. The red-eye reduction feature reduces the red-eye effect.</rdfs:comment>
    <belongsToModule xml:lang="en">DigitalCamera</belongsToModule>
    <rdfs:label xml:lang="de">Rote-Augen-Effekt Reduktion</rdfs:label>
    <rdfs:label xml:lang="en">red eye reduction</rdfs:label>
  </owl:DatatypeProperty>
  <owl:DatatypeProperty rdf:ID="hasNetworkAbility">
    <rdfs:comment xml:lang="en">Ability to connect the product to a network.</rdfs:comment>
    <rdfs:isDefinedBy rdf:resource="http://www.ebusiness-unibw.org/ontologies/consumerelectronics/v1"/>
    <rdfs:label xml:lang="de">Netzwerkfähigkeit</rdfs:label>
    <rdfs:label xml:lang="en">network ability</rdfs:label>
    <rdfs:subPropertyOf rdf:resource="http://purl.org/goodrelations/v1#datatypeProductOrServiceProperty"/>
    <rdfs:range rdf:resource="http://www.w3.org/2001/XMLSchema#boolean"/>
  </owl:DatatypeProperty>
  <owl:DatatypeProperty rdf:ID="hasTouchscreen">
    <rdfs:subPropertyOf rdf:resource="http://purl.org/goodrelations/v1#datatypeProductOrServiceProperty"/>
    <belongsToModule xml:lang="en">MP3Player, Printer, DigitalCamera, Camcorder</belongsToModule>
    <rdfs:comment xml:lang="en">Defines the ability to operate an object by touching its screen.</rdfs:comment>
    <rdfs:isDefinedBy rdf:resource="http://www.ebusiness-unibw.org/ontologies/consumerelectronics/v1"/>
    <rdfs:range rdf:resource="http://www.w3.org/2001/XMLSchema#boolean"/>
    <rdfs:label xml:lang="de">Sensorbildschirm</rdfs:label>
    <rdfs:label xml:lang="en">touch screen</rdfs:label>
  </owl:DatatypeProperty>
  <owl:DatatypeProperty rdf:ID="hasVideoResolution">
    <rdfs:range rdf:resource="http://www.w3.org/2001/XMLSchema#string"/>
    <rdfs:label xml:lang="de">Videoauflösung</rdfs:label>
    <rdfs:label xml:lang="en">video resolution</rdfs:label>
    <belongsToModule xml:lang="en">DigitalCamera, Camcorder</belongsToModule>
    <rdfs:subPropertyOf rdf:resource="http://purl.org/goodrelations/v1#datatypeProductOrServiceProperty"/>
    <rdfs:isDefinedBy rdf:resource="http://www.ebusiness-unibw.org/ontologies/consumerelectronics/v1"/>
    <rdfs:comment xml:lang="en">Defines the digital resolution of the videos (Common unit of measurement pixel, E37). (Example: 1024x768)</rdfs:comment>
  </owl:DatatypeProperty>
  <owl:DatatypeProperty rdf:ID="hasDRMSupport">
    <rdfs:subPropertyOf rdf:resource="http://purl.org/goodrelations/v1#datatypeProductOrServiceProperty"/>
    <rdfs:isDefinedBy rdf:resource="http://www.ebusiness-unibw.org/ontologies/consumerelectronics/v1"/>
    <rdfs:comment xml:lang="en">Defines the support of a generic term that refers to access control technologies used by hardware manufacturers.</rdfs:comment>
    <rdfs:label xml:lang="de">DRM Unterstützung</rdfs:label>
    <rdfs:label xml:lang="en">DRM support</rdfs:label>
    <belongsToModule xml:lang="en">MP3Player</belongsToModule>
    <rdfs:range rdf:resource="http://www.w3.org/2001/XMLSchema#boolean"/>
  </owl:DatatypeProperty>
  <owl:DatatypeProperty rdf:ID="hasAudioInputSource">
    <rdfs:isDefinedBy rdf:resource="http://www.ebusiness-unibw.org/ontologies/consumerelectronics/v1"/>
    <rdfs:subPropertyOf rdf:resource="http://purl.org/goodrelations/v1#datatypeProductOrServiceProperty"/>
    <rdfs:comment xml:lang="en">Defines which audio input devices can be used with this object.</rdfs:comment>
    <rdfs:label xml:lang="de">Audioeingang</rdfs:label>
    <rdfs:label xml:lang="en">audio input source</rdfs:label>
    <belongsToModule xml:lang="en">DigitalCamera</belongsToModule>
    <rdfs:range rdf:resource="http://www.w3.org/2001/XMLSchema#boolean"/>
  </owl:DatatypeProperty>
  <gr:BusinessEntity rdf:ID="Nikon">
    <rdfs:comment xml:lang="en">The business entity Nikon Corporation.</rdfs:comment>
    <belongsToModule xml:lang="en">DigitalCamera</belongsToModule>
    <rdfs:seeAlso rdf:resource="http://www.nikon.com/"/>
    <gr:legalName rdf:datatype="http://www.w3.org/2001/XMLSchema#string"
    >Nikon Corporation</gr:legalName>
    <rdfs:label rdf:datatype="http://www.w3.org/2001/XMLSchema#string"
    >Nikon</rdfs:label>
  </gr:BusinessEntity>
  <gr:BusinessEntity rdf:ID="Phoenix">
    <rdfs:label rdf:datatype="http://www.w3.org/2001/XMLSchema#string"
    >Phoenix</rdfs:label>
    <belongsToModule xml:lang="en">Camcorder</belongsToModule>
    <rdfs:seeAlso rdf:resource="http://www.phoenixcontact.com/"/>
    <rdfs:comment xml:lang="en">The business entity Phoenix.</rdfs:comment>
    <gr:legalName rdf:datatype="http://www.w3.org/2001/XMLSchema#string"
    >Phoenix Contact GmbH Co. KG</gr:legalName>
  </gr:BusinessEntity>
  <gr:BusinessEntity rdf:ID="MPIO">
    <belongsToModule xml:lang="en">MP3Player</belongsToModule>
    <rdfs:label rdf:datatype="http://www.w3.org/2001/XMLSchema#string"
    >MPIO</rdfs:label>
    <rdfs:seeAlso rdf:resource="http://www.mpio.com/"/>
    <gr:legalName rdf:datatype="http://www.w3.org/2001/XMLSchema#string"
    >MPIO Inc.</gr:legalName>
    <rdfs:comment xml:lang="en">The business entity MPIO Inc.</rdfs:comment>
  </gr:BusinessEntity>
  <gr:BusinessEntity rdf:ID="Oppo">
    <rdfs:label rdf:datatype="http://www.w3.org/2001/XMLSchema#string"
    >Oppo</rdfs:label>
    <rdfs:comment xml:lang="en">The business entity Oppo.</rdfs:comment>
    <belongsToModule xml:lang="en">TV</belongsToModule>
    <gr:legalName rdf:datatype="http://www.w3.org/2001/XMLSchema#string"
    >Elmarc BV</gr:legalName>
    <rdfs:seeAlso rdf:resource="http://www.oppo.nl/"/>
  </gr:BusinessEntity>
  <DataFormatVideo rdf:ID="MPEG">
    <rdfs:label xml:lang="en">MPEG</rdfs:label>
    <rdfs:label xml:lang="de">MPEG</rdfs:label>
    <rdfs:comment xml:lang="en">Includes all kinds of MPEG formats.</rdfs:comment>
    <belongsToModule xml:lang="en">MP3Player, DigitalCamera, Camcorder</belongsToModule>
  </DataFormatVideo>
  <CompatibleOperatingSystems rdf:ID="Linux">
    <belongsToModule xml:lang="en">MP3Player, Printer, DigitalCamera, Camcorder</belongsToModule>
    <rdfs:label xml:lang="en">Linux</rdfs:label>
    <rdfs:label xml:lang="de">Linux</rdfs:label>
    <rdfs:comment xml:lang="en">Linux is a generic term commonly used to refer to Unix-like computer operating systems which use the Linux kernel.</rdfs:comment>
  </CompatibleOperatingSystems>
  <gr:BusinessEntity rdf:ID="Toshiba">
    <gr:legalName rdf:datatype="http://www.w3.org/2001/XMLSchema#string"
    >Toshiba Corporation</gr:legalName>
    <rdfs:seeAlso rdf:resource="http://www.toshiba.com/"/>
    <rdfs:comment xml:lang="en">The business entity Toshiba Corporation.</rdfs:comment>
    <rdfs:label rdf:datatype="http://www.w3.org/2001/XMLSchema#string"
    >Toshiba</rdfs:label>
    <belongsToModule xml:lang="en">MP3Player, TV, DigitalCamera, Camcorder</belongsToModule>
  </gr:BusinessEntity>
  <gr:BusinessEntity rdf:ID="Dane-Elec">
    <rdfs:seeAlso rdf:resource="http://www.dane-elec.com/"/>
    <rdfs:comment xml:lang="en">The business entity Dane-Elec GmbH.</rdfs:comment>
    <rdfs:label rdf:datatype="http://www.w3.org/2001/XMLSchema#string"
    >Dane-Elec</rdfs:label>
    <gr:legalName rdf:datatype="http://www.w3.org/2001/XMLSchema#string"
    >Dane-Elec GmbH</gr:legalName>
    <belongsToModule xml:lang="en">MP3Player</belongsToModule>
  </gr:BusinessEntity>
  <gr:BusinessEntity rdf:ID="Ricoh">
    <rdfs:label rdf:datatype="http://www.w3.org/2001/XMLSchema#string"
    >Ricoh</rdfs:label>
    <rdfs:comment xml:lang="en">The business entity Ricoh.</rdfs:comment>
    <belongsToModule xml:lang="en">Printer, DigitalCamera</belongsToModule>
    <rdfs:seeAlso rdf:resource="http://www.ebusiness-unibw.org/ontologies/consumerelectronics/v1"/>
    <gr:legalName rdf:datatype="http://www.w3.org/2001/XMLSchema#string"
    >Ricoh Company, Ltd.</gr:legalName>
  </gr:BusinessEntity>
  <DataInterfaceType rdf:ID="USB2.0">
    <rdfs:comment xml:lang="en">Maximum speed of 480 Mbit/s.</rdfs:comment>
    <rdfs:label xml:lang="en">USB 2.0</rdfs:label>
    <rdfs:label xml:lang="de">USB 2.0</rdfs:label>
    <belongsToModule xml:lang="en">MP3Player, TV, Printer, DigitalCamera, Camcorder</belongsToModule>
  </DataInterfaceType>
  <gr:BusinessEntity rdf:ID="Tatung">
    <rdfs:label rdf:datatype="http://www.w3.org/2001/XMLSchema#string"
    >Tatung</rdfs:label>
    <belongsToModule xml:lang="en">MP3Player, TV</belongsToModule>
    <gr:legalName rdf:datatype="http://www.w3.org/2001/XMLSchema#string"
    >Tatung Co.</gr:legalName>
    <rdfs:comment xml:lang="en">The business entity Tatung Co.</rdfs:comment>
    <rdfs:seeAlso rdf:resource="http://www.tatung.com/"/>
  </gr:BusinessEntity>
  <GeneralFeatures rdf:ID="TeletextFunction">
    <rdfs:label xml:lang="de">Teletext Funktion</rdfs:label>
    <rdfs:label xml:lang="en">Teletext function</rdfs:label>
    <rdfs:comment xml:lang="en">Teletext (or "broadcast Teletext") is a television information retrieval service developed in the United Kingdom in the early 1970s. It offers a range of text-based information, typically including national, international and sporting news, weather and TV schedules.

(This description is partly based on or reuses content from the Wikipedia article "Teletext" (http://en.wikipedia.org/wiki/Teletext) and is licensed under the GNU Free Documentation License (http://www.gnu.org/copyleft/fdl.html).)</rdfs:comment>
    <belongsToModule xml:lang="en">TV</belongsToModule>
  </GeneralFeatures>
  <Features rdf:ID="FaceIdendification">
    <rdfs:label xml:lang="de">Gesichtserkennung</rdfs:label>
    <rdfs:label xml:lang="en">Face identification</rdfs:label>
    <belongsToModule xml:lang="en">DigitalCamera, Camcorder</belongsToModule>
    <rdfs:comment xml:lang="en">Ability to identify the face and to justify the picture to it.</rdfs:comment>
  </Features>
  <VideoFeatures rdf:ID="CombFilter">
    <rdfs:label xml:lang="en">Comb filter</rdfs:label>
    <rdfs:label xml:lang="de">Comb Filter</rdfs:label>
    <rdfs:comment xml:lang="en">In signal processing, a comb filter adds a delayed version of a signal to itself, causing constructive and destructive interference. The frequency response of a comb filter consists of a series of regularly-spaced spikes, giving the appearance of a comb.

(This description is partly based on or reuses content from the Wikipedia article "Comb filter" (http://en.wikipedia.org/wiki/Comb_filter) and is licensed under the GNU Free Documentation License (http://www.gnu.org/copyleft/fdl.html).)</rdfs:comment>
    <belongsToModule xml:lang="en">TV</belongsToModule>
  </VideoFeatures>
  <gr:BusinessEntity rdf:ID="Griffin">
    <belongsToModule xml:lang="en">MP3Player</belongsToModule>
    <rdfs:comment xml:lang="en">The business entity Griffin Technology.</rdfs:comment>
    <rdfs:label rdf:datatype="http://www.w3.org/2001/XMLSchema#string"
    >Griffin</rdfs:label>
    <rdfs:seeAlso rdf:resource="http://www.griffintechnology.com/"/>
    <gr:legalName rdf:datatype="http://www.w3.org/2001/XMLSchema#string"
    >Griffin Technology</gr:legalName>
  </gr:BusinessEntity>
  <DataFormatVideo rdf:ID="AVI">
    <belongsToModule xml:lang="en">MP3Player, DigitalCamera, Camcorder</belongsToModule>
    <rdfs:comment xml:lang="en">A multimedia container format introduced by Microsoft.</rdfs:comment>
    <rdfs:label xml:lang="en">AVI</rdfs:label>
    <rdfs:label rdf:datatype="http://www.w3.org/2001/XMLSchema#string"
    >AVI</rdfs:label>
  </DataFormatVideo>
  <gr:BusinessEntity rdf:ID="Sanyo">
    <rdfs:seeAlso rdf:resource="http://sanyo.com/"/>
    <rdfs:label rdf:datatype="http://www.w3.org/2001/XMLSchema#string"
    >Sanyo</rdfs:label>
    <rdfs:comment xml:lang="en">The business entity Sanyo.</rdfs:comment>
    <belongsToModule xml:lang="en">TV, DigitalCamera, Camcorder</belongsToModule>
    <gr:legalName rdf:datatype="http://www.w3.org/2001/XMLSchema#string"
    >SANYO Electric Co., Ltd.</gr:legalName>
  </gr:BusinessEntity>
  <DataInterfaceType rdf:ID="USB1.0">
    <rdfs:label xml:lang="en">USB 1.0</rdfs:label>
    <rdfs:label xml:lang="de">USB 1.0</rdfs:label>
    <rdfs:comment xml:lang="en">Specified data rates of 1.5 Mbit/s and 12 Mbit/s.</rdfs:comment>
    <belongsToModule xml:lang="en">MP3Player, TV, Printer, DigitalCamera, Camcorder</belongsToModule>
  </DataInterfaceType>
  <gr:BusinessEntity rdf:ID="Samsung">
    <gr:legalName rdf:datatype="http://www.w3.org/2001/XMLSchema#string"
    >Samsung Group</gr:legalName>
    <rdfs:seeAlso rdf:resource="http://www.samsung.com/"/>
    <rdfs:label rdf:datatype="http://www.w3.org/2001/XMLSchema#string"
    >Samsung</rdfs:label>
    <rdfs:comment xml:lang="en">The business entity Samsung Group.</rdfs:comment>
    <belongsToModule xml:lang="en">MP3Player, TV, Printer, DigitalCamera, Camcorder</belongsToModule>
  </gr:BusinessEntity>
  <DisplayType rdf:ID="LCD">
    <rdfs:comment xml:lang="en">A liquid crystal display (LCD) is an electronically-modulated optical device shaped into a thin, flat panel made up of any number of color or monochrome pixels filled with liquid crystals and arrayed in front of a light source (backlight) or reflector.

(This description is partly based on or reuses content from the Wikipedia article "Liquid crystal display" (http://en.wikipedia.org/wiki/Liquid_crystal_display) and is licensed under the GNU Free Documentation License (http://www.gnu.org/copyleft/fdl.html).)</rdfs:comment>
    <rdfs:label xml:lang="en">LCD</rdfs:label>
    <rdfs:label xml:lang="de">LCD</rdfs:label>
    <belongsToModule xml:lang="en">TV, Camcorder</belongsToModule>
  </DisplayType>
  <AudioFeatures rdf:ID="SmartSoundControl">
    <rdfs:label xml:lang="en">SmartSound control</rdfs:label>
    <rdfs:label xml:lang="de">SmartSound control</rdfs:label>
    <rdfs:comment xml:lang="en">SmartSound’s technology benefits television producers and editors by giving enhanced creative options through special music technology that delivers multiple musical variations for different moods.</rdfs:comment>
    <belongsToModule xml:lang="en">TV</belongsToModule>
  </AudioFeatures>
  <GeneralFeatures rdf:ID="EPG">
    <belongsToModule xml:lang="en">TV</belongsToModule>
    <rdfs:comment xml:lang="en">An electronic program(me) guide (EPG) or interactive program(me) guide (IPG) or electronic service guide (ESG) is an digital guide to scheduled broadcast television or radio programs, typically displayed on-screen with functions allowing a viewer to navigate, select, and discover content by time, title, channel, genre, etc. by use of their remote control, a keyboard, or other input devices such as a phone keypad.

(This description is partly based on or reuses content from the Wikipedia article "Electronic program guide" (http://en.wikipedia.org/wiki/Electronic_program_guide) and is licensed under the GNU Free Documentation License (http://www.gnu.org/copyleft/fdl.html).)</rdfs:comment>
    <rdfs:label xml:lang="en">EPG</rdfs:label>
    <rdfs:label xml:lang="de">EPG</rdfs:label>
  </GeneralFeatures>
  <gr:BusinessEntity rdf:ID="Pacific_Digital">
    <rdfs:label rdf:datatype="http://www.w3.org/2001/XMLSchema#string"
    >Pacific Digital</rdfs:label>
    <rdfs:seeAlso rdf:resource="http://www.pacificdigitalhome.com/"/>
    <rdfs:comment xml:lang="en">The business entity Pacific Digital Home.</rdfs:comment>
    <gr:legalName rdf:datatype="http://www.w3.org/2001/XMLSchema#string"
    >Pacific Digital Home</gr:legalName>
    <belongsToModule xml:lang="en">MP3Player</belongsToModule>
  </gr:BusinessEntity>
  <Connectivity rdf:ID="SCART">
    <rdfs:comment xml:lang="en">SCART (from Syndicat des Constructeurs d'Appareils Radiorécepteurs et Téléviseurs, Radio and Television Receiver Manufacturer's Association) is a French-originated standard and associated 21-pin connector for connecting audio-visual (AV) equipment together.

(This description is partly based on or reuses content from the Wikipedia article "SCART" (http://en.wikipedia.org/wiki/SCART) and is licensed under the GNU Free Documentation License (http://www.gnu.org/copyleft/fdl.html).)</rdfs:comment>
    <rdfs:label xml:lang="en">SCART</rdfs:label>
    <rdfs:label xml:lang="de">SCART</rdfs:label>
    <belongsToModule xml:lang="en">TV</belongsToModule>
  </Connectivity>
  <GeneralFeatures rdf:ID="GameMode">
    <rdfs:comment xml:lang="en">A special mode providing more performance of the television to optimize pictures when games are played on a LCD or plasma panel.</rdfs:comment>
    <rdfs:label xml:lang="de">Spielemodus</rdfs:label>
    <rdfs:label xml:lang="en">Game mode</rdfs:label>
    <belongsToModule xml:lang="en">TV</belongsToModule>
  </GeneralFeatures>
  <StorageMedia rdf:ID="InternalHDD">
    <belongsToModule xml:lang="en">MP3Player, DigitalCamera, Camcorder</belongsToModule>
    <rdfs:comment xml:lang="en">Hard disk drive, a computer device which stores digitally encoded data.</rdfs:comment>
    <rdfs:label xml:lang="de">Interne HDD</rdfs:label>
    <rdfs:label xml:lang="en">Internal HDD</rdfs:label>
  </StorageMedia>
  <Connectivity rdf:ID="CVBS_out">
    <rdfs:label xml:lang="en">CVBS out</rdfs:label>
    <rdfs:label xml:lang="de">CVBS out</rdfs:label>
    <belongsToModule xml:lang="en">TV</belongsToModule>
    <rdfs:comment xml:lang="en">Composite video is often designated by the CVBS acronym, meaning any of "Color, Video, Blank and Sync", "Composite Video Baseband Signal", "Composite Video Burst Signal", or "Composite Video with Burst and Sync". Here the output is meant.</rdfs:comment>
  </Connectivity>
  <gr:BusinessEntity rdf:ID="Grundig">
    <rdfs:comment xml:lang="en">The business entity GRUNDIG Intermedia GmbH.</rdfs:comment>
    <gr:legalName rdf:datatype="http://www.w3.org/2001/XMLSchema#string"
    >GRUNDIG Intermedia GmbH </gr:legalName>
    <belongsToModule xml:lang="en">MP3Player, TV</belongsToModule>
    <rdfs:label rdf:datatype="http://www.w3.org/2001/XMLSchema#string"
    >Grundig</rdfs:label>
    <rdfs:seeAlso rdf:resource="http://www.grundig.de/"/>
  </gr:BusinessEntity>
  <SceneMode rdf:ID="Portrait">
    <rdfs:comment xml:lang="en">Ability of the camcorder to adapt to special environments.</rdfs:comment>
    <belongsToModule xml:lang="en">Camcorder</belongsToModule>
    <rdfs:label xml:lang="en">Portrait</rdfs:label>
    <rdfs:label xml:lang="de">Portrait</rdfs:label>
  </SceneMode>
  <MediaType rdf:ID="Envelope">
    <belongsToModule xml:lang="en">Printer</belongsToModule>
    <rdfs:label xml:lang="en">Envelope</rdfs:label>
    <rdfs:label xml:lang="de">Briefkuvert</rdfs:label>
    <rdfs:comment xml:lang="en">Is a packaging product, usually made of flat material such as paper or cardboard.</rdfs:comment>
  </MediaType>
  <MediaFormat rdf:ID="A5">
    <rdfs:label xml:lang="de">A5</rdfs:label>
    <rdfs:label xml:lang="en">A5</rdfs:label>
    <rdfs:comment xml:lang="en">Format of the german institute for standardization: 148 x 210 mm.</rdfs:comment>
    <belongsToModule xml:lang="en">Printer</belongsToModule>
  </MediaFormat>
  <Features rdf:ID="RedEyeReduction">
    <rdfs:label xml:lang="de">Rote-Augen-Effekt Reduktion</rdfs:label>
    <rdfs:label xml:lang="en">Red eye reduction</rdfs:label>
    <belongsToModule xml:lang="en">Camcorder</belongsToModule>
    <rdfs:comment xml:lang="en">Defines the ability to precede the flash with a series of short, low-power flashes, or a continuous piercing bright light triggering the iris to contract.</rdfs:comment>
  </Features>
  <DataInterfaceType rdf:ID="USB3.0">
    <rdfs:comment xml:lang="en">Maximum speed of 4,8 Gbit/s.</rdfs:comment>
    <belongsToModule xml:lang="en">MP3Player, TV, Printer, DigitalCamera, Camcorder</belongsToModule>
    <rdfs:label xml:lang="en">USB 3.0</rdfs:label>
    <rdfs:label xml:lang="de">USB 3.0</rdfs:label>
  </DataInterfaceType>
  <gr:BusinessEntity rdf:ID="Aiwa">
    <gr:legalName rdf:datatype="http://www.w3.org/2001/XMLSchema#string"
    >Sony Corporation  </gr:legalName>
    <belongsToModule xml:lang="en">MP3Player</belongsToModule>
    <rdfs:seeAlso rdf:resource="http://www.aiwa.com/"/>
    <rdfs:comment xml:lang="en">The business entity Sony Corporation.</rdfs:comment>
    <rdfs:label rdf:datatype="http://www.w3.org/2001/XMLSchema#string"
    >Aiwa</rdfs:label>
  </gr:BusinessEntity>
  <DisplayType rdf:ID="Monochrome">
    <belongsToModule xml:lang="en">MP3Player</belongsToModule>
    <rdfs:label xml:lang="en">Monochrome</rdfs:label>
    <rdfs:label xml:lang="de">Monochrom</rdfs:label>
    <rdfs:comment xml:lang="en">Ability to display just two colors (black/white).</rdfs:comment>
  </DisplayType>
  <VideoFeatures rdf:ID="FullHD">
    <rdfs:comment xml:lang="en">Usually assumes a widescreen aspect ratio of 16:9, implying a horizontal resolution of 1920 pixels. This creates a frame resolution of 1920×1080, or 2,073,600 pixels in total.

(This description is partly based on or reuses content from the Wikipedia article "1080p" (http://en.wikipedia.org/wiki/1080p) and is licensed under the GNU Free Documentation License (http://www.gnu.org/copyleft/fdl.html).)</rdfs:comment>
    <rdfs:label xml:lang="en">Full HD</rdfs:label>
    <rdfs:label xml:lang="de">Full HD</rdfs:label>
    <belongsToModule xml:lang="en">TV</belongsToModule>
  </VideoFeatures>
  <Connectivity rdf:ID="RGB">
    <belongsToModule xml:lang="en">TV</belongsToModule>
    <rdfs:label xml:lang="en">RGB</rdfs:label>
    <rdfs:label xml:lang="de">RGB</rdfs:label>
    <rdfs:comment xml:lang="en">The RGB color model is an additive color model in which red, green, and blue light are added together in various ways to reproduce a broad array of colors. The name of the model comes from the initials of the three additive primary colors, red, green, and blue. Typical RGB input devices are color TV and video cameras, image scanners, and digital cameras. Typical RGB output devices are TV sets of various technologies (CRT, LCD, plasma, etc.), computer and mobile phone displays, video projectors, multicolor LED displays, and large screens as JumboTron, etc. Color printers, on the other hand, are usually not RGB devices, but subtractive color devices (typically CMYK color model).

(This description is partly based on or reuses content from the Wikipedia article "RGB" (http://en.wikipedia.org/wiki/RGB) and is licensed under the GNU Free Documentation License (http://www.gnu.org/copyleft/fdl.html).)</rdfs:comment>
  </Connectivity>
  <DataFormatVideo rdf:ID="MOV">
    <rdfs:label xml:lang="en">MOV</rdfs:label>
    <rdfs:label xml:lang="de">MOV</rdfs:label>
    <belongsToModule xml:lang="en">MP3Player, DigitalCamera, Camcorder</belongsToModule>
    <rdfs:comment xml:lang="en">The QuickTime (.mov) file format functions as a multimedia container file that contains one or more tracks, each of which stores a particular type of data: audio, video, effects, or text (e.g. for subtitles).

(This description is partly based on or reuses content from the Wikipedia article "QuickTime" (http://en.wikipedia.org/wiki/QuickTime) and is licensed under the GNU Free Documentation License (http://www.gnu.org/copyleft/fdl.html).)</rdfs:comment>
  </DataFormatVideo>
  <AudioFeatures rdf:ID="Equalizer">
    <rdfs:label xml:lang="en">Equalizer</rdfs:label>
    <rdfs:label xml:lang="de">Equalizer</rdfs:label>
    <rdfs:comment xml:lang="en">Equalization, equalisation or EQ is the process of using passive or active electronic elements or digital algorithms for the purpose of altering (originally flattening) the frequency response characteristics of a system.

(This description is partly based on or reuses content from the Wikipedia article "Equalization" (http://en.wikipedia.org/wiki/Equalization) and is licensed under the GNU Free Documentation License (http://www.gnu.org/copyleft/fdl.html).)</rdfs:comment>
    <belongsToModule xml:lang="en">TV</belongsToModule>
  </AudioFeatures>
  <Color rdf:ID="Navy">
    <rdfs:label xml:lang="en">Navy</rdfs:label>
    <rdfs:label xml:lang="de">Marineblau</rdfs:label>
    <rdfs:comment xml:lang="en">RGB Value 0,0,128</rdfs:comment>
    <belongsToModule xml:lang="en">MP3Player, TV, Printer, DigitalCamera, Camcorder</belongsToModule>
  </Color>
  <VideoFeatures rdf:ID="PixelPlusHD">
    <belongsToModule xml:lang="en">TV</belongsToModule>
    <rdfs:comment xml:lang="en">Pixel Plus HD is a picture processing technology that enables viewers to watch content that is vivid, natural and real.</rdfs:comment>
    <rdfs:label xml:lang="en">Pixel Plus HD</rdfs:label>
    <rdfs:label xml:lang="de">Pixel Plus HD</rdfs:label>
  </VideoFeatures>
  <MediaFormat rdf:ID="A3">
    <belongsToModule xml:lang="en">Printer</belongsToModule>
    <rdfs:label xml:lang="de">A3</rdfs:label>
    <rdfs:label xml:lang="en">A3</rdfs:label>
    <rdfs:comment xml:lang="en">Format of the german institute for standardization: 297 x 420 mm.</rdfs:comment>
  </MediaFormat>
  <gr:BusinessEntity rdf:ID="TallyGenicom">
    <rdfs:label rdf:datatype="http://www.w3.org/2001/XMLSchema#string"
    >TallyGenicom</rdfs:label>
    <belongsToModule xml:lang="en">Printer</belongsToModule>
    <rdfs:seeAlso rdf:resource="http://www.tallygenicom.com/"/>
    <gr:legalName rdf:datatype="http://www.w3.org/2001/XMLSchema#string"
    >TallyGenicom</gr:legalName>
    <rdfs:comment xml:lang="en">The business entity TallyGenicom.</rdfs:comment>
  </gr:BusinessEntity>
  <TVDisplayResolution rdf:ID="HDTV_1080p">
    <rdfs:comment xml:lang="en">1080p is the shorthand name for a category of HDTV video modes. The number "1080" represents 1,080 lines of vertical resolution (1080 horizontal scan lines), while the letter p stands for progressive scan (meaning the image is not interlaced). 1080p can be referred to as full HD or full high definition to differentiate it from other HDTV video modes.

(This description is partly based on or reuses content from the Wikipedia article "1080p" (http://en.wikipedia.org/wiki/1080p) and is licensed under the GNU Free Documentation License (http://www.gnu.org/copyleft/fdl.html).)</rdfs:comment>
    <rdfs:label xml:lang="de">HDTV 1080p</rdfs:label>
    <rdfs:label xml:lang="en">HDTV 1080p</rdfs:label>
    <belongsToModule xml:lang="en">TV</belongsToModule>
  </TVDisplayResolution>
  <SignalFormat rdf:ID="UHF">
    <rdfs:comment xml:lang="en">Ultra high frequency (UHF) designates a range (band) of electromagnetic waves with frequencies between 300 MHz and 3 GHz (3,000 MHz).

(This description is partly based on or reuses content from the Wikipedia article "UHF" (http://en.wikipedia.org/wiki/UHF) and is licensed under the GNU Free Documentation License (http://www.gnu.org/copyleft/fdl.html).)</rdfs:comment>
    <rdfs:label xml:lang="en">UHF</rdfs:label>
    <rdfs:label xml:lang="de">VHF</rdfs:label>
    <belongsToModule xml:lang="en">TV</belongsToModule>
  </SignalFormat>
  <DataFormatImage rdf:ID="PNG">
    <belongsToModule xml:lang="en">MP3Player, DigitalCamera, Camcorder</belongsToModule>
    <rdfs:comment xml:lang="en">The PNG (Portable Network Graphics) file format was created as the free, open-source successor to the GIF.

(This description is partly based on or reuses content from the Wikipedia article "Graphics file format" (http://en.wikipedia.org/wiki/Graphics_file_format) and is licensed under the GNU Free Documentation License (http://www.gnu.org/copyleft/fdl.html).)</rdfs:comment>
    <rdfs:label xml:lang="en">PNG</rdfs:label>
    <rdfs:label xml:lang="de">PNG</rdfs:label>
  </DataFormatImage>
  <CompatibleOperatingSystems rdf:ID="MacOSXJaguar">
    <rdfs:label xml:lang="en">Mac OS X Jaguar</rdfs:label>
    <rdfs:label xml:lang="de">Mac OS X Jaguar</rdfs:label>
    <rdfs:comment xml:lang="en">Mac OS is the trademarked name for a series of graphical user interface-based operating systems developed by Apple Inc. for their Macintosh line of computer systems.</rdfs:comment>
    <belongsToModule xml:lang="en">MP3Player, Printer, DigitalCamera, Camcorder</belongsToModule>
  </CompatibleOperatingSystems>
  <gr:BusinessEntity rdf:ID="TwinMOS">
    <rdfs:seeAlso rdf:resource="http://www.twinmos.com/"/>
    <rdfs:comment xml:lang="en">The business entity TwinMOS Technologies Inc</rdfs:comment>
    <belongsToModule xml:lang="en">MP3Player</belongsToModule>
    <gr:legalName rdf:datatype="http://www.w3.org/2001/XMLSchema#string"
    >TwinMOS Technologies Inc</gr:legalName>
    <rdfs:label rdf:datatype="http://www.w3.org/2001/XMLSchema#string"
    >TwinMOS</rdfs:label>
  </gr:BusinessEntity>
  <Connectivity rdf:ID="SubwooferOut">
    <belongsToModule xml:lang="en">TV</belongsToModule>
    <rdfs:comment xml:lang="en">A connection port for a subwoover. Subwoofer is a woofer, or a complete loudspeaker dedicated to the reproduction of bass audio frequencies, from perhaps 150 Hz down as far as 20 Hz, or in rare cases lower.

(This description is partly based on or reuses content from the Wikipedia article "Subwoofer" (http://en.wikipedia.org/wiki/Subwoofer) and is licensed under the GNU Free Documentation License (http://www.gnu.org/copyleft/fdl.html).)</rdfs:comment>
    <rdfs:label xml:lang="en">Subwoofer out</rdfs:label>
    <rdfs:label xml:lang="de">Subwoofer out</rdfs:label>
  </Connectivity>
  <VideoFeatures rdf:ID="Acuity">
    <belongsToModule xml:lang="en">TV</belongsToModule>
    <rdfs:comment xml:lang="en">Is acuteness or clearness of vision, especially form vision, which is dependent on the sharpness of the retinal focus within the eye and the sensitivity of the interpretative faculty of the brain.

(This description is partly based on or reuses content from the Wikipedia article "Visual acuity" (http://en.wikipedia.org/wiki/Visual_acuity) and is licensed under the GNU Free Documentation License (http://www.gnu.org/copyleft/fdl.html).)</rdfs:comment>
    <rdfs:label xml:lang="de">Acuity</rdfs:label>
    <rdfs:label xml:lang="en">Acuity</rdfs:label>
  </VideoFeatures>
  <gr:BusinessEntity rdf:ID="ATEC">
    <belongsToModule xml:lang="en">TV</belongsToModule>
    <rdfs:comment xml:lang="en">The business entity ATEC.</rdfs:comment>
    <rdfs:label rdf:datatype="http://www.w3.org/2001/XMLSchema#string"
    >ATEC</rdfs:label>
    <gr:legalName rdf:datatype="http://www.w3.org/2001/XMLSchema#string"
    >ATEC</gr:legalName>
  </gr:BusinessEntity>
  <GeneralFeatures rdf:ID="CommonInterface">
    <rdfs:comment xml:lang="en">The Common Interface is an extensible digital interconnect found in the digital TV market.

(This description is partly based on or reuses content from the Wikipedia article "Common Interface" (http://en.wikipedia.org/wiki/Common_Interface) and is licensed under the GNU Free Documentation License (http://www.gnu.org/copyleft/fdl.html).)</rdfs:comment>
    <belongsToModule xml:lang="en">TV</belongsToModule>
    <rdfs:label xml:lang="en">Common interface</rdfs:label>
    <rdfs:label xml:lang="de">Common interface</rdfs:label>
  </GeneralFeatures>
  <gr:BusinessEntity rdf:ID="Brother">
    <rdfs:comment xml:lang="en">The business entity Brother.</rdfs:comment>
    <gr:legalName rdf:datatype="http://www.w3.org/2001/XMLSchema#string"
    >Brother International GmbH</gr:legalName>
    <belongsToModule xml:lang="en">Printer</belongsToModule>
    <rdfs:label rdf:datatype="http://www.w3.org/2001/XMLSchema#string"
    >Brother</rdfs:label>
    <rdfs:seeAlso rdf:resource="http://www.brother.de/"/>
  </gr:BusinessEntity>
  <SignalFormat rdf:ID="SECAM-D_K">
    <belongsToModule xml:lang="en">TV</belongsToModule>
    <rdfs:comment xml:lang="en">SECAM, also written SÉCAM (Séquentiel couleur à mémoire, French for "Sequential Color with Memory"), is an analog color television system first used in France. SECAM D/K is used in the Commonwealth of Independent States and Eastern Europe (this is simply SECAM used with the D and K monochrome TV transmission standards).

(This description is partly based on or reuses content from the Wikipedia article "SECAM" (http://en.wikipedia.org/wiki/SECAM) and is licensed under the GNU Free Documentation License (http://www.gnu.org/copyleft/fdl.html).)</rdfs:comment>
    <rdfs:label xml:lang="en">SECAM-D K</rdfs:label>
    <rdfs:label xml:lang="de">SECAM-D K</rdfs:label>
  </SignalFormat>
  <Accessory rdf:ID="DC_Cable">
    <rdfs:comment xml:lang="en">The mean amplitude of a waveform.</rdfs:comment>
    <rdfs:label xml:lang="de">DC Kabel</rdfs:label>
    <rdfs:label xml:lang="en">DC cable</rdfs:label>
    <belongsToModule xml:lang="en">Camcorder</belongsToModule>
  </Accessory>
  <gr:BusinessEntity rdf:ID="GNR">
    <rdfs:label rdf:datatype="http://www.w3.org/2001/XMLSchema#string"
    >GNR</rdfs:label>
    <belongsToModule xml:lang="en">TV</belongsToModule>
    <rdfs:seeAlso rdf:resource="http://www.gnr.co.uk/"/>
    <rdfs:comment xml:lang="en">The business entity GNR.</rdfs:comment>
    <gr:legalName rdf:datatype="http://www.w3.org/2001/XMLSchema#string"
    >GNR</gr:legalName>
  </gr:BusinessEntity>
  <Color rdf:ID="MulticoloredBody">
    <rdfs:comment xml:lang="en">The body of the Product has more than one color.</rdfs:comment>
    <rdfs:label xml:lang="de">Mehrfarbig</rdfs:label>
    <rdfs:label xml:lang="en">multicolored</rdfs:label>
    <belongsToModule xml:lang="en">MP3Player, TV, Printer, DigitalCamera, Camcorder</belongsToModule>
  </Color>
  <Color rdf:ID="Green">
    <rdfs:comment xml:lang="en">RGB Value 0,128,0</rdfs:comment>
    <rdfs:label xml:lang="en">Green</rdfs:label>
    <rdfs:label xml:lang="de">Grün</rdfs:label>
    <belongsToModule xml:lang="en">MP3Player, TV, Printer, DigitalCamera, Camcorder</belongsToModule>
  </Color>
  <gr:BusinessEntity rdf:ID="Cowon">
    <belongsToModule xml:lang="en">MP3Player</belongsToModule>
    <rdfs:seeAlso rdf:resource="http://www.cowonglobal.com/"/>
    <rdfs:label rdf:datatype="http://www.w3.org/2001/XMLSchema#string"
    >Cowon</rdfs:label>
    <rdfs:comment xml:lang="en">The business entity COWON SYSTEMS, Inc.</rdfs:comment>
    <gr:legalName rdf:datatype="http://www.w3.org/2001/XMLSchema#string"
    >COWON SYSTEMS, Inc. </gr:legalName>
  </gr:BusinessEntity>
  <Features rdf:ID="ColorPrint">
    <rdfs:comment xml:lang="en">The reproduction of an image or text in color on a paper.</rdfs:comment>
    <belongsToModule xml:lang="en">Printer</belongsToModule>
    <rdfs:label xml:lang="en">Color print</rdfs:label>
    <rdfs:label xml:lang="de">Farbdruck</rdfs:label>
  </Features>
  <DataFormatAudio rdf:ID="ALE">
    <rdfs:label xml:lang="en">ALE</rdfs:label>
    <rdfs:label xml:lang="de">ALE</rdfs:label>
    <belongsToModule xml:lang="en">MP3Player, DigitalCamera, Camcorder</belongsToModule>
    <rdfs:comment xml:lang="en">Apple Lossless (also known as Apple Lossless Encoder, ALE, or Apple Lossless Audio Codec, ALAC) is an audio codec developed by Apple Inc. for lossless data compression of digital music.

(This description is partly based on or reuses content from the Wikipedia article "Apple Lossless" (http://en.wikipedia.org/wiki/Apple_Lossless) and is licensed under the GNU Free Documentation License (http://www.gnu.org/copyleft/fdl.html).)</rdfs:comment>
  </DataFormatAudio>
  <Features rdf:ID="VideoRecording">
    <rdfs:comment xml:lang="en">Ability to record videos.</rdfs:comment>
    <rdfs:label xml:lang="de">Videoaufnahme</rdfs:label>
    <rdfs:label xml:lang="en">Video recording</rdfs:label>
    <belongsToModule xml:lang="en">DigitalCamera</belongsToModule>
  </Features>
  <TVDisplayResolution rdf:ID="EDTV_480p">
    <belongsToModule xml:lang="en">TV</belongsToModule>
    <rdfs:comment xml:lang="en">480p is the shorthand name for a video display resolution. The p stands for progressive scan, i.e. non-interlaced. The 480 denotes a vertical resolution of 480 vertically scanning lines, usually with a horizontal resolution of 640 pixels and 4:3 aspect ratio or a horizontal resolution of 854 pixels and 16:9 aspect ratio.

(This description is partly based on or reuses content from the Wikipedia article "480p" (http://en.wikipedia.org/wiki/480p) and is licensed under the GNU Free Documentation License (http://www.gnu.org/copyleft/fdl.html).)</rdfs:comment>
    <rdfs:label xml:lang="de">EDTV 480p</rdfs:label>
    <rdfs:label xml:lang="en">EDTV 480p</rdfs:label>
  </TVDisplayResolution>
  <StorageMedia rdf:ID="MemoryStick">
    <belongsToModule xml:lang="en">MP3Player, DigitalCamera, Camcorder</belongsToModule>
    <rdfs:comment xml:lang="en">Memory Stick is a removable flash memory card format.</rdfs:comment>
    <rdfs:label xml:lang="de">MemoryStick</rdfs:label>
    <rdfs:label xml:lang="en">MemoryStick</rdfs:label>
  </StorageMedia>
  <TunerType rdf:ID="Digital">
    <rdfs:comment xml:lang="en">A digital system uses discrete (discontinuous) values, usually but not always symbolized numerically (hence called "digital") to represent information for input, processing, transmission, storage.

(This description is partly based on or reuses content from the Wikipedia article "Digital" (http://en.wikipedia.org/wiki/Digital) and is licensed under the GNU Free Documentation License (http://www.gnu.org/copyleft/fdl.html).)</rdfs:comment>
    <rdfs:label xml:lang="de">Digital</rdfs:label>
    <rdfs:label xml:lang="en">Digital</rdfs:label>
    <belongsToModule xml:lang="en">TV</belongsToModule>
  </TunerType>
  <CompatibleOperatingSystems rdf:ID="MacOSXCheetah">
    <rdfs:label xml:lang="en">Mac OS X Cheetah</rdfs:label>
    <rdfs:label xml:lang="de">Mac OS X Cheetah</rdfs:label>
    <belongsToModule xml:lang="en">MP3Player, Printer, DigitalCamera, Camcorder</belongsToModule>
    <rdfs:comment xml:lang="en">Mac OS is the trademarked name for a series of graphical user interface-based operating systems developed by Apple Inc. for their Macintosh line of computer systems.</rdfs:comment>
  </CompatibleOperatingSystems>
  <gr:BusinessEntity rdf:ID="Casio">
    <rdfs:label rdf:datatype="http://www.w3.org/2001/XMLSchema#string"
    >Casio</rdfs:label>
    <gr:legalName rdf:datatype="http://www.w3.org/2001/XMLSchema#string"
    >Casio Computer Co., Ltd</gr:legalName>
    <belongsToModule xml:lang="en">DigitalCamera</belongsToModule>
    <rdfs:seeAlso rdf:resource="http://world.casio.com/"/>
    <rdfs:comment xml:lang="en">The business entity Casio Computer Co., Ltd.</rdfs:comment>
  </gr:BusinessEntity>
  <Zoom rdf:ID="ZoomOptical">
    <belongsToModule xml:lang="en">DigitalCamera</belongsToModule>
    <rdfs:comment xml:lang="en">An optical zoom is a mechanical assembly of lens elements with the ability to vary its focal length (and thus angle of view), as opposed to a fixed focal length (FFL) lens (see prime lens).

(This description is partly based on or reuses content from the Wikipedia article "Zoom lens" (http://en.wikipedia.org/wiki/Zoom_lens) and is licensed under the GNU Free Documentation License (http://www.gnu.org/copyleft/fdl.html).)</rdfs:comment>
    <rdfs:label xml:lang="de">Optischer Zoom</rdfs:label>
    <rdfs:label xml:lang="en">Zoom optical</rdfs:label>
  </Zoom>
  <gr:BusinessEntity rdf:ID="Lexmark">
    <rdfs:comment xml:lang="en">The business entity Lexmark.</rdfs:comment>
    <gr:legalName rdf:datatype="http://www.w3.org/2001/XMLSchema#string"
    >Lexmark International, Inc.</gr:legalName>
    <rdfs:label rdf:datatype="http://www.w3.org/2001/XMLSchema#string"
    >Lexmark.</rdfs:label>
    <rdfs:seeAlso rdf:resource="http://www.lexmark.com/"/>
    <belongsToModule xml:lang="en">Printer</belongsToModule>
  </gr:BusinessEntity>
  <Features rdf:ID="LineInRecorder">
    <rdfs:label xml:lang="en">Line in recorder</rdfs:label>
    <rdfs:label xml:lang="de">Audioaufnahme</rdfs:label>
    <belongsToModule xml:lang="en">MP3Player</belongsToModule>
    <rdfs:comment xml:lang="en">Ability to record sounds via cable connection.</rdfs:comment>
  </Features>
  <MediaFormat rdf:ID="A4">
    <rdfs:comment xml:lang="en">Format of the german institute for standardization: 210 x 297 mm.</rdfs:comment>
    <rdfs:label xml:lang="de">A4</rdfs:label>
    <rdfs:label xml:lang="en">A4</rdfs:label>
    <belongsToModule xml:lang="en">Printer</belongsToModule>
  </MediaFormat>
  <TunerType rdf:ID="Analog">
    <rdfs:comment xml:lang="en">An analog or analogue signal is any continuous signal for which the time varying feature (variable) of the signal is a representation of some other time varying quantity, i.e analogous to another time varying signal.

(This description is partly based on or reuses content from the Wikipedia article "Analog signal" (http://en.wikipedia.org/wiki/Analog_signal) and is licensed under the GNU Free Documentation License (http://www.gnu.org/copyleft/fdl.html).)</rdfs:comment>
    <belongsToModule xml:lang="en">TV</belongsToModule>
    <rdfs:label xml:lang="en">Analog</rdfs:label>
    <rdfs:label xml:lang="de">Digital</rdfs:label>
  </TunerType>
  <DataFormatAudio rdf:ID="MP4_Audio">
    <rdfs:label xml:lang="en">MP4 Audio</rdfs:label>
    <rdfs:label xml:lang="de">MP4 Audio</rdfs:label>
    <rdfs:comment xml:lang="en">A collection of methods defining compression of audio digital data.</rdfs:comment>
    <belongsToModule xml:lang="en">MP3Player, DigitalCamera, Camcorder</belongsToModule>
  </DataFormatAudio>
  <gr:BusinessEntity rdf:ID="New_Universe">
    <belongsToModule xml:lang="en">MP3Player, TV</belongsToModule>
    <rdfs:seeAlso rdf:resource="http://www.nu-europe.com/"/>
    <gr:legalName rdf:datatype="http://www.w3.org/2001/XMLSchema#string"
    >New Universe B.V.</gr:legalName>
    <rdfs:comment xml:lang="en">The business entity New Universe B.V.</rdfs:comment>
    <rdfs:label rdf:datatype="http://www.w3.org/2001/XMLSchema#string"
    >New Universe</rdfs:label>
  </gr:BusinessEntity>
  <gr:BusinessEntity rdf:ID="Victory">
    <rdfs:comment xml:lang="en">The business entity Victory Niederland B.V.</rdfs:comment>
    <belongsToModule xml:lang="en">MP3Player</belongsToModule>
    <rdfs:label rdf:datatype="http://www.w3.org/2001/XMLSchema#string"
    >Victory</rdfs:label>
    <rdfs:seeAlso rdf:resource="http://www.123victory.eu/"/>
    <gr:legalName rdf:datatype="http://www.w3.org/2001/XMLSchema#string"
    >Victory Niederland B.V.</gr:legalName>
  </gr:BusinessEntity>
  <DataInterfaceType rdf:ID="IEEE_1394">
    <belongsToModule xml:lang="en">Printer, Printer, DigitalCamera, Camcorder</belongsToModule>
    <rdfs:label xml:lang="de">IEEE_1394</rdfs:label>
    <rdfs:label xml:lang="en">IEEE_1394</rdfs:label>
    <rdfs:comment xml:lang="en">The IEEE 1394 interface is a serial bus interface standard for high-speed communications and isochronous real-time data transfer, frequently used by personal computers, as well as in digital audio, digital video, automotive, and aeronautics applications.  

(This description is partly based on or reuses content from the Wikipedia article "firewire" (http://en.wikipedia.org/wiki/FireWire) and is licensed under the GNU Free Documentation License (http://www.gnu.org/copyleft/fdl.html).)</rdfs:comment>
  </DataInterfaceType>
  <MediaFormat rdf:ID="A9">
    <belongsToModule xml:lang="en">Printer</belongsToModule>
    <rdfs:label xml:lang="de">A9</rdfs:label>
    <rdfs:label xml:lang="en">A9</rdfs:label>
    <rdfs:comment xml:lang="en">Format of the german institute for standardization: 37 x 52 mm.</rdfs:comment>
  </MediaFormat>
  <gr:BusinessEntity rdf:ID="ODYS">
    <rdfs:label rdf:datatype="http://www.w3.org/2001/XMLSchema#string"
    >ODYS</rdfs:label>
    <rdfs:seeAlso rdf:resource="http://www.odys.de/"/>
    <rdfs:comment xml:lang="en">The business entity ODYS.</rdfs:comment>
    <gr:legalName rdf:datatype="http://www.w3.org/2001/XMLSchema#string"
    >ODYS</gr:legalName>
    <belongsToModule xml:lang="en">MP3Player, TV, DigitalCamera, Camcorder</belongsToModule>
  </gr:BusinessEntity>
  <GeneralFeatures rdf:ID="Anti-ReflectionCoatedScreen">
    <rdfs:label xml:lang="de">Antireflektierende Bildschirmbeschichtung</rdfs:label>
    <rdfs:label xml:lang="en">Anti-reflection coated screen</rdfs:label>
    <rdfs:comment xml:lang="en">The screen has a short persistence phosphor with an anti-reflection and anti-static coating.</rdfs:comment>
    <belongsToModule xml:lang="en">TV</belongsToModule>
  </GeneralFeatures>
  <Connectivity rdf:ID="DigitalAudioOpticalOut">
    <rdfs:comment xml:lang="en">Digital audio uses digital signals for sound reproduction. This includes analog-to-digital conversion, digital-to-analog conversion, storage, and transmission. TOSLINK or Optical Cable is a standardized optical fiber connection system.

(This description is partly based on or reuses content from the Wikipedia article "Digital audio" (http://en.wikipedia.org/wiki/Digital_audio) and is licensed under the GNU Free Documentation License (http://www.gnu.org/copyleft/fdl.html).)</rdfs:comment>
    <belongsToModule xml:lang="en">TV</belongsToModule>
    <rdfs:label xml:lang="en">Digital audio optical out</rdfs:label>
    <rdfs:label xml:lang="de">Digital audio optical out</rdfs:label>
  </Connectivity>
  <gr:BusinessEntity rdf:ID="ATMT">
    <rdfs:seeAlso rdf:resource="http://www.atmt.co.uk/"/>
    <belongsToModule xml:lang="en">MP3Player</belongsToModule>
    <rdfs:label rdf:datatype="http://www.w3.org/2001/XMLSchema#string"
    >ATMT</rdfs:label>
    <rdfs:comment xml:lang="en">ATMT</rdfs:comment>
    <gr:legalName rdf:datatype="http://www.w3.org/2001/XMLSchema#string"
    >ATMT Group</gr:legalName>
  </gr:BusinessEntity>
  <DataFormatImage rdf:ID="Bitmap">
    <rdfs:comment xml:lang="en">In computer graphics, a bitmap or pixmap is a type of memory organization or image file format used to store digital images.

(This description is partly based on or reuses content from the Wikipedia article "Bitmap" (http://en.wikipedia.org/wiki/Bitmap) and is licensed under the GNU Free Documentation License (http://www.gnu.org/copyleft/fdl.html).)</rdfs:comment>
    <belongsToModule xml:lang="en">MP3Player, DigitalCamera, Camcorder</belongsToModule>
    <rdfs:label xml:lang="en">Bitmap</rdfs:label>
    <rdfs:label xml:lang="de">Bitmap</rdfs:label>
  </DataFormatImage>
  <gr:BusinessEntity rdf:ID="Acer">
    <gr:legalName rdf:datatype="http://www.w3.org/2001/XMLSchema#string"
    >Acer, Inc</gr:legalName>
    <belongsToModule xml:lang="en">MP3Player, TV, DigitalCamera</belongsToModule>
    <rdfs:comment xml:lang="en">The business entity Acer, Inc.</rdfs:comment>
    <rdfs:label rdf:datatype="http://www.w3.org/2001/XMLSchema#string"
    >Acer</rdfs:label>
    <rdfs:seeAlso rdf:resource="http://www.acer.com/"/>
  </gr:BusinessEntity>
  <gr:BusinessEntity rdf:ID="PQI">
    <gr:legalName rdf:datatype="http://www.w3.org/2001/XMLSchema#string"
    >Power Quotient International Co., Ltd.</gr:legalName>
    <rdfs:comment xml:lang="en">The business entity Power Quotient International Co., Ltd.</rdfs:comment>
    <rdfs:seeAlso rdf:resource="http://www.pqi.com.tw/"/>
    <belongsToModule xml:lang="en">MP3Player</belongsToModule>
    <rdfs:label rdf:datatype="http://www.w3.org/2001/XMLSchema#string"
    >PQI</rdfs:label>
  </gr:BusinessEntity>
  <gr:BusinessEntity rdf:ID="TRUST">
    <belongsToModule xml:lang="en">MP3Player, DigitalCamera, Camcorder</belongsToModule>
    <rdfs:label rdf:datatype="http://www.w3.org/2001/XMLSchema#string"
    >TRUST</rdfs:label>
    <rdfs:comment xml:lang="en">The business entity TRUST International B.V.</rdfs:comment>
    <rdfs:seeAlso rdf:resource="http://www.trust.com/"/>
    <gr:legalName rdf:datatype="http://www.w3.org/2001/XMLSchema#string"
    >TRUST International B.V.</gr:legalName>
  </gr:BusinessEntity>
  <GeneralFeatures rdf:ID="FirmwareUpgradable">
    <belongsToModule xml:lang="en">TV</belongsToModule>
    <rdfs:label xml:lang="de">Firmware aufrüstbar</rdfs:label>
    <rdfs:label xml:lang="en">Firmware upgradable</rdfs:label>
    <rdfs:comment xml:lang="en">The term upgrade refers to the replacement of a product with a newer version of that same product, here it is the replacement of the firmware with a newer version of it.</rdfs:comment>
  </GeneralFeatures>
  <gr:BusinessEntity rdf:ID="Prestigio">
    <gr:legalName rdf:datatype="http://www.w3.org/2001/XMLSchema#string"
    >Prestigio Plaza Ltd.</gr:legalName>
    <belongsToModule xml:lang="en">TV</belongsToModule>
    <rdfs:comment xml:lang="en">The business entity Prestigio.</rdfs:comment>
    <rdfs:label rdf:datatype="http://www.w3.org/2001/XMLSchema#string"
    >Prestigio</rdfs:label>
    <rdfs:seeAlso rdf:resource="http://www.prestigio.com/"/>
  </gr:BusinessEntity>
  <CompatibleOperatingSystems rdf:ID="MacOSXLeopard">
    <rdfs:label xml:lang="en">Mac OS X Leopard</rdfs:label>
    <rdfs:label xml:lang="de">Mac OS X Leopard</rdfs:label>
    <rdfs:comment xml:lang="en">Mac OS is the trademarked name for a series of graphical user interface-based operating systems developed by Apple Inc. for their Macintosh line of computer systems.</rdfs:comment>
    <belongsToModule xml:lang="en">MP3Player, Printer, DigitalCamera, Camcorder</belongsToModule>
  </CompatibleOperatingSystems>
  <TVDisplayResolution rdf:ID="SDTV_576i">
    <belongsToModule xml:lang="en">TV</belongsToModule>
    <rdfs:label xml:lang="en">SDTV 576i</rdfs:label>
    <rdfs:label xml:lang="de">SDTV 576i</rdfs:label>
    <rdfs:comment xml:lang="en">576i is a standard-definition video mode used in (former) PAL and SECAM countries. In digital applications it's usually referred to as "576i", in analogue contexts it's often quoted as "625 lines". The 576 identifies a vertical resolution of 576 lines (usually with a horizontal resolution of 720 or 704 pixels), and the i identifies it as an interlaced resolution.

(This description is partly based on or reuses content from the Wikipedia article "576ii" (http://en.wikipedia.org/wiki/576i) and is licensed under the GNU Free Documentation License (http://www.gnu.org/copyleft/fdl.html).)</rdfs:comment>
  </TVDisplayResolution>
  <gr:BusinessEntity rdf:ID="InfoPrint">
    <gr:legalName rdf:datatype="http://www.w3.org/2001/XMLSchema#string"
    >InfoPrint Solutions Company</gr:legalName>
    <rdfs:seeAlso rdf:resource="http://www.infoprintsolutionscompany.com/"/>
    <rdfs:comment xml:lang="en">The business entity InfoPrint.</rdfs:comment>
    <rdfs:label rdf:datatype="http://www.w3.org/2001/XMLSchema#string"
    >InfoPrint</rdfs:label>
    <belongsToModule xml:lang="en">Printer</belongsToModule>
  </gr:BusinessEntity>
  <MediaFormat rdf:ID="B5">
    <rdfs:comment xml:lang="en">Format of the german institute for standardization: 176 x 250 mm.</rdfs:comment>
    <rdfs:label xml:lang="de">B5</rdfs:label>
    <rdfs:label xml:lang="en">B5</rdfs:label>
    <belongsToModule xml:lang="en">Printer</belongsToModule>
  </MediaFormat>
  <MediaFormat rdf:ID="B4">
    <rdfs:comment xml:lang="en">Format of the german institute for standardization: 250 x 353 mm.</rdfs:comment>
    <rdfs:label xml:lang="de">B4</rdfs:label>
    <rdfs:label xml:lang="en">B4</rdfs:label>
    <belongsToModule xml:lang="en">Printer</belongsToModule>
  </MediaFormat>
  <CompatibleOperatingSystems rdf:ID="MacOSXPanther">
    <belongsToModule xml:lang="en">MP3Player, Printer, DigitalCamera, Camcorder</belongsToModule>
    <rdfs:label xml:lang="en">Mac OS X Panther</rdfs:label>
    <rdfs:label xml:lang="de">Mac OS X Panther</rdfs:label>
    <rdfs:comment xml:lang="en">Mac OS is the trademarked name for a series of graphical user interface-based operating systems developed by Apple Inc. for their Macintosh line of computer systems.</rdfs:comment>
  </CompatibleOperatingSystems>
  <Accessory rdf:ID="USB_Cable">
    <belongsToModule xml:lang="en">Camcorder</belongsToModule>
    <rdfs:comment xml:lang="en">A serial bus standard to connect devices to a host computer.</rdfs:comment>
    <rdfs:label xml:lang="en">USB cable</rdfs:label>
    <rdfs:label xml:lang="de">USB Kabel</rdfs:label>
  </Accessory>
  <gr:BusinessEntity rdf:ID="Smartdisk">
    <gr:legalName rdf:datatype="http://www.w3.org/2001/XMLSchema#string"
    >Verbatim Corporation </gr:legalName>
    <belongsToModule xml:lang="en">MP3Player</belongsToModule>
    <rdfs:comment xml:lang="en">The business entity Verbatim Corporation.</rdfs:comment>
    <rdfs:seeAlso rdf:resource="http://www.smartdisk.com/"/>
    <rdfs:label rdf:datatype="http://www.w3.org/2001/XMLSchema#string"
    >Smartdisk</rdfs:label>
  </gr:BusinessEntity>
  <gr:BusinessEntity rdf:ID="Decktron">
    <rdfs:label rdf:datatype="http://www.w3.org/2001/XMLSchema#string"
    >Decktron</rdfs:label>
    <belongsToModule xml:lang="en">MP3Player</belongsToModule>
    <rdfs:seeAlso rdf:resource="http://decktron.de/"/>
    <gr:legalName rdf:datatype="http://www.w3.org/2001/XMLSchema#string"
    >Decktron Europe GmbH</gr:legalName>
    <rdfs:comment xml:lang="en">The business entity Decktron Europe GmbH.</rdfs:comment>
  </gr:BusinessEntity>
  <gr:BusinessEntity rdf:ID="CTX">
    <belongsToModule xml:lang="en">TV</belongsToModule>
    <rdfs:seeAlso rdf:resource="http://www.ctxeurope.com/"/>
    <rdfs:label rdf:datatype="http://www.w3.org/2001/XMLSchema#string"
    >CTX</rdfs:label>
    <rdfs:comment xml:lang="en">The business entity CTX.</rdfs:comment>
    <gr:legalName rdf:datatype="http://www.w3.org/2001/XMLSchema#string"
    >CTX Technology Corporation</gr:legalName>
  </gr:BusinessEntity>
  <DataFormatImage rdf:ID="DPOF">
    <rdfs:label xml:lang="de">DPOF</rdfs:label>
    <rdfs:label xml:lang="en">DPOF</rdfs:label>
    <belongsToModule xml:lang="en">DigitalCamera, Camcorder</belongsToModule>
    <rdfs:comment xml:lang="en">DPOF (Digital Print Order format) is a format which allows the user of a digital camera or other device such as a Mobile Phone or PDA to define which captured images on the storage card are to be printed, together with information on the number of copies or other image information such as paper size, image title text, image orientation, contact information and more.

(This description is partly based on or reuses content from the Wikipedia article "DPOF" (http://en.wikipedia.org/wiki/DPOF) and is licensed under the GNU Free Documentation License (http://www.gnu.org/copyleft/fdl.html).)</rdfs:comment>
  </DataFormatImage>
  <gr:BusinessEntity rdf:ID="Coby">
    <rdfs:seeAlso rdf:resource="http://www.cobyusa.com/"/>
    <belongsToModule xml:lang="en">MP3Player, TV</belongsToModule>
    <rdfs:label rdf:datatype="http://www.w3.org/2001/XMLSchema#string"
    >Coby</rdfs:label>
    <rdfs:comment xml:lang="en">The business entity Coby Electronics Corporation.</rdfs:comment>
    <gr:legalName rdf:datatype="http://www.w3.org/2001/XMLSchema#string"
    >Coby Electronics Corporation</gr:legalName>
  </gr:BusinessEntity>
  <DataInterfaceType rdf:ID="S-Video_out">
    <belongsToModule xml:lang="en">Camcorder</belongsToModule>
    <rdfs:comment xml:lang="en">Is an analog video signal that carries the video data as two separate signals, lumen (luminance) and chroma (color).

(This description is partly based on or reuses content from the Wikipedia article "S-Video" (http://en.wikipedia.org/wiki/S-Video) and is licensed under the GNU Free Documentation License (http://www.gnu.org/copyleft/fdl.html).)</rdfs:comment>
    <rdfs:label xml:lang="de">S-Video out</rdfs:label>
    <rdfs:label xml:lang="en">S-Video out</rdfs:label>
  </DataInterfaceType>
  <gr:BusinessEntity rdf:ID="Denver">
    <rdfs:seeAlso rdf:resource="http://www.denver-electronics.com/"/>
    <rdfs:comment xml:lang="en">The business entity Denver.</rdfs:comment>
    <rdfs:label rdf:datatype="http://www.w3.org/2001/XMLSchema#string"
    >Denver</rdfs:label>
    <gr:legalName rdf:datatype="http://www.w3.org/2001/XMLSchema#string"
    >Denver Electronics</gr:legalName>
    <belongsToModule xml:lang="en">TV</belongsToModule>
  </gr:BusinessEntity>
  <gr:BusinessEntity rdf:ID="Oki">
    <rdfs:comment xml:lang="en">The business entity Oki.</rdfs:comment>
    <belongsToModule xml:lang="en">TV, Printer</belongsToModule>
    <rdfs:label rdf:datatype="http://www.w3.org/2001/XMLSchema#string"
    >Oki</rdfs:label>
    <gr:legalName rdf:datatype="http://www.w3.org/2001/XMLSchema#string"
    >Oki Electric Industry Co., Ltd.</gr:legalName>
    <rdfs:seeAlso rdf:resource="http://www.oki.com/"/>
  </gr:BusinessEntity>
  <Connectivity rdf:ID="CompositeVideoIn">
    <rdfs:label xml:lang="en">Composite video in</rdfs:label>
    <rdfs:label xml:lang="de">Composite video in</rdfs:label>
    <rdfs:comment xml:lang="en">Composite video is the format of an analog television (picture only) signal before it is combined with a sound signal and modulated onto an RF carrier. It is usually in a standard format such as NTSC, PAL, or SECAM. It is a composite of three source signals called Y, U and V (together referred to as YUV) with sync pulses. Here the input is meant.

(This description is partly based on or reuses content from the Wikipedia article "Composite video" (http://en.wikipedia.org/wiki/Composite_video) and is licensed under the GNU Free Documentation License (http://www.gnu.org/copyleft/fdl.html).)</rdfs:comment>
    <belongsToModule xml:lang="en">TV</belongsToModule>
  </Connectivity>
  <gr:BusinessEntity rdf:ID="Yukai">
    <rdfs:comment xml:lang="en">The business entity Yukai.</rdfs:comment>
    <gr:legalName rdf:datatype="http://www.w3.org/2001/XMLSchema#string"
    >Mustek Optic-Computer and Communication International GmbH</gr:legalName>
    <rdfs:label rdf:datatype="http://www.w3.org/2001/XMLSchema#string"
    >Yukai</rdfs:label>
    <belongsToModule xml:lang="en">Camcorder</belongsToModule>
    <rdfs:seeAlso rdf:resource="http://www.yukai.eu/"/>
  </gr:BusinessEntity>
  <SensorType rdf:ID="SensorType_3CCD">
    <rdfs:comment xml:lang="en">3CCD is a term used to describe an imaging system employed by some still cameras, video cameras, telecine and camcorders.

(This description is partly based on or reuses content from the Wikipedia article "Three-CCD" (http://en.wikipedia.org/wiki/Three-CCD) and is licensed under the GNU Free Documentation License (http://www.gnu.org/copyleft/fdl.html).)</rdfs:comment>
    <rdfs:label xml:lang="en">Three-CCD</rdfs:label>
    <rdfs:label xml:lang="de">Three-CCD</rdfs:label>
    <belongsToModule xml:lang="en">Camcorder</belongsToModule>
  </SensorType>
  <Focus rdf:ID="FocusFixed">
    <rdfs:label xml:lang="de">Starrer Fokus</rdfs:label>
    <rdfs:label xml:lang="en">Focus fixed</rdfs:label>
    <belongsToModule xml:lang="en">DigitalCamera, Camcorder</belongsToModule>
    <rdfs:comment xml:lang="en">A photographic lens for which the focus is not adjustable is called a fixed-focus lens.

(This description is partly based on or reuses content from the Wikipedia article "Fixed focus" (http://en.wikipedia.org/wiki/Fixed_focus) and is licensed under the GNU Free Documentation License (http://www.gnu.org/copyleft/fdl.html).)</rdfs:comment>
  </Focus>
  <gr:BusinessEntity rdf:ID="Apple">
    <rdfs:comment xml:lang="en">The business entity Apple, Inc.</rdfs:comment>
    <belongsToModule xml:lang="en">MP3Player</belongsToModule>
    <rdfs:label rdf:datatype="http://www.w3.org/2001/XMLSchema#string"
    >Apple</rdfs:label>
    <rdfs:seeAlso rdf:resource="http://www.apple.com/"/>
    <gr:legalName rdf:datatype="http://www.w3.org/2001/XMLSchema#string"
    >Apple Inc.</gr:legalName>
  </gr:BusinessEntity>
  <SignalFormat rdf:ID="DVB_COFDM">
    <rdfs:comment xml:lang="en">Digital Video Broadcasting (DVB) is a suite of internationally accepted open standards for digital television. Coded OFDM (COFDM) and Discrete multi-tone modulation (DMT) is a frequency-division multiplexing (FDM) scheme utilized as a digital multi-carrier modulation method. A large number of closely-spaced orthogonal sub-carriers are used to carry data. The data is divided into several parallel data streams or channels, one for each sub-carrier. Each sub-carrier is modulated with a conventional modulation scheme (such as quadrature amplitude modulation or phase shift keying) at a low symbol rate, maintaining total data rates similar to conventional single-carrier modulation schemes in the same bandwidth.

(This description is partly based on or reuses content from the Wikipedia article "Digital Video Broadcasting" (http://en.wikipedia.org/wiki/Digital_Video_Broadcasting) and is licensed under the GNU Free Documentation License (http://www.gnu.org/copyleft/fdl.html).)</rdfs:comment>
    <rdfs:label xml:lang="en">DVB COFDM</rdfs:label>
    <rdfs:label xml:lang="de">DVB COFDM</rdfs:label>
    <belongsToModule xml:lang="en">TV</belongsToModule>
  </SignalFormat>
  <ProcessorType rdf:ID="G4_Class_Processor">
    <rdfs:label xml:lang="de">G4 Class Processor</rdfs:label>
    <rdfs:label xml:lang="en">G4 Class Processor</rdfs:label>
    <belongsToModule xml:lang="en">Printer</belongsToModule>
    <rdfs:comment xml:lang="en">A designation used by Apple Computer to describe a fourth generation of 32-bit PowerPC microprocessors.

(This description is partly based on or reuses content from the Wikipedia article "PowerPC_G4" (http://en.wikipedia.org/wiki/PowerPC_G4) and is licensed under the GNU Free Documentation License (http://www.gnu.org/copyleft/fdl.html).)</rdfs:comment>
  </ProcessorType>
  <Connectivity rdf:ID="YPbPr">
    <rdfs:comment xml:lang="en">YPbPR is the analog video signal carried by component video cable in consumer electronics. The green cable carries Y, the blue cable carries PB and the red cable carries PR.

(This description is partly based on or reuses content from the Wikipedia article "YPbPr" (http://en.wikipedia.org/wiki/YPbPr) and is licensed under the GNU Free Documentation License (http://www.gnu.org/copyleft/fdl.html).)</rdfs:comment>
    <rdfs:label xml:lang="de">YPbPr</rdfs:label>
    <rdfs:label xml:lang="en">YPbPr</rdfs:label>
    <belongsToModule xml:lang="en">TV</belongsToModule>
  </Connectivity>
  <AudioFeatures rdf:ID="NoiseReduction">
    <belongsToModule xml:lang="en">TV</belongsToModule>
    <rdfs:comment xml:lang="en">Noise reduction is the process of removing noise from a signal.</rdfs:comment>
    <rdfs:label xml:lang="en">Noise reduction</rdfs:label>
    <rdfs:label xml:lang="de">Geräuschunterdrückung</rdfs:label>
  </AudioFeatures>
  <Color rdf:ID="Yellow">
    <rdfs:comment xml:lang="en">RGB Value 255,255,0</rdfs:comment>
    <belongsToModule xml:lang="en">MP3Player, TV, Printer, DigitalCamera, Camcorder</belongsToModule>
    <rdfs:label xml:lang="en">Yellow</rdfs:label>
    <rdfs:label xml:lang="de">Gelb</rdfs:label>
  </Color>
  <AudioFeatures rdf:ID="BuiltInSpeakers">
    <rdfs:comment xml:lang="en">Speakers that are integrated in the hull of a electronical device, that is able to play audio signals.</rdfs:comment>
    <rdfs:label xml:lang="de">Eingebaute Lautsprecher</rdfs:label>
    <rdfs:label xml:lang="en">Built in speakers</rdfs:label>
    <belongsToModule xml:lang="en">TV, Camcorder</belongsToModule>
  </AudioFeatures>
  <gr:BusinessEntity rdf:ID="Haier">
    <rdfs:label rdf:datatype="http://www.w3.org/2001/XMLSchema#string"
    >Haier</rdfs:label>
    <belongsToModule xml:lang="en">TV</belongsToModule>
    <rdfs:seeAlso rdf:resource="http://www.haier.com/"/>
    <gr:legalName rdf:datatype="http://www.w3.org/2001/XMLSchema#string"
    >Haier Group</gr:legalName>
    <rdfs:comment xml:lang="en">The business entity Haier.</rdfs:comment>
  </gr:BusinessEntity>
  <gr:BusinessEntity rdf:ID="Yakumo">
    <rdfs:comment xml:lang="en">The business entity Yakumo GmbH.</rdfs:comment>
    <belongsToModule xml:lang="en">DigitalCamera</belongsToModule>
    <rdfs:label rdf:datatype="http://www.w3.org/2001/XMLSchema#string"
    >Yakumo</rdfs:label>
    <gr:legalName rdf:datatype="http://www.w3.org/2001/XMLSchema#string"
    >Yakumo GmbH</gr:legalName>
  </gr:BusinessEntity>
  <gr:BusinessEntity rdf:ID="Techsolo">
    <rdfs:seeAlso rdf:resource="http://www.techsolo.com/"/>
    <rdfs:label rdf:datatype="http://www.w3.org/2001/XMLSchema#string"
    >Techsolo</rdfs:label>
    <belongsToModule xml:lang="en">MP3Player</belongsToModule>
    <gr:legalName rdf:datatype="http://www.w3.org/2001/XMLSchema#string"
    >Techsolo Europe B.V.</gr:legalName>
    <rdfs:comment xml:lang="en">The business entity Techsolo Europe B.V.</rdfs:comment>
  </gr:BusinessEntity>
  <Features rdf:ID="DocumentViewing">
    <belongsToModule xml:lang="en">MP3Player, DigitalCamera, Camcorder</belongsToModule>
    <rdfs:comment xml:lang="en">Ability to display documents.</rdfs:comment>
    <rdfs:label xml:lang="en">Document viewing</rdfs:label>
    <rdfs:label xml:lang="de">Dokumentdarstellung</rdfs:label>
  </Features>
  <VideoFeatures rdf:ID="AmbilightSpectraActiveFrame">
    <rdfs:comment xml:lang="en">Active Frame is a single soft halo of light powered by 126 LEDs.</rdfs:comment>
    <rdfs:label xml:lang="en">Ambilight Spectra Active Frame</rdfs:label>
    <rdfs:label xml:lang="de">Ambilight Spectra Active Frame</rdfs:label>
    <belongsToModule xml:lang="en">TV</belongsToModule>
  </VideoFeatures>
  <MediaFormat rdf:ID="A1">
    <belongsToModule xml:lang="en">Printer</belongsToModule>
    <rdfs:label xml:lang="de">A1</rdfs:label>
    <rdfs:label xml:lang="en">A1</rdfs:label>
    <rdfs:comment xml:lang="en">Format of the german institute for standardization: 594 x 841 mm.</rdfs:comment>
  </MediaFormat>
  <owl:AnnotationProperty rdf:about="http://purl.org/dc/elements/1.1/rights"/>
  <gr:BusinessEntity rdf:ID="Esselte">
    <belongsToModule xml:lang="en">Printer</belongsToModule>
    <rdfs:comment xml:lang="en">The business entity Esselte.</rdfs:comment>
    <gr:legalName rdf:datatype="http://www.w3.org/2001/XMLSchema#string"
    >Esselte Corporation</gr:legalName>
    <rdfs:label rdf:datatype="http://www.w3.org/2001/XMLSchema#string"
    >Esselte</rdfs:label>
    <rdfs:seeAlso rdf:resource="http://www.esselte.com/"/>
  </gr:BusinessEntity>
  <gr:BusinessEntity rdf:ID="Netgear">
    <gr:legalName rdf:datatype="http://www.w3.org/2001/XMLSchema#string"
    >NETGEAR, Inc.</gr:legalName>
    <rdfs:label rdf:datatype="http://www.w3.org/2001/XMLSchema#string"
    >Netgear</rdfs:label>
    <rdfs:seeAlso rdf:resource="http://www.netgear.de/"/>
    <rdfs:comment xml:lang="en">The business entity NETGEAR, Inc.</rdfs:comment>
    <belongsToModule xml:lang="en">MP3Player</belongsToModule>
  </gr:BusinessEntity>
  <SignalFormat rdf:ID="PAL-I">
    <rdfs:label xml:lang="en">PAL-I</rdfs:label>
    <rdfs:label xml:lang="de">PAL-L</rdfs:label>
    <rdfs:comment xml:lang="en">PAL, short for Phase Alternating Line, is a colour-encoding system used in broadcast television systems in large parts of the world. This is only used in Ireland, the UK, Hongkong and Macau.

(This description is partly based on or reuses content from the Wikipedia article "PAL" (http://en.wikipedia.org/wiki/PAL) and is licensed under the GNU Free Documentation License (http://www.gnu.org/copyleft/fdl.html).)</rdfs:comment>
    <belongsToModule xml:lang="en">TV</belongsToModule>
  </SignalFormat>
  <CompatibleOperatingSystems rdf:ID="WindowsME">
    <belongsToModule xml:lang="en">MP3Player, Printer, DigitalCamera, Camcorder</belongsToModule>
    <rdfs:label xml:lang="en">Windows ME</rdfs:label>
    <rdfs:label xml:lang="de">Windows ME</rdfs:label>
    <rdfs:comment xml:lang="en">A version of a Microsoft operating system.</rdfs:comment>
  </CompatibleOperatingSystems>
  <Features rdf:ID="LightExposureControl">
    <rdfs:label xml:lang="en">Light exposure control</rdfs:label>
    <rdfs:label xml:lang="de">Belichtungsregelung</rdfs:label>
    <rdfs:comment xml:lang="en">Is the total amount of light allowed to fall on the photographic medium during the process of taking a photograph.</rdfs:comment>
    <belongsToModule xml:lang="en">Camcorder</belongsToModule>
  </Features>
  <gr:BusinessEntity rdf:ID="Eaconn">
    <rdfs:seeAlso rdf:resource="http://www.eaconn.com/"/>
    <gr:legalName rdf:datatype="http://www.w3.org/2001/XMLSchema#string"
    >EACONN B.V.</gr:legalName>
    <rdfs:comment xml:lang="en">The business entity EACONN B.V.</rdfs:comment>
    <belongsToModule xml:lang="en">MP3Player</belongsToModule>
    <rdfs:label rdf:datatype="http://www.w3.org/2001/XMLSchema#string"
    >Eaconn</rdfs:label>
  </gr:BusinessEntity>
  <GeneralFeatures rdf:ID="DVB-T">
    <rdfs:comment xml:lang="en">DVB-T is an abbreviation for Digital Video Broadcasting - Terrestrial; it is the DVB European-based consortium standard for the broadcast transmission of digital terrestrial television. This system transmits compressed digital audio, video and other data in an MPEG transport stream, using COFDM modulation.

(This description is partly based on or reuses content from the Wikipedia article "DVB-T" (http://en.wikipedia.org/wiki/DVB-T) and is licensed under the GNU Free Documentation License (http://www.gnu.org/copyleft/fdl.html).)</rdfs:comment>
    <belongsToModule xml:lang="en">TV</belongsToModule>
    <rdfs:label xml:lang="en">DVB-T</rdfs:label>
    <rdfs:label xml:lang="de">DVB-T</rdfs:label>
  </GeneralFeatures>
  <VideoFeatures rdf:ID="PixelPlus2">
    <rdfs:label xml:lang="de">Pixelplus 2</rdfs:label>
    <rdfs:label xml:lang="en">Pixelplus 2</rdfs:label>
    <rdfs:comment xml:lang="en">Pixelplus 2 is a technology which allows motion reinterpolation on 480p and 576p material.</rdfs:comment>
    <belongsToModule xml:lang="en">TV</belongsToModule>
  </VideoFeatures>
  <gr:BusinessEntity rdf:ID="Harwa">
    <rdfs:comment xml:lang="en">The business entity Harwa.</rdfs:comment>
    <gr:legalName rdf:datatype="http://www.w3.org/2001/XMLSchema#string"
    >Harwa Electronics GmbH</gr:legalName>
    <belongsToModule xml:lang="en">TV</belongsToModule>
    <rdfs:label rdf:datatype="http://www.w3.org/2001/XMLSchema#string"
    >Harwa</rdfs:label>
  </gr:BusinessEntity>
  <gr:BusinessEntity rdf:ID="Gembird">
    <gr:legalName rdf:datatype="http://www.w3.org/2001/XMLSchema#string"
    >GEMBIRD ® Deutschland GmbH </gr:legalName>
    <rdfs:label rdf:datatype="http://www.w3.org/2001/XMLSchema#string"
    >Gembird</rdfs:label>
    <rdfs:comment xml:lang="en">The business entity GEMBIRD ® Deutschland GmbH.</rdfs:comment>
    <rdfs:seeAlso rdf:resource="http://www.gembird.com/"/>
    <belongsToModule xml:lang="en">MP3Player</belongsToModule>
  </gr:BusinessEntity>
  <DataInterfaceType rdf:ID="Bluetooth">
    <rdfs:label xml:lang="en">Bluetooth</rdfs:label>
    <rdfs:label xml:lang="de">Bluetooth</rdfs:label>
    <belongsToModule xml:lang="en">MP3Player, Printer, DigitalCamera, Camcorder</belongsToModule>
    <rdfs:comment xml:lang="en">Bluetooth is a wireless protocol utilizing short-range communications technology facilitating data transmission over short distances from fixed and mobile devices, creating wireless personal area networks.</rdfs:comment>
  </DataInterfaceType>
  <MediaFormat rdf:ID="MediaFormatEnvelope">
    <belongsToModule xml:lang="en">Printer</belongsToModule>
    <rdfs:comment xml:lang="en">Media format that is able to assume different shapes.</rdfs:comment>
    <rdfs:label xml:lang="en">Media format Envelope</rdfs:label>
    <rdfs:label xml:lang="de">Medienformat Briefkuvert</rdfs:label>
  </MediaFormat>
  <Accessory rdf:ID="AC_Cable">
    <rdfs:comment xml:lang="en">A net transfer of energy over a complete cycle of the alternating current waveform.</rdfs:comment>
    <belongsToModule xml:lang="en">Camcorder</belongsToModule>
    <rdfs:label xml:lang="en">AC cable</rdfs:label>
    <rdfs:label xml:lang="de">AC Kabel</rdfs:label>
  </Accessory>
  <RechargeableEnergySource rdf:ID="Lit-Ion">
    <belongsToModule xml:lang="en">MP3Player, DigitalCamera, Camcorder</belongsToModule>
    <rdfs:comment xml:lang="en">Type of rechargeable battery in which a lithium ion moves between the anode and cathode.

(This description is partly based on or reuses content from the Wikipedia article "Lithium ion battery" (http://en.wikipedia.org/wiki/Lithium_ion_battery) and is licensed under the GNU Free Documentation License (http://www.gnu.org/copyleft/fdl.html).)</rdfs:comment>
    <rdfs:label xml:lang="en">Lit-Ion</rdfs:label>
    <rdfs:label xml:lang="de">Lit-Ion</rdfs:label>
  </RechargeableEnergySource>
  <GeneralFeatures rdf:ID="IntegratedClock">
    <rdfs:comment xml:lang="en">Clock integrated in a device.</rdfs:comment>
    <rdfs:label xml:lang="de">Integrierte Uhr</rdfs:label>
    <rdfs:label xml:lang="en">Integrated clock</rdfs:label>
    <belongsToModule xml:lang="en">TV</belongsToModule>
  </GeneralFeatures>
  <gr:BusinessEntity rdf:ID="Sagem">
    <rdfs:label rdf:datatype="http://www.w3.org/2001/XMLSchema#string"
    >Sagem</rdfs:label>
    <rdfs:comment xml:lang="en">The business entity Sagem.</rdfs:comment>
    <rdfs:seeAlso rdf:resource="http://www.sagem.com/"/>
    <gr:legalName rdf:datatype="http://www.w3.org/2001/XMLSchema#string"
    >Sagem Télécommunications</gr:legalName>
    <belongsToModule xml:lang="en">TV, Printer</belongsToModule>
  </gr:BusinessEntity>
  <gr:BusinessEntity rdf:ID="SMS">
    <gr:legalName rdf:datatype="http://www.w3.org/2001/XMLSchema#string"
    >SMS Printing Graphics</gr:legalName>
    <belongsToModule xml:lang="en">Printer</belongsToModule>
    <rdfs:comment xml:lang="en">The business entity SMS.</rdfs:comment>
    <rdfs:label rdf:datatype="http://www.w3.org/2001/XMLSchema#string"
    >SMS</rdfs:label>
    <rdfs:seeAlso rdf:resource="http://www.smsprintingngraphics.com/"/>
  </gr:BusinessEntity>
  <SceneMode rdf:ID="PhotoMode">
    <belongsToModule xml:lang="en">Camcorder</belongsToModule>
    <rdfs:comment xml:lang="en">Ability of the camcorder to adapt to special environments.</rdfs:comment>
    <rdfs:label xml:lang="de">Photo modus</rdfs:label>
    <rdfs:label xml:lang="en">Photo mode</rdfs:label>
  </SceneMode>
  <gr:BusinessEntity rdf:ID="Viewpia">
    <rdfs:label rdf:datatype="http://www.w3.org/2001/XMLSchema#string"
    >Viewpia</rdfs:label>
    <belongsToModule xml:lang="en">TV</belongsToModule>
    <rdfs:comment xml:lang="en">The business entity Viewpia.</rdfs:comment>
    <rdfs:seeAlso rdf:resource="http://www.gt-24.de/"/>
    <gr:legalName rdf:datatype="http://www.w3.org/2001/XMLSchema#string"
    >Global-Tech 24 Ltd.</gr:legalName>
  </gr:BusinessEntity>
  <gr:BusinessEntity rdf:ID="TechniSat">
    <gr:legalName rdf:datatype="http://www.w3.org/2001/XMLSchema#string"
    >TechniSat Digital GmbH </gr:legalName>
    <belongsToModule xml:lang="en">MP3Player, TV</belongsToModule>
    <rdfs:comment xml:lang="en">The business entity TechniSat.</rdfs:comment>
    <rdfs:label rdf:datatype="http://www.w3.org/2001/XMLSchema#string"
    >TechniSat</rdfs:label>
    <rdfs:seeAlso rdf:resource="http://www.technisat.com/"/>
  </gr:BusinessEntity>
  <gr:BusinessEntity rdf:ID="Typhoon">
    <rdfs:comment xml:lang="en">The business entity COS Distribution GmbH</rdfs:comment>
    <rdfs:seeAlso rdf:resource="http://www.typhoon.de/"/>
    <rdfs:label rdf:datatype="http://www.w3.org/2001/XMLSchema#string"
    >Typhoon</rdfs:label>
    <gr:legalName rdf:datatype="http://www.w3.org/2001/XMLSchema#string"
    >COS Distribution GmbH</gr:legalName>
    <belongsToModule xml:lang="en">MP3Player</belongsToModule>
  </gr:BusinessEntity>
  <gr:BusinessEntity rdf:ID="Sharp">
    <rdfs:label rdf:datatype="http://www.w3.org/2001/XMLSchema#string"
    >Sharp</rdfs:label>
    <rdfs:comment xml:lang="en">The business entity Sharp.</rdfs:comment>
    <rdfs:seeAlso rdf:resource="http://www.sharp-world.com/"/>
    <gr:legalName rdf:datatype="http://www.w3.org/2001/XMLSchema#string"
    >Sharp Corporation</gr:legalName>
    <belongsToModule xml:lang="en">TV</belongsToModule>
  </gr:BusinessEntity>
  <Connectivity rdf:ID="RF">
    <rdfs:label xml:lang="de">RF</rdfs:label>
    <rdfs:label xml:lang="en">RF</rdfs:label>
    <rdfs:comment xml:lang="en">An RF connector is an electrical connector designed to work at radio frequencies in the multi-megahertz range. RF connectors are typically used with coaxial cables and are designed to maintain the shielding that the coaxial design offers. Better models also minimize the change in transmission line impedance at the connection. Mechanically they provide a fastening mechanism (thread, bayonet, braces, push pull) and springs for a low ohmic electric contact while sparing the gold surface thus allowing above 1000 reconnects and reducing the insertion force. Research activity in the area of radio-frequency (RF) circuit design has surged in the last decade in direct response to the enormous market demand for inexpensive, high data rate wireless transceivers.

(This description is partly based on or reuses content from the Wikipedia article "RF connector" (http://en.wikipedia.org/wiki/RF_connector) and is licensed under the GNU Free Documentation License (http://www.gnu.org/copyleft/fdl.html).)</rdfs:comment>
  </Connectivity>
  <Features rdf:ID="Microphon">
    <rdfs:comment xml:lang="en">Ability to record voices and sounds.</rdfs:comment>
    <rdfs:label xml:lang="de">Mikrofon</rdfs:label>
    <rdfs:label xml:lang="en">Microphon</rdfs:label>
    <belongsToModule xml:lang="en">DigitalCamera, Camcorder</belongsToModule>
  </Features>
  <gr:BusinessEntity rdf:ID="Nintendo">
    <belongsToModule xml:lang="en">MP3Player</belongsToModule>
    <rdfs:comment xml:lang="en">The business entity Nintendo Company Ltd.</rdfs:comment>
    <gr:legalName rdf:datatype="http://www.w3.org/2001/XMLSchema#string"
    >Nintendo Company Ltd.</gr:legalName>
    <rdfs:seeAlso rdf:resource="http://www.nintendo.com/"/>
    <rdfs:label rdf:datatype="http://www.w3.org/2001/XMLSchema#string"
    >Nintendo</rdfs:label>
  </gr:BusinessEntity>
  <gr:BusinessEntity rdf:ID="NEC">
    <rdfs:comment xml:lang="en">The business entity NEC Corporation.</rdfs:comment>
    <rdfs:seeAlso rdf:resource="http://www.necel.com/"/>
    <rdfs:label rdf:datatype="http://www.w3.org/2001/XMLSchema#string"
    >NEC</rdfs:label>
    <belongsToModule xml:lang="en">MP3Player, TV</belongsToModule>
    <gr:legalName rdf:datatype="http://www.w3.org/2001/XMLSchema#string"
    >NEC Corporation</gr:legalName>
  </gr:BusinessEntity>
  <gr:BusinessEntity rdf:ID="Vivitar">
    <gr:legalName rdf:datatype="http://www.w3.org/2001/XMLSchema#string"
    >Vivitar Corporation</gr:legalName>
    <rdfs:label rdf:datatype="http://www.w3.org/2001/XMLSchema#string"
    >Vivitar</rdfs:label>
    <belongsToModule xml:lang="en">DigitalCamera</belongsToModule>
    <rdfs:comment xml:lang="en">The business entity Vivitar Corporation.</rdfs:comment>
    <rdfs:seeAlso rdf:resource="http://www.syntaxbrillian.com/"/>
  </gr:BusinessEntity>
  <gr:BusinessEntity rdf:ID="Apacer">
    <gr:legalName rdf:datatype="http://www.w3.org/2001/XMLSchema#string"
    >Apacer Technology, Inc.</gr:legalName>
    <rdfs:label rdf:datatype="http://www.w3.org/2001/XMLSchema#string"
    >Apacer</rdfs:label>
    <rdfs:seeAlso rdf:resource="http://www.apacer.com/"/>
    <belongsToModule xml:lang="en">MP3Player</belongsToModule>
    <rdfs:comment xml:lang="en">The business entity Apacer Technology, Inc.</rdfs:comment>
  </gr:BusinessEntity>
  <GeneralFeatures rdf:ID="AutoChannelSearch">
    <rdfs:comment xml:lang="en">Gives an indication of preprogrammed channels for the user of a television so that he does not need to programm it himself.</rdfs:comment>
    <belongsToModule xml:lang="en">TV</belongsToModule>
    <rdfs:label xml:lang="de">Automatischer Sendersuchlauf</rdfs:label>
    <rdfs:label xml:lang="en">Auto channel search</rdfs:label>
  </GeneralFeatures>
  <gr:BusinessEntity rdf:ID="MPMAN">
    <rdfs:seeAlso rdf:resource="http://www.mpmaneurope.com/"/>
    <belongsToModule xml:lang="en">MP3Player</belongsToModule>
    <rdfs:comment xml:lang="en">The business entity MPMAN Europe.</rdfs:comment>
    <gr:legalName rdf:datatype="http://www.w3.org/2001/XMLSchema#string"
    >MPMAN Europe</gr:legalName>
    <rdfs:label rdf:datatype="http://www.w3.org/2001/XMLSchema#string"
    >MPAN</rdfs:label>
  </gr:BusinessEntity>
  <gr:BusinessEntity rdf:ID="Energy_Sistem">
    <belongsToModule xml:lang="en">MP3Player</belongsToModule>
    <rdfs:seeAlso rdf:resource="http://www.energysistem.com/"/>
    <rdfs:label rdf:datatype="http://www.w3.org/2001/XMLSchema#string"
    >Energy Sistem</rdfs:label>
    <gr:legalName rdf:datatype="http://www.w3.org/2001/XMLSchema#string"
    >Energy Sistem Soyntec S.A.</gr:legalName>
    <rdfs:comment xml:lang="en">The business entity Energy Sistem Soyntec S.A.</rdfs:comment>
  </gr:BusinessEntity>
  <MediaType rdf:ID="Label">
    <rdfs:comment xml:lang="en">Media type that can be printed on one side and has a glued area on the other side.</rdfs:comment>
    <belongsToModule xml:lang="en">Printer</belongsToModule>
    <rdfs:label xml:lang="de">Etikett</rdfs:label>
    <rdfs:label xml:lang="en">Label</rdfs:label>
  </MediaType>
  <GeneralFeatures rdf:ID="Timer">
    <belongsToModule xml:lang="en">TV</belongsToModule>
    <rdfs:label xml:lang="de">Zeitgeber</rdfs:label>
    <rdfs:label xml:lang="en">Timer</rdfs:label>
    <rdfs:comment xml:lang="en">A timer is a specialized type of clock counting backwards to a predefined end.

(This description is partly based on or reuses content from the Wikipedia article "Timer" (http://en.wikipedia.org/wiki/Timer) and is licensed under the GNU Free Documentation License (http://www.gnu.org/copyleft/fdl.html).)</rdfs:comment>
  </GeneralFeatures>
  <gr:BusinessEntity rdf:ID="Chimei">
    <rdfs:comment xml:lang="en">The business entity Chimei.</rdfs:comment>
    <rdfs:seeAlso rdf:resource="http://www.chimei.com.tw/"/>
    <rdfs:label rdf:datatype="http://www.w3.org/2001/XMLSchema#string"
    >Chimei</rdfs:label>
    <gr:legalName rdf:datatype="http://www.w3.org/2001/XMLSchema#string"
    >CHIE MEI Optoelectronics Corp(CMO)</gr:legalName>
    <belongsToModule xml:lang="en">TV</belongsToModule>
  </gr:BusinessEntity>
  <gr:BusinessEntity rdf:ID="Difrnce">
    <rdfs:seeAlso rdf:resource="http://www.difrnce.nl/"/>
    <belongsToModule xml:lang="en">MP3Player</belongsToModule>
    <gr:legalName rdf:datatype="http://www.w3.org/2001/XMLSchema#string"
    >DIFRNCE B.V.</gr:legalName>
    <rdfs:comment xml:lang="en">The business entity DIFRNCE B.V.</rdfs:comment>
    <rdfs:label rdf:datatype="http://www.w3.org/2001/XMLSchema#string"
    >Difrnce</rdfs:label>
  </gr:BusinessEntity>
  <Color rdf:ID="Black">
    <rdfs:comment xml:lang="en">RGB Value 0,0,0</rdfs:comment>
    <rdfs:label xml:lang="en">Black</rdfs:label>
    <rdfs:label xml:lang="de">Schwarz</rdfs:label>
    <belongsToModule xml:lang="en">MP3Player, TV, Printer, DigitalCamera, Camcorder</belongsToModule>
  </Color>
  <PrintResolution rdf:ID="HP_REt">
    <belongsToModule xml:lang="en">Printer</belongsToModule>
    <rdfs:comment xml:lang="en">Special printing technology invented and used by HP.</rdfs:comment>
    <rdfs:label xml:lang="de">HP REt</rdfs:label>
    <rdfs:label xml:lang="en">HP REt</rdfs:label>
  </PrintResolution>
  <DataFormatVideo rdf:ID="MP4_Video">
    <belongsToModule xml:lang="en">MP3Player, DigitalCamera, Camcorder</belongsToModule>
    <rdfs:label xml:lang="en">MP4 Video</rdfs:label>
    <rdfs:label xml:lang="de">MP4 Video</rdfs:label>
    <rdfs:comment xml:lang="en">A collection of methods defining compression of video digital data.</rdfs:comment>
  </DataFormatVideo>
  <gr:BusinessEntity rdf:ID="GE">
    <rdfs:comment xml:lang="en">The business entity General Electric Company.</rdfs:comment>
    <rdfs:label rdf:datatype="http://www.w3.org/2001/XMLSchema#string"
    >GE</rdfs:label>
    <rdfs:seeAlso rdf:resource="http://www.ge.com/"/>
    <gr:legalName rdf:datatype="http://www.w3.org/2001/XMLSchema#string"
    >General Electric Company</gr:legalName>
    <belongsToModule xml:lang="en">DigitalCamera</belongsToModule>
  </gr:BusinessEntity>
  <MediaFormat rdf:ID="A7">
    <rdfs:comment xml:lang="en">Format of the german institute for standardization: 74 x 105 mm.</rdfs:comment>
    <belongsToModule xml:lang="en">Printer</belongsToModule>
    <rdfs:label xml:lang="de">A7</rdfs:label>
    <rdfs:label xml:lang="en">A7</rdfs:label>
  </MediaFormat>
  <Color rdf:ID="Beige">
    <rdfs:comment xml:lang="en">RGB Value 245,245,220</rdfs:comment>
    <rdfs:label xml:lang="en">Beige</rdfs:label>
    <rdfs:label xml:lang="de">Beige</rdfs:label>
    <belongsToModule xml:lang="en">MP3Player, TV, Printer, DigitalCamera, Camcorder</belongsToModule>
  </Color>
  <Color rdf:ID="Pink">
    <rdfs:label xml:lang="en">Pink</rdfs:label>
    <rdfs:label xml:lang="de">Pink</rdfs:label>
    <rdfs:comment xml:lang="en">RGB Value 255,192,203</rdfs:comment>
    <belongsToModule xml:lang="en">MP3Player, TV, Printer, DigitalCamera, Camcorder</belongsToModule>
  </Color>
  <Features rdf:ID="VoiceRecording">
    <rdfs:label xml:lang="de">Voicerekorder</rdfs:label>
    <rdfs:label xml:lang="en">Voicerecorder</rdfs:label>
    <rdfs:comment xml:lang="en">Ability to record sounds with a micro.</rdfs:comment>
    <belongsToModule xml:lang="en">MP3Player, DigitalCamera</belongsToModule>
  </Features>
  <SignalFormat rdf:ID="PAL">
    <rdfs:label xml:lang="en">PAL</rdfs:label>
    <rdfs:label xml:lang="de">PAL</rdfs:label>
    <rdfs:comment xml:lang="en">PAL, short for Phase Alternating Line, is a colour-encoding system used in broadcast television systems in large parts of the world.

(This description is partly based on or reuses content from the Wikipedia article "PAL" (http://en.wikipedia.org/wiki/PAL) and is licensed under the GNU Free Documentation License (http://www.gnu.org/copyleft/fdl.html).)</rdfs:comment>
    <belongsToModule xml:lang="en">TV</belongsToModule>
  </SignalFormat>
  <MediaFormat rdf:ID="B8">
    <rdfs:label xml:lang="de">B8</rdfs:label>
    <rdfs:label xml:lang="en">B8</rdfs:label>
    <belongsToModule xml:lang="en">Printer</belongsToModule>
    <rdfs:comment xml:lang="en">Format of the german institute for standardization: 62 x 88 mm.</rdfs:comment>
  </MediaFormat>
  <gr:BusinessEntity rdf:ID="Actebis">
    <rdfs:comment xml:lang="en">The business entity Actebis Peacock GmbH.</rdfs:comment>
    <rdfs:seeAlso rdf:resource="http://www.actebis.com/"/>
    <belongsToModule xml:lang="en">MP3Player</belongsToModule>
    <gr:legalName rdf:datatype="http://www.w3.org/2001/XMLSchema#string"
    >Actebis Peacock GmbH </gr:legalName>
    <rdfs:label rdf:datatype="http://www.w3.org/2001/XMLSchema#string"
    >Actebis</rdfs:label>
  </gr:BusinessEntity>
  <gr:BusinessEntity rdf:ID="PackardBell">
    <rdfs:comment xml:lang="en">The business entity Packard Bell.</rdfs:comment>
    <rdfs:label rdf:datatype="http://www.w3.org/2001/XMLSchema#string"
    >Packard Bell</rdfs:label>
    <belongsToModule xml:lang="en">MP3Player, TV</belongsToModule>
    <rdfs:seeAlso rdf:resource="http://www.packardbell.com/"/>
    <gr:legalName rdf:datatype="http://www.w3.org/2001/XMLSchema#string"
    >Packard Bell</gr:legalName>
  </gr:BusinessEntity>
  <Features rdf:ID="PictureViewing">
    <rdfs:label xml:lang="de">Bildbetrachtung</rdfs:label>
    <rdfs:label xml:lang="en">Picture viewing</rdfs:label>
    <belongsToModule xml:lang="en">MP3Player</belongsToModule>
    <rdfs:comment xml:lang="en">Ability to display digital pictures.</rdfs:comment>
  </Features>
  <Zoom rdf:ID="ZoomDigital">
    <rdfs:label xml:lang="de">Digitaler Zoom</rdfs:label>
    <rdfs:label xml:lang="en">Zoom digital</rdfs:label>
    <belongsToModule xml:lang="en">DigitalCamera</belongsToModule>
    <rdfs:comment xml:lang="en">Zoom is a method of decreasing (narrowing) the apparent angle of view of a photographic or video image.

(This description is partly based on or reuses content from the Wikipedia article "Digital zoom" (http://en.wikipedia.org/wiki/Digital_zoom) and is licensed under the GNU Free Documentation License (http://www.gnu.org/copyleft/fdl.html).)</rdfs:comment>
  </Zoom>
  <gr:BusinessEntity rdf:ID="Orion">
    <gr:legalName rdf:datatype="http://www.w3.org/2001/XMLSchema#string"
    >ORION - ISP Kommanditgesellschaft Dieter Lather</gr:legalName>
    <rdfs:comment xml:lang="en">The business entity Orion.</rdfs:comment>
    <belongsToModule xml:lang="en">TV</belongsToModule>
    <rdfs:seeAlso rdf:resource="http://www.orion-europa.de/"/>
    <rdfs:label rdf:datatype="http://www.w3.org/2001/XMLSchema#string"
    >Orion</rdfs:label>
  </gr:BusinessEntity>
  <VideoFeatures rdf:ID="ProgressiveScan">
    <rdfs:comment xml:lang="en">Progressive or noninterlaced scanning is a method for displaying, storing or transmitting moving images in which all the lines of each frame are drawn in sequence.

(This description is partly based on or reuses content from the Wikipedia article "Progressive scan" (http://en.wikipedia.org/wiki/Progressive_scan) and is licensed under the GNU Free Documentation License (http://www.gnu.org/copyleft/fdl.html).)</rdfs:comment>
    <rdfs:label xml:lang="en">Progressive Scan</rdfs:label>
    <rdfs:label xml:lang="de">Progressive Scan</rdfs:label>
    <belongsToModule xml:lang="en">TV</belongsToModule>
  </VideoFeatures>
  <Features rdf:ID="Alert">
    <rdfs:label xml:lang="en">Alert</rdfs:label>
    <rdfs:label xml:lang="de">Alarm</rdfs:label>
    <rdfs:comment xml:lang="en">Has wakeup-function.</rdfs:comment>
    <belongsToModule xml:lang="en">MP3Player</belongsToModule>
  </Features>
  <GeneralFeatures rdf:ID="PlugAndPlay">
    <rdfs:label xml:lang="en">Plug and Play</rdfs:label>
    <rdfs:label xml:lang="de">Plug and Play</rdfs:label>
    <rdfs:comment xml:lang="en">Describes any hardware specification that alleviates the need for user configuration of device resources.

(This description is partly based on or reuses content from the Wikipedia article "Legacy Plug and Play" (http://en.wikipedia.org/wiki/Legacy_Plug_and_Play) and is licensed under the GNU Free Documentation License (http://www.gnu.org/copyleft/fdl.html).)</rdfs:comment>
  </GeneralFeatures>
  <gr:BusinessEntity rdf:ID="Finlux">
    <rdfs:label rdf:datatype="http://www.w3.org/2001/XMLSchema#string"
    >Finlux</rdfs:label>
    <rdfs:seeAlso rdf:resource="http://www.finlux.fi/"/>
    <belongsToModule xml:lang="en">TV</belongsToModule>
    <rdfs:comment xml:lang="en">The business entity Finlux.</rdfs:comment>
    <gr:legalName rdf:datatype="http://www.w3.org/2001/XMLSchema#string"
    >Finlux Inc.</gr:legalName>
  </gr:BusinessEntity>
  <CompatibleOperatingSystems rdf:ID="MacOSXPuma">
    <rdfs:label xml:lang="en">Mac OS X Puma</rdfs:label>
    <rdfs:label xml:lang="de">Mac OS X Puma</rdfs:label>
    <belongsToModule xml:lang="en">MP3Player, Printer, DigitalCamera, Camcorder</belongsToModule>
    <rdfs:comment xml:lang="en">Mac OS is the trademarked name for a series of graphical user interface-based operating systems developed by Apple Inc. for their Macintosh line of computer systems.</rdfs:comment>
  </CompatibleOperatingSystems>
  <Color rdf:ID="Blue">
    <rdfs:comment xml:lang="en">RGB Value 0,0,255</rdfs:comment>
    <rdfs:label xml:lang="en">Blue</rdfs:label>
    <rdfs:label xml:lang="de">Blau</rdfs:label>
    <belongsToModule xml:lang="en">MP3Player, TV, Printer, DigitalCamera, Camcorder</belongsToModule>
  </Color>
  <gr:BusinessEntity rdf:ID="JVC">
    <rdfs:label rdf:datatype="http://www.w3.org/2001/XMLSchema#string"
    >JVC</rdfs:label>
    <rdfs:seeAlso rdf:resource="http://jdl.jvc-europe.com/"/>
    <gr:legalName rdf:datatype="http://www.w3.org/2001/XMLSchema#string"
    >Victor Company of Japan, limited</gr:legalName>
    <rdfs:comment xml:lang="en">The business entity Victor Company of Japan, Limited.</rdfs:comment>
    <belongsToModule xml:lang="en">MP3Player, TV, Camcorder</belongsToModule>
  </gr:BusinessEntity>
  <MediaType rdf:ID="PlainPaper">
    <belongsToModule xml:lang="en">Printer</belongsToModule>
    <rdfs:label xml:lang="de">Normalpapier</rdfs:label>
    <rdfs:label xml:lang="en">Plain paper</rdfs:label>
    <rdfs:comment xml:lang="en">Thin material mainly used for writing upon, printing upon or packaging.</rdfs:comment>
  </MediaType>
  <RechargeableEnergySource rdf:ID="NIH2">
    <rdfs:comment xml:lang="en">A nickel hydrogen battery (NIH2 or Ni-H2) is a rechargeable electrochemical power source based on nickel and hydrogen.</rdfs:comment>
    <rdfs:label xml:lang="en">NIH2</rdfs:label>
    <rdfs:label xml:lang="de">NIH2</rdfs:label>
    <belongsToModule xml:lang="en">MP3Player, DigitalCamera, Camcorder</belongsToModule>
  </RechargeableEnergySource>
  <DataFormatAudio rdf:ID="Format5.1ch">
    <belongsToModule xml:lang="en">Camcorder</belongsToModule>
    <rdfs:label xml:lang="de">Format 5.1ch</rdfs:label>
    <rdfs:label xml:lang="en">Format 5.1ch</rdfs:label>
    <rdfs:comment xml:lang="en">Encompasses a range of techniques for enriching (expanding and deepening) the sound reproduction quality, of an audio source, with additional audio channels reproduced via additional, discrete speakers.</rdfs:comment>
  </DataFormatAudio>
  <Color rdf:ID="Silver">
    <rdfs:label xml:lang="de">Silber</rdfs:label>
    <rdfs:label xml:lang="en">Silver</rdfs:label>
    <rdfs:comment xml:lang="en">RGB Value 192,192,192</rdfs:comment>
    <belongsToModule xml:lang="en">MP3Player, TV, Printer, DigitalCamera, Camcorder</belongsToModule>
  </Color>
  <DataFormatAudio rdf:ID="FLAC">
    <rdfs:label xml:lang="en">FLAC</rdfs:label>
    <rdfs:label xml:lang="de">FLAC</rdfs:label>
    <rdfs:comment xml:lang="en">Free Lossless Audio Codec (FLAC) is a file format for lossless audio data compression.

(This description is partly based on or reuses content from the Wikipedia article "Free Lossless Audio Codec" (http://en.wikipedia.org/wiki/Free_Lossless_Audio_Codec) and is licensed under the GNU Free Documentation License (http://www.gnu.org/copyleft/fdl.html).)</rdfs:comment>
    <belongsToModule xml:lang="en">MP3Player, DigitalCamera, Camcorder</belongsToModule>
  </DataFormatAudio>
  <MediaFormat rdf:ID="A0">
    <rdfs:label xml:lang="de">A0</rdfs:label>
    <rdfs:label xml:lang="en">A0</rdfs:label>
    <rdfs:comment xml:lang="en">Format of the german institute for standardization: 841 x 1189 mm.</rdfs:comment>
    <belongsToModule xml:lang="en">Printer</belongsToModule>
  </MediaFormat>
  <SignalFormat rdf:ID="NICAM">
    <rdfs:comment xml:lang="en">NICAM stands for Near Instantaneous Companded Audio Multiplex. It is an early form of lossy compression for digital audio.

(This description is partly based on or reuses content from the Wikipedia article "NICAM" (http://en.wikipedia.org/wiki/NICAM) and is licensed under the GNU Free Documentation License (http://www.gnu.org/copyleft/fdl.html).)</rdfs:comment>
    <belongsToModule xml:lang="en">TV</belongsToModule>
    <rdfs:label xml:lang="en">NICAM</rdfs:label>
    <rdfs:label xml:lang="de">NICAM</rdfs:label>
  </SignalFormat>
  <Features rdf:ID="Flash">
    <belongsToModule xml:lang="en">Camcorder</belongsToModule>
    <rdfs:comment xml:lang="en">Is a device used in photography that produces an instantaneous flash of artificial light.</rdfs:comment>
    <rdfs:label xml:lang="de">Blitz</rdfs:label>
    <rdfs:label xml:lang="en">Flash</rdfs:label>
  </Features>
  <GeneralFeatures rdf:ID="PowerLED">
    <rdfs:comment xml:lang="en">It is a semiconductor diode that emits light when an electric current is applied in the forward direction of the device used to show the power status of an electrical device.

(This description is partly based on or reuses content from the Wikipedia article "LED" (http://en.wikipedia.org/wiki/Led) and is licensed under the GNU Free Documentation License (http://www.gnu.org/copyleft/fdl.html).)</rdfs:comment>
    <belongsToModule xml:lang="en">TV, Camcorder</belongsToModule>
    <rdfs:label xml:lang="de">In-Betrieb Ledanzeige</rdfs:label>
    <rdfs:label xml:lang="en">Power LED</rdfs:label>
  </GeneralFeatures>
  <Features rdf:ID="WindFilter">
    <rdfs:label xml:lang="de">Windfilter</rdfs:label>
    <rdfs:label xml:lang="en">Wind filter</rdfs:label>
    <rdfs:comment xml:lang="en">Ability to filter out wind noises.</rdfs:comment>
    <belongsToModule xml:lang="en">Camcorder</belongsToModule>
  </Features>
  <gr:BusinessEntity rdf:ID="Kyocera">
    <belongsToModule xml:lang="en">Printer</belongsToModule>
    <gr:legalName rdf:datatype="http://www.w3.org/2001/XMLSchema#string"
    >Kyocera Corporation</gr:legalName>
    <rdfs:comment xml:lang="en">The business entity Kyocera.</rdfs:comment>
    <rdfs:label rdf:datatype="http://www.w3.org/2001/XMLSchema#string"
    >Kyocera</rdfs:label>
    <rdfs:seeAlso rdf:resource="http://global.kyocera.com/"/>
  </gr:BusinessEntity>
  <gr:BusinessEntity rdf:ID="Differo">
    <rdfs:seeAlso rdf:resource="http://www.differo.es/"/>
    <rdfs:label rdf:datatype="http://www.w3.org/2001/XMLSchema#string"
    >Differo</rdfs:label>
    <rdfs:comment xml:lang="en">The business entity Differo Ltd.</rdfs:comment>
    <belongsToModule xml:lang="en">MP3Player</belongsToModule>
    <gr:legalName rdf:datatype="http://www.w3.org/2001/XMLSchema#string"
    >Differo Ltd.</gr:legalName>
  </gr:BusinessEntity>
  <gr:BusinessEntity rdf:ID="Humax">
    <rdfs:seeAlso rdf:resource="http://www.humaxdigital.com/"/>
    <rdfs:comment xml:lang="en">The business entity Humax.</rdfs:comment>
    <gr:legalName rdf:datatype="http://www.w3.org/2001/XMLSchema#string"
    >HUMAX Electronics Co Ltd.</gr:legalName>
    <rdfs:label rdf:datatype="http://www.w3.org/2001/XMLSchema#string"
    >Humax</rdfs:label>
    <belongsToModule rdf:datatype="http://www.w3.org/2001/XMLSchema#string"
    >TV</belongsToModule>
  </gr:BusinessEntity>
  <gr:BusinessEntity rdf:ID="Pendrive">
    <rdfs:seeAlso rdf:resource="http://www.pendrive.com/"/>
    <rdfs:comment xml:lang="en">The business entity dynaTRON Electronics GmbH &amp; Co KG.</rdfs:comment>
    <rdfs:label rdf:datatype="http://www.w3.org/2001/XMLSchema#string"
    >Pendrive</rdfs:label>
    <belongsToModule xml:lang="en">MP3Player, DigitalCamera</belongsToModule>
    <gr:legalName rdf:datatype="http://www.w3.org/2001/XMLSchema#string"
    >dynaTRON Electronics GmbH &amp; Co. KG </gr:legalName>
  </gr:BusinessEntity>
  <ComputerDisplayResolution rdf:ID="ComputerDisplayResolution_1024x768_60_70_75_85Hz">
    <belongsToModule xml:lang="en">TV</belongsToModule>
    <rdfs:label xml:lang="en">Computer display resolution 1024x768 60 70 75 85Hz</rdfs:label>
    <rdfs:label xml:lang="de">Computerbildschirmauflösung 1024x768 60 70 75 85Hz</rdfs:label>
    <rdfs:comment xml:lang="en">Display resolution specified as the width and height in pixels, color depth measured in bits, and refresh rate expressed in hertz; here Extended Graphics Array.

(This description is partly based on or reuses content from the Wikipedia article "Display resolution" (http://en.wikipedia.org/wiki/Display_resolution) and is licensed under the GNU Free Documentation License (http://www.gnu.org/copyleft/fdl.html).)</rdfs:comment>
  </ComputerDisplayResolution>
  <DataFormatImage rdf:ID="SVG">
    <rdfs:comment xml:lang="en">SVG (Scalable Vector Graphics) is an open standard created and developed by the World Wide Web Consortium to address the need (and attempts of several corporations) for a versatile, scriptable and all-purpose vector format for the web and otherwise.

(This description is partly based on or reuses content from the Wikipedia article "Vector graphics" (http://en.wikipedia.org/wiki/Vector_graphics) and is licensed under the GNU Free Documentation License (http://www.gnu.org/copyleft/fdl.html).)</rdfs:comment>
    <belongsToModule xml:lang="en">MP3Player, , DigitalCamera, Camcorder</belongsToModule>
    <rdfs:label xml:lang="en">SVG</rdfs:label>
    <rdfs:label xml:lang="de">SVG</rdfs:label>
  </DataFormatImage>
  <ViewFinder rdf:ID="ViewFinderOptical">
    <belongsToModule xml:lang="en">DigitalCamera</belongsToModule>
    <rdfs:comment xml:lang="en">An optical viewfinder is simply a reversed telescope mounted to see what the camera will see.

(This description is partly based on or reuses content from the Wikipedia article "Viewfinder" (http://en.wikipedia.org/wiki/Viewfinder) and is licensed under the GNU Free Documentation License (http://www.gnu.org/copyleft/fdl.html).)</rdfs:comment>
    <rdfs:label xml:lang="en">Viewfinder optical</rdfs:label>
    <rdfs:label xml:lang="de">Optischer Bildsucher</rdfs:label>
  </ViewFinder>
  <gr:BusinessEntity rdf:ID="Aigo">
    <rdfs:label rdf:datatype="http://www.w3.org/2001/XMLSchema#string"
    >Aigo</rdfs:label>
    <belongsToModule xml:lang="en">MP3Player</belongsToModule>
    <rdfs:seeAlso rdf:resource="http://www.aigo.com/"/>
    <rdfs:comment xml:lang="en">The business entity Beijing Huaqi Information Digital Technology Co., Ltd.</rdfs:comment>
    <gr:legalName rdf:datatype="http://www.w3.org/2001/XMLSchema#string"
    >Beijing Huaqi Information Digital Technology Co., Ltd.</gr:legalName>
  </gr:BusinessEntity>
  <owl:AnnotationProperty rdf:about="http://purl.org/dc/elements/1.1/contributor"/>
  <DisplayType rdf:ID="PDP">
    <rdfs:label xml:lang="en">PDP</rdfs:label>
    <rdfs:label xml:lang="de">PDP</rdfs:label>
    <rdfs:comment xml:lang="en">A plasma display panel (PDP) is a type of flat panel display common to large TV displays (37in. [940mm]). Many tiny cells between two panels of glass hold an inert mixture of noble gases. The gas in the cells is electrically turned into a plasma which then excites phosphors to emit light.

(This description is partly based on or reuses content from the Wikipedia article "Digital newspaper technology - Plasma" (http://en.wikipedia.org/wiki/Digital_newspaper_technology#Plasma) and is licensed under the GNU Free Documentation License (http://www.gnu.org/copyleft/fdl.html).)</rdfs:comment>
  </DisplayType>
  <VideoFeatures rdf:ID="PerfectPixelHD">
    <rdfs:label xml:lang="en">Perfect Pixel HD</rdfs:label>
    <rdfs:label xml:lang="de">Perfect Pixel HD</rdfs:label>
    <rdfs:comment xml:lang="en">Perfect Pixel HD Engine offers the unique combination of ultimate sharpness, natural detail, vivid colours and smooth natural motion on all qualities of HD, standard TV signals and multimedia content, for high definition displays. Each pixel of the incoming picture is enhanced to better match the surrounding pixels, resulting in a more natural picture.</rdfs:comment>
    <belongsToModule xml:lang="en">TV</belongsToModule>
  </VideoFeatures>
  <SignalFormat rdf:ID="NTSC">
    <rdfs:label xml:lang="en">NTSC</rdfs:label>
    <rdfs:label xml:lang="de">NTSC</rdfs:label>
    <belongsToModule xml:lang="en">TV</belongsToModule>
    <rdfs:comment xml:lang="en">NTSC (National Television Standard Conversion) is the analog television system used in most of the Americas, Japan, South Korea, Taiwan, the Philippines, Burma, and some Pacific island nations and territories.

(This description is partly based on or reuses content from the Wikipedia article "NTSC" (http://en.wikipedia.org/wiki/NTSC) and is licensed under the GNU Free Documentation License (http://www.gnu.org/copyleft/fdl.html).)</rdfs:comment>
  </SignalFormat>
  <gr:BusinessEntity rdf:ID="Yusmart">
    <rdfs:seeAlso rdf:resource="http://www.yusmart-lcd.co.uk/"/>
    <rdfs:comment xml:lang="en">The business entity Yusmart.</rdfs:comment>
    <gr:legalName rdf:datatype="http://www.w3.org/2001/XMLSchema#string"
    >Yusmart B.V.</gr:legalName>
    <belongsToModule xml:lang="en">TV</belongsToModule>
    <rdfs:label rdf:datatype="http://www.w3.org/2001/XMLSchema#string"
    >Yusmart</rdfs:label>
  </gr:BusinessEntity>
  <DataFormatAudio rdf:ID="WMA">
    <rdfs:label xml:lang="en">WMA</rdfs:label>
    <rdfs:label xml:lang="de">WMA</rdfs:label>
    <rdfs:comment xml:lang="en">An audio data compression technology developed by Microsoft.</rdfs:comment>
    <belongsToModule xml:lang="en">MP3Player, DigitalCamera, Camcorder</belongsToModule>
  </DataFormatAudio>
  <MediaType rdf:ID="Postcard">
    <rdfs:label xml:lang="de">Postkarte</rdfs:label>
    <rdfs:label xml:lang="en">Postcard</rdfs:label>
    <rdfs:comment xml:lang="en">Rectangular piece of thick paper or thin cardboard intended for writing and mailing without an envelope.</rdfs:comment>
    <belongsToModule xml:lang="en">Printer</belongsToModule>
  </MediaType>
  <gr:BusinessEntity rdf:ID="Panasonic">
    <rdfs:label rdf:datatype="http://www.w3.org/2001/XMLSchema#string"
    >Panasonic</rdfs:label>
    <gr:legalName rdf:datatype="http://www.w3.org/2001/XMLSchema#string"
    >Panasonic Corporation</gr:legalName>
    <belongsToModule xml:lang="en">MP3Player, TV, Printer, DigitalCamera, Camcorder</belongsToModule>
    <rdfs:seeAlso rdf:resource="http://www.panasonic.com/"/>
    <rdfs:comment xml:lang="en">The business entity Panasonic Corporation.</rdfs:comment>
  </gr:BusinessEntity>
  <gr:BusinessEntity rdf:ID="Maxfield">
    <rdfs:label rdf:datatype="http://www.w3.org/2001/XMLSchema#string"
    >Maxfield</rdfs:label>
    <belongsToModule xml:lang="en">MP3Player</belongsToModule>
    <rdfs:seeAlso rdf:resource="http://www.maxfield.de/"/>
    <gr:legalName rdf:datatype="http://www.w3.org/2001/XMLSchema#string"
    >Maxfield GmbH</gr:legalName>
    <rdfs:comment xml:lang="en">The business entity Maxfield GmbH.</rdfs:comment>
  </gr:BusinessEntity>
  <MediaType rdf:ID="Cardstock">
    <rdfs:label xml:lang="de">Fotokarton</rdfs:label>
    <rdfs:label xml:lang="en">cardstock</rdfs:label>
    <rdfs:comment xml:lang="en">A paper stock that is thicker and more durable than normal writing or printing paper, but thinner and more flexible than other forms of paperboard.

(This description is partly based on or reuses content from the Wikipedia article "Cardstock" (http://en.wikipedia.org/wiki/Card_stock) and is licensed under the GNU Free Documentation License (http://www.gnu.org/copyleft/fdl.html).)</rdfs:comment>
    <belongsToModule xml:lang="en">Printer</belongsToModule>
  </MediaType>
  <owl:AnnotationProperty rdf:about="http://purl.org/dc/elements/1.1/subject"/>
  <PrintResolution rdf:ID="HP_FastRes_1200_DPI">
    <belongsToModule xml:lang="en">Printer</belongsToModule>
    <rdfs:comment xml:lang="en">Special printing technology invented and used by HP.</rdfs:comment>
    <rdfs:label xml:lang="de">HP FastRes 1200 DPI</rdfs:label>
    <rdfs:label xml:lang="en">HP FastRes 1200 DPI</rdfs:label>
  </PrintResolution>
  <gr:BusinessEntity rdf:ID="IBM">
    <rdfs:label rdf:datatype="http://www.w3.org/2001/XMLSchema#string"
    >IBM</rdfs:label>
    <rdfs:comment xml:lang="en">The business entity IBM.</rdfs:comment>
    <belongsToModule xml:lang="en">Printer</belongsToModule>
    <gr:legalName rdf:datatype="http://www.w3.org/2001/XMLSchema#string"
    >International Business Machines Corporation</gr:legalName>
    <rdfs:seeAlso rdf:resource="http://www.ibm.com/"/>
  </gr:BusinessEntity>
  <gr:BusinessEntity rdf:ID="SanDisk">
    <rdfs:comment xml:lang="en">The business entity SanDisk Corporation.</rdfs:comment>
    <gr:legalName rdf:datatype="http://www.w3.org/2001/XMLSchema#string"
    >SanDisk Corporation</gr:legalName>
    <rdfs:label rdf:datatype="http://www.w3.org/2001/XMLSchema#string"
    >Sandisk</rdfs:label>
    <rdfs:seeAlso rdf:resource="http://sandisk.de/"/>
    <belongsToModule xml:lang="en">MP3Player</belongsToModule>
  </gr:BusinessEntity>
  <VideoFeatures rdf:ID="DigitalCrystalClear">
    <rdfs:label xml:lang="en">Digital Crystal Clear</rdfs:label>
    <rdfs:label xml:lang="de">Digital Crystal Clear</rdfs:label>
    <rdfs:comment xml:lang="en">Digital Crystal Clear is a package of picture innovations that digitally adjusts and optimises picture quality to optimal contrast, colour and sharpness levels.</rdfs:comment>
    <belongsToModule xml:lang="en">TV</belongsToModule>
  </VideoFeatures>
  <VideoFeatures rdf:ID="AmbilightSpectra2">
    <rdfs:comment xml:lang="en">Ambilight Spectra 2 generates reactive ambient lighting on both sides of a Flat TV.</rdfs:comment>
    <rdfs:label xml:lang="en">Ambilight Spectra 2</rdfs:label>
    <rdfs:label xml:lang="de">Ambilight Spectra 2</rdfs:label>
    <belongsToModule xml:lang="en">TV</belongsToModule>
  </VideoFeatures>
  <Connectivity rdf:ID="TRSConnector">
    <rdfs:comment xml:lang="en">A TRS connector (tip, ring, sleeve) also called an audio jack, phone plug, jack plug, stereo plug, mini-jack, or mini-stereo, is a common audio connector. It is cylindrical in shape, typically with three contacts, although sometimes with two (a TS connector) or four (a TRRS connector).

(This description is partly based on or reuses content from the Wikipedia article "TRS connector" (http://en.wikipedia.org/wiki/TRS_connector) and is licensed under the GNU Free Documentation License (http://www.gnu.org/copyleft/fdl.html).)</rdfs:comment>
    <belongsToModule xml:lang="en">TV</belongsToModule>
    <rdfs:label xml:lang="en">TRS connector</rdfs:label>
    <rdfs:label xml:lang="de">TRS Verbindungsstecker</rdfs:label>
  </Connectivity>
  <DataFormatAudio rdf:ID="MP3">
    <rdfs:comment xml:lang="en">A digital audio encoding format using a form of lossy data compression.</rdfs:comment>
    <belongsToModule xml:lang="en">MP3Player, DigitalCamera, Camcorder</belongsToModule>
    <rdfs:label xml:lang="en">MP3</rdfs:label>
    <rdfs:label xml:lang="de">MP3</rdfs:label>
  </DataFormatAudio>
  <DataInterfaceType rdf:ID="PictBridge">
    <rdfs:comment xml:lang="en">Is an industry standard from the Camera &amp; Imaging Products Association (CIPA) for direct printing.</rdfs:comment>
    <rdfs:label xml:lang="de">PictBridge</rdfs:label>
    <rdfs:label xml:lang="en">PictBridge</rdfs:label>
    <belongsToModule xml:lang="en">Camcorder</belongsToModule>
  </DataInterfaceType>
  <Focus rdf:ID="FocusManual">
    <belongsToModule xml:lang="en">DigitalCamera, Camcorder</belongsToModule>
    <rdfs:label xml:lang="de">Manueller Fokus</rdfs:label>
    <rdfs:label xml:lang="en">Focus manual</rdfs:label>
    <rdfs:comment xml:lang="en">A manual focus allows the operator to adjust the focus of the lens by hand.

(This description is partly based on or reuses content from the Wikipedia article "Manual focus" (http://en.wikipedia.org/wiki/Manual_focus) and is licensed under the GNU Free Documentation License (http://www.gnu.org/copyleft/fdl.html).)</rdfs:comment>
  </Focus>
  <AudioFeatures rdf:ID="DynamicBassEnhancement">
    <rdfs:comment xml:lang="en">Dynamic settlement of bass audiosignals.</rdfs:comment>
    <rdfs:label xml:lang="de">Dynamischer Bass</rdfs:label>
    <rdfs:label xml:lang="en">Dynamic bass enhancement</rdfs:label>
    <belongsToModule xml:lang="en">TV</belongsToModule>
  </AudioFeatures>
  <gr:BusinessEntity rdf:ID="Intuix">
    <rdfs:label rdf:datatype="http://www.w3.org/2001/XMLSchema#string"
    >Intuix</rdfs:label>
    <gr:legalName rdf:datatype="http://www.w3.org/2001/XMLSchema#string"
    >Intuix LLC</gr:legalName>
    <belongsToModule xml:lang="en">MP3Player</belongsToModule>
    <rdfs:seeAlso rdf:resource="http://www.intuix.net/"/>
    <rdfs:comment xml:lang="en">The business entity Intuix LLC.</rdfs:comment>
  </gr:BusinessEntity>
  <GeneralFeatures rdf:ID="ChildSafetyLock">
    <rdfs:comment xml:lang="en">A child safety lock is a special-purpose lock that is designed to help prevent children from getting at any dangerous contents.

(This description is partly based on or reuses content from the Wikipedia article "Child safety lock" (http://en.wikipedia.org/wiki/Child_safety_lock) and is licensed under the GNU Free Documentation License (http://www.gnu.org/copyleft/fdl.html).)</rdfs:comment>
    <rdfs:label xml:lang="de">Kindersicherung</rdfs:label>
    <rdfs:label xml:lang="en">Child safety lock</rdfs:label>
    <belongsToModule xml:lang="en">TV</belongsToModule>
  </GeneralFeatures>
  <SceneMode rdf:ID="Spotlight">
    <belongsToModule xml:lang="en">Camcorder</belongsToModule>
    <rdfs:comment xml:lang="en">Ability of the camcorder to adapt to special environments.</rdfs:comment>
    <rdfs:label xml:lang="de">Spotlight</rdfs:label>
    <rdfs:label xml:lang="en">Spotlight</rdfs:label>
  </SceneMode>
  <MediaFormat rdf:ID="B1">
    <rdfs:label xml:lang="de">B1</rdfs:label>
    <rdfs:label xml:lang="en">B1</rdfs:label>
    <belongsToModule xml:lang="en">Printer</belongsToModule>
    <rdfs:comment xml:lang="en">Format of the german institute for standardization: 707 x 1000 mm.</rdfs:comment>
  </MediaFormat>
  <DataFormatVideo rdf:ID="DV">
    <rdfs:label xml:lang="de">DV</rdfs:label>
    <rdfs:label xml:lang="en">DV</rdfs:label>
    <rdfs:comment xml:lang="en">Digital Video (DV) is a digital video format created by Sony, JVC, Panasonic and other video camera producers, and launched in 1995. The DV specification (originally known as the Blue Book, current official name IEC 61834) defines both the codec and the tape format.

(This description is partly based on or reuses content from the Wikipedia article "DV" (http://en.wikipedia.org/wiki/DV) and is licensed under the GNU Free Documentation License (http://www.gnu.org/copyleft/fdl.html).)</rdfs:comment>
    <belongsToModule xml:lang="en">DigitalCamera, Camcorder</belongsToModule>
  </DataFormatVideo>
  <gr:BusinessEntity rdf:ID="Dell">
    <rdfs:comment xml:lang="en">The business entity Dell.</rdfs:comment>
    <belongsToModule xml:lang="en">Printer</belongsToModule>
    <gr:legalName rdf:datatype="http://www.w3.org/2001/XMLSchema#string"
    >Dell Inc.</gr:legalName>
    <rdfs:label rdf:datatype="http://www.w3.org/2001/XMLSchema#string"
    >Dell</rdfs:label>
    <rdfs:seeAlso rdf:resource="http://www.dell.com/"/>
  </gr:BusinessEntity>
  <DisplayType rdf:ID="Multicolor">
    <rdfs:comment xml:lang="en">Ability to display more than two different kinds of color.</rdfs:comment>
    <rdfs:label xml:lang="en">Multicolor</rdfs:label>
    <rdfs:label xml:lang="de">Mehrfarbig</rdfs:label>
    <belongsToModule xml:lang="en">MP3Player</belongsToModule>
  </DisplayType>
  <DataFormatAudio rdf:ID="DolbyDigital">
    <rdfs:comment xml:lang="en">The marketing name for a series of lossy audio compression technologies developed by Dolby Laboratories.

(This description is partly based on or reuses content from the Wikipedia article "Dolby Digital" (http://en.wikipedia.org/wiki/Dolby_Digital) and is licensed under the GNU Free Documentation License (http://www.gnu.org/copyleft/fdl.html).)</rdfs:comment>
    <rdfs:label xml:lang="de">DolbyDigital</rdfs:label>
    <rdfs:label xml:lang="en">DolbyDigital</rdfs:label>
    <belongsToModule xml:lang="en">Camcorder</belongsToModule>
  </DataFormatAudio>
  <gr:BusinessEntity rdf:ID="TrekStor">
    <rdfs:seeAlso rdf:resource="http://www.trekstor.de/"/>
    <gr:legalName rdf:datatype="http://www.w3.org/2001/XMLSchema#string"
    >TrekStor GmbH &amp; Co. KG</gr:legalName>
    <belongsToModule xml:lang="en">MP3Player</belongsToModule>
    <rdfs:comment xml:lang="en">The business entity TrekStore GmbH &amp; Co. KG</rdfs:comment>
    <rdfs:label rdf:datatype="http://www.w3.org/2001/XMLSchema#string"
    >Trekstor</rdfs:label>
  </gr:BusinessEntity>
  <gr:BusinessEntity rdf:ID="V7">
    <gr:legalName rdf:datatype="http://www.w3.org/2001/XMLSchema#string"
    >V7</gr:legalName>
    <rdfs:label rdf:datatype="http://www.w3.org/2001/XMLSchema#string"
    >V7</rdfs:label>
    <belongsToModule xml:lang="en">TV</belongsToModule>
    <rdfs:seeAlso rdf:resource="http://www.v7-world.com/"/>
    <rdfs:comment xml:lang="en">The business entity Videoseven.</rdfs:comment>
  </gr:BusinessEntity>
  <ProcessorType rdf:ID="PowerPC_32_bit">
    <rdfs:comment xml:lang="en">A RISC instruction set architecture created by the 1991 Apple-IBM-Motorola alliance, known as AIM. Originally intended for personal computers, PowerPC CPUs have since become popular embedded and high-performance processors.</rdfs:comment>
    <belongsToModule xml:lang="en">Printer</belongsToModule>
    <rdfs:label xml:lang="de">PowerPC 32 bit</rdfs:label>
    <rdfs:label xml:lang="en">PowerPC 32 bit</rdfs:label>
  </ProcessorType>
  <gr:BusinessEntity rdf:ID="DK_digital">
    <rdfs:comment xml:lang="en">The business entity DK digital GmbH.</rdfs:comment>
    <rdfs:seeAlso rdf:resource="http://www.dk-digital.com/"/>
    <belongsToModule xml:lang="en">MP3Player</belongsToModule>
    <rdfs:label rdf:datatype="http://www.w3.org/2001/XMLSchema#string"
    >DK digital</rdfs:label>
    <gr:legalName rdf:datatype="http://www.w3.org/2001/XMLSchema#string"
    >DK digital GmbH</gr:legalName>
  </gr:BusinessEntity>
  <gr:BusinessEntity rdf:ID="Archos">
    <rdfs:seeAlso rdf:resource="http://www.archos.com/"/>
    <belongsToModule xml:lang="en">MP3Player, Camcorder</belongsToModule>
    <rdfs:label rdf:datatype="http://www.w3.org/2001/XMLSchema#string"
    >Archos</rdfs:label>
    <gr:legalName rdf:datatype="http://www.w3.org/2001/XMLSchema#string"
    >Archos GmbH</gr:legalName>
    <rdfs:comment xml:lang="en">The business entity Archos GmbH.</rdfs:comment>
  </gr:BusinessEntity>
  <gr:BusinessEntity rdf:ID="Intenso">
    <belongsToModule xml:lang="en">MP3Player</belongsToModule>
    <rdfs:label rdf:datatype="http://www.w3.org/2001/XMLSchema#string"
    >Intenso</rdfs:label>
    <rdfs:comment xml:lang="en">The business entity Intenso GmbH.</rdfs:comment>
    <gr:legalName rdf:datatype="http://www.w3.org/2001/XMLSchema#string"
    >Intenso GmbH</gr:legalName>
    <rdfs:seeAlso rdf:resource="http://www.intenso.de/"/>
  </gr:BusinessEntity>
  <AudioInterfaceType rdf:ID="Audio3.5mm">
    <rdfs:comment xml:lang="en">Audio interface type of a specific diameter.</rdfs:comment>
    <rdfs:label xml:lang="en">Audio 3.5mm</rdfs:label>
    <rdfs:label xml:lang="de">Audio 3.5mm</rdfs:label>
    <belongsToModule xml:lang="en">MP3Player</belongsToModule>
  </AudioInterfaceType>
  <gr:BusinessEntity rdf:ID="Olympus">
    <rdfs:label rdf:datatype="http://www.w3.org/2001/XMLSchema#string"
    >Olympus</rdfs:label>
    <rdfs:comment xml:lang="en">The business entity Olympus Europa Holding GmbH.</rdfs:comment>
    <belongsToModule xml:lang="en">MP3Player, DigitalCamera</belongsToModule>
    <gr:legalName rdf:datatype="http://www.w3.org/2001/XMLSchema#string"
    >Olympus Europa Holding GmbH Corporate Communications</gr:legalName>
    <rdfs:seeAlso rdf:resource="http://www.olympus.de/"/>
  </gr:BusinessEntity>
  <AudioFeatures rdf:ID="AutoVolumeLeveller">
    <belongsToModule xml:lang="en">TV</belongsToModule>
    <rdfs:label xml:lang="de">Automatische Lautstärkenanpassung</rdfs:label>
    <rdfs:label xml:lang="en">Auto volume leveller</rdfs:label>
    <rdfs:comment xml:lang="en">Levels the audio volume of televisions automatically so that undesired peaks in the sound can be reduced.</rdfs:comment>
  </AudioFeatures>
  <DataFormatOffice rdf:ID="PDF">
    <rdfs:comment xml:lang="en">Portable Document Format (PDF) is a file format created by Adobe Systems in 1993 for document exchange.

(This description is partly based on or reuses content from the Wikipedia article "Pdf" (http://en.wikipedia.org/wiki/Pdf) and is licensed under the GNU Free Documentation License (http://www.gnu.org/copyleft/fdl.html).)</rdfs:comment>
    <belongsToModule xml:lang="en">MP3Player, DigitalCamera</belongsToModule>
    <rdfs:label xml:lang="en">PDF</rdfs:label>
    <rdfs:label xml:lang="de">PDF</rdfs:label>
  </DataFormatOffice>
  <gr:BusinessEntity rdf:ID="AIPTEK">
    <belongsToModule xml:lang="en">DigitalCamera, Camcorder</belongsToModule>
    <rdfs:comment xml:lang="en">The business entity AIPTEK, Inc.</rdfs:comment>
    <rdfs:label rdf:datatype="http://www.w3.org/2001/XMLSchema#string"
    >AIPTEK</rdfs:label>
    <rdfs:seeAlso rdf:resource="http://www.aiptek.com/"/>
    <gr:legalName rdf:datatype="http://www.w3.org/2001/XMLSchema#string"
    >AIPTEK, Inc.</gr:legalName>
  </gr:BusinessEntity>
  <gr:BusinessEntity rdf:ID="Nanopoint">
    <rdfs:seeAlso rdf:resource="http://www.nanopoint.co.uk/"/>
    <gr:legalName rdf:datatype="http://www.w3.org/2001/XMLSchema#string"
    >Nanopoint Technology Inc.</gr:legalName>
    <rdfs:comment xml:lang="en">The business entity Nanopoint Technology Inc.</rdfs:comment>
    <rdfs:label rdf:datatype="http://www.w3.org/2001/XMLSchema#string"
    >Nanopoint</rdfs:label>
    <belongsToModule xml:lang="en">MP3Player</belongsToModule>
  </gr:BusinessEntity>
  <gr:BusinessEntity rdf:ID="TakeMS">
    <rdfs:seeAlso rdf:resource="http://www.takems.de/"/>
    <rdfs:comment xml:lang="en">The business entity takeMS International AG.</rdfs:comment>
    <belongsToModule xml:lang="en">MP3Player</belongsToModule>
    <rdfs:label rdf:datatype="http://www.w3.org/2001/XMLSchema#string"
    >takeMS</rdfs:label>
    <gr:legalName rdf:datatype="http://www.w3.org/2001/XMLSchema#string"
    >takeMS International AG</gr:legalName>
  </gr:BusinessEntity>
  <gr:BusinessEntity rdf:ID="Hannspree">
    <rdfs:seeAlso rdf:resource="http://www.hannspree.com/"/>
    <gr:legalName rdf:datatype="http://www.w3.org/2001/XMLSchema#string"
    >Hannspree Inc.</gr:legalName>
    <rdfs:label rdf:datatype="http://www.w3.org/2001/XMLSchema#string"
    >Hannspree</rdfs:label>
    <rdfs:comment xml:lang="en">The business entity Hannspree.</rdfs:comment>
    <belongsToModule xml:lang="en">TV</belongsToModule>
  </gr:BusinessEntity>
  <MediaFormat rdf:ID="A2">
    <belongsToModule xml:lang="en">Printer</belongsToModule>
    <rdfs:comment xml:lang="en">Format of the german institute for standardization: 420 x 594 mm.</rdfs:comment>
    <rdfs:label xml:lang="de">A2</rdfs:label>
    <rdfs:label xml:lang="en">A2</rdfs:label>
  </MediaFormat>
  <RechargeableEnergySource rdf:ID="Li-Ion_Polymer">
    <rdfs:label xml:lang="en">Li-ion Polymer</rdfs:label>
    <rdfs:label xml:lang="de">Li-ion Polymer</rdfs:label>
    <rdfs:comment xml:lang="en">Lithium polymer batteries (abbreviated Li-poly, Li-Pol, LiPo, LIP, PLI or LiP) are rechargeable batteries which have technologically evolved from lithium-ion batteries.

(This description is partly based on or reuses content from the Wikipedia article "Lithium-polymer" (http://en.wikipedia.org/wiki/Lithium-polymer) and is licensed under the GNU Free Documentation License (http://www.gnu.org/copyleft/fdl.html).)</rdfs:comment>
    <belongsToModule xml:lang="en">MP3Player, DigitalCamera, Camcorder</belongsToModule>
  </RechargeableEnergySource>
  <Accessory rdf:ID="AV_Cable">
    <rdfs:comment xml:lang="en">A cable to carry video and audio signals from a device, to a tv; in digital or analog format.</rdfs:comment>
    <belongsToModule xml:lang="en">Camcorder</belongsToModule>
    <rdfs:label xml:lang="en">AV cable</rdfs:label>
    <rdfs:label xml:lang="de">AV Kabel</rdfs:label>
  </Accessory>
  <gr:BusinessEntity rdf:ID="Lenco">
    <rdfs:label rdf:datatype="http://www.w3.org/2001/XMLSchema#string"
    >Lenco</rdfs:label>
    <belongsToModule xml:lang="en">MP3Player, TV</belongsToModule>
    <rdfs:seeAlso rdf:resource="http://www.lenco-audiovideo.com/"/>
    <rdfs:comment xml:lang="en">The business entity Lenco Audio-Video.</rdfs:comment>
    <gr:legalName rdf:datatype="http://www.w3.org/2001/XMLSchema#string"
    >Lenco Audio-Video</gr:legalName>
  </gr:BusinessEntity>
  <gr:BusinessEntity rdf:ID="AOC">
    <rdfs:seeAlso rdf:resource="http://www.aoc-europe.com/"/>
    <rdfs:comment xml:lang="en">The business entity AOC.</rdfs:comment>
    <gr:legalName rdf:datatype="http://www.w3.org/2001/XMLSchema#string"
    >AOC</gr:legalName>
    <rdfs:label rdf:datatype="http://www.w3.org/2001/XMLSchema#string"
    >AOC</rdfs:label>
  </gr:BusinessEntity>
  <SignalFormat rdf:ID="DVB">
    <rdfs:comment xml:lang="en">Digital Video Broadcasting (DVB) is a suite of internationally accepted open standards for digital television. DVB systems distribute data using a variety of approaches, including by satellite (DVB-S, DVB-S2 and DVB-SH; also DVB-SMATV for distribution via SMATV); cable (DVB-C); terrestrial television (DVB-T, DVB-T2) and digital terrestrial television for handhelds (DVB-H,DVB-SH); and via microwave using DTT (DVB-MT), the MMDS (DVB-MC), and/or MVDS standards (DVB-MS).

(This description is partly based on or reuses content from the Wikipedia article "Digital Video Broadcasting" (http://en.wikipedia.org/wiki/Digital_Video_Broadcasting) and is licensed under the GNU Free Documentation License (http://www.gnu.org/copyleft/fdl.html).)</rdfs:comment>
    <belongsToModule xml:lang="en">TV</belongsToModule>
    <rdfs:label xml:lang="en">DVB</rdfs:label>
    <rdfs:label xml:lang="de">DVB</rdfs:label>
  </SignalFormat>
  <DataFormatOffice rdf:ID="DOC">
    <rdfs:comment xml:lang="en">A file extension for word processing documents.</rdfs:comment>
    <belongsToModule xml:lang="en">MP3Player, DigitalCamera</belongsToModule>
    <rdfs:label xml:lang="en">DOC</rdfs:label>
    <rdfs:label xml:lang="de">DOC</rdfs:label>
  </DataFormatOffice>
  <gr:BusinessEntity rdf:ID="Pentax">
    <rdfs:seeAlso rdf:resource="http://www.pentax.jp/english/"/>
    <belongsToModule xml:lang="en">DigitalCamera</belongsToModule>
    <rdfs:comment xml:lang="en">The business entity Pentax Corporation.</rdfs:comment>
    <gr:legalName rdf:datatype="http://www.w3.org/2001/XMLSchema#string"
    >Pentax Corporation</gr:legalName>
    <rdfs:label rdf:datatype="http://www.w3.org/2001/XMLSchema#string"
    >Pentax</rdfs:label>
  </gr:BusinessEntity>
  <gr:BusinessEntity rdf:ID="Vestel">
    <belongsToModule xml:lang="en">TV</belongsToModule>
    <rdfs:seeAlso rdf:resource="http://www.vestel.com/"/>
    <rdfs:label rdf:datatype="http://www.w3.org/2001/XMLSchema#string"
    >Vestel</rdfs:label>
    <rdfs:comment xml:lang="en">The business entity Vestel.</rdfs:comment>
    <gr:legalName rdf:datatype="http://www.w3.org/2001/XMLSchema#string"
    >Vestel Electronics</gr:legalName>
  </gr:BusinessEntity>
  <gr:BusinessEntity rdf:ID="Yuraku">
    <rdfs:comment xml:lang="en">The business entity Yuraku.</rdfs:comment>
    <rdfs:label rdf:datatype="http://www.w3.org/2001/XMLSchema#string"
    >Yuraku</rdfs:label>
    <belongsToModule xml:lang="en">TV</belongsToModule>
    <gr:legalName rdf:datatype="http://www.w3.org/2001/XMLSchema#string"
    >YURAKU Pte Ltd.</gr:legalName>
    <rdfs:seeAlso rdf:resource="http://www.yuraku.com.sg/"/>
  </gr:BusinessEntity>
  <CompatibleOperatingSystems rdf:ID="Windows95">
    <rdfs:label xml:lang="en">Windows 95</rdfs:label>
    <rdfs:label xml:lang="de">Windows 95</rdfs:label>
    <rdfs:comment xml:lang="en">A version of a Microsoft operating system.</rdfs:comment>
    <belongsToModule xml:lang="en">MP3Player, Printer, DigitalCamera, Camcorder</belongsToModule>
  </CompatibleOperatingSystems>
  <gr:BusinessEntity rdf:ID="Akai">
    <rdfs:comment xml:lang="en">The business entity Akai.</rdfs:comment>
    <gr:legalName rdf:datatype="http://www.w3.org/2001/XMLSchema#string"
    >Akai</gr:legalName>
    <belongsToModule xml:lang="en">MP3Player, TV</belongsToModule>
    <rdfs:seeAlso rdf:resource="http://www.akai.com/"/>
    <rdfs:label rdf:datatype="http://www.w3.org/2001/XMLSchema#string"
    >Akai</rdfs:label>
  </gr:BusinessEntity>
  <DataFormatImage rdf:ID="CGM">
    <rdfs:comment xml:lang="en">CGM (Computer Graphics Metafile) is a file format for 2D vector graphics, raster graphics, and text, and is defined by ISO/IEC 8632.

(This description is partly based on or reuses content from the Wikipedia article "Computer Graphics Metafile" (http://en.wikipedia.org/wiki/Computer_Graphics_Metafile) and is licensed under the GNU Free Documentation License (http://www.gnu.org/copyleft/fdl.html).)</rdfs:comment>
    <belongsToModule xml:lang="en">MP3Player, DigitalCamera, Camcorder</belongsToModule>
    <rdfs:label xml:lang="en">CGM</rdfs:label>
    <rdfs:label xml:lang="de">CGM</rdfs:label>
  </DataFormatImage>
  <CompatibleOperatingSystems rdf:ID="Windows2000">
    <rdfs:label xml:lang="en">Windows 2000</rdfs:label>
    <rdfs:label xml:lang="de">Windows 2000</rdfs:label>
    <belongsToModule xml:lang="en">MP3Player, Printer, DigitalCamera, Camcorder</belongsToModule>
    <rdfs:comment xml:lang="en">A version of a Microsoft operating system.</rdfs:comment>
  </CompatibleOperatingSystems>
  <MediaFormat rdf:ID="B7">
    <rdfs:label xml:lang="de">B7</rdfs:label>
    <rdfs:label xml:lang="en">B7</rdfs:label>
    <belongsToModule xml:lang="en">Printer</belongsToModule>
    <rdfs:comment xml:lang="en">Format of the german institute for standardization: 88 x 125 mm.</rdfs:comment>
  </MediaFormat>
  <Connectivity rdf:ID="AV">
    <rdfs:label xml:lang="en">AV</rdfs:label>
    <rdfs:label xml:lang="de">AV</rdfs:label>
    <belongsToModule xml:lang="en">TV</belongsToModule>
    <rdfs:comment xml:lang="en">Audio connectors and video connectors are electrical connectors for carrying an audio signal or video signal, either in an analog or digital format. Analog A/V connectors often use shielded cable to inhibit RF interference and noise.

(This description is partly based on or reuses content from the Wikipedia article "Audio and video connector" (http://en.wikipedia.org/wiki/Audio_and_video_connector) and is licensed under the GNU Free Documentation License (http://www.gnu.org/copyleft/fdl.html).)</rdfs:comment>
  </Connectivity>
  <owl:AnnotationProperty rdf:about="http://purl.org/dc/elements/1.1/title"/>
  <TVDisplayResolution rdf:ID="HDTV_720p">
    <rdfs:label xml:lang="en">HDTV 720p</rdfs:label>
    <rdfs:label xml:lang="de">HDTV 720p</rdfs:label>
    <rdfs:comment xml:lang="en">720p is the shorthand name for a category of HDTV video modes. The number 720 stands for the 720 vertical scan lines of display resolution (also known as 720 pixels of vertical resolution), while the letter p stands for progressive scan or non-interlaced.

(This description is partly based on or reuses content from the Wikipedia article "720p" (http://en.wikipedia.org/wiki/720p) and is licensed under the GNU Free Documentation License (http://www.gnu.org/copyleft/fdl.html).)</rdfs:comment>
    <belongsToModule xml:lang="en">TV</belongsToModule>
  </TVDisplayResolution>
  <VideoFeatures rdf:ID="ScreenFormatAdjustments">
    <rdfs:comment xml:lang="en">Includes the possibility to switch between different screen formats.</rdfs:comment>
    <rdfs:label xml:lang="en">Screen format adjustments</rdfs:label>
    <rdfs:label xml:lang="de">Bildschirmformatanpassung</rdfs:label>
    <belongsToModule xml:lang="en">TV</belongsToModule>
  </VideoFeatures>
  <MediaFormat rdf:ID="B2">
    <rdfs:comment xml:lang="en">Format of the german institute for standardization: 500 x 707 mm.</rdfs:comment>
    <belongsToModule xml:lang="en">Printer</belongsToModule>
    <rdfs:label xml:lang="de">B2</rdfs:label>
    <rdfs:label xml:lang="en">B2</rdfs:label>
  </MediaFormat>
  <GeneralFeatures rdf:ID="OnScreenDisplay">
    <rdfs:comment xml:lang="en">An on-screen display (abbreviated OSD) is an image superimposed on a screen picture, commonly used by modern televisions, VCRs, and DVD players to display information such as volume, channel, and time.

(This description is partly based on or reuses content from the Wikipedia article "On-screen display" (http://en.wikipedia.org/wiki/On-screen_display) and is licensed under the GNU Free Documentation License (http://www.gnu.org/copyleft/fdl.html).)</rdfs:comment>
    <rdfs:label xml:lang="en">on screen display</rdfs:label>
    <rdfs:label xml:lang="de">Bildschirmanzeige</rdfs:label>
    <belongsToModule xml:lang="en">TV</belongsToModule>
  </GeneralFeatures>
  <gr:BusinessEntity rdf:ID="Canyon">
    <rdfs:label rdf:datatype="http://www.w3.org/2001/XMLSchema#string"
    >Canyon</rdfs:label>
    <gr:legalName rdf:datatype="http://www.w3.org/2001/XMLSchema#string"
    >Canyon</gr:legalName>
    <rdfs:seeAlso rdf:resource="http://www.canyon-tech.it/"/>
    <rdfs:comment xml:lang="en">The business entity Canyon.</rdfs:comment>
    <belongsToModule xml:lang="en">MP3Player</belongsToModule>
  </gr:BusinessEntity>
  <DataFormatVideo rdf:ID="AVCH">
    <rdfs:label xml:lang="de">AVCH</rdfs:label>
    <rdfs:label xml:lang="en">AVCH</rdfs:label>
    <rdfs:comment xml:lang="en">A high-definition and standard-definition recording format for use in digital tapeless camcorders. The format is comparable to other handheld video camera recording formats, particularly HDV and TOD.

(This description is partly based on or reuses content from the Wikipedia article "HDV" (http://en.wikipedia.org/wiki/HDV) and is licensed under the GNU Free Documentation License (http://www.gnu.org/copyleft/fdl.html).)</rdfs:comment>
    <belongsToModule xml:lang="en">Camcorder</belongsToModule>
  </DataFormatVideo>
  <Connectivity rdf:ID="PCIn">
    <belongsToModule xml:lang="en">TV</belongsToModule>
    <rdfs:comment xml:lang="en">Port to connect a PC with the electronical device.</rdfs:comment>
    <rdfs:label xml:lang="en">PC in</rdfs:label>
    <rdfs:label xml:lang="de">PC in</rdfs:label>
  </Connectivity>
  <StorageMedia rdf:ID="SmartMediaCard">
    <rdfs:label xml:lang="de">SmartMediaCard</rdfs:label>
    <rdfs:label xml:lang="en">SmartMediaCard</rdfs:label>
    <belongsToModule xml:lang="en">MP3Player, DigitalCamera, Camcorder</belongsToModule>
    <rdfs:comment xml:lang="en">SmartMedia is a flash memory card standard.</rdfs:comment>
  </StorageMedia>
  <DataInterfaceType rdf:ID="Infrared">
    <rdfs:label xml:lang="en">Infrared</rdfs:label>
    <rdfs:label xml:lang="de">Infrarot</rdfs:label>
    <rdfs:comment xml:lang="en">Infrared (IR) radiation is electromagnetic radiation whose wavelength is longer than that of visible light, but shorter than that of terahertz radiation and microwaves.

(This description is partly based on or reuses content from the Wikipedia article "Infrared" (http://en.wikipedia.org/wiki/Infrared) and is licensed under the GNU Free Documentation License (http://www.gnu.org/copyleft/fdl.html).)</rdfs:comment>
    <belongsToModule xml:lang="en">MP3Player, Printer, DigitalCamera, Camcorder</belongsToModule>
  </DataInterfaceType>
  <MediaFormat rdf:ID="B6">
    <belongsToModule xml:lang="en">Printer</belongsToModule>
    <rdfs:label xml:lang="de">B6</rdfs:label>
    <rdfs:label xml:lang="en">B6</rdfs:label>
    <rdfs:comment xml:lang="en">Format of the german institute for standardization: 125 x 176 mm.</rdfs:comment>
  </MediaFormat>
  <AudioInterfaceType rdf:ID="Audio2.5mm">
    <rdfs:label xml:lang="en">Audio 2.5mm</rdfs:label>
    <rdfs:label xml:lang="de">Audio 2.5mm</rdfs:label>
    <rdfs:comment xml:lang="en">Audio interface type of a specific diameter.</rdfs:comment>
    <belongsToModule xml:lang="en">MP3Player</belongsToModule>
  </AudioInterfaceType>
  <VideoFeatures rdf:ID="PixelPlus3HD">
    <rdfs:label xml:lang="en">Pixel Plus 3 HD</rdfs:label>
    <rdfs:label xml:lang="de">Pixel Plus 3 HD</rdfs:label>
    <belongsToModule xml:lang="en">TV</belongsToModule>
    <rdfs:comment xml:lang="en">Pixel Plus 3 HD offers the unique combination of ultimate sharpness, natural detail, vivid colours and smooth natural motion on all qualities of HD, standard TV signals and multimedia content for high definition displays. Each pixel of the incoming picture is enhanced to better match the surrounding pixels, resulting in a more natural picture. Artefacts and noise in all sources from multimedia to standard TV and also in highly compressed HD are detected and reduced.</rdfs:comment>
  </VideoFeatures>
  <gr:BusinessEntity rdf:ID="Guillemot">
    <rdfs:seeAlso rdf:resource="http://www.guillemot.biz/"/>
    <belongsToModule xml:lang="en">MP3Player</belongsToModule>
    <rdfs:comment xml:lang="en">The business entity Guillemot Corporation.</rdfs:comment>
    <rdfs:label rdf:datatype="http://www.w3.org/2001/XMLSchema#string"
    >Guillemot</rdfs:label>
    <gr:legalName rdf:datatype="http://www.w3.org/2001/XMLSchema#string"
    >Guillemot Corporation</gr:legalName>
  </gr:BusinessEntity>
  <gr:BusinessEntity rdf:ID="Thomson">
    <gr:legalName rdf:datatype="http://www.w3.org/2001/XMLSchema#string"
    >The Thomson Corporation</gr:legalName>
    <rdfs:label rdf:datatype="http://www.w3.org/2001/XMLSchema#string"
    >Thomson</rdfs:label>
    <belongsToModule xml:lang="en">MP3Player, TV</belongsToModule>
    <rdfs:seeAlso rdf:resource="http://www.thomson.net/"/>
    <rdfs:comment xml:lang="en">The business entity The Thomson Corporation.</rdfs:comment>
  </gr:BusinessEntity>
  <StorageMedia rdf:ID="MicroDrive">
    <rdfs:comment xml:lang="en">A miniature, 1-inch hard disk designed to fit in a CompactFlash (CF) Type II slot.</rdfs:comment>
    <rdfs:label xml:lang="de">MicroDrive</rdfs:label>
    <rdfs:label xml:lang="en">MicroDrive</rdfs:label>
    <belongsToModule xml:lang="en">MP3Player, DigitalCamera, Camcorder</belongsToModule>
  </StorageMedia>
  <LensSystem rdf:ID="OneStepFixed">
    <belongsToModule xml:lang="en">Camcorder</belongsToModule>
    <rdfs:comment xml:lang="en">A special lens system.</rdfs:comment>
    <rdfs:label xml:lang="de">One step fixed</rdfs:label>
    <rdfs:label xml:lang="en">One step fixed</rdfs:label>
  </LensSystem>
  <Features rdf:ID="Clock">
    <rdfs:comment xml:lang="en">Can display the current time.</rdfs:comment>
    <rdfs:label xml:lang="en">Clock</rdfs:label>
    <rdfs:label xml:lang="de">Uhr</rdfs:label>
    <belongsToModule xml:lang="en">MP3Player</belongsToModule>
  </Features>
  <DataFormatAudio rdf:ID="WAV">
    <rdfs:label xml:lang="en">WAV</rdfs:label>
    <rdfs:label xml:lang="de">WAV</rdfs:label>
    <rdfs:comment xml:lang="en">WAV (or WAVE), short for Waveform audio format, is a Microsoft and IBM audio file format standard for storing an audio bitstream on PCs.

(This description is partly based on or reuses content from the Wikipedia article "WAV" (http://en.wikipedia.org/wiki/WAV) and is licensed under the GNU Free Documentation License (http://www.gnu.org/copyleft/fdl.html).)</rdfs:comment>
    <belongsToModule xml:lang="en">MP3Player, DigitalCamera, Camcorder</belongsToModule>
  </DataFormatAudio>
  <WhiteBalance rdf:ID="IndoorWhiteBalance">
    <rdfs:comment xml:lang="en">Ability to adapt of different adjustments of the intensities of the colors.</rdfs:comment>
    <belongsToModule xml:lang="en">Camcorder</belongsToModule>
    <rdfs:label xml:lang="de">Weißabgleich innen</rdfs:label>
    <rdfs:label xml:lang="en">Indoor white balance</rdfs:label>
  </WhiteBalance>
  <DataFormatAudio rdf:ID="AAC-LC">
    <rdfs:comment xml:lang="en">Advanced Audio Coding (AAC) is a standardized, lossy compression and encoding scheme for digital audio.

(This description is partly based on or reuses content from the Wikipedia article "Advanced Audio Coding" (http://en.wikipedia.org/wiki/Advanced_Audio_Coding) and is licensed under the GNU Free Documentation License (http://www.gnu.org/copyleft/fdl.html).)</rdfs:comment>
    <rdfs:label xml:lang="en">AAC-LC</rdfs:label>
    <rdfs:label xml:lang="de">AAC-LC</rdfs:label>
    <belongsToModule xml:lang="en">MP3Player, DigitalCamera, Camcorder</belongsToModule>
  </DataFormatAudio>
  <gr:BusinessEntity rdf:ID="HP">
    <rdfs:seeAlso rdf:resource="http://www.hp.com/"/>
    <rdfs:comment xml:lang="en">The business entity Hewlett-Packard Company.</rdfs:comment>
    <rdfs:label rdf:datatype="http://www.w3.org/2001/XMLSchema#string"
    >HP</rdfs:label>
    <gr:legalName rdf:datatype="http://www.w3.org/2001/XMLSchema#string"
    >Hewlett-Packard Company</gr:legalName>
    <belongsToModule xml:lang="en">MP3Player, Printer, DigitalCamera</belongsToModule>
  </gr:BusinessEntity>
  <Color rdf:ID="Grey">
    <rdfs:label xml:lang="en">Grey</rdfs:label>
    <rdfs:label xml:lang="de">Grau</rdfs:label>
    <belongsToModule xml:lang="en">MP3Player, TV, Printer, DigitalCamera, Camcorder</belongsToModule>
    <rdfs:comment xml:lang="en">RGB Value 128,128,128</rdfs:comment>
  </Color>
  <gr:BusinessEntity rdf:ID="iRiver">
    <belongsToModule xml:lang="en">MP3Player</belongsToModule>
    <rdfs:comment xml:lang="en">The business entity iriver Europe GmbH.</rdfs:comment>
    <gr:legalName rdf:datatype="http://www.w3.org/2001/XMLSchema#string"
    >iriver Europe GmbH</gr:legalName>
    <rdfs:seeAlso rdf:resource="http://www.iriver.de/"/>
    <rdfs:label rdf:datatype="http://www.w3.org/2001/XMLSchema#string"
    >iriver</rdfs:label>
  </gr:BusinessEntity>
  <gr:BusinessEntity rdf:ID="Fujifilm">
    <rdfs:seeAlso rdf:resource="http://www.fujifilm.com/"/>
    <rdfs:label rdf:datatype="http://www.w3.org/2001/XMLSchema#string"
    >Fujifilm</rdfs:label>
    <belongsToModule xml:lang="en">DigitalCamera</belongsToModule>
    <rdfs:comment xml:lang="en">The business entity Fujifilm Holdings Corporation.</rdfs:comment>
    <gr:legalName rdf:datatype="http://www.w3.org/2001/XMLSchema#string"
    >Fujifilm Holdings Corporation</gr:legalName>
  </gr:BusinessEntity>
  <gr:BusinessEntity rdf:ID="Lexar">
    <rdfs:comment xml:lang="en">The business entity Lexar Media, Inc.</rdfs:comment>
    <gr:legalName rdf:datatype="http://www.w3.org/2001/XMLSchema#string"
    >Lexar Media, Inc. </gr:legalName>
    <belongsToModule xml:lang="en">MP3Player</belongsToModule>
    <rdfs:seeAlso rdf:resource="http://www.lexar.com/"/>
    <rdfs:label rdf:datatype="http://www.w3.org/2001/XMLSchema#string"
    >Lexar</rdfs:label>
  </gr:BusinessEntity>
  <Features rdf:ID="AutomaticPictureStabilizer">
    <belongsToModule xml:lang="en">DigitalCamera, Camcorder</belongsToModule>
    <rdfs:comment xml:lang="en">A device used to stabilize a picture in order to keep it in a steady position.</rdfs:comment>
    <rdfs:label xml:lang="de">Automatischer Bildstabilisator</rdfs:label>
    <rdfs:label xml:lang="en">Automatic picture stabilizer</rdfs:label>
  </Features>
  <gr:BusinessEntity rdf:ID="Medion">
    <rdfs:seeAlso rdf:resource="http://www.medion.com/"/>
    <rdfs:comment xml:lang="en">The business entity Medion AG.</rdfs:comment>
    <gr:legalName rdf:datatype="http://www.w3.org/2001/XMLSchema#string"
    >Medion AG</gr:legalName>
    <rdfs:label rdf:datatype="http://www.w3.org/2001/XMLSchema#string"
    >Medion</rdfs:label>
    <belongsToModule xml:lang="en">MP3Player, TV</belongsToModule>
  </gr:BusinessEntity>
  <ComputerDisplayResolution rdf:ID="ComputerDisplayResolution_800x600_60_72_75_85Hz">
    <rdfs:label xml:lang="en">Computer display resolution 800x600 60 72 75 85Hz</rdfs:label>
    <rdfs:label xml:lang="de">Computerbildschirmauflösung 800x600 60 72 75 85Hz</rdfs:label>
    <rdfs:comment xml:lang="en">Display resolution specified as the width and height in pixels, color depth measured in bits, and refresh rate expressed in hertz; here Super Video Graphics Array.

(This description is partly based on or reuses content from the Wikipedia article "Display resolution" (http://en.wikipedia.org/wiki/Display_resolution) and is licensed under the GNU Free Documentation License (http://www.gnu.org/copyleft/fdl.html).)</rdfs:comment>
    <belongsToModule xml:lang="en">TV</belongsToModule>
  </ComputerDisplayResolution>
  <gr:BusinessEntity rdf:ID="TEAC">
    <rdfs:seeAlso rdf:resource="http://www.teac.de/"/>
    <gr:legalName rdf:datatype="http://www.w3.org/2001/XMLSchema#string"
    >TEAC Europe GmbH </gr:legalName>
    <rdfs:comment xml:lang="en">The business entity TEAC Europe GmbH.</rdfs:comment>
    <belongsToModule xml:lang="en">MP3Player, TV</belongsToModule>
    <rdfs:label rdf:datatype="http://www.w3.org/2001/XMLSchema#string"
    >TEAC</rdfs:label>
  </gr:BusinessEntity>
  <gr:BusinessEntity rdf:ID="Sony">
    <rdfs:comment xml:lang="en">The business entity Sony Corporation</rdfs:comment>
    <belongsToModule xml:lang="en">MP3Player, TV, DigitalCamera, Camcorder</belongsToModule>
    <rdfs:seeAlso rdf:resource="http://www.sony.com/"/>
    <gr:legalName rdf:datatype="http://www.w3.org/2001/XMLSchema#string"
    >Sony Corporation </gr:legalName>
    <rdfs:label rdf:datatype="http://www.w3.org/2001/XMLSchema#string"
    >Sony</rdfs:label>
  </gr:BusinessEntity>
  <gr:BusinessEntity rdf:ID="Olivetti">
    <rdfs:label rdf:datatype="http://www.w3.org/2001/XMLSchema#string"
    >Olivetti</rdfs:label>
    <belongsToModule xml:lang="en">Printer</belongsToModule>
    <rdfs:comment xml:lang="en">The business entity Olivetti.</rdfs:comment>
    <rdfs:seeAlso rdf:resource="http://www.olivetti.com/"/>
    <gr:legalName rdf:datatype="http://www.w3.org/2001/XMLSchema#string"
    >Olivetti Tecnost</gr:legalName>
  </gr:BusinessEntity>
  <gr:BusinessEntity rdf:ID="ViewSonic">
    <rdfs:comment xml:lang="en">The business entity ViewSonic.</rdfs:comment>
    <belongsToModule xml:lang="en">TV</belongsToModule>
    <rdfs:label rdf:datatype="http://www.w3.org/2001/XMLSchema#string"
    >ViewSonic</rdfs:label>
    <rdfs:seeAlso rdf:resource="http://www.viewsonic.com/"/>
    <gr:legalName rdf:datatype="http://www.w3.org/2001/XMLSchema#string"
    >ViewSonic Corporation</gr:legalName>
  </gr:BusinessEntity>
  <gr:BusinessEntity rdf:ID="Creative_Labs">
    <rdfs:label rdf:datatype="http://www.w3.org/2001/XMLSchema#string"
    >Creative Labs</rdfs:label>
    <rdfs:comment xml:lang="en">The business entity Creative Technology Limited.</rdfs:comment>
    <rdfs:seeAlso rdf:resource="http://www.creative.com/"/>
    <gr:legalName rdf:datatype="http://www.w3.org/2001/XMLSchema#string"
    >Creative Technology Limited</gr:legalName>
    <belongsToModule xml:lang="en">MP3Player, DigitalCamera, Camcorder</belongsToModule>
  </gr:BusinessEntity>
  <gr:BusinessEntity rdf:ID="Logitech">
    <rdfs:comment xml:lang="en">The business entity Logitech International S.A.</rdfs:comment>
    <rdfs:seeAlso rdf:resource="http://www.logitech.com/"/>
    <gr:legalName rdf:datatype="http://www.w3.org/2001/XMLSchema#string"
    >Logitech International S.A.</gr:legalName>
    <rdfs:label rdf:datatype="http://www.w3.org/2001/XMLSchema#string"
    >Logitech</rdfs:label>
    <belongsToModule xml:lang="en">DigitalCamera</belongsToModule>
  </gr:BusinessEntity>
  <Features rdf:ID="Playlist">
    <belongsToModule xml:lang="en">MP3Player</belongsToModule>
    <rdfs:comment xml:lang="en">Ability to put audiofiles in a playlist.</rdfs:comment>
    <rdfs:label xml:lang="de">Wiedergabeliste</rdfs:label>
    <rdfs:label xml:lang="en">Playlist</rdfs:label>
  </Features>
  <AudioFeatures rdf:ID="IncredibleSurround">
    <rdfs:comment xml:lang="en">Psycho-acoustic method of widening the stereo spatial image especially suited for applications with limited separation of left and right speakers.</rdfs:comment>
    <belongsToModule xml:lang="en">TV</belongsToModule>
    <rdfs:label xml:lang="en">Incredible Surround</rdfs:label>
    <rdfs:label xml:lang="de">Incredible Surround</rdfs:label>
  </AudioFeatures>
  <Connectivity rdf:ID="RS-232">
    <rdfs:label xml:lang="en">RS-232</rdfs:label>
    <rdfs:label xml:lang="de">RS-232</rdfs:label>
    <rdfs:comment xml:lang="en">In telecommunications, RS-232 (Recommended Standard 232) is a standard for serial binary data signals connecting between a DTE (Data Terminal Equipment) and a DCE (Data Circuit-terminating Equipment). It is commonly used in computer serial ports.

(This description is partly based on or reuses content from the Wikipedia article "RS-232" (http://en.wikipedia.org/wiki/RS-232) and is licensed under the GNU Free Documentation License (http://www.gnu.org/copyleft/fdl.html).)</rdfs:comment>
    <belongsToModule xml:lang="en">TV</belongsToModule>
  </Connectivity>
  <gr:BusinessEntity rdf:ID="Asus">
    <rdfs:comment xml:lang="en">The business entity Asus.</rdfs:comment>
    <rdfs:label rdf:datatype="http://www.w3.org/2001/XMLSchema#string"
    >Asus</rdfs:label>
    <gr:legalName rdf:datatype="http://www.w3.org/2001/XMLSchema#string"
    >ASUSTeK Computer Inc.</gr:legalName>
    <belongsToModule xml:lang="en">TV</belongsToModule>
    <rdfs:seeAlso rdf:resource="http://www.asus.com/"/>
  </gr:BusinessEntity>
  <Features rdf:ID="TextViewing">
    <belongsToModule xml:lang="en">MP3Player</belongsToModule>
    <rdfs:label xml:lang="de">Textdarstellung</rdfs:label>
    <rdfs:label xml:lang="en">Text viewing</rdfs:label>
    <rdfs:comment xml:lang="en">Ability to display text.</rdfs:comment>
  </Features>
  <RechargeableEnergySource rdf:ID="NiMH">
    <rdfs:comment xml:lang="en">A nickel-metal hydride battery, abbreviated NiMH, is a type of rechargeable battery similar to a nickel-cadmium (NiCd) battery but using a hydrogen-absorbing alloy for the negative electrode instead of cadmium.

(This description is partly based on or reuses content from the Wikipedia article "Nickel metal hydride battery" (http://en.wikipedia.org/wiki/Nickel_metal_hydride_battery) and is licensed under the GNU Free Documentation License (http://www.gnu.org/copyleft/fdl.html).)</rdfs:comment>
    <rdfs:label xml:lang="en">NiMH</rdfs:label>
    <rdfs:label xml:lang="de">NiMH</rdfs:label>
    <belongsToModule xml:lang="en">MP3Player, DigitalCamera, Camcorder</belongsToModule>
  </RechargeableEnergySource>
  <SignalFormat rdf:ID="Hyperband">
    <rdfs:comment xml:lang="en">Hyperband designates a range (band) of electromagnetic waves with frequencies between 300 MHz and 470 MHz. This is designated for kable TV especially to recieve digital TV normed for DVB-C.</rdfs:comment>
    <belongsToModule xml:lang="en">TV</belongsToModule>
    <rdfs:label xml:lang="en">Hyperband</rdfs:label>
    <rdfs:label xml:lang="de">Hyperband</rdfs:label>
  </SignalFormat>
  <gr:BusinessEntity rdf:ID="Pioneer">
    <gr:legalName rdf:datatype="http://www.w3.org/2001/XMLSchema#string"
    >Pioneer Corporation</gr:legalName>
    <belongsToModule xml:lang="en">TV</belongsToModule>
    <rdfs:label rdf:datatype="http://www.w3.org/2001/XMLSchema#string"
    >Pioneer</rdfs:label>
    <rdfs:seeAlso rdf:resource="http://pioneer.jp/"/>
    <rdfs:comment xml:lang="en">The business entity Pioneer.</rdfs:comment>
  </gr:BusinessEntity>
  <gr:BusinessEntity rdf:ID="LG">
    <rdfs:seeAlso rdf:resource="http://www.lge.com/"/>
    <rdfs:comment xml:lang="en">The business entity LG Group.</rdfs:comment>
    <belongsToModule xml:lang="en">MP3Player, TV</belongsToModule>
    <rdfs:label rdf:datatype="http://www.w3.org/2001/XMLSchema#string"
    >LG</rdfs:label>
    <gr:legalName rdf:datatype="http://www.w3.org/2001/XMLSchema#string"
    >LG Group</gr:legalName>
  </gr:BusinessEntity>
  <gr:BusinessEntity rdf:ID="Xerox">
    <rdfs:comment xml:lang="en">The business entity Xerox.</rdfs:comment>
    <belongsToModule xml:lang="en">Printer</belongsToModule>
    <rdfs:seeAlso rdf:resource="http://www.xerox.com/"/>
    <rdfs:label rdf:datatype="http://www.w3.org/2001/XMLSchema#string"
    >Xerox</rdfs:label>
    <gr:legalName rdf:datatype="http://www.w3.org/2001/XMLSchema#string"
    >Xerox Corporation</gr:legalName>
  </gr:BusinessEntity>
  <Connectivity rdf:ID="ComponentVideoOut">
    <rdfs:label xml:lang="en">Component video out</rdfs:label>
    <rdfs:label xml:lang="de">Component video out</rdfs:label>
    <rdfs:comment xml:lang="en">Component video is a video signal that has been split into two or more components. In popular use, it refers to a type of analog video information that is transmitted or stored as three separate signals. Component video can be contrasted with composite video (NTSC, PAL or SECAM) in which all the video information is combined into a single line-level signal. Like composite, component video cables do not carry audio and are often paired with audio cables. Here the output is meant.

(This description is partly based on or reuses content from the Wikipedia article "Component video" (http://en.wikipedia.org/wiki/Component_video) and is licensed under the GNU Free Documentation License (http://www.gnu.org/copyleft/fdl.html).)</rdfs:comment>
  </Connectivity>
  <SignalFormat rdf:ID="SECAM">
    <belongsToModule xml:lang="en">TV</belongsToModule>
    <rdfs:comment xml:lang="en">SECAM, also written SÉCAM (Séquentiel couleur à mémoire, French for "Sequential Color with Memory"), is an analog color television system first used in France.

(This description is partly based on or reuses content from the Wikipedia article "SECAM" (http://en.wikipedia.org/wiki/SECAM) and is licensed under the GNU Free Documentation License (http://www.gnu.org/copyleft/fdl.html).)</rdfs:comment>
    <rdfs:label xml:lang="en">SECAM</rdfs:label>
    <rdfs:label xml:lang="de">SECAM</rdfs:label>
  </SignalFormat>
  <gr:BusinessEntity rdf:ID="Philips">
    <gr:legalName rdf:datatype="http://www.w3.org/2001/XMLSchema#string"
    >Koninklijke Philips Electronics N.V.</gr:legalName>
    <belongsToModule xml:lang="en">MP3Player, TV, DigitalCamera</belongsToModule>
    <rdfs:comment xml:lang="en">The business entity Koninklijke Philips Electronics N.V.</rdfs:comment>
    <rdfs:seeAlso rdf:resource="http://www.philips.com/"/>
    <rdfs:label rdf:datatype="http://www.w3.org/2001/XMLSchema#string"
    >Philips</rdfs:label>
  </gr:BusinessEntity>
  <CompatibleOperatingSystems rdf:ID="Windows98">
    <belongsToModule xml:lang="en">MP3Player, Printer, DigitalCamera, Camcorder</belongsToModule>
    <rdfs:comment xml:lang="en">A version of a Microsoft operating system.</rdfs:comment>
    <rdfs:label xml:lang="en">Windows 98</rdfs:label>
    <rdfs:label xml:lang="de">Windows 98</rdfs:label>
  </CompatibleOperatingSystems>
  <Features rdf:ID="SelfTimer">
    <rdfs:label xml:lang="de">Selbstauslöser</rdfs:label>
    <rdfs:label xml:lang="en">Self-timer</rdfs:label>
    <belongsToModule xml:lang="en">DigitalCamera, Camcorder</belongsToModule>
    <rdfs:comment xml:lang="en">Ability to give a delay between the pressing of the shutter release and the shutter firing.</rdfs:comment>
  </Features>
  <gr:BusinessEntity rdf:ID="Iiyama">
    <rdfs:comment xml:lang="en">The business entity Iiyama.</rdfs:comment>
    <rdfs:seeAlso rdf:resource="http://www.iiyama.com/"/>
    <rdfs:label rdf:datatype="http://www.w3.org/2001/XMLSchema#string"
    >Iiyama</rdfs:label>
    <gr:legalName rdf:datatype="http://www.w3.org/2001/XMLSchema#string"
    >Iiyama</gr:legalName>
    <belongsToModule xml:lang="en">TV</belongsToModule>
  </gr:BusinessEntity>
  <Connectivity rdf:ID="DigitalAudioCoaxialOut">
    <belongsToModule xml:lang="en">TV</belongsToModule>
    <rdfs:label xml:lang="en">Digital audio coaxial out</rdfs:label>
    <rdfs:label xml:lang="de">Digital audio coaxial out</rdfs:label>
    <rdfs:comment xml:lang="en">Digital audio uses digital signals for sound reproduction. This includes analog-to-digital conversion, digital-to-analog conversion, storage and transmission. From the signal point of view, a connector can be viewed as a short, rigid cable. The connector usually has the same impedance as the related cable and probably has a similar cutoff frequency although its dielectric may be different. Some connectors are gold or rhodium plated, while some connectors use nickel or tin plating. Silver is also used due to its excellent conductivity. Although silver tends to oxidize rather quickly, the silver oxide that is produced is still conductive. This may pose a cosmetic issue but it does not degrade the performance of the connector. Here the output is meant.

(This description is partly based on or reuses content from the Wikipedia article "Digital audio" (http://en.wikipedia.org/wiki/Digital_audio) and is licensed under the GNU Free Documentation License (http://www.gnu.org/copyleft/fdl.html).)</rdfs:comment>
  </Connectivity>
  <SignalFormat rdf:ID="PAL-B_G">
    <rdfs:comment xml:lang="en">PAL, short for Phase Alternating Line, is a colour-encoding system used in broadcast television systems in large parts of the world. This is used in western europe.

(This description is partly based on or reuses content from the Wikipedia article "PAL" (http://en.wikipedia.org/wiki/PAL) and is licensed under the GNU Free Documentation License (http://www.gnu.org/copyleft/fdl.html).)</rdfs:comment>
    <rdfs:label xml:lang="en">PAL-B G</rdfs:label>
    <rdfs:label xml:lang="de">PAL-B G</rdfs:label>
    <belongsToModule xml:lang="en">TV</belongsToModule>
  </SignalFormat>
  <Connectivity rdf:ID="PCMCIA">
    <belongsToModule xml:lang="en">TV</belongsToModule>
    <rdfs:comment xml:lang="en">The Personal Computer Memory Card International Association is an international standards body that defines and promotes the PC Card (formerly known as "PCMCIA card") and ExpressCard standards. Although the organization's name refers to memory cards, their standards are not limited to memory devices. These cards can be used for wireless connectivity, modem and other functions in laptop/notebook PCs that may be lacking them natively.

(This description is partly based on or reuses content from the Wikipedia article "PCMCIA" (http://en.wikipedia.org/wiki/PCMCIA) and is licensed under the GNU Free Documentation License (http://www.gnu.org/copyleft/fdl.html).)</rdfs:comment>
    <rdfs:label xml:lang="en">PCMCIA</rdfs:label>
    <rdfs:label xml:lang="de">PCMCIA</rdfs:label>
  </Connectivity>
  <MediaFormat rdf:ID="B0">
    <rdfs:label xml:lang="de">B0</rdfs:label>
    <rdfs:label xml:lang="en">B0</rdfs:label>
    <belongsToModule xml:lang="en">Printer</belongsToModule>
    <rdfs:comment xml:lang="en">Format of the german institute for standardization: 1000 x 1414 mm.</rdfs:comment>
  </MediaFormat>
  <ProcessorType rdf:ID="RISC">
    <belongsToModule xml:lang="en">Printer</belongsToModule>
    <rdfs:label xml:lang="de">RISC</rdfs:label>
    <rdfs:label xml:lang="en">RISC</rdfs:label>
    <rdfs:comment xml:lang="en">Reduced instruction set computing, represents a CPU design strategy emphasizing the insight that simplified instructions that "do less" may still provide for higher performance if this simplicity can be utilized to make instructions execute very quickly.</rdfs:comment>
  </ProcessorType>
  <Features rdf:ID="AudioInput">
    <rdfs:comment xml:lang="en">Defines the support of a computer soundcard driver protocol for digital audio specified by Steinberg, providing a low-latency and high fidelity interface between a software application and a computer's sound card.</rdfs:comment>
    <belongsToModule xml:lang="en">Camcorder</belongsToModule>
    <rdfs:label xml:lang="en">Audio input</rdfs:label>
    <rdfs:label xml:lang="de">Audioeingang</rdfs:label>
  </Features>
  <gr:BusinessEntity rdf:ID="Eizo">
    <rdfs:comment xml:lang="en">The business entity Eizo.</rdfs:comment>
    <rdfs:seeAlso rdf:resource="http://www.eizo.com/"/>
    <rdfs:label rdf:datatype="http://www.w3.org/2001/XMLSchema#string"
    >Eizo</rdfs:label>
    <belongsToModule xml:lang="en">TV</belongsToModule>
    <gr:legalName rdf:datatype="http://www.w3.org/2001/XMLSchema#string"
    >Eizo Nano Technologies Inc.</gr:legalName>
  </gr:BusinessEntity>
  <gr:BusinessEntity rdf:ID="Konica_Minolta">
    <rdfs:seeAlso rdf:resource="http://www.konicaminolta.com/"/>
    <rdfs:comment xml:lang="en">The business entity Konica Minolta.</rdfs:comment>
    <rdfs:label rdf:datatype="http://www.w3.org/2001/XMLSchema#string"
    >Konica Minolta</rdfs:label>
    <gr:legalName rdf:datatype="http://www.w3.org/2001/XMLSchema#string"
    >Konica Minolta Holdings, Inc.</gr:legalName>
    <belongsToModule xml:lang="en">Printer, DigitalCamera</belongsToModule>
  </gr:BusinessEntity>
  <gr:BusinessEntity rdf:ID="Transcend">
    <rdfs:seeAlso rdf:resource="http://www.transcendusa.com/"/>
    <belongsToModule xml:lang="en">MP3Player</belongsToModule>
    <gr:legalName rdf:datatype="http://www.w3.org/2001/XMLSchema#string"
    >Transcend Information, Inc. </gr:legalName>
    <rdfs:comment xml:lang="en">The business entity Transcend Information, Inc.</rdfs:comment>
    <rdfs:label rdf:datatype="http://www.w3.org/2001/XMLSchema#string"
    >Transcend</rdfs:label>
  </gr:BusinessEntity>
  <WhiteBalance rdf:ID="AutoWhiteBalance">
    <rdfs:label xml:lang="de">Automatischer Weißabgleich</rdfs:label>
    <rdfs:label xml:lang="en">Auto white balance</rdfs:label>
    <rdfs:comment xml:lang="en">Ability to adapt of different adjustments of the intensities of the colors.</rdfs:comment>
    <belongsToModule xml:lang="en">Camcorder</belongsToModule>
  </WhiteBalance>
  <MediaType rdf:ID="LaserPrintingPaper">
    <rdfs:comment xml:lang="en">Special sort of paper used in laser printers.</rdfs:comment>
    <belongsToModule xml:lang="en">Printer</belongsToModule>
    <rdfs:label xml:lang="de">Laserdruckpapier</rdfs:label>
    <rdfs:label xml:lang="en">Laser printing paper</rdfs:label>
  </MediaType>
  <DataFormatOffice rdf:ID="TXT">
    <belongsToModule xml:lang="en">MP3Player, DigitalCamera</belongsToModule>
    <rdfs:label xml:lang="en">TXT</rdfs:label>
    <rdfs:label xml:lang="de">TXT</rdfs:label>
    <rdfs:comment xml:lang="en">Is a filename extension for files consisting of text usually contain very little formatting.</rdfs:comment>
  </DataFormatOffice>
  <Focus rdf:ID="FocusAuto">
    <rdfs:comment xml:lang="en">Autofocus (or AF) is a feature of some optical systems that allows them to obtain (and in some systems to also continuously maintain) correct focus on a subject, instead of requiring the operator to adjust focus manually.

(This description is partly based on or reuses content from the Wikipedia article "Autofocus" (http://en.wikipedia.org/wiki/Autofocus) and is licensed under the GNU Free Documentation License (http://www.gnu.org/copyleft/fdl.html).)</rdfs:comment>
    <belongsToModule xml:lang="en">DigitalCamera, Camcorder</belongsToModule>
    <rdfs:label xml:lang="de">Autofokus</rdfs:label>
    <rdfs:label xml:lang="en">Focus auto</rdfs:label>
  </Focus>
  <gr:BusinessEntity rdf:ID="Palm">
    <rdfs:comment xml:lang="en">The business entity Palm Inc.</rdfs:comment>
    <gr:legalName rdf:datatype="http://www.w3.org/2001/XMLSchema#string"
    >Palm Inc</gr:legalName>
    <rdfs:seeAlso rdf:resource="http://www.palm.com/"/>
    <rdfs:label rdf:datatype="http://www.w3.org/2001/XMLSchema#string"
    >Palm</rdfs:label>
    <belongsToModule xml:lang="en">MP3Player</belongsToModule>
  </gr:BusinessEntity>
  <Features rdf:ID="Shuffle">
    <belongsToModule xml:lang="en">MP3Player</belongsToModule>
    <rdfs:label xml:lang="en">Shuffle</rdfs:label>
    <rdfs:label xml:lang="de">Zufällige Wiedergabe</rdfs:label>
    <rdfs:comment xml:lang="en">Ability to play files in random order.</rdfs:comment>
  </Features>
  <GeneralFeatures rdf:ID="OnOffTimer">
    <belongsToModule xml:lang="en">TV</belongsToModule>
    <rdfs:label xml:lang="de">Ein- und Ausschalttimer</rdfs:label>
    <rdfs:label xml:lang="en">On off timer</rdfs:label>
    <rdfs:comment xml:lang="en">Describes the possibility to maintain a designated  time when the television or electrical device should be switched off or on automatically.</rdfs:comment>
  </GeneralFeatures>
  <StorageMedia rdf:ID="XDPictureCard">
    <belongsToModule xml:lang="en">MP3Player, DigitalCamera, Camcorder</belongsToModule>
    <rdfs:comment xml:lang="en">The xD-Picture Card is a type of flash memory card.</rdfs:comment>
    <rdfs:label xml:lang="de">XDPictureCard</rdfs:label>
    <rdfs:label xml:lang="en">XDPictureCard</rdfs:label>
  </StorageMedia>
  <DataFormatVideo rdf:ID="H.264">
    <rdfs:label xml:lang="en">H.264</rdfs:label>
    <rdfs:label xml:lang="de">H.264</rdfs:label>
    <rdfs:comment xml:lang="en">H.264 is a standard for video compression, and is equivalent to MPEG-4 Part 10, or MPEG-4 AVC (for Advanced Video Coding). As of 2008, it is the latest block-oriented motion-compensation-based codec standard developed by the ITU-T Video Coding Experts Group (VCEG) together with the ISO/IEC Moving Picture Experts Group (MPEG), and it was the product of a partnership effort known as the Joint Video Team (JVT).

(This description is partly based on or reuses content from the Wikipedia article "H.264" (http://en.wikipedia.org/wiki/H.264) and is licensed under the GNU Free Documentation License (http://www.gnu.org/copyleft/fdl.html).)</rdfs:comment>
    <belongsToModule xml:lang="en">MP3Player, DigitalCamera, Camcorder</belongsToModule>
  </DataFormatVideo>
  <GeneralFeatures rdf:ID="SleepTimer">
    <rdfs:comment xml:lang="en">A sleep timer is a function on many modern televisions that shut off the power after a preset amount of time. The setting is usually made either from the remote control or the television menus. They are intended to allow viewers to watch as they fall asleep.

(This description is partly based on or reuses content from the Wikipedia article "Sleep timer" (http://en.wikipedia.org/wiki/Sleep_timer) and is licensed under the GNU Free Documentation License (http://www.gnu.org/copyleft/fdl.html).)</rdfs:comment>
    <rdfs:label xml:lang="en">Sleep timer</rdfs:label>
    <rdfs:label xml:lang="de">Schlafzeitgeber</rdfs:label>
    <belongsToModule xml:lang="en">TV</belongsToModule>
  </GeneralFeatures>
  <SceneMode rdf:ID="NightMode">
    <rdfs:label xml:lang="de">Nachtmodus</rdfs:label>
    <rdfs:label xml:lang="en">Night mode</rdfs:label>
    <rdfs:comment xml:lang="en">Ability of the camcorder to adapt to special environments.</rdfs:comment>
    <belongsToModule xml:lang="en">Camcorder</belongsToModule>
  </SceneMode>
  <Color rdf:ID="White">
    <rdfs:comment xml:lang="en">RGB Value 255,255,255</rdfs:comment>
    <rdfs:label xml:lang="en">White</rdfs:label>
    <rdfs:label xml:lang="de">Weiß</rdfs:label>
    <belongsToModule xml:lang="en">MP3Player, TV, Printer, DigitalCamera, Camcorder</belongsToModule>
  </Color>
  <gr:BusinessEntity rdf:ID="VIVOTEK">
    <rdfs:seeAlso rdf:resource="http://www.vivotek.com/"/>
    <rdfs:label rdf:datatype="http://www.w3.org/2001/XMLSchema#string"
    >VIVOTEK</rdfs:label>
    <belongsToModule xml:lang="en">DigitalCamera</belongsToModule>
    <rdfs:comment xml:lang="en">The business entity VIVOTEK Inc.</rdfs:comment>
    <gr:legalName rdf:datatype="http://www.w3.org/2001/XMLSchema#string"
    >VIVOTEK Inc.</gr:legalName>
  </gr:BusinessEntity>
  <ComputerDisplayResolution rdf:ID="ComputerDisplayResolution_640x480_60_72_75_85Hz">
    <rdfs:label xml:lang="en">Computer display resolution 640x480 60 72 75 85Hz</rdfs:label>
    <rdfs:label xml:lang="de">Computerbildschirmauflösung 640x480 60 72 75 85Hz</rdfs:label>
    <rdfs:comment xml:lang="en">Display resolution specified as the width and height in pixels, color depth measured in bits, and refresh rate expressed in hertz; here Video Graphics Array.

(This description is partly based on or reuses content from the Wikipedia article "Display resolution" (http://en.wikipedia.org/wiki/Display_resolution) and is licensed under the GNU Free Documentation License (http://www.gnu.org/copyleft/fdl.html).)</rdfs:comment>
    <belongsToModule xml:lang="en">TV</belongsToModule>
  </ComputerDisplayResolution>
  <StorageMedia rdf:ID="SD">
    <belongsToModule xml:lang="en">MP3Player, DigitalCamera, Camcorder</belongsToModule>
    <rdfs:label xml:lang="en">SD</rdfs:label>
    <rdfs:label xml:lang="de">SD</rdfs:label>
    <rdfs:comment xml:lang="en">A flash memory card format used in portable device.</rdfs:comment>
  </StorageMedia>
  <AudioInterfaceType rdf:ID="BluetoothAudio">
    <rdfs:comment xml:lang="en">Bluetooth is a wireless protocol utilizing short-range communications technology facilitating data transmission over short distances from fixed and mobile devices, creating wireless personal area networks (refers to audio).</rdfs:comment>
    <belongsToModule xml:lang="en">MP3Player</belongsToModule>
    <rdfs:label xml:lang="en">Bluetooth audio</rdfs:label>
    <rdfs:label xml:lang="de">Bluetooth Audio</rdfs:label>
  </AudioInterfaceType>
  <gr:BusinessEntity rdf:ID="Sapphire">
    <rdfs:comment xml:lang="en">The business entity Sapphire Technology Limited</rdfs:comment>
    <belongsToModule xml:lang="en">MP3Player</belongsToModule>
    <gr:legalName rdf:datatype="http://www.w3.org/2001/XMLSchema#string"
    >Sapphire Technology Limited</gr:legalName>
    <rdfs:seeAlso rdf:resource="http://www.sapphiretech.com/"/>
    <rdfs:label rdf:datatype="http://www.w3.org/2001/XMLSchema#string"
    >Sapphire</rdfs:label>
  </gr:BusinessEntity>
  <VideoFeatures rdf:ID="AmbilightSpectra3">
    <belongsToModule xml:lang="en">TV</belongsToModule>
    <rdfs:comment xml:lang="en">Enlarges the screen further by projecting a glow of light from the back of the screen onto the surrounding wall. Ambilight adjusts automatically the colour and brightness of the light surrounding the TV to match with the picture.</rdfs:comment>
    <rdfs:label xml:lang="de">Ambilight Spectra 3</rdfs:label>
    <rdfs:label xml:lang="en">Ambilight Spectra 3</rdfs:label>
  </VideoFeatures>
  <DataInterfaceType rdf:ID="HDMI_Interface">
    <rdfs:label xml:lang="de">HDMI Schnittstelle</rdfs:label>
    <rdfs:label xml:lang="en">HDMI interface</rdfs:label>
    <rdfs:comment xml:lang="en">HDMI (High-Definition Multimedia Interface) is a compact audio/video interface for transmitting uncompressed digital data.

(This description is partly based on or reuses content from the Wikipedia article "HDMI" (http://en.wikipedia.org/wiki/HDMI) and is licensed under the GNU Free Documentation License (http://www.gnu.org/copyleft/fdl.html).)</rdfs:comment>
    <belongsToModule xml:lang="en">DigitalCamera, Camcorder</belongsToModule>
  </DataInterfaceType>
  <DataFormatAudio rdf:ID="ASF">
    <rdfs:comment xml:lang="en">Advanced Systems Format (formerly Advanced Streaming Format, Active Streaming Format) is Microsoft's proprietary digital audio/digital video container format, especially meant for streaming media. ASF is part of the Windows Media framework.

(This description is partly based on or reuses content from the Wikipedia article "Advanced Systems Format" (http://en.wikipedia.org/wiki/Advanced_Systems_Format) and is licensed under the GNU Free Documentation License (http://www.gnu.org/copyleft/fdl.html).)</rdfs:comment>
    <belongsToModule xml:lang="en">MP3Player, DigitalCamera, Camcorder</belongsToModule>
    <rdfs:label xml:lang="en">ASF</rdfs:label>
    <rdfs:label xml:lang="de">ASF</rdfs:label>
  </DataFormatAudio>
  <Accessory rdf:ID="Headphones">
    <rdfs:comment xml:lang="en">A pair of small loudspeakers, or less commonly a single speaker, with a way of holding them close to a user's ears and a means of connecting them to a signal source such as an audio amplifier, radio or CD player.</rdfs:comment>
    <rdfs:label xml:lang="de">Kopfhörer</rdfs:label>
    <rdfs:label xml:lang="en">Headphones</rdfs:label>
    <belongsToModule xml:lang="en">Camcorder</belongsToModule>
  </Accessory>
  <MediaFormat rdf:ID="B3">
    <belongsToModule xml:lang="en">Printer</belongsToModule>
    <rdfs:label xml:lang="de">B3</rdfs:label>
    <rdfs:label xml:lang="en">B3</rdfs:label>
    <rdfs:comment xml:lang="en">Format of the german institute for standardization: 353 x 500 mm.</rdfs:comment>
  </MediaFormat>
  <Color rdf:ID="Olive">
    <rdfs:label xml:lang="en">Olive</rdfs:label>
    <rdfs:label xml:lang="de">Olivgrün</rdfs:label>
    <belongsToModule xml:lang="en">MP3Player, TV, Printer, DigitalCamera, Camcorder</belongsToModule>
    <rdfs:comment xml:lang="en">RGB Value 128,128,0</rdfs:comment>
  </Color>
  <CompatibleOperatingSystems rdf:ID="Windows2003">
    <rdfs:comment xml:lang="en">A version of a Microsoft operating system.</rdfs:comment>
    <rdfs:label xml:lang="en">Windows 2003</rdfs:label>
    <rdfs:label xml:lang="de">Windows 2003</rdfs:label>
    <belongsToModule xml:lang="en">MP3Player, Printer, DigitalCamera, Camcorder</belongsToModule>
  </CompatibleOperatingSystems>
  <owl:AnnotationProperty rdf:ID="belongsToModule">
    <rdfs:comment xml:lang="en">Describes to which product categories the property or concept belongs (comma seperated, e.g. "MP3Player, TV").</rdfs:comment>
    <rdfs:isDefinedBy rdf:resource="http://www.ebusiness-unibw.org/ontologies/consumerelectronics/v1"/>
  </owl:AnnotationProperty>
  <gr:BusinessEntity rdf:ID="Kye_Genius">
    <rdfs:seeAlso rdf:resource="http://www.geniusnet.com/"/>
    <rdfs:label rdf:datatype="http://www.w3.org/2001/XMLSchema#string"
    >Kye Genius</rdfs:label>
    <gr:legalName rdf:datatype="http://www.w3.org/2001/XMLSchema#string"
    >Genius, KYE Systems Corp.</gr:legalName>
    <rdfs:comment xml:lang="en">The business entity Genius, KYE Systems Corp.</rdfs:comment>
    <belongsToModule xml:lang="en">MP3Player, Camcorder</belongsToModule>
  </gr:BusinessEntity>
  <gr:BusinessEntity rdf:ID="Seiko">
    <rdfs:seeAlso rdf:resource="http://www.seikoinstruments.com/"/>
    <rdfs:label rdf:datatype="http://www.w3.org/2001/XMLSchema#string"
    >Seiko</rdfs:label>
    <rdfs:comment xml:lang="en">The business entity Seiko.</rdfs:comment>
    <belongsToModule xml:lang="en">Printer</belongsToModule>
    <gr:legalName rdf:datatype="http://www.w3.org/2001/XMLSchema#string"
    >Seiko Holdings Corporation</gr:legalName>
  </gr:BusinessEntity>
  <gr:BusinessEntity rdf:ID="Lavod">
    <rdfs:comment xml:lang="en">The business entity LAVOD CORPORATION.</rdfs:comment>
    <rdfs:label rdf:datatype="http://www.w3.org/2001/XMLSchema#string"
    >Lavod</rdfs:label>
    <rdfs:seeAlso rdf:resource="http://www.lavod.com/"/>
    <belongsToModule xml:lang="en">MP3Player</belongsToModule>
    <gr:legalName rdf:datatype="http://www.w3.org/2001/XMLSchema#string"
    >LAVOD CORPOPATION</gr:legalName>
  </gr:BusinessEntity>
  <gr:BusinessEntity rdf:ID="SIGMA">
    <rdfs:label rdf:datatype="http://www.w3.org/2001/XMLSchema#string"
    >SIGMA</rdfs:label>
    <rdfs:comment xml:lang="en">The business entity SIGMA GmbH.</rdfs:comment>
    <gr:legalName rdf:datatype="http://www.w3.org/2001/XMLSchema#string"
    >SIGMA GmbH</gr:legalName>
    <belongsToModule xml:lang="en">DigitalCamera</belongsToModule>
    <rdfs:seeAlso rdf:resource="http://www.sigma-foto.de/"/>
  </gr:BusinessEntity>
  <Connectivity rdf:ID="CVBS_in">
    <rdfs:comment xml:lang="en">Composite video is often designated by the CVBS acronym, meaning any of "Color, Video, Blank and Sync", "Composite Video Baseband Signal", "Composite Video Burst Signal", or "Composite Video with Burst and Sync". Here the input is meant.</rdfs:comment>
    <rdfs:label xml:lang="de">CVBS in</rdfs:label>
    <rdfs:label xml:lang="en">CVBS in</rdfs:label>
    <belongsToModule xml:lang="en">TV</belongsToModule>
  </Connectivity>
  <Connectivity rdf:ID="HeadphoneLineOut_2.5mm">
    <belongsToModule xml:lang="en">TV</belongsToModule>
    <rdfs:comment xml:lang="en">Port to connect headphones with an electronical device. Here the port has the diameter of 2,5 millimetres.</rdfs:comment>
    <rdfs:label xml:lang="en">Headphone line out 2.5mm</rdfs:label>
    <rdfs:label xml:lang="de">Kopfhörerausgang 2.5 mm</rdfs:label>
  </Connectivity>
  <DataFormatImage rdf:ID="JPEG">
    <rdfs:label xml:lang="en">JPEG</rdfs:label>
    <rdfs:label xml:lang="de">JPEG</rdfs:label>
    <belongsToModule xml:lang="en">MP3Player, DigitalCamera, Camcorder</belongsToModule>
    <rdfs:comment xml:lang="en">JPEG compression is used in a number of image file formats. JPEG/Exif is the most common image format used by digital cameras and other photographic image capture devices; along with JPEG/JFIF, it is the most common format for storing and transmitting photographic images on the World Wide Web.

(This description is partly based on or reuses content from the Wikipedia article "JPEG" (http://en.wikipedia.org/wiki/JPEG) and is licensed under the GNU Free Documentation License (http://www.gnu.org/copyleft/fdl.html).)</rdfs:comment>
  </DataFormatImage>
  <gr:BusinessEntity rdf:ID="Fujitsu_Siemens">
    <rdfs:seeAlso rdf:resource="http://www.fujitsu.com/"/>
    <gr:legalName rdf:datatype="http://www.w3.org/2001/XMLSchema#string"
    >Fujitsu Siemens Computers</gr:legalName>
    <rdfs:comment xml:lang="en">The business entity Fujitsu Siemens.</rdfs:comment>
    <rdfs:label rdf:datatype="http://www.w3.org/2001/XMLSchema#string"
    >Fujitsu Siemens</rdfs:label>
    <belongsToModule xml:lang="en">TV, Printer, DigitalCamera</belongsToModule>
  </gr:BusinessEntity>
  <gr:BusinessEntity rdf:ID="Mustek">
    <rdfs:seeAlso rdf:resource="http://www.mustek.com/"/>
    <rdfs:comment xml:lang="en">The business entity Mustek Ltd.</rdfs:comment>
    <belongsToModule xml:lang="en">MP3Player, Camcorder</belongsToModule>
    <gr:legalName rdf:datatype="http://www.w3.org/2001/XMLSchema#string"
    >Mustek Ltd.</gr:legalName>
    <rdfs:label rdf:datatype="http://www.w3.org/2001/XMLSchema#string"
    >Mustek</rdfs:label>
  </gr:BusinessEntity>
  <VideoFeatures rdf:ID="Ambilight1">
    <belongsToModule xml:lang="en">TV</belongsToModule>
    <rdfs:comment xml:lang="en">Ambilight, which is short for Ambient Lighting Technology, is a feature invented by Philips Electronics, generating light effects around the TV that correspond to the video content.

(This description is partly based on or reuses content from the Wikipedia article "Ambilight" (http://en.wikipedia.org/wiki/Ambilight) and is licensed under the GNU Free Documentation License (http://www.gnu.org/copyleft/fdl.html).)</rdfs:comment>
    <rdfs:label xml:lang="en">Ambilight 1</rdfs:label>
    <rdfs:label rdf:datatype="http://www.w3.org/2001/XMLSchema#string"
    >Ambilight 1</rdfs:label>
  </VideoFeatures>
  <Color rdf:ID="Orange">
    <belongsToModule xml:lang="en">MP3Player, TV, Printer, DigitalCamera, Camcorder</belongsToModule>
    <rdfs:label xml:lang="en">Orange</rdfs:label>
    <rdfs:label xml:lang="de">Orange</rdfs:label>
    <rdfs:comment xml:lang="en">RGB Value 255,165,0</rdfs:comment>
  </Color>
  <PowerSupplyUnit rdf:ID="ACAdapter">
    <rdfs:comment xml:lang="en">A linear or switched-mode power supply (or in some cases just a transformer) that is built into the top of a plug and needed for the conversion of one form of electrical power to another desired form and voltage.

(This description is partly based on or reuses content from the Wikipedia article "Power supply" (http://en.wikipedia.org/wiki/Power_supply) and is licensed under the GNU Free Documentation License (http://www.gnu.org/copyleft/fdl.html).)</rdfs:comment>
    <belongsToModule xml:lang="en">MP3Player, Printer, DigitalCamera, Camcorder</belongsToModule>
    <rdfs:label xml:lang="en">AC Adapter</rdfs:label>
    <rdfs:label xml:lang="de">AC Adapter</rdfs:label>
  </PowerSupplyUnit>
  <Connectivity rdf:ID="HeadphoneLineOut_3.5mm">
    <rdfs:comment xml:lang="en">Port to connect headphones with an electronical device. Here the port has the diameter of 3,5 millimetres.</rdfs:comment>
    <belongsToModule xml:lang="en">TV</belongsToModule>
    <rdfs:label xml:lang="en">Headphone line out 3,5 mm</rdfs:label>
    <rdfs:label xml:lang="de">Kopfhörerausgang 3,5 mm</rdfs:label>
  </Connectivity>
  <gr:BusinessEntity rdf:ID="Sweex">
    <rdfs:label rdf:datatype="http://www.w3.org/2001/XMLSchema#string"
    >Sweex</rdfs:label>
    <gr:legalName rdf:datatype="http://www.w3.org/2001/XMLSchema#string"
    >Sweex</gr:legalName>
    <belongsToModule xml:lang="en">TV</belongsToModule>
    <rdfs:comment xml:lang="en">The business entity Sweex.</rdfs:comment>
    <rdfs:seeAlso rdf:resource="http://www.sweex.com/"/>
  </gr:BusinessEntity>
  <SceneMode rdf:ID="Sports">
    <rdfs:comment xml:lang="en">Ability of the camcorder to adapt to special environments.</rdfs:comment>
    <belongsToModule xml:lang="en">Camcorder</belongsToModule>
    <rdfs:label xml:lang="en">Sport</rdfs:label>
    <rdfs:label xml:lang="en">Sports</rdfs:label>
  </SceneMode>
  <gr:BusinessEntity rdf:ID="Sitecom">
    <rdfs:comment xml:lang="en">The business entity Sitecom</rdfs:comment>
    <rdfs:label rdf:datatype="http://www.w3.org/2001/XMLSchema#string"
    >Sitecom</rdfs:label>
    <belongsToModule xml:lang="en">MP3Player</belongsToModule>
    <rdfs:seeAlso rdf:resource="http://www.sitecom.com/"/>
    <gr:legalName rdf:datatype="http://www.w3.org/2001/XMLSchema#string"
    >Sitecom</gr:legalName>
  </gr:BusinessEntity>
  <gr:BusinessEntity rdf:ID="Agfa">
    <rdfs:label rdf:datatype="http://www.w3.org/2001/XMLSchema#string"
    >Agfa</rdfs:label>
    <gr:legalName rdf:datatype="http://www.w3.org/2001/XMLSchema#string"
    >Agfa-Gevaert N.V.</gr:legalName>
    <belongsToModule xml:lang="en">DigitalCamera</belongsToModule>
    <rdfs:seeAlso rdf:resource="http://www.agfa.com/"/>
    <rdfs:comment xml:lang="en">The business entity Agfa-Gevaert N.V.</rdfs:comment>
  </gr:BusinessEntity>
  <gr:BusinessEntity rdf:ID="Ricatech">
    <rdfs:seeAlso rdf:resource="http://www.ricatech.com/"/>
    <rdfs:label rdf:datatype="http://www.w3.org/2001/XMLSchema#string"
    >Ricatech</rdfs:label>
    <rdfs:comment xml:lang="en">The business entity Ricatech B.V.</rdfs:comment>
    <gr:legalName rdf:datatype="http://www.w3.org/2001/XMLSchema#string"
    >Ricatech B.V.</gr:legalName>
    <belongsToModule xml:lang="en">MP3Player</belongsToModule>
  </gr:BusinessEntity>
  <Color rdf:ID="Gold">
    <rdfs:comment xml:lang="en">RGB Value 255,215,0</rdfs:comment>
    <rdfs:label xml:lang="en">Gold</rdfs:label>
    <rdfs:label xml:lang="de">Gold</rdfs:label>
    <belongsToModule xml:lang="en">MP3Player, TV, Printer, DigitalCamera, Camcorder</belongsToModule>
  </Color>
  <WhiteBalance rdf:ID="OutdoorWhiteBalance">
    <rdfs:comment xml:lang="en">Ability to adapt of different adjustments of the intensities of the colors.</rdfs:comment>
    <rdfs:label xml:lang="de">Weißabgleich außen</rdfs:label>
    <rdfs:label xml:lang="en">Outdoor white balance</rdfs:label>
    <belongsToModule xml:lang="en">Camcorder</belongsToModule>
  </WhiteBalance>
  <Accessory rdf:ID="IR_Remote">
    <rdfs:label xml:lang="de">Infrarotfernbedienung</rdfs:label>
    <rdfs:label xml:lang="en">IR remote control</rdfs:label>
    <rdfs:comment xml:lang="en">Remote control with a electromagnetic radiation whose wavelength is longer than that of visible light (400-700 nm), but shorter than that of terahertz radiation (3-300 µm) and microwaves (~30,000 µm). Infrared radiation spans roughly three orders of magnitude (750 nm and 1000 µm)</rdfs:comment>
    <belongsToModule xml:lang="en">Camcorder</belongsToModule>
  </Accessory>
  <DataFormatAudio rdf:ID="AIFF">
    <rdfs:comment xml:lang="en">Audio Interchange File Format (AIFF) is an audio file format standard used for storing sound data for personal computers and other electronic audio devices.

(This description is partly based on or reuses content from the Wikipedia article "Audio Interchange File Format" (http://en.wikipedia.org/wiki/Audio_Interchange_File_Format) and is licensed under the GNU Free Documentation License (http://www.gnu.org/copyleft/fdl.html).)</rdfs:comment>
    <belongsToModule xml:lang="en">MP3Player, DigitalCamera, Camcorder</belongsToModule>
    <rdfs:label xml:lang="en">AIFF</rdfs:label>
    <rdfs:label xml:lang="de">AIFF</rdfs:label>
  </DataFormatAudio>
  <gr:BusinessEntity rdf:ID="Memorex">
    <belongsToModule xml:lang="en">MP3Player, TV</belongsToModule>
    <rdfs:label rdf:datatype="http://www.w3.org/2001/XMLSchema#string"
    >Memorex</rdfs:label>
    <rdfs:seeAlso rdf:resource="http://www.memorex.com/"/>
    <rdfs:comment xml:lang="en">The business entity Memorex Products, Inc.</rdfs:comment>
    <gr:legalName rdf:datatype="http://www.w3.org/2001/XMLSchema#string"
    >Memorex Products, Inc.</gr:legalName>
  </gr:BusinessEntity>
  <Color rdf:ID="Purple">
    <rdfs:comment xml:lang="en">RGB Value 128,0,128</rdfs:comment>
    <rdfs:label xml:lang="en">Purple</rdfs:label>
    <rdfs:label xml:lang="de">Purpurrot</rdfs:label>
    <belongsToModule xml:lang="en">MP3Player, TV, Printer, DigitalCamera, Camcorder</belongsToModule>
  </Color>
  <Features rdf:ID="Radio">
    <belongsToModule xml:lang="en">MP3Player</belongsToModule>
    <rdfs:comment xml:lang="en">Ability to recieve radiosignal.</rdfs:comment>
    <rdfs:label xml:lang="en">Radio</rdfs:label>
    <rdfs:label xml:lang="de">Radio</rdfs:label>
  </Features>
  <gr:BusinessEntity rdf:ID="Tektronix">
    <rdfs:seeAlso rdf:resource="http://www.tek.com/"/>
    <gr:legalName rdf:datatype="http://www.w3.org/2001/XMLSchema#string"
    >Tektronix, Inc.</gr:legalName>
    <rdfs:comment xml:lang="en">The business entity Tektronix.</rdfs:comment>
    <rdfs:label rdf:datatype="http://www.w3.org/2001/XMLSchema#string"
    >Tektronix</rdfs:label>
    <belongsToModule xml:lang="en">Printer</belongsToModule>
  </gr:BusinessEntity>
  <DataInterfaceType rdf:ID="DVI_in">
    <rdfs:label xml:lang="de">DV in</rdfs:label>
    <rdfs:label xml:lang="en">DV in</rdfs:label>
    <belongsToModule xml:lang="en">Camcorder</belongsToModule>
    <rdfs:comment xml:lang="en">A digital video format created by Sony, JVC, Panasonic and other video camera producers.</rdfs:comment>
  </DataInterfaceType>
  <DataFormatImage rdf:ID="TIFF">
    <rdfs:label xml:lang="en">TIFF</rdfs:label>
    <rdfs:label xml:lang="de">TIFF</rdfs:label>
    <rdfs:comment xml:lang="en">The TIFF (Tagged Image File Format) is a flexible format that normally saves 8 bits or 16 bits per color (red, green, blue) for 24-bit and 48-bit totals, respectively, using either the TIFF or the TIF filenames.

(This description is partly based on or reuses content from the Wikipedia article "Graphics file format" (http://en.wikipedia.org/wiki/Graphics_file_format) and is licensed under the GNU Free Documentation License (http://www.gnu.org/copyleft/fdl.html).)</rdfs:comment>
    <belongsToModule xml:lang="en">MP3Player, DigitalCamera, Camcorder</belongsToModule>
  </DataFormatImage>
  <StorageMedia rdf:ID="MMC">
    <rdfs:comment xml:lang="en">A solid state disk or flash memory data storage device.</rdfs:comment>
    <belongsToModule xml:lang="en">MP3Player, DigitalCamera, Camcorder</belongsToModule>
    <rdfs:label xml:lang="en">MMC</rdfs:label>
    <rdfs:label xml:lang="de">MMC</rdfs:label>
  </StorageMedia>
  <RechargeableEnergySource rdf:ID="Solar">
    <rdfs:label xml:lang="en">Solar</rdfs:label>
    <rdfs:label xml:lang="de">Solar</rdfs:label>
    <rdfs:comment xml:lang="en">Solar cell or photovoltaic cell is a wide area electronic device that converts solar energy into electricity by the photovoltaic effect.

(This description is partly based on or reuses content from the Wikipedia article "Solar cell" (http://en.wikipedia.org/wiki/Solar_cell) and is licensed under the GNU Free Documentation License (http://www.gnu.org/copyleft/fdl.html).)</rdfs:comment>
    <belongsToModule xml:lang="en">MP3Player, DigitalCamera, Camcorder</belongsToModule>
  </RechargeableEnergySource>
  <CompatibleOperatingSystems rdf:ID="WindowsXP">
    <belongsToModule xml:lang="en">MP3Player, Printer, DigitalCamera, Camcorder</belongsToModule>
    <rdfs:label xml:lang="en">Windows XP</rdfs:label>
    <rdfs:label xml:lang="de">Windows XP</rdfs:label>
    <rdfs:comment xml:lang="en">A version of a Microsoft operating system.</rdfs:comment>
  </CompatibleOperatingSystems>
  <Color rdf:ID="Brown">
    <belongsToModule xml:lang="en">MP3Player, TV, Printer, DigitalCamera, Camcorder</belongsToModule>
    <rdfs:comment xml:lang="en">RGB Value 165,42,42</rdfs:comment>
    <rdfs:label xml:lang="en">Brown</rdfs:label>
    <rdfs:label xml:lang="de">Braun</rdfs:label>
  </Color>
  <SignalFormat rdf:ID="PAL-L">
    <belongsToModule xml:lang="en">TV</belongsToModule>
    <rdfs:label xml:lang="en">PAL-L</rdfs:label>
    <rdfs:label xml:lang="de">PAL-L</rdfs:label>
    <rdfs:comment xml:lang="en">PAL, short for Phase Alternating Line, is a colour-encoding system used in broadcast television systems in large parts of the world. PAL L is used on some hotel internal distribution systems, as well as other public display and plant television systems.

(This description is partly based on or reuses content from the Wikipedia article "PAL" (http://en.wikipedia.org/wiki/PAL) and is licensed under the GNU Free Documentation License (http://www.gnu.org/copyleft/fdl.html).)</rdfs:comment>
  </SignalFormat>
  <DisposableEnergySource rdf:ID="DisposableBattery">
    <rdfs:label xml:lang="de">Batterie</rdfs:label>
    <rdfs:label xml:lang="en">Disposable battery</rdfs:label>
    <belongsToModule xml:lang="en">MP3Player, DigitalCamera, Camcorder</belongsToModule>
    <rdfs:comment xml:lang="en">Is any kind of electrochemical cell in which the electrochemical reaction of interest is not reversible.</rdfs:comment>
  </DisposableEnergySource>
  <Connectivity rdf:ID="PCAudioIn">
    <belongsToModule xml:lang="en">TV</belongsToModule>
    <rdfs:comment xml:lang="en">Port to connect the audio cables for a PC with the electronical device.</rdfs:comment>
    <rdfs:label xml:lang="de">PC Audio in</rdfs:label>
    <rdfs:label xml:lang="en">PC Audio out</rdfs:label>
  </Connectivity>
  <GeneralFeatures rdf:ID="StandbyLED">
    <belongsToModule xml:lang="en">TV</belongsToModule>
    <rdfs:label xml:lang="de">Standby Ledanzeige</rdfs:label>
    <rdfs:label xml:lang="en">Standby LED</rdfs:label>
    <rdfs:comment xml:lang="en">It is a semiconductor diode that emits light when an electric current is applied in the forward direction of the device used to show the standby status of an electrical device.

(This description is partly based on or reuses content from the Wikipedia article "LED" (http://en.wikipedia.org/wiki/Led) and is licensed under the GNU Free Documentation License (http://www.gnu.org/copyleft/fdl.html).)</rdfs:comment>
  </GeneralFeatures>
  <VideoFeatures rdf:ID="PictureInPicture">
    <rdfs:comment xml:lang="en">Picture in Picture (PiP) is a feature of some television receivers and similar devices. One program (channel) is displayed on the full TV screen at the same time as one or more other programs are displayed in inset windows. Sound is usually from the main program only.

(This description is partly based on or reuses content from the Wikipedia article "Picture in picture" (http://en.wikipedia.org/wiki/Picture-in-picture) and is licensed under the GNU Free Documentation License (http://www.gnu.org/copyleft/fdl.html).)</rdfs:comment>
    <belongsToModule xml:lang="en">TV</belongsToModule>
    <rdfs:label xml:lang="en">Picture in Picture</rdfs:label>
    <rdfs:label xml:lang="de">Bild in Bild Funktion</rdfs:label>
  </VideoFeatures>
  <MediaFormat rdf:ID="MediaFormaPostcard">
    <belongsToModule xml:lang="en">Printer</belongsToModule>
    <rdfs:label xml:lang="de">Medienformat Postkarte</rdfs:label>
    <rdfs:label xml:lang="en">Media format postcard</rdfs:label>
    <rdfs:comment xml:lang="en">Media format that is able to assume different shapes.</rdfs:comment>
  </MediaFormat>
  <SignalFormat rdf:ID="VHF">
    <rdfs:comment xml:lang="en">VHF (Very high frequency) is the radio frequency range from 30 MHz to 300 MHz.

(This description is partly based on or reuses content from the Wikipedia article "VHF" (http://en.wikipedia.org/wiki/VHF) and is licensed under the GNU Free Documentation License (http://www.gnu.org/copyleft/fdl.html).)</rdfs:comment>
    <belongsToModule xml:lang="en">TV</belongsToModule>
    <rdfs:label xml:lang="en">VHF</rdfs:label>
    <rdfs:label xml:lang="de">VHF</rdfs:label>
  </SignalFormat>
  <CompatibleOperatingSystems rdf:ID="WindowsNT">
    <rdfs:comment xml:lang="en">A version of a Microsoft operating system.</rdfs:comment>
    <belongsToModule xml:lang="en">MP3Player, Printer, DigitalCamera, Camcorder</belongsToModule>
    <rdfs:label xml:lang="en">Windows NT</rdfs:label>
    <rdfs:label xml:lang="de">Windows NT</rdfs:label>
  </CompatibleOperatingSystems>
  <Connectivity rdf:ID="DLNA_Ethernet">
    <rdfs:comment xml:lang="en">The Digital Living Network Alliance is an international, cross-industry collaboration of consumer electronics, computing industry and mobile device companies. Members of DLNA develop a concept of wired and wireless interoperable networks where digital content such as photos, music, and videos can be shared through consumer electronics (CE), personal computers (PCs), and mobile devices in and beyond the home.

(This description is partly based on or reuses content from the Wikipedia article "Digital Living Network Alliance" (http://en.wikipedia.org/wiki/Digital_Living_Network_Alliance) and is licensed under the GNU Free Documentation License (http://www.gnu.org/copyleft/fdl.html).)</rdfs:comment>
    <rdfs:label xml:lang="en">DLNA Ethernet</rdfs:label>
    <rdfs:label xml:lang="de">DLNA Ethernet</rdfs:label>
    <belongsToModule xml:lang="en">TV</belongsToModule>
  </Connectivity>
  <StorageMedia rdf:ID="CompactFlash">
    <rdfs:comment xml:lang="en">CompactFlash (CF) is a mass storage device format used in portable electronic devices. For storage, CompactFlash typically uses flash memory in a standardized enclosure.

(This description is partly based on or reuses content from the Wikipedia article "CompactFlash" (http://en.wikipedia.org/wiki/CompactFlash) and is licensed under the GNU Free Documentation License (http://www.gnu.org/copyleft/fdl.html).)</rdfs:comment>
    <rdfs:label xml:lang="de">CompactFlash</rdfs:label>
    <rdfs:label xml:lang="en">CompactFlash</rdfs:label>
    <belongsToModule xml:lang="en">MP3Player, DigitalCamera, Camcorder</belongsToModule>
  </StorageMedia>
  <gr:BusinessEntity rdf:ID="Mirai">
    <rdfs:label rdf:datatype="http://www.w3.org/2001/XMLSchema#string"
    >Mirai</rdfs:label>
    <gr:legalName rdf:datatype="http://www.w3.org/2001/XMLSchema#string"
    >Mirai</gr:legalName>
    <rdfs:seeAlso rdf:resource="http://www.mirai.eu/"/>
    <belongsToModule xml:lang="en">TV</belongsToModule>
    <rdfs:comment xml:lang="en">The business entity Mirai.</rdfs:comment>
  </gr:BusinessEntity>
  <gr:BusinessEntity rdf:ID="Salora">
    <rdfs:seeAlso rdf:resource="http://www.salora.com/"/>
    <rdfs:label rdf:datatype="http://www.w3.org/2001/XMLSchema#string"
    >Salora</rdfs:label>
    <rdfs:comment xml:lang="en">The business entity Salora.</rdfs:comment>
    <belongsToModule xml:lang="en">TV</belongsToModule>
    <gr:legalName rdf:datatype="http://www.w3.org/2001/XMLSchema#string"
    >SALORA</gr:legalName>
  </gr:BusinessEntity>
  <MediaFormat rdf:ID="A8">
    <belongsToModule xml:lang="en">Printer</belongsToModule>
    <rdfs:comment xml:lang="en">Format of the german institute for standardization: 52 x 74 mm.</rdfs:comment>
    <rdfs:label xml:lang="de">A8</rdfs:label>
    <rdfs:label xml:lang="en">A8</rdfs:label>
  </MediaFormat>
  <DataFormatVideo rdf:ID="WMV">
    <belongsToModule xml:lang="en">MP3Player, DigitalCamera, Camcorder</belongsToModule>
    <rdfs:comment xml:lang="en">A compressed video file format for several proprietary codecs developed by Microsoft.</rdfs:comment>
    <rdfs:label xml:lang="en">WMV</rdfs:label>
    <rdfs:label xml:lang="de">WMV</rdfs:label>
  </DataFormatVideo>
  <VideoFeatures rdf:ID="ContrastPlus">
    <rdfs:comment xml:lang="en">Ensures that, according to the scene, the screen always displays the best possible contrast. This results in a depth of focus, which lends an extraordinary power to the television image, making it appear almost touchable.</rdfs:comment>
    <belongsToModule xml:lang="en">TV</belongsToModule>
    <rdfs:label xml:lang="en">Contrast Plus</rdfs:label>
    <rdfs:label xml:lang="de">Contrast Plus</rdfs:label>
  </VideoFeatures>
  <gr:BusinessEntity rdf:ID="Nokia">
    <belongsToModule xml:lang="en">DigitalCamera</belongsToModule>
    <rdfs:seeAlso rdf:resource="http://www.nokia.com/"/>
    <rdfs:label rdf:datatype="http://www.w3.org/2001/XMLSchema#string"
    >Nokia</rdfs:label>
    <rdfs:comment xml:lang="en">The business entity Nokia Corporation.</rdfs:comment>
    <gr:legalName rdf:datatype="http://www.w3.org/2001/XMLSchema#string"
    >Nokia Corporation</gr:legalName>
  </gr:BusinessEntity>
  <ViewFinder rdf:ID="ViewFinderElectronic">
    <rdfs:label xml:lang="en">Viewfinder electronic</rdfs:label>
    <rdfs:label xml:lang="de">Elektronischer Bildsucher</rdfs:label>
    <rdfs:comment xml:lang="en">An electronic viewfinder or EVF is a viewfinder where the image captured by the lens is projected electronically onto a miniature display. The image on this display is used to assist in aiming the camera at the scene to be photographed.

(This description is partly based on or reuses content from the Wikipedia article "Electronic viewfinder" (http://en.wikipedia.org/wiki/Electronic_viewfinder) and is licensed under the GNU Free Documentation License (http://www.gnu.org/copyleft/fdl.html).)</rdfs:comment>
    <belongsToModule xml:lang="en">DigitalCamera</belongsToModule>
  </ViewFinder>
  <CompatibleOperatingSystems rdf:ID="WindowsVista">
    <rdfs:label xml:lang="en">Windows Vista</rdfs:label>
    <rdfs:label xml:lang="de">Windows Vista</rdfs:label>
    <belongsToModule xml:lang="en">MP3Player, Printer, DigitalCamera, Camcorder</belongsToModule>
    <rdfs:comment xml:lang="en">A version of a Microsoft operating system.</rdfs:comment>
  </CompatibleOperatingSystems>
  <gr:BusinessEntity rdf:ID="iDream">
    <rdfs:seeAlso rdf:resource="http://www.idream.be/"/>
    <rdfs:label rdf:datatype="http://www.w3.org/2001/XMLSchema#string"
    >iDream</rdfs:label>
    <belongsToModule xml:lang="en">MP3Player</belongsToModule>
    <gr:legalName rdf:datatype="http://www.w3.org/2001/XMLSchema#string"
    >iDream Production Pvt. Ltd.</gr:legalName>
    <rdfs:comment xml:lang="en">The business entity iDream Production Pvt. Ltd.</rdfs:comment>
  </gr:BusinessEntity>
  <Certificate rdf:ID="RoHS">
    <belongsToModule xml:lang="en">TV</belongsToModule>
    <rdfs:comment xml:lang="en">The Directive on the restriction of the use of certain hazardous substances in electrical and electronic equipment 2002/95/EC.

(This description is partly based on or reuses content from the Wikipedia article "ROHS" (http://en.wikipedia.org/wiki/ROHS) and is licensed under the GNU Free Documentation License (http://www.gnu.org/copyleft/fdl.html).)</rdfs:comment>
    <rdfs:label xml:lang="en">RoHS</rdfs:label>
    <rdfs:label xml:lang="de">RoHS</rdfs:label>
  </Certificate>
  <MediaFormat rdf:ID="A6">
    <rdfs:comment xml:lang="en">Format of the german institute for standardization: 105 x 148 mm.</rdfs:comment>
    <belongsToModule xml:lang="en">Printer</belongsToModule>
    <rdfs:label xml:lang="de">A6</rdfs:label>
    <rdfs:label xml:lang="en">A6</rdfs:label>
  </MediaFormat>
  <USB rdf:ID="USBEnergyInterface">
    <rdfs:comment xml:lang="en">USB-interface used to provide power to low-consumption devices without the need for an external power supply.</rdfs:comment>
    <rdfs:label xml:lang="en">USB energy interface</rdfs:label>
    <rdfs:label xml:lang="de">USB Stromschnittstelle</rdfs:label>
    <belongsToModule xml:lang="en">MP3Player, Printer, DigitalCamera</belongsToModule>
  </USB>
  <DataFormatImage rdf:ID="PSD">
    <rdfs:label xml:lang="en">PSD</rdfs:label>
    <rdfs:label xml:lang="de">PSD</rdfs:label>
    <rdfs:comment xml:lang="en">The .PSD (Photoshop Document) format stores an image with support for most imaging options available in Photoshop. These include layers with masks, color spaces, ICC profiles, transparency, text, alpha channels and spot colors, clipping paths, and duotone settings.

(This description is partly based on or reuses content from the Wikipedia article "Adobe Photoshop" (http://en.wikipedia.org/wiki/Adobe_Photoshop) and is licensed under the GNU Free Documentation License (http://www.gnu.org/copyleft/fdl.html).)</rdfs:comment>
    <belongsToModule xml:lang="en">MP3Player, DigitalCamera, Camcorder</belongsToModule>
  </DataFormatImage>
  <gr:BusinessEntity rdf:ID="Memup">
    <belongsToModule xml:lang="en">MP3Player</belongsToModule>
    <gr:legalName rdf:datatype="http://www.w3.org/2001/XMLSchema#string"
    >Modul Burotic SAS </gr:legalName>
    <rdfs:seeAlso rdf:resource="http://www.memup.de/"/>
    <rdfs:comment xml:lang="en">The business entity Modul Burotic SAS.</rdfs:comment>
    <rdfs:label rdf:datatype="http://www.w3.org/2001/XMLSchema#string"
    >Memup</rdfs:label>
  </gr:BusinessEntity>
  <Connectivity rdf:ID="DVI">
    <rdfs:label xml:lang="en">DVI</rdfs:label>
    <rdfs:label xml:lang="de">DVI</rdfs:label>
    <rdfs:comment xml:lang="en">The Digital Visual Interface (DVI) is a video interface standard designed to maximize the visual quality of digital display devices such as flat panel LCD computer displays and digital projectors. It is designed for carrying uncompressed digital video data to a display. It is partially compatible with the High-Definition Multimedia Interface (HDMI) standard in digital mode (DVI-D), and VGA in analog mode (DVI-A).

(This description is partly based on or reuses content from the Wikipedia article "Digital Visual Interface" (http://en.wikipedia.org/wiki/Digital_Visual_Interface) and is licensed under the GNU Free Documentation License (http://www.gnu.org/copyleft/fdl.html).)</rdfs:comment>
    <belongsToModule xml:lang="en">TV</belongsToModule>
  </Connectivity>
  <gr:BusinessEntity rdf:ID="MSI">
    <gr:legalName rdf:datatype="http://www.w3.org/2001/XMLSchema#string"
    >Micro-Star Int'l Co., Ltd.</gr:legalName>
    <rdfs:seeAlso rdf:resource="http://www.msi.com.tw/"/>
    <rdfs:comment xml:lang="en">The business entity Micro-Star Int'l Co., Ltd.</rdfs:comment>
    <belongsToModule xml:lang="en">MP3Player, TV</belongsToModule>
    <rdfs:label rdf:datatype="http://www.w3.org/2001/XMLSchema#string"
    >MSI</rdfs:label>
  </gr:BusinessEntity>
  <Features rdf:ID="EconomicalMode">
    <rdfs:comment xml:lang="en">Equipment that allows economical printing.</rdfs:comment>
    <rdfs:label xml:lang="en">Economical mode</rdfs:label>
    <rdfs:label xml:lang="de">Energiesparmodus</rdfs:label>
    <belongsToModule xml:lang="en">Printer</belongsToModule>
  </Features>
  <gr:BusinessEntity rdf:ID="InFocus">
    <rdfs:label rdf:datatype="http://www.w3.org/2001/XMLSchema#string"
    >InFocus</rdfs:label>
    <rdfs:seeAlso rdf:resource="http://www.infocus.com/"/>
    <rdfs:comment xml:lang="en">The business entity InFocus.</rdfs:comment>
    <belongsToModule xml:lang="en">TV</belongsToModule>
    <gr:legalName rdf:datatype="http://www.w3.org/2001/XMLSchema#string"
    >InFocus Co</gr:legalName>
  </gr:BusinessEntity>
  <DataFormatImage rdf:ID="GIF">
    <rdfs:label xml:lang="en">GIF</rdfs:label>
    <rdfs:label xml:lang="de">GIF</rdfs:label>
    <belongsToModule xml:lang="en">MP3Player, DigitalCamera, Camcorder</belongsToModule>
    <rdfs:comment xml:lang="en">The format supports up to 8 bits per pixel, allowing a single image to reference a palette of up to 256 distinct colors chosen from the 24-bit RGB color space.

(This description is partly based on or reuses content from the Wikipedia article "Graphics Interchange Format" (http://en.wikipedia.org/wiki/Graphics_Interchange_Format) and is licensed under the GNU Free Documentation License (http://www.gnu.org/copyleft/fdl.html).)</rdfs:comment>
  </DataFormatImage>
  <StorageMedia rdf:ID="SDHC">
    <rdfs:label xml:lang="de">SDHC</rdfs:label>
    <rdfs:label xml:lang="en">SDHC</rdfs:label>
    <rdfs:comment xml:lang="en">SDHC (Secure Digital High Capacity, SD 2.0) is an extension of the SD standard that appeared in June 2006.

(This description is partly based on or reuses content from the Wikipedia article "Secure Digital card" (http://en.wikipedia.org/wiki/Secure_Digital_card) and is licensed under the GNU Free Documentation License (http://www.gnu.org/copyleft/fdl.html).)</rdfs:comment>
    <belongsToModule xml:lang="en">Camcorder</belongsToModule>
  </StorageMedia>
  <VideoFeatures rdf:ID="DigitalImageScalingTechnology">
    <rdfs:label xml:lang="en">Digital Image Scaling Technology</rdfs:label>
    <rdfs:label xml:lang="de">Digital Image Scaling Technology</rdfs:label>
    <rdfs:comment xml:lang="en">Seamlessly up-scales any video source to display at full high definition 1080p.</rdfs:comment>
    <belongsToModule xml:lang="en">TV</belongsToModule>
  </VideoFeatures>
  <gr:BusinessEntity rdf:ID="Polaroid">
    <gr:legalName rdf:datatype="http://www.w3.org/2001/XMLSchema#string"
    >Polaroid Corporation</gr:legalName>
    <rdfs:comment xml:lang="en">The business entity Polaroid.</rdfs:comment>
    <rdfs:label rdf:datatype="http://www.w3.org/2001/XMLSchema#string"
    >Polaroid</rdfs:label>
    <rdfs:seeAlso rdf:resource="http://www.polaroid.com/"/>
    <belongsToModule xml:lang="en">TV, DigitalCamera</belongsToModule>
  </gr:BusinessEntity>
  <Features rdf:ID="Snapshot">
    <rdfs:label xml:lang="de">Snapshot</rdfs:label>
    <rdfs:label xml:lang="en">Snapshot</rdfs:label>
    <rdfs:comment xml:lang="en">Is a shot that is aimed and fired very quickly at a target that appears suddenly and for a very short period of time.</rdfs:comment>
    <belongsToModule xml:lang="en">Camcorder</belongsToModule>
  </Features>
  <gr:BusinessEntity rdf:ID="Kodak">
    <rdfs:comment xml:lang="en">The business entity Eastman Kodak Company.</rdfs:comment>
    <rdfs:seeAlso rdf:resource="http://www.kodak.com/"/>
    <rdfs:label rdf:datatype="http://www.w3.org/2001/XMLSchema#string"
    >Kodak</rdfs:label>
    <belongsToModule xml:lang="en">DigitalCamera, Camcorder</belongsToModule>
    <gr:legalName rdf:datatype="http://www.w3.org/2001/XMLSchema#string"
    >Eastman Kodak Company</gr:legalName>
  </gr:BusinessEntity>
  <gr:BusinessEntity rdf:ID="Hitachi">
    <belongsToModule xml:lang="en">TV, DigitalCamera, Camcorder</belongsToModule>
    <gr:legalName rdf:datatype="http://www.w3.org/2001/XMLSchema#string"
    >HITACHI Digital Media</gr:legalName>
    <rdfs:seeAlso rdf:resource="http://www.hitachidigitalmedia.com/"/>
    <rdfs:label rdf:datatype="http://www.w3.org/2001/XMLSchema#string"
    >Hitachi</rdfs:label>
    <rdfs:comment xml:lang="en">The business entity Hitachi.</rdfs:comment>
  </gr:BusinessEntity>
  <TVDisplayResolution rdf:ID="SDTV_480i">
    <belongsToModule xml:lang="en">TV</belongsToModule>
    <rdfs:comment xml:lang="en">480i is the shorthand name for a video mode, namely the U.S. NTSC television system or digital television systems with the same characteristics. The i, which is sometimes uppercase, stands for interlaced, the 480 for a vertical frame resolution of 480 lines containing picture information; while NTSC has a total of 525 lines, only 480 of these are used to display the image.

(This description is partly based on or reuses content from the Wikipedia article "480i" (http://en.wikipedia.org/wiki/480i) and is licensed under the GNU Free Documentation License (http://www.gnu.org/copyleft/fdl.html).)</rdfs:comment>
    <rdfs:label xml:lang="de">SDTV 480i</rdfs:label>
    <rdfs:label xml:lang="en">SDTV 480i</rdfs:label>
  </TVDisplayResolution>
  <StorageMedia rdf:ID="InternalFlashMemory">
    <rdfs:label xml:lang="de">Interner Flashspeicher</rdfs:label>
    <rdfs:label xml:lang="en">Internal flash memory</rdfs:label>
    <rdfs:comment xml:lang="en">Flash memory is non-volatile computer memory that can be electrically erased and reprogrammed.</rdfs:comment>
    <belongsToModule xml:lang="en">MP3Player, DigitalCamera, Camcorder</belongsToModule>
  </StorageMedia>
  <Features rdf:ID="VideoPlayBack">
    <rdfs:comment xml:lang="en">Ability to display video files.</rdfs:comment>
    <belongsToModule xml:lang="en">MP3Player</belongsToModule>
    <rdfs:label xml:lang="en">Video play back</rdfs:label>
    <rdfs:label xml:lang="de">Videowiedergabe</rdfs:label>
  </Features>
  <CompatibleOperatingSystems rdf:ID="MacOSXSnowLeopard">
    <rdfs:comment xml:lang="en">Mac OS is the trademarked name for a series of graphical user interface-based operating systems developed by Apple Inc. for their Macintosh line of computer systems.</rdfs:comment>
    <belongsToModule xml:lang="en">MP3Player, Printer, DigitalCamera, Camcorder</belongsToModule>
    <rdfs:label xml:lang="en">Mac OS X Snow Leopard</rdfs:label>
    <rdfs:label xml:lang="de">Mac OS X Snow Leopard</rdfs:label>
  </CompatibleOperatingSystems>
  <Connectivity rdf:ID="ComponentVideoIn">
    <rdfs:comment xml:lang="en">Component video is a video signal that has been split into two or more components. In popular use, it refers to a type of analog video information that is transmitted or stored as three separate signals. Component video can be contrasted with composite video (NTSC, PAL or SECAM) in which all the video information is combined into a single line-level signal. Like composite, component video cables do not carry audio and are often paired with audio cables. Here the input is meant.

(This description is partly based on or reuses content from the Wikipedia article "Component video" (http://en.wikipedia.org/wiki/Component_video) and is licensed under the GNU Free Documentation License (http://www.gnu.org/copyleft/fdl.html).)</rdfs:comment>
    <belongsToModule xml:lang="en">TV</belongsToModule>
    <rdfs:label xml:lang="en">Component video in</rdfs:label>
    <rdfs:label xml:lang="de">Component video in</rdfs:label>
  </Connectivity>
  <gr:BusinessEntity rdf:ID="Canon">
    <gr:legalName rdf:datatype="http://www.w3.org/2001/XMLSchema#string"
    >Canon Inc.</gr:legalName>
    <rdfs:label rdf:datatype="http://www.w3.org/2001/XMLSchema#string"
    >Canon</rdfs:label>
    <rdfs:comment xml:lang="en">The business entity Canon.</rdfs:comment>
    <rdfs:seeAlso rdf:resource="http://www.canon.com/"/>
    <belongsToModule xml:lang="en">Printer, DigitalCamera, Camcorder</belongsToModule>
  </gr:BusinessEntity>
  <gr:BusinessEntity rdf:ID="Hisense">
    <rdfs:seeAlso rdf:resource="http://www.hisense.com/"/>
    <rdfs:comment xml:lang="en">The business entity Hisense.</rdfs:comment>
    <gr:legalName rdf:datatype="http://www.w3.org/2001/XMLSchema#string"
    >Hisense Group</gr:legalName>
    <belongsToModule xml:lang="en">TV</belongsToModule>
    <rdfs:label rdf:datatype="http://www.w3.org/2001/XMLSchema#string"
    >Hisense</rdfs:label>
  </gr:BusinessEntity>
  <Features rdf:ID="DuplexPrint">
    <belongsToModule xml:lang="en">Printer</belongsToModule>
    <rdfs:comment xml:lang="en">A feature of computer printers and MFPs that allows the automatic printing of a sheet of paper on both sides.</rdfs:comment>
    <rdfs:label xml:lang="de">Duplexdruck</rdfs:label>
    <rdfs:label xml:lang="en">Duplex print</rdfs:label>
  </Features>
  <DataInterfaceType rdf:ID="IEEE_802.11">
    <rdfs:comment xml:lang="en">IEEE 802.11 is a set of standards for wireless local area network (WLAN) computer communication, developed by the IEEE LAN/MAN Standards Committee (IEEE 802) in the 5 GHz and 2.4 GHz public spectrum bands.

(This description is partly based on or reuses content from the Wikipedia article "802.11" (http://en.wikipedia.org/wiki/802.11) and is licensed under the GNU Free Documentation License (http://www.gnu.org/copyleft/fdl.html).)</rdfs:comment>
    <rdfs:label xml:lang="en">IEEE 802.11</rdfs:label>
    <rdfs:label xml:lang="de">IEEE 802.11</rdfs:label>
    <belongsToModule xml:lang="en">MP3Player, Printer, DigitalCamera, Camcorder</belongsToModule>
  </DataInterfaceType>
  <gr:BusinessEntity rdf:ID="Phillar">
    <gr:legalName rdf:datatype="http://www.w3.org/2001/XMLSchema#string"
    >Phillar electronics b. V.</gr:legalName>
    <belongsToModule xml:lang="en">TV</belongsToModule>
    <rdfs:label rdf:datatype="http://www.w3.org/2001/XMLSchema#string"
    >Phillar</rdfs:label>
    <rdfs:comment xml:lang="en">The business entity Phillar.</rdfs:comment>
  </gr:BusinessEntity>
  <gr:BusinessEntity rdf:ID="Microsoft">
    <gr:legalName rdf:datatype="http://www.w3.org/2001/XMLSchema#string"
    >Microsoft Corporation</gr:legalName>
    <rdfs:seeAlso rdf:resource="http://www.microsoft.com/"/>
    <belongsToModule xml:lang="en">MP3Player</belongsToModule>
    <rdfs:label rdf:datatype="http://www.w3.org/2001/XMLSchema#string"
    >Microsoft</rdfs:label>
    <rdfs:comment xml:lang="en">The business entity Microsoft Corporation.</rdfs:comment>
  </gr:BusinessEntity>
  <Features rdf:ID="BacklightMode">
    <rdfs:label xml:lang="de">Hintergrundbeleuchtungsmodus</rdfs:label>
    <rdfs:label xml:lang="en">Backlight mode</rdfs:label>
    <belongsToModule xml:lang="en">DigitalCamera, Camcorder</belongsToModule>
    <rdfs:comment xml:lang="en">Ability to photograph against a light source.</rdfs:comment>
  </Features>
  <DataFormatAudio rdf:ID="OGG">
    <rdfs:label xml:lang="en">OGG</rdfs:label>
    <rdfs:label xml:lang="de">OGG</rdfs:label>
    <rdfs:comment xml:lang="en">Ogg is a free, open standard container format maintained by the Xiph.Org Foundation.</rdfs:comment>
    <belongsToModule xml:lang="en">MP3Player, DigitalCamera, Camcorder</belongsToModule>
  </DataFormatAudio>
  <SignalFormat rdf:ID="SECAM-L">
    <rdfs:label xml:lang="en">SECAM-L</rdfs:label>
    <rdfs:label xml:lang="de">SECAM-L</rdfs:label>
    <belongsToModule xml:lang="en">TV</belongsToModule>
    <rdfs:comment xml:lang="en">SECAM, also written SÉCAM (Séquentiel couleur à mémoire, French for "Sequential Color with Memory"), is an analog color television system first used in France. French SECAM (SECAM-L) is used only in France, Luxembourg (only RTL9 on CH 21 from Dudelange) and Tele Monte-Carlo Transmitters in the south of France.

(This description is partly based on or reuses content from the Wikipedia article "SECAM" (http://en.wikipedia.org/wiki/SECAM) and is licensed under the GNU Free Documentation License (http://www.gnu.org/copyleft/fdl.html).)</rdfs:comment>
  </SignalFormat>
  <RechargeableEnergySource rdf:ID="NiCd">
    <belongsToModule xml:lang="en">MP3Player, DigitalCamera, Camcorder</belongsToModule>
    <rdfs:label xml:lang="en">NiCd</rdfs:label>
    <rdfs:label xml:lang="de">NiCd</rdfs:label>
    <rdfs:comment xml:lang="en">A type of rechargeable battery using nickel oxide hydroxide and metallic cadmium as electrodes.

(This description is partly based on or reuses content from the Wikipedia article "Nickel-cadmium battery" (http://en.wikipedia.org/wiki/Nickel-cadmium_battery) and is licensed under the GNU Free Documentation License (http://www.gnu.org/copyleft/fdl.html).)</rdfs:comment>
  </RechargeableEnergySource>
  <gr:BusinessEntity rdf:ID="Belkin">
    <rdfs:seeAlso rdf:resource="http://www.belkin.com/"/>
    <gr:legalName rdf:datatype="http://www.w3.org/2001/XMLSchema#string"
    >Belkin International Inc</gr:legalName>
    <rdfs:comment xml:lang="en">The business entity Belkin International Inc.</rdfs:comment>
    <rdfs:label rdf:datatype="http://www.w3.org/2001/XMLSchema#string"
    >Belkin</rdfs:label>
    <belongsToModule xml:lang="en">MP3Player</belongsToModule>
  </gr:BusinessEntity>
  <MediaType rdf:ID="Transparency">
    <belongsToModule xml:lang="en">Printer</belongsToModule>
    <rdfs:comment xml:lang="en">A thin sheet of transparent flexible material, typically cellulose acetate, onto which you can print.</rdfs:comment>
    <rdfs:label xml:lang="de">Folie</rdfs:label>
    <rdfs:label xml:lang="en">Transparency</rdfs:label>
  </MediaType>
  <owl:AnnotationProperty rdf:about="http://purl.org/dc/elements/1.1/creator"/>
  <MediaFormat rdf:ID="DL">
    <belongsToModule xml:lang="en">Printer</belongsToModule>
    <rdfs:label xml:lang="de">DL</rdfs:label>
    <rdfs:label xml:lang="en">DL</rdfs:label>
    <rdfs:comment xml:lang="en">Format of the german institute for standardization: 110 x 220 mm.</rdfs:comment>
  </MediaFormat>
  <DataInterfaceType rdf:ID="DVI_out">
    <belongsToModule xml:lang="en">Camcorder</belongsToModule>
    <rdfs:label xml:lang="de">DVI out</rdfs:label>
    <rdfs:label xml:lang="en">DVI out</rdfs:label>
    <rdfs:comment xml:lang="en">A digital video format created by Sony, JVC, Panasonic and other video camera producers.</rdfs:comment>
  </DataInterfaceType>
  <Accessory rdf:ID="VideoComponent_Cable">
    <rdfs:comment xml:lang="en">A video signal that has been split into two or more components.</rdfs:comment>
    <rdfs:label xml:lang="de">Videokomponentenkabel</rdfs:label>
    <rdfs:label xml:lang="en">Video component cable</rdfs:label>
    <belongsToModule xml:lang="en">Camcorder</belongsToModule>
  </Accessory>
  <TVDisplayResolution rdf:ID="HDTV_1080i">
    <rdfs:label xml:lang="de">HDTV 1080i</rdfs:label>
    <rdfs:label xml:lang="en">HDTV 1080i</rdfs:label>
    <belongsToModule xml:lang="en">TV</belongsToModule>
    <rdfs:comment xml:lang="en">1080i is the shorthand name of a format of high-definition video modes. 1080 denotes the number of horizontal scan lines - also known as vertical resolution - and the letter i stands for interlaced.

(This description is partly based on or reuses content from the Wikipedia article "1080i" (http://en.wikipedia.org/wiki/1080i) and is licensed under the GNU Free Documentation License (http://www.gnu.org/copyleft/fdl.html).)</rdfs:comment>
  </TVDisplayResolution>
  <SignalFormat rdf:ID="SECAM-B_G">
    <rdfs:comment xml:lang="en">SECAM, also written SÉCAM (Séquentiel couleur à mémoire, French for "Sequential Color with Memory"), is an analog color television system first used in France. SECAM-B/G is used in the Middle East, former East Germany and Greece.

(This description is partly based on or reuses content from the Wikipedia article "SECAM" (http://en.wikipedia.org/wiki/SECAM) and is licensed under the GNU Free Documentation License (http://www.gnu.org/copyleft/fdl.html).)</rdfs:comment>
    <belongsToModule xml:lang="en">TV</belongsToModule>
    <rdfs:label xml:lang="en">SECAM-B G</rdfs:label>
    <rdfs:label xml:lang="de">SECAM-B G</rdfs:label>
  </SignalFormat>
  <gr:BusinessEntity rdf:ID="Daewoo">
    <rdfs:seeAlso rdf:resource="http://www.daewoo-electronics.de/"/>
    <belongsToModule xml:lang="en">TV</belongsToModule>
    <gr:legalName rdf:datatype="http://www.w3.org/2001/XMLSchema#string"
    >Daewoo Electronics</gr:legalName>
    <rdfs:comment xml:lang="en">The business entity Daewoo.</rdfs:comment>
    <rdfs:label rdf:datatype="http://www.w3.org/2001/XMLSchema#string"
    >Daewoo</rdfs:label>
  </gr:BusinessEntity>
  <Certificate rdf:ID="CE_Mark">
    <rdfs:comment xml:lang="en">The CE marking (also known as CE mark) is a mandatory conformity mark on many products placed on the single market in the European Economic Area (EEA).

(This description is partly based on or reuses content from the Wikipedia article "CE mark" (http://en.wikipedia.org/wiki/CE_mark) and is licensed under the GNU Free Documentation License (http://www.gnu.org/copyleft/fdl.html).)</rdfs:comment>
    <rdfs:label xml:lang="en">CE Mark</rdfs:label>
    <rdfs:label xml:lang="de">CE Mark</rdfs:label>
    <belongsToModule xml:lang="en">TV</belongsToModule>
  </Certificate>
  <gr:BusinessEntity rdf:ID="Axago">
    <rdfs:label rdf:datatype="http://www.w3.org/2001/XMLSchema#string"
    >Axago</rdfs:label>
    <belongsToModule xml:lang="en">MP3Player</belongsToModule>
    <rdfs:comment xml:lang="en">The business entity Axago.</rdfs:comment>
    <rdfs:seeAlso rdf:resource="http://www.axago.cz/"/>
    <gr:legalName rdf:datatype="http://www.w3.org/2001/XMLSchema#string"
    >Axago</gr:legalName>
  </gr:BusinessEntity>
  <gr:BusinessEntity rdf:ID="Hyundai">
    <rdfs:label rdf:datatype="http://www.w3.org/2001/XMLSchema#string"
    >Hyundai</rdfs:label>
    <gr:legalName rdf:datatype="http://www.w3.org/2001/XMLSchema#string"
    >Hyundai IT Europe GmbH</gr:legalName>
    <rdfs:seeAlso rdf:resource="http://www.hyundaiit.eu/"/>
    <belongsToModule xml:lang="en">TV</belongsToModule>
    <rdfs:comment xml:lang="en">The business entity Hyundai.</rdfs:comment>
  </gr:BusinessEntity>
  <MediaType rdf:ID="Photopaper">
    <belongsToModule xml:lang="en">Printer</belongsToModule>
    <rdfs:comment xml:lang="en">Kind of paper that is specifically designed to print high quality digital photos.</rdfs:comment>
    <rdfs:label xml:lang="de">Fotopapier</rdfs:label>
    <rdfs:label xml:lang="en">Photo paper</rdfs:label>
  </MediaType>
  <DataInterfaceType rdf:ID="S-Video_in">
    <belongsToModule xml:lang="en">TV, Camcorder</belongsToModule>
    <rdfs:label xml:lang="de">S-Video in</rdfs:label>
    <rdfs:label xml:lang="en">S-Video in</rdfs:label>
    <rdfs:comment xml:lang="en">Is an analog video signal that carries the video data as two separate signals, lumen (luminance) and chroma (color).

(This description is partly based on or reuses content from the Wikipedia article "S-Video" (http://en.wikipedia.org/wiki/S-Video) and is licensed under the GNU Free Documentation License (http://www.gnu.org/copyleft/fdl.html).)</rdfs:comment>
  </DataInterfaceType>
  <gr:BusinessEntity rdf:ID="Freecom">
    <rdfs:label rdf:datatype="http://www.w3.org/2001/XMLSchema#string"
    >Freecom</rdfs:label>
    <belongsToModule xml:lang="en">MP3Player</belongsToModule>
    <rdfs:comment xml:lang="en">The business entity Freecom Technologies GmbH.</rdfs:comment>
    <rdfs:seeAlso rdf:resource="http://www.freecom.de/"/>
    <gr:legalName rdf:datatype="http://www.w3.org/2001/XMLSchema#string"
    >Freecom Technologies GmbH</gr:legalName>
  </gr:BusinessEntity>
  <SceneMode rdf:ID="BeachAndSnow">
    <belongsToModule xml:lang="en">Camcorder</belongsToModule>
    <rdfs:comment xml:lang="en">Ability of the camcorder to adapt to special environments.</rdfs:comment>
    <rdfs:label xml:lang="en">Beach and snow</rdfs:label>
    <rdfs:label xml:lang="de">Strand und Schnee</rdfs:label>
  </SceneMode>
  <gr:BusinessEntity rdf:ID="Epson">
    <rdfs:comment xml:lang="en">The business entity Seiko Epson Corporation.</rdfs:comment>
    <gr:legalName rdf:datatype="http://www.w3.org/2001/XMLSchema#string"
    >Seiko Epson Corporation</gr:legalName>
    <rdfs:label rdf:datatype="http://www.w3.org/2001/XMLSchema#string"
    >Epson</rdfs:label>
    <rdfs:seeAlso rdf:resource="http://www.epson.co.jp/e/"/>
    <belongsToModule xml:lang="en">MP3Player, Printer, DigitalCamera</belongsToModule>
  </gr:BusinessEntity>
  <gr:BusinessEntity rdf:ID="BenQ">
    <rdfs:seeAlso rdf:resource="http://www.aoc-europe.com/"/>
    <gr:legalName rdf:datatype="http://www.w3.org/2001/XMLSchema#string"
    >BenQ Corporation</gr:legalName>
    <rdfs:label rdf:datatype="http://www.w3.org/2001/XMLSchema#string"
    >BenQ</rdfs:label>
    <belongsToModule xml:lang="en">MP3Player, TV, DigitalCamera</belongsToModule>
    <rdfs:comment xml:lang="en">The business entity BenQ Corporation.</rdfs:comment>
  </gr:BusinessEntity>
  <DataInterfaceType rdf:ID="MiniUSB">
    <rdfs:label xml:lang="en">Mini USB</rdfs:label>
    <rdfs:label rdf:datatype="http://www.w3.org/2001/XMLSchema#string"
    >Mini USB</rdfs:label>
    <rdfs:comment xml:lang="en">The non-standard Mini-USB's, official Mini-B, Micro-A, and Micro-B connectors are used for smaller devices such as PDAs, mobile phones or digital cameras. The Standard-A plug is approximately 4 by 12 mm, the Standard-B approximately 7 by 8 mm, and the Mini-A and Mini-B plugs approximately 2 by 7 mm.

(This description is partly based on or reuses content from the Wikipedia article "Universial Serial Bus" (http://en.wikipedia.org/wiki/Universal_Serial_Bus) and is licensed under the GNU Free Documentation License (http://www.gnu.org/copyleft/fdl.html).)</rdfs:comment>
    <belongsToModule xml:lang="en">MP3Player, Printer, DigitalCamera, Camcorder</belongsToModule>
  </DataInterfaceType>
  <Color rdf:ID="Red">
    <rdfs:label xml:lang="en">Red</rdfs:label>
    <rdfs:label xml:lang="de">Rot</rdfs:label>
    <belongsToModule xml:lang="en">MP3Player, TV, Printer, DigitalCamera, Camcorder</belongsToModule>
    <rdfs:comment xml:lang="en">RGB Value 255,0,0</rdfs:comment>
  </Color>
  <gr:BusinessEntity rdf:ID="Sharkoon">
    <rdfs:seeAlso rdf:resource="http://www.sharkoon.com/"/>
    <belongsToModule xml:lang="en">MP3Player</belongsToModule>
    <gr:legalName rdf:datatype="http://www.w3.org/2001/XMLSchema#string"
    >SHARKOON Technologies GmbH </gr:legalName>
    <rdfs:label rdf:datatype="http://www.w3.org/2001/XMLSchema#string"
    >Sharkoon</rdfs:label>
    <rdfs:comment xml:lang="en">The business entity SHARKOON Technologies GmbH.</rdfs:comment>
  </gr:BusinessEntity>
  <gr:BusinessEntity rdf:ID="Verbatim">
    <rdfs:comment xml:lang="en">The business entity Verbatim Corporation.</rdfs:comment>
    <rdfs:label rdf:datatype="http://www.w3.org/2001/XMLSchema#string"
    >Verbatim</rdfs:label>
    <belongsToModule xml:lang="en">MP3Player</belongsToModule>
    <rdfs:seeAlso rdf:resource="http://www.verbatim.com/"/>
    <gr:legalName rdf:datatype="http://www.w3.org/2001/XMLSchema#string"
    >Verbatim Corporation </gr:legalName>
  </gr:BusinessEntity>
  <MediaFormat rdf:ID="B9">
    <rdfs:comment xml:lang="en">Format of the german institute for standardization: 44 x 62 mm.</rdfs:comment>
    <belongsToModule xml:lang="en">Printer</belongsToModule>
    <rdfs:label xml:lang="de">B9</rdfs:label>
    <rdfs:label xml:lang="en">B9</rdfs:label>
  </MediaFormat>
  <CompatibleOperatingSystems rdf:ID="MacOSXTiger">
    <belongsToModule xml:lang="en">MP3Player, Printer, DigitalCamera, Camcorder</belongsToModule>
    <rdfs:comment xml:lang="en">Mac OS is the trademarked name for a series of graphical user interface-based operating systems developed by Apple Inc. for their Macintosh line of computer systems.</rdfs:comment>
    <rdfs:label xml:lang="en">Mac OS X Tiger</rdfs:label>
    <rdfs:label xml:lang="de">Mac OS X Tiger</rdfs:label>
  </CompatibleOperatingSystems>
  <SensorType rdf:ID="CMOS">
    <belongsToModule xml:lang="en">Camcorder</belongsToModule>
    <rdfs:comment xml:lang="en">Complementary metal-oxide-semiconductor (CMOS) (pronounced "see-moss", IPA: /&#712;si&#720;m&#594;s/), is a major class of integrated circuits. CMOS technology is used in microprocessors, microcontrollers, static RAM, and other digital logic circuits. CMOS technology is also used for a wide variety of analog circuits such as image sensors, data converters, and highly integrated transceivers for many types of communication. Frank Wanlass successfully patented CMOS in 1967 (US Patent 3,356,858).

(This description is partly based on or reuses content from the Wikipedia article "CMOS" (http://en.wikipedia.org/wiki/CMOS) and is licensed under the GNU Free Documentation License (http://www.gnu.org/copyleft/fdl.html).)</rdfs:comment>
    <rdfs:label xml:lang="en">CMOS</rdfs:label>
    <rdfs:label xml:lang="de">CMOS</rdfs:label>
  </SensorType>
  <Connectivity rdf:ID="HDMI">
    <belongsToModule xml:lang="en">TV</belongsToModule>
    <rdfs:label xml:lang="de">HDMI</rdfs:label>
    <rdfs:label xml:lang="en">HDMI</rdfs:label>
    <rdfs:comment xml:lang="en">HDMI (High-Definition Multimedia Interface) is a compact audio/video interface for transmitting uncompressed digital data. It represents a digital alternative to consumer analog standards such as Radio Frequency (RF) coaxial cable, composite video, S-Video, SCART, component video, D-Terminal, and VGA. HDMI connects digital audio/video sources such as set-top boxes, Blu-ray Disc players, personal computers (PCs), video game consoles, and AV receivers to compatible digital audio devices, computer monitors, and digital televisions.

(This description is partly based on or reuses content from the Wikipedia article "HDMI" (http://en.wikipedia.org/wiki/HDMI) and is licensed under the GNU Free Documentation License (http://www.gnu.org/copyleft/fdl.html).)</rdfs:comment>
  </Connectivity>
</rdf:RDF>

<!-- Created with Protege (with OWL Plugin 3.3.1, Build 430)  http://protege.stanford.edu -->